@prefix : <http://buildvoc.co.uk/resource/> .
@prefix dc: <http://purl.org/dc/elements/1.1/> .
@prefix dcat: <http://www.w3.org/ns/dcat#> .
@prefix dct: <http://purl.org/dc/terms/> .
@prefix grddl: <http://www.w3.org/2003/g/data-view#> .
@prefix ns: <http://www.w3.org/2003/06/sw-vocab-status/ns#> .
@prefix olo: <http://purl.org/ontology/olo/core#> .
@prefix owl: <http://www.w3.org/2002/07/owl#> .
@prefix rdf: <http://www.w3.org/1999/02/22-rdf-syntax-ns#> .
@prefix rdfs: <http://www.w3.org/2000/01/rdf-schema#> .
@prefix skos: <http://www.w3.org/2004/02/skos/core#> .
@prefix skosxl: <http://www.w3.org/2008/05/skos-xl#> .
@prefix xsd: <http://www.w3.org/2001/XMLSchema#> .

<http://buildvoc.co.uk/resource/> a owl:Ontology .

:c_4cdc3b72 a skos:Concept;
  skos:prefLabel "compartment wall or floor"@en .

:c_79a3679f dc:source :c_6c82c09f .

:c_6c82c09f a skos:Concept;
  dc:publisher "Department for Communities and Local Government"@en, <http://viaf.org/viaf/143434596>;
  dc:subject """Building Regulations 2010: Approved Documents B
"""@en;
  dct:created "2019-11-30T07:32:03.382Z"^^xsd:dateTime;
  skos:broader :c_d4480e31;
  skos:definition "Presents the functional requirements for complying with fire safety in buildings other than dwellings in the building regulations. The sections cover: B1 - Means of warning and escape, B2 - Internal fire spread (linings), B3 - Internal fire spread (structure), B4 - External fire spread and B5 - Access and facilities for the fire service. Also includes Regulations 6(3), 7(2) and 38. Volume 1 deals with dwellings and blocks of flats and Volume 2 deals with all other types of building covered by the Building Regulations."@en;
  skos:inScheme :conceptScheme_751925ed;
  skos:prefLabel "fire safety - volume 2: buildings other than dwellings. 2019 edition - for use in england"@en .

:c_ca00c020 a skos:Concept;
  dc:publisher "Department for Communities and Local Government"@en, <http://viaf.org/viaf/143434596>;
  dc:subject """Building Regulations 2010: Approved Documents B
"""@en;
  dct:created "2019-11-30T07:34:38.949Z"^^xsd:dateTime;
  dct:modified "2020-10-23T17:17:44.557Z"^^xsd:dateTime;
  skos:broader :c_d4480e31;
  skos:definition "Presents the functional requirements for complying with fire safety in dwellings in the building regulations. The sections cover: B1 - Means of warning and escape, B2 - Internal fire spread (linings), B3 - Internal fire spread (structure), B4 - External fire spread and B5 - Access and facilities for the fire service. Also includes Regulations 6(3), 7(2) and 38. Approved Document B (fire safety) has been published in two volumes. Volume 1 deals with dwellings and blocks of flats and Volume 2 deals with all other types of building covered by the Building Regulations."@en;
  skos:example <https://assets.publishing.service.gov.uk/government/uploads/system/uploads/attachment_data/file/832631/Approved_Document_B__fire_safety__volume_1_-_2019_edition.pdf>;
  skos:inScheme :conceptScheme_751925ed;
  skos:prefLabel "fire safety - volume 1: dwellings. 2019 edition - for use in england"@en .

:c_75f7c82b skos:narrower :c_007625df, :c_139d3767, :c_1d287961, :c_1dfadb92, :c_3a5b7e76,
    :c_454526b8, :c_659ab1b8, :c_851c02b0, :c_da079e58, :c_daa05efb, :c_e756ef49, :c_f127ef1e,
    :c_f340cba7, :c_fabf0784 .

:c_502a871c skos:changeNote "changed from guidance documents "@en;
  skos:narrower :c_37246cae;
  skos:prefLabel "building regulations guidance"@en .

:c_d4480e31 skos:narrower :c_6c82c09f .

:xl_en_d2f47531 dct:modified "2019-11-30T07:27:51.385Z"^^xsd:dateTime;
  skosxl:literalForm "building regulations guidance"@en .

:c_f9b32acf a skos:Concept;
  dct:created "2018-03-28T19:03:52.286Z"^^xsd:dateTime;
  skos:closeMatch <https://www.eionet.europa.eu/gemet/en/concept/11514>;
  skos:definition "The act of regulating; a rule or order prescribed for management or government; a regulating principle; a precept. Rule of order prescribed by superior or competent authority relating to action on those under its control."@en;
  skos:inScheme :conceptScheme_751925ed;
  skos:narrower :c_0e0d001c, :c_86cfaae6;
  skos:topConceptOf :conceptScheme_751925ed .

:c_37246cae dct:modified "2020-11-04T06:54:21.843Z"^^xsd:dateTime .

:c_86cfaae6 skos:notation "uksi 2010 2214"@en .

:c_132d79ca dc:source :c_6c82c09f, :c_ca00c020 .

:c_727adfdb dc:source :c_ca00c020 .

:c_5724a233 dc:source :c_ca00c020;
  dct:modified "2019-12-21T07:22:01.689Z"^^xsd:dateTime .

:c_b44f46e0 dc:source :c_ca00c020;
  skos:prefLabel "specified attachment"@en .

:c_a4eaf123 dc:source :c_ca00c020;
  skos:definition "(fire-protecting) A ceiling suspended below a floor that adds to the fire resistance of the floor."@en .

:c_228ee3b0 dc:publisher """HM Government
"""@en;
  dct:created "2019-11-30T11:58:19.854Z"^^xsd:dateTime;
  skos:definition "A room that the only escape route from an inner room passes through."@en;
  skos:prefLabel "access room"@en .

:c_da6168d8 dct:created "2019-12-12T20:41:23.654Z"^^xsd:dateTime;
  dct:modified "2019-12-28T07:17:46.911Z"^^xsd:dateTime;
  skos:broader :c_13911a49 .

:c_7fc5469b skos:definition "A space enclosed by elements of a building (including a suspended ceiling) or contained within an element, but that is not a room, cupboard, circulation space, protected shaft, or space within a flue, chute, duct, pipe or conduit."@en;
  skos:inScheme :conceptScheme_751925ed;
  skos:prefLabel "cavity"@en .

:c_6284471b a skos:Concept .

:xl_en_42f4c7a1 a skosxl:Label;
  skosxl:literalForm "air"@en .

:c_56fef4b5 dc:source :c_6c82c09f;
  skos:inScheme :conceptScheme_751925ed .

:c_bed063fd skos:inScheme :conceptScheme_751925ed .

:c_f5536b7d dct:modified "2019-12-13T23:33:59.284Z"^^xsd:dateTime .

:c_83464c52 dct:created "2019-12-12T20:50:45.745Z"^^xsd:dateTime .

:c_33c0e1b5 dc:source :c_ca00c020;
  skos:inScheme :conceptScheme_751925ed .

:c_9b7f9eb7 dct:modified "2019-12-13T22:36:18.618Z"^^xsd:dateTime .

:c_4a90e0e1 dct:created "2019-12-13T23:19:04.145Z"^^xsd:dateTime;
  skos:definition "A building or part of a building, comprising one or more rooms, spaces or storeys, that is constructed to prevent the spread of fire to or from another part of the same building or an adjoining building."@en .

:c_13911a49 skos:narrower :c_056e5a0a, :c_10ea4ecc, :c_4cb80404, :c_4cdc3b72, :c_7d862abe,
    :c_858351ef, :c_a4eaf123, :c_b3f65603 .

:c_b2cab8d9 skos:inScheme :conceptScheme_751925ed .

:c_4553c077 dct:created "2018-07-22T14:24:33.455Z"^^xsd:dateTime .

:c_feba40b2 dct:modified "2020-10-23T17:04:12.702Z"^^xsd:dateTime .

:c_e7e6b110 dc:source :c_ca00c020 .



:c_8258611b dc:source :c_6c82c09f .

:xl_en_2de5ebbe a skosxl:Label .

:conceptScheme_751925ed a skos:ConceptScheme;
  dc:contributor "British Standards Institution"@en;
  dc:creator "P Stacey"@en;
  dct:created "2018-04-07T19:41:18.052Z"^^xsd:dateTime;
  dct:license <http://creativecommons.org/licenses/by/4.0/>;
  dct:modified "2019-11-30T10:41:58.827Z"^^xsd:dateTime;
  skos:prefLabel "Drawing information"@en, "General"@en, "Information and communication"@en,
    "Labour"@en, "Legislation"@en, "Materials"@en, "Phases of development (construction)"@en .

:c_6c82c09f dct:modified "2020-10-23T17:18:08.995Z"^^xsd:dateTime .

:xl_en_91bd8550 skosxl:literalForm "attma"@en .

:c_38ba0f99 dct:created "2019-12-15T08:42:47.378Z"^^xsd:dateTime;
  skos:broader :c_13911a49 .

:xl_en_96c8608e a skosxl:Label;
  skosxl:literalForm "loi"@en .

:c_3e5063e6 skos:definition "A storey with a floor that, at some point, is more than 1200mm below the highest level of ground beside the outside walls. (However, see Appendix B, paragraph B26c, for situations where the storey is considered to be a basement only because of a sloping site.)"@en;
  skos:inScheme :conceptScheme_751925ed .

:c_34f295d5 rdfs:isDefinedBy <http://www.legislation.gov.uk/uksi/2010/2214/regulation/2>;
  skos:prefLabel "dwelling"@en .

:xl_en_45e6bbda a skosxl:Label .

:c_b3f65603 a skos:Concept;
  dct:modified "2020-10-26T07:36:45.280Z"^^xsd:dateTime;
  skos:definition "A flat that is a workplace for people who live there, its occupants, and for people who do not live on the premises."@en;
  skos:inScheme :conceptScheme_751925ed;
  skos:prefLabel "live/work unit"@en .

:c_10ea4ecc a skos:Concept;
  dct:created "2019-12-15T08:28:48.957Z"^^xsd:dateTime;
  dct:modified "2019-12-15T08:34:09.621Z"^^xsd:dateTime;
  skos:broader :c_13911a49;
  skos:definition "Structural means that provide one or more safe routes for people to go, during a fire, from any point in the building to a place of safety."@en;
  skos:inScheme :conceptScheme_751925ed;
  skos:prefLabel "means of escape"@en .

:c_056e5a0a dc:source :c_6c82c09f;
  dct:created "2019-12-15T08:25:31.904Z"^^xsd:dateTime;
  dct:modified "2019-12-15T08:34:09.992Z"^^xsd:dateTime;
  skos:note "Room from which escape is possible only by passing through another room (the access room)."@en .

:c_4cb80404 a skos:Concept;
  dc:source :c_6c82c09f, :c_ca00c020;
  dct:created "2019-12-15T08:34:53.951Z"^^xsd:dateTime;
  dct:modified "2019-12-15T08:38:34.953Z"^^xsd:dateTime;
  skos:broader :c_13911a49;
  skos:definition "The internal arrangement of a building in which more than one storey or level is contained in one undivided volume, e.g. split-level floors. For the purposes of this document there is a distinction between open spatial planning and an atrium space."@en;
  skos:inScheme :conceptScheme_751925ed;
  skos:prefLabel "open spatial planning"@en .

:c_f4139893 a skos:Concept;
  dc:source :c_6c82c09f, :c_ca00c020;
  dct:created "2019-12-21T06:28:24.441Z"^^xsd:dateTime;
  skos:broader :c_13911a49;
  skos:definition "A place of education for children between 2 and 19 years old. The term includes nursery schools, primary schools and secondary schools as defined in the Education Act 1996."@en;
  skos:inScheme :conceptScheme_751925ed;
  skos:prefLabel "school"@en .

:c_1f1f7725 a skos:Concept;
  dc:source :c_6c82c09f, :c_ca00c020;
  dct:created "2019-12-15T08:30:42.736Z"^^xsd:dateTime;
  dct:modified "2019-12-15T08:34:09.545Z"^^xsd:dateTime;
  skos:broader :c_13911a49;
  skos:definition """<ul><li>Width of a doorway, cubic capacity, area, height of a building and number of storeys are measured as shown in Appendix D, Diagrams D1 to D6.
<li>Occupant number, travel distance, escape route and stairs are measured as described in Appendix D, paragraphs D1 to D4.</ul>"""@en;
  skos:inScheme :conceptScheme_751925ed;
  skos:prefLabel "measurement"@en .

:c_35d3a535 a skos:Concept;
  dct:modified "2019-12-15T08:46:59.170Z"^^xsd:dateTime;
  skos:broader :c_13911a49;
  skos:definition "Includes pipe fittings and accessories. The definition of ‘pipe’ excludes a flue pipe and a pipe used for ventilating purposes, other than a ventilating pipe for an above-ground drainage system."@en;
  skos:inScheme :conceptScheme_751925ed;
  skos:prefLabel "pipe"@en .

:c_ee10273a skos:inScheme :conceptScheme_751925ed .

:c_7c12f560 dc:source :c_ca00c020;
  skos:definition "A stair that leads to a final exit to a place of safety and that is adequately enclosed with fire resisting construction. Included in the definition is any exit passageway between the foot of the stair and the final exit."@en .

:c_cc61a0f4 dct:modified "2019-12-21T06:27:11.448Z"^^xsd:dateTime .

:c_d5c15327 dct:modified "2019-12-15T08:47:29.723Z"^^xsd:dateTime;
  skos:definition "An electrical circuit that is protected against fire."@en .

:c_d32d8045 a skos:Concept;
  skos:prefLabel "single storey"@en .

:c_46be855e skos:broader :c_13911a49 .

:c_7d862abe a skos:Concept;
  dc:source :c_ca00c020;
  dct:created "2019-12-21T06:32:03.423Z"^^xsd:dateTime;
  skos:broader :c_13911a49;
  skos:definition "A device that closes a door, when open at any angle, against a door frame."@en;
  skos:inScheme :conceptScheme_751925ed;
  skos:prefLabel "self-closing device"@en .

:c_132d79ca skos:inScheme :conceptScheme_751925ed;
  skos:prefLabel "site"@en .

:c_7b85eda3 dct:modified "2019-12-21T06:27:12.227Z"^^xsd:dateTime;
  skos:definition "A corridor or lobby that is adequately protected from fire in adjoining areas by fire resisting construction."@en .

:c_b6083e42 dc:source :c_6c82c09f .

:c_b44f46e0 skos:definition """Includes any of the following. 
<ul><li>A balcony attached to an external wall.
<li>A device for reducing heat gain within a building by deflecting sunlight which is attached to an external wall. </ul>
A solar panel attached to an external wall."""@en .

:c_cb3d4c10 a skos:Concept .

:c_727adfdb a skos:Concept;
  skos:prefLabel "storey exit"@en .

:c_13543964 dct:modified "2019-12-21T06:27:12.116Z"^^xsd:dateTime .

:c_a4eaf123 dct:modified "2019-12-21T07:22:01.421Z"^^xsd:dateTime .

:xl_en_310fdd79 a skosxl:Label;
  skosxl:literalForm "sap"@en .

:c_c02d4d7d dct:modified "2019-12-28T07:15:27.051Z"^^xsd:dateTime;
  rdfs:isDefinedBy <http://www.legislation.gov.uk/uksi/2010/2214/regulation/2> .

:xl_en_76bd2153 a skosxl:Label;
  skosxl:literalForm """2.1.1
"""@en .

:c_b975b2d2 dc:source :c_6c82c09f .

:c_da6168d8 rdfs:isDefinedBy <http://www.legislation.gov.uk/uksi/2010/2214/regulation/2> .

:xl_en_b9ef8f0c a skosxl:Label;
  skosxl:literalForm "part r - physical infrastructure for high speed electronic communications networks"@en .

:c_7400b440 a skos:Concept;
  skos:prefLabel "purpose group"@en .

:c_06f29df7 a skos:Concept;
  dct:created "2018-03-28T19:12:00.921Z"^^xsd:dateTime;
  skos:inScheme :conceptScheme_751925ed;
  skos:prefLabel "regulation 7 - materials and workmanship"@en;
  skosxl:prefLabel :xl_en_f65b5e23 .

:c_502a871c a skos:Concept;
  dct:created "2018-03-28T19:04:56.970Z"^^xsd:dateTime;
  skos:inScheme :conceptScheme_751925ed;
  skos:topConceptOf :conceptScheme_751925ed;
  skosxl:prefLabel :xl_en_d2f47531 .

:c_f851b292 skos:prefLabel "habitable room"@en .

:c_86cfaae6 a skos:Concept;
  dct:created "2020-10-19T16:31:48.703Z"^^xsd:dateTime;
  skos:broader :c_f9b32acf;
  skos:inScheme :conceptScheme_751925ed;
  skos:narrower :c_9d708081;
  skos:prefLabel "building regulations 2010"@en .

:c_d10595f3 skos:inScheme :conceptScheme_751925ed .

:c_90aedbdc skos:narrower :c_e47ea7fb .

:c_76c8b363 skos:inScheme :conceptScheme_751925ed;
  skos:prefLabel "extract ventilation"@en .

:c_59a3ae21 skos:narrower :c_4d4c50dd, :c_eeea044b, :c_f851b292 .

:c_4fe84b3b skos:inScheme :conceptScheme_751925ed .

:c_feba40b2 dct:created "2020-10-23T17:02:27.325Z"^^xsd:dateTime .

:xl_en_f65b5e23 a skosxl:Label;
  skosxl:literalForm "regulation 7 - materials and workmanship"@en .

:c_13911a49 a skos:Concept;
  dct:created "2019-11-30T11:56:26.982Z"^^xsd:dateTime;
  rdfs:isDefinedBy :c_f9b32acf;
  skos:narrower :c_132d79ca, :c_1f1f7725, :c_34f295d5, :c_35d3a535, :c_38ba0f99, :c_3e5063e6,
    :c_40560ccd, :c_46be855e, :c_da6168d8, :c_f4139893;
  skos:note "NOTE: Except for the items marked * (which are from the Building Regulations 2010), these definitions apply only to Approved Document B.<p>NOTE: The terms defined below are key terms used in this document only. Refer to BS 4422 for further guidance on the definitions of common terms used in the fire safety industry which are not listed below.</p>"@en .

:xl_en_45e6bbda skosxl:literalForm "construct spec"@en .

:c_f70bb786 dct:modified "2019-12-12T21:17:46.146Z"^^xsd:dateTime .

:c_9b7f9eb7 skos:prefLabel "firefighting lift"@en .

:xl_en_ca2d0e57 a skosxl:Label .

:c_858351ef a skos:Concept;
  dc:source :c_6c82c09f, :c_ca00c020;
  dct:modified "2019-12-15T08:34:09.479Z"^^xsd:dateTime;
  skos:definition "A boundary presumed to exist between two buildings on the same site."@en;
  skos:prefLabel "notional boundary"@en .

:c_10ea4ecc dc:source :c_ca00c020 .

:c_b3f65603 dc:source :c_ca00c020 .

:c_056e5a0a dc:source :c_ca00c020 .

:c_0e0d001c a skos:Concept;
  dct:created "2018-03-29T10:47:59.314Z"^^xsd:dateTime;
  skos:definition "This Order reforms the law relating to fire safety in non-domestic premises. It replaces fire certification under the Fire Precautions Act 1971 with a general duty to ensure, so far as is reasonably practicable, the safety of employees, a general duty, in relation to non-employees to take such fire precautions as may reasonably be required in the circumstances to ensure that premises are safe and a duty to carry out a risk assessment."@en;
  skos:inScheme :conceptScheme_751925ed;
  skos:prefLabel "regulatory reform (fire safety) order 2005"@en;
  skos:related :c_d4480e31;
  skosxl:prefLabel :xl_en_a359d04b .

:c_851c02b0 skos:prefLabel "traffic route"@en .

:c_9d708081 skos:broader :c_86cfaae6 .

:c_e756ef49 a skos:Concept;
  skos:broader :c_75f7c82b;
  skos:definition " includes any mobile work equipment work equipment means any machinery, appliance, apparatus, tool or installation for use at work (whether exclusively or not)"@en;
  skos:notation "uksi 2015 51"@en;
  skos:prefLabel "vehicle"@en .

:c_139d3767 a skos:Concept;
  skos:broader :c_75f7c82b;
  skos:definition " means any day on which construction work takes place workplace means a workplace within the meaning of regulation 2(1) of the Workplace (Health, Safety and Welfare) Regulations 1992(a) other than a construction site. (2) Any reference in these Regulations to a plan, rule, document, report or copy includes a copy or electronic version which is(a)"@en;
  skos:notation "uksi 2015 51"@en;
  skos:prefLabel "working day"@en .

:c_1e8a7cbf skos:inScheme :conceptScheme_751925ed .

:c_c31ddac5 skos:inScheme :conceptScheme_751925ed .

:c_d4480e31 a skos:Concept;
  dc:source "Building a Safer Future – Independent Review of Building Regulations and Fire Safety: Final Report"@en;
  dct:created "2018-03-28T19:09:47.835Z"^^xsd:dateTime;
  skos:broader :c_502a871c;
  skos:definition "Guidance on ways to comply with the fire safety requirements in Part B of Schedule 1 to the Building Regulations 2010"@en;
  skos:inScheme :conceptScheme_751925ed;
  skos:prefLabel "part b - fire safety"@en .

:c_0a3a129e skos:narrower :c_17ac084f, :c_9480d322, :c_968e7c1f .

:c_ef1c9d78 skos:inScheme :conceptScheme_751925ed .

:c_c07e16c5 skos:inScheme :conceptScheme_751925ed .

:xl_en_a359d04b a skosxl:Label;
  skosxl:literalForm "regulatory reform (fire safety) order 2005"@en .

:c_6b24d6e2 a skos:Concept;
  dct:created "2018-03-29T10:24:41.329Z"^^xsd:dateTime;
  rdfs:isDefinedBy <http://www.legislation.gov.uk/uksi/2010/2214/part/9/made>;
  skos:broader :c_86cfaae6;
  skos:inScheme :conceptScheme_751925ed;
  skos:notation "part 09"@en;
  skos:prefLabel "testing and commissioning (building regulation)"@en;
  skosxl:prefLabel :xl_en_e99200e0 .


:xl_en_453bc190 a skosxl:Label;
  skosxl:literalForm """2.1.6
"""@en .

:xl_en_913b3693 a skosxl:Label .

:c_75ffd205 dct:created "2018-04-21T15:09:31.302Z"^^xsd:dateTime .

:xl_en_e99200e0 a skosxl:Label;
  skosxl:literalForm "testing and commissioning (building regulation)"@en .

:c_46be855e dct:created "2019-12-21T06:13:29.946Z"^^xsd:dateTime .

:xl_en_1445c137 a skosxl:Label;
  skosxl:literalForm "air tightness testing and measurement association certificate"@en .

:c_a4eaf123 dc:source :c_6c82c09f .

:c_79a3679f dct:modified "2019-12-13T23:33:59.692Z"^^xsd:dateTime .

:xl_en_1b847882 skosxl:literalForm "legal"@en .

:c_228ee3b0 skos:broader :c_13911a49;
  skos:inScheme :conceptScheme_751925ed .

:xl_en_80102184 skosxl:literalForm """2.1.10
"""@en .

:xl_en_ecb8813d skosxl:literalForm "health"@en .

:c_83464c52 dc:source :c_6c82c09f;
  dct:modified "2019-12-28T06:46:32.538Z"^^xsd:dateTime .

:c_58df2af5 skos:broader :c_86cfaae6;
  skos:note "Requirements Regulations 4 and 6"@en .



:c_61f82d61 a skos:Concept;
  dc:source :c_6c82c09f, :c_ca00c020 .

:c_533afc9b dct:created "2018-07-20T21:00:25.877Z"^^xsd:dateTime .

:c_132d79ca dct:created "2019-12-21T06:56:02.209Z"^^xsd:dateTime;
  skos:broader :c_13911a49 .

:c_10030a9a dct:modified "2019-12-13T23:33:58.982Z"^^xsd:dateTime;
  skos:broader :c_13911a49 .

:c_727adfdb dc:source :c_6c82c09f;
  skos:broader :c_13911a49;
  skos:inScheme :conceptScheme_751925ed .

:c_04c52352 dc:source :c_6c82c09f .

:c_7d862abe dc:source :c_6c82c09f .

:c_c1a78f4b dc:source :c_6c82c09f .

:c_40560ccd a skos:Concept;
  dct:created "2019-12-21T06:48:21.375Z"^^xsd:dateTime;
  skos:broader :c_13911a49;
  skos:inScheme :conceptScheme_751925ed;
  skos:prefLabel "sheltered housing"@en .

:c_35d3a535 dct:created "2019-12-15T08:39:34.693Z"^^xsd:dateTime .

:c_13543964 a skos:Concept;
  skos:inScheme :conceptScheme_751925ed;
  skos:prefLabel "protected entrance hall/landing"@en .

:c_f97db0fd skos:inScheme :conceptScheme_751925ed .

:c_5918929b skos:inScheme :conceptScheme_751925ed .

:c_1dfadb92 skos:inScheme :conceptScheme_751925ed .

:c_3cae7829 dct:modified "2019-12-14T08:48:46.738Z"^^xsd:dateTime .

:xl_en_0049082b a skosxl:Label;
  skosxl:literalForm "bass"@en .

:c_b975b2d2 a skos:Concept;
  dct:created "2019-12-21T07:15:28.445Z"^^xsd:dateTime;
  skos:broader :c_13911a49;
  skos:inScheme :conceptScheme_751925ed;
  skos:prefLabel "thermoplastic material"@en .

:c_cb86c2ff dc:source :c_ca00c020 .


:c_5ef03467 dc:source :c_ca00c020 .

:skosCollection_42952ecf dct:created "2018-08-11T08:35:23.556Z"^^xsd:dateTime .

:c_9a0f5e20 dc:source :c_6c82c09f;
  dct:modified "2019-12-14T08:48:46.832Z"^^xsd:dateTime .

:c_88af4873 dc:source :c_6c82c09f;
  skos:notation "B2"@en .

:c_c02d4d7d a skos:Concept;
  skos:inScheme :conceptScheme_751925ed;
  skos:prefLabel "building"@en .

:c_5724a233 dc:source :c_6c82c09f .

:c_56fef4b5 skos:broader :c_13911a49 .

:xl_en_6cb57c20 a skosxl:Label;
  skosxl:literalForm """2.1.3
"""@en .

:xl_en_91bd8550 a skosxl:Label .

:c_e162c613 dct:created "2018-05-26T11:01:47.267Z"^^xsd:dateTime .

:xl_en_c14ad7c7 a skosxl:Label;
  skosxl:literalForm "part c - site preparation and resistance to contaminates and moisture"@en .

:c_da6168d8 a skos:Concept;
  skos:definition "Includes a dwellinghouse and a flat."@en;
  skos:inScheme :conceptScheme_751925ed;
  skos:prefLabel "dwelling"@en .

:c_9b7f9eb7 dc:source :c_ca00c020;
  skos:notation "B1"@en .

:c_b2cab8d9 dc:source :c_ca00c020;
  skos:definition "The maximum aggregate plan perimeter, found by vertical projection onto a horizontal plane. (See Section 15 of Approved Document B Volume 2.)"@en .

:c_a965ecce dc:source :c_6c82c09f;
  dct:modified "2019-12-28T06:46:06.436Z"^^xsd:dateTime;
  skos:notation "B2"@en .

:c_b0f3b4fb a skos:Concept;
  dc:source :c_ca00c020;
  skos:notation "B1"@en .

:c_34f295d5 a skos:Concept;
  dct:created "2019-12-12T20:41:01.583Z"^^xsd:dateTime;
  dct:modified "2019-12-28T07:19:31.525Z"^^xsd:dateTime;
  skos:broader :c_13911a49;
  skos:inScheme :conceptScheme_751925ed;
  skos:notation "*B1"@en .

:c_858351ef dct:created "2019-12-15T08:31:59.287Z"^^xsd:dateTime;
  skos:broader :c_13911a49;
  skos:inScheme :conceptScheme_751925ed .

:xl_en_44ca1675 a skosxl:Label .

:xl_en_3c41ea90 a skosxl:Label;
  skosxl:literalForm "lod"@en .

:xl_en_cff63d0f a skosxl:Label .

:c_6284471b dc:source :c_6c82c09f;
  skos:prefLabel "automatic release mechanism"@en .

:c_8258611b dc:source :c_ca00c020;
  skos:prefLabel "atrium (plural atria)"@en .

:xl_en_fd21eb9e a skosxl:Label;
  skosxl:literalForm """2.1.2
"""@en .

:c_3e5063e6 skos:broader :c_13911a49 .

:c_06f29df7 dct:modified "2020-11-04T19:45:22.646Z"^^xsd:dateTime;
  skos:notation "uksi 2010 2214"@en .

:c_75f7c82b skos:narrower :c_2f92acaa, :c_9d2dac79 .

:xl_en_f2eee9b5 skosxl:literalForm "cde"@en .

:c_33c0e1b5 a skos:Concept .

:xl_en_0a7cb84d a skosxl:Label;
  skosxl:literalForm "midp"@en .

:c_d4480e31 skos:narrower :c_ca00c020 .

:c_bed063fd dc:source :c_ca00c020 .

:c_38ba0f99 dct:modified "2019-12-15T08:46:58.872Z"^^xsd:dateTime;
  skos:definition "(also called an access or raised floor) A floor that is supported by a structural floor, but with an intervening cavity to house services."@en .

:conceptScheme_751925ed dc:description "Scope of controlled vocabulary to follow"@en .

:c_14b52896 dc:source :c_6c82c09f, :c_ca00c020;
  dct:modified "2019-12-14T08:48:46.962Z"^^xsd:dateTime .

:xl_en_1b847882 a skosxl:Label .

:c_7804ad6c dc:source :c_6c82c09f;
  dct:modified "2019-12-14T08:48:47.639Z"^^xsd:dateTime .

:c_59a3ae21 skos:narrower :c_830012c2 .

:c_d5c15327 a skos:Concept .

:xl_en_d1eea4cb a skosxl:Label;
  skosxl:literalForm "cml"@en .

:xl_en_7274bb0f a skosxl:Label;
  skosxl:literalForm "pim"@en .

:xl_en_24febe8b a skosxl:Label;
  skosxl:literalForm """2.1.9
"""@en .

:c_7400b440 skos:inScheme :conceptScheme_751925ed .

:c_1a6e1e92 a skos:Concept;
  dct:created "2018-03-28T19:10:14.402Z"^^xsd:dateTime;
  skos:inScheme :conceptScheme_751925ed;
  skos:prefLabel "part e - resistance to the passage of sound"@en;
  skosxl:prefLabel :xl_en_1fd9fca8 .

:c_8cba3c82 dct:modified "2020-10-23T17:08:13.914Z"^^xsd:dateTime;
  skos:broader :c_502a871c .

:xl_en_1fd9fca8 a skosxl:Label;
  skosxl:literalForm "part e - resistance to the passage of sound"@en .

:c_f4139893 dct:modified "2019-12-28T06:54:53.684Z"^^xsd:dateTime;
  rdfs:isDefinedBy <http://www.legislation.gov.uk/ukpga/1996/56/section/4>;
  rdfs:seeAlso <http://www.legislation.gov.uk/ukpga/1996/56/section/4> .

:xl_en_1ec12f25 a skosxl:Label .

:c_1b060096 a skos:Concept;
  dct:created "2018-03-28T19:09:39.123Z"^^xsd:dateTime;
  dct:modified "2020-10-23T17:06:18.179Z"^^xsd:dateTime;
  skos:broader :c_502a871c;
  skos:inScheme :conceptScheme_751925ed;
  skos:prefLabel "part a - structure"@en .

:c_0a3a129e skos:narrower :c_58b42d76, :c_6f581d4d, :c_a7557993, :c_da334512 .

:c_9e4931f7 a skos:Concept;
  dct:created "2019-12-13T23:09:23.909Z"^^xsd:dateTime;
  skos:broader :c_13911a49;
  skos:inScheme :conceptScheme_751925ed;
  skos:prefLabel "cavity barrier"@en .

:c_13911a49 skos:narrower :c_33c0e1b5, :c_56fef4b5, :c_83464c52, :c_9b7f9eb7, :c_9e4931f7;
  skos:broader :c_ca00c020;
  skos:inScheme :conceptScheme_751925ed;
  skos:narrower :c_04c52352, :c_13543964, :c_228ee3b0, :c_727adfdb, :c_b0f3b4fb, :c_b6083e42,
    :c_bed063fd, :c_f5536b7d, :c_f70bb786;
  skos:prefLabel "appendix a: key terms"@en .

:c_c02d4d7d skos:notation "*"@en .

:c_83464c52 a skos:Concept;
  skos:broader :c_13911a49;
  skos:definition "(unless otherwise specified, e.g. as in the case of flats) The distance that a person would travel from any point within the floor area to the nearest storey exit, determined by the layout of walls, partitions and fittings."@en;
  skos:notation "B2"@en;
  skos:prefLabel "travel distance"@en .

<http://buildvoc.co.uk/resource/> owl:imports <http://www.w3.org/ns/dcat> .

:c_52aaa84e dct:created "2018-07-24T17:09:26.522Z"^^xsd:dateTime .

:c_277602e6 dct:created "2018-08-11T09:08:09.653Z"^^xsd:dateTime .

:c_4a90e0e1 dc:source :c_ca00c020 .

:c_7d862abe skos:note "NOTE: If the door is in a cavity barrier, rising butt hinges (which are different from the self-closing device mentioned above) are acceptable."@en .

:xl_en_ca2d0e57 skosxl:literalForm "bep"@en .

:xl_en_8715993d a skosxl:Label .

:c_5ef03467 dc:source :c_6c82c09f;
  dct:modified "2019-12-13T23:33:58.622Z"^^xsd:dateTime;
  skos:definition "One of two or more exits, each of which is separate from the other."@en .

:c_04c52352 a skos:Concept;
  dct:created "2019-12-21T06:34:39.568Z"^^xsd:dateTime;
  skos:broader :c_13911a49;
  skos:inScheme :conceptScheme_751925ed;
  skos:prefLabel "separated part"@en .

:c_dc99fe05 dct:created "2018-04-07T19:42:55.911Z"^^xsd:dateTime .

:c_b44f46e0 a skos:Concept;
  dc:source :c_6c82c09f;
  dct:modified "2019-12-21T07:22:01.754Z"^^xsd:dateTime .

:c_da6168d8 skos:note "NOTE: A dwelling is a unit where one or more people live (whether or not as a sole or main residence) in either of the following situations.<ul><li> A single person or people living together as a family.<li> A maximum of six people living together as a single household, including where care is provided for residents.</ul>"@en .

:c_13543964 dct:created "2019-12-21T06:12:19.585Z"^^xsd:dateTime;
  skos:broader :c_13911a49 .

:c_132d79ca dct:modified "2019-12-21T07:22:01.802Z"^^xsd:dateTime;
  skos:definition """ 
(of a building) The land occupied by the building, up to the boundaries with land in other ownership."""@en .

:c_b304ed8a dct:modified "2019-12-28T07:20:58.374Z"^^xsd:dateTime;
  rdfs:isDefinedBy <http://www.legislation.gov.uk/uksi/2010/2214/regulation/2> .



:c_b4ccd5f2 rdfs:isDefinedBy <http://www.legislation.gov.uk/uksi/2010/2214/regulation/2> .

:xl_en_6bbf3d9b a skosxl:Label;
  skosxl:literalForm "part d - toxic substances"@en .

:c_10ea4ecc dc:source :c_6c82c09f .

:c_b3f65603 dc:source :c_6c82c09f .

:c_56fef4b5 dct:created "2019-12-21T07:19:11.868Z"^^xsd:dateTime;
  skos:definition """(in relation to a side or external wall of a building) All of the following are classed as unprotected areas.
<ul><li>Any part of the external wall that has less than the relevant fire resistance set out in Section 13.
<li>  Any part of the external wall constructed of material more than 1mm thick if that material does not have a class B-s3, d2 rating or better, which is attached or applied, whether for cladding or any other purpose. 
<li>  Windows, doors or other openings. This does not include windows that are designed and glazed to give the necessary level of fire resistance and that are not openable.</ul>"""@en .

:c_28013078 a skos:Concept;
  dc:source :c_ca00c020;
  skos:inScheme :conceptScheme_751925ed .

:xl_en_400b0017 a skosxl:Label .

:c_34f295d5 dc:source :c_ca00c020;
  skos:definition "Includes a dwellinghouse and a flat."@en;
  skos:note "NOTE: A dwelling is a unit where one or more people live (whether or not as a sole or main residence) in either of the following situations.<ul><li> A single person or people living together as a family.<li> A maximum of six people living together as a single household, including where care is provided for residents.</ul>"@en .

:c_9b7f9eb7 skos:definition "A lift with additional protection and with controls that enable it to be used by the fire and rescue service when fighting a fire. (See Section 15.)"@en .

:c_88af4873 dct:modified "2019-12-28T06:44:59.815Z"^^xsd:dateTime .

:c_b2cab8d9 dct:created "2019-12-12T20:47:12.799Z"^^xsd:dateTime;
  dct:modified "2019-12-13T22:39:26.964Z"^^xsd:dateTime;
  skos:broader :c_13911a49;
  skos:notation "B1"@en .

:c_9d708081 dct:modified "2020-11-04T18:00:52.757Z"^^xsd:dateTime;
  skos:notation "uksi 2010 2214"@en .

:c_a965ecce a skos:Concept;
  dct:created "2019-12-12T20:47:00.103Z"^^xsd:dateTime;
  skos:broader :c_13911a49;
  skos:definition "The maximum aggregate plan perimeter, found by vertical projection onto a horizontal plane. (See Section 15.)"@en;
  skos:inScheme :conceptScheme_751925ed;
  skos:prefLabel "perimeter (of a building)"@en .

:c_be34e7b3 dc:source :c_6c82c09f .

:c_8258611b skos:note "NOTE: Enclosed lift wells, enclosed escalator wells, building services ducts and stairs are not classified as atria."@en .

:xl_en_44ca1675 skosxl:literalForm "aim"@en .

:xl_en_3e905d0b a skosxl:Label;
  skosxl:literalForm "part k - protection from falling, collision and impact"@en .

:c_f5536b7d dc:source :c_ca00c020;
  dct:created "2019-12-13T23:11:41.791Z"^^xsd:dateTime;
  skos:broader :c_13911a49;
  skos:inScheme :conceptScheme_751925ed;
  skos:prefLabel "ceiling"@en .

:c_7fc5469b dct:created "2019-12-13T23:07:38.815Z"^^xsd:dateTime;
  skos:broader :c_13911a49 .

:c_b0f3b4fb dct:created "2019-12-12T20:50:36.136Z"^^xsd:dateTime;
  dct:modified "2019-12-13T22:42:18.989Z"^^xsd:dateTime;
  skos:broader :c_13911a49;
  skos:inScheme :conceptScheme_751925ed .

:c_33c0e1b5 dct:created "2019-12-13T23:16:16.374Z"^^xsd:dateTime;
  dct:modified "2019-12-13T23:33:59.393Z"^^xsd:dateTime;
  skos:broader :c_13911a49;
  skos:definition "A walkway, open to the air on one or more sides, that forms part of the escape route from more than one flat."@en .

:c_bed063fd a skos:Concept;
  dct:created "2019-12-13T23:17:32.193Z"^^xsd:dateTime;
  dct:modified "2020-10-26T07:33:12.073Z"^^xsd:dateTime;
  skos:definition "An escape stair that serves more than one flat."@en;
  skos:prefLabel "common stair"@en .

:xl_en_f259c22d a skosxl:Label;
  skosxl:literalForm "part j - combustion appliances and fuel storage systems"@en .

:xl_en_718751b0 a skosxl:Label;
  skosxl:literalForm """2.1.8
"""@en .

:c_6284471b dc:source :c_ca00c020 .

:c_3e5063e6 a skos:Concept;
  dc:source :c_ca00c020;
  dct:created "2019-12-13T23:02:15.181Z"^^xsd:dateTime;
  dct:modified "2019-12-13T23:33:58.928Z"^^xsd:dateTime .

:c_727adfdb dct:created "2019-12-21T07:12:19.397Z"^^xsd:dateTime;
  skos:definition "A final exit, or a doorway that gives direct access into a protected stairway, firefighting lobby or external escape route."@en .

:xl_en_0460024f a skosxl:Label;
  skosxl:literalForm "part l - conservation of fuel and power"@en .

:c_b6083e42 a skos:Concept;
  dc:source :c_ca00c020;
  dct:created "2019-11-30T12:49:44.067Z"^^xsd:dateTime;
  dct:isPartOf :c_6c82c09f, :c_ca00c020;
  skos:broader :c_13911a49;
  skos:definition "Escape routes that are sufficiently separated by direction and space or by fire resisting construction to ensure that one is still available if the other is affected by fire."@en;
  skos:inScheme :conceptScheme_751925ed;
  skos:prefLabel "alternative escape routes"@en;
  skos:scopeNote "NOTE: A second stair, balcony or flat roof which enables a person to reach a place free from danger from fire is considered an alternative escape route for the purposes of a dwellinghouse."@en .

:c_10030a9a a skos:Concept;
  dc:source :c_6c82c09f, :c_ca00c020;
  skos:prefLabel "boundary"@en .

:c_c02d4d7d dc:source :c_6c82c09f, :c_ca00c020;
  skos:broader :c_13911a49;
  skos:definition "Any permanent or temporary building but not any other kind of structure or erection. A reference to a building includes a reference to part of a building."@en .

:xl_en_913b3693 skosxl:literalForm "plqs"@en .

:xl_en_1ec12f25 skosxl:literalForm "oir"@en .

:c_4a90e0e1 a skos:Concept;
  dc:source :c_6c82c09f;
  dct:modified "2019-12-13T23:33:59.592Z"^^xsd:dateTime;
  skos:broader :c_13911a49;
  skos:inScheme :conceptScheme_751925ed;
  skos:note "NOTE: A roof space above the top storey of a compartment is included in that compartment. (See also ‘Separated part’.)"@en;
  skos:prefLabel "compartment (fire)"@en .

:c_b44f46e0 dct:created "2019-12-21T06:58:14.334Z"^^xsd:dateTime;
  skos:broader :c_13911a49;
  skos:inScheme :conceptScheme_751925ed .

:xl_en_f987d3fd a skosxl:Label;
  skosxl:literalForm "smp"@en .

:xl_en_e99200e0 dct:modified "2018-07-20T21:02:30.704Z"^^xsd:dateTime .

:c_47c790ae dc:source :c_6c82c09f .

:c_f70bb786 a skos:Concept .

:c_04c52352 dct:modified "2019-12-21T06:40:53.009Z"^^xsd:dateTime;
  skos:definition "(of a building) Part of a building that is separated from another part of the same building by a compartment wall. The wall runs the full height of the part and is in one vertical plane. (See Appendix D, Diagram D5.)"@en .

:c_4cdc3b72 dct:created "2019-11-30T13:35:56.186Z"^^xsd:dateTime;
  dct:isPartOf :c_ca00c020;
  dct:modified "2019-12-12T21:17:12.203Z"^^xsd:dateTime;
  dct:source :c_ca00c020;
  skos:broader :c_13911a49;
  skos:definition "A fire resisting wall or floor to separate one fire compartment from another."@en;
  skos:inScheme :conceptScheme_751925ed;
  skos:notation "B1"@en;
  skos:note " NOTE: Provisions relating to construction are given in Section 7."@en .

<http://buildvoc.co.uk/resource/> owl:imports <http://purl.org/dc/elements/1.1/> .

:c_5db451a3 dc:source "https://www.rics.org/globalassets/rics-website/media/upholding-professional-standards/sector-standards/construction/nrm-1-order-of-cost-estimating-and-cost-planning-2nd-edition-rics.pdf"@en .

:c_228ee3b0 dc:source :c_6c82c09f, :c_ca00c020;
  dct:isPartOf :c_6c82c09f, :c_ca00c020 .

:c_79a3679f dc:source :c_ca00c020 .

:c_ca00c020 skos:exactMatch <http://www.worldcat.org/oclc/1120217476> .

:c_58df2af5 a skos:Concept;
  dct:modified "2020-11-04T19:50:21.107Z"^^xsd:dateTime;
  skos:notation "uksi 2010 2214"@en;
  skos:prefLabel "schedule 1"@en .

:c_2a34c0b8 a skos:Concept;
  dct:created "2018-03-28T19:11:31.113Z"^^xsd:dateTime;
  skos:inScheme :conceptScheme_751925ed;
  skos:prefLabel "part p - electrical safety"@en;
  skosxl:prefLabel :xl_en_2a32cf6f .

:c_1a6e1e92 dct:modified "2020-10-23T17:08:24.565Z"^^xsd:dateTime;
  skos:broader :c_502a871c .

:xl_en_2a32cf6f a skosxl:Label;
  skosxl:literalForm "part p - electrical safety"@en .

:c_b4ccd5f2 dct:modified "2019-12-28T07:24:42.666Z"^^xsd:dateTime .

:c_d5c15327 skos:inScheme :conceptScheme_751925ed;
  skos:prefLabel "protected circuit"@en .

:c_75f7c82b skos:narrower :c_a4cdd233 .

:xl_en_80102184 a skosxl:Label .

:xl_en_74ce780a a skosxl:Label;
  skosxl:literalForm """2
"""@en .

:conceptScheme_751925ed dc:contributor """HM Government
"""@en .

:c_2ca1576c a skos:Concept;
  dct:created "2018-03-28T19:10:21.168Z"^^xsd:dateTime;
  skos:broader :c_502a871c;
  skos:inScheme :conceptScheme_751925ed;
  skos:prefLabel "part f - ventilation"@en;
  skosxl:prefLabel :xl_en_a94d8a2b .

:c_62cc4d78 skos:broader :c_59a3ae21 .

:xl_en_a94d8a2b a skosxl:Label;
  skosxl:literalForm "part f - ventilation"@en .

:c_46be855e a skos:Concept;
  skos:definition "A shaft that enables people, air or objects to pass from one compartment to another, and which is enclosed with fire resisting construction."@en;
  skos:inScheme :conceptScheme_751925ed;
  skos:prefLabel "protected shaft"@en .

:c_40560ccd dct:modified "2019-12-21T06:53:32.043Z"^^xsd:dateTime;
  skos:definition "Includes two or more dwellings in the same building or on adjacent sites, designed and constructed as residential accommodation for vulnerable or elderly people who receive, or will receive, a support service."@en .

:c_28013078 dc:source :c_6c82c09f;
  dct:created "2019-12-13T23:06:17.075Z"^^xsd:dateTime;
  dct:modified "2020-10-25T07:07:36.633Z"^^xsd:dateTime;
  skos:broader :c_13911a49;
  skos:definition "A term that includes both local authority building control and approved inspectors."@en;
  skos:prefLabel "building control body (tba)"@en .

:c_7fc5469b a skos:Concept;
  dc:source :c_6c82c09f, :c_ca00c020;
  dct:modified "2019-12-13T23:33:59.168Z"^^xsd:dateTime .

:c_9e4931f7 dc:source :c_6c82c09f;
  skos:definition "A construction within a cavity, other than a smoke curtain, to perform either of the following functions.<ul><li>Close a cavity to stop smoke or flame entering.<li>Restrict the movement of smoke or flame within a cavity.</ul>"@en .

:c_f5536b7d dc:source :c_6c82c09f;
  skos:definition "Part of a building that encloses a room, protected shaft or circulation space and is exposed overhead. "@en .

:c_e7e6b110 dc:source :c_6c82c09f;
  skos:prefLabel "circulation space"@en .

:c_33c0e1b5 dc:source :c_6c82c09f .

:c_bed063fd dc:source :c_6c82c09f;
  skos:broader :c_13911a49 .

:c_13911a49 skos:broader :c_6c82c09f;
  skos:narrower :c_10030a9a, :c_28013078, :c_28e7c922, :c_4a90e0e1, :c_5724a233, :c_5ef03467,
    :c_79a3679f, :c_7fc5469b, :c_88af4873, :c_a965ecce, :c_b44f46e0, :c_b975b2d2, :c_c02d4d7d .



:xl_en_2de5ebbe skosxl:literalForm "sb-imp"@en .

:c_cb3d4c10 dc:source :c_6c82c09f .

:c_7c12f560 a skos:Concept;
  skos:broader :c_13911a49;
  skos:inScheme :conceptScheme_751925ed;
  skos:prefLabel "protected stairway"@en .

:xl_en_8c98a903 a skosxl:Label;
  skosxl:literalForm """2.1.11
"""@en .

:c_b975b2d2 skos:definition "Any synthetic polymeric material that has a softening point below 200°C if tested to BS EN ISO 306 Method A120. Specimens for this test may be fabricated from the original polymer where the thickness of material of the end product is less than 2.5mm."@en .

:c_13543964 skos:definition "A circulation area, consisting of a hall or space in a flat, that is enclosed with fire resisting construction other than an external wall of a building."@en .

:c_3e5063e6 dc:source :c_6c82c09f;
  skos:prefLabel "basement storey"@en .

:c_b65b6f3f dct:created "2018-07-22T13:43:09.626Z"^^xsd:dateTime .

:c_6c82c09f skos:example <https://assets.publishing.service.gov.uk/government/uploads/system/uploads/attachment_data/file/832633/Approved_Document_B__fire_safety__volume_2_-_2019_edition.pdf> .

:c_706598d3 dc:source :c_6c82c09f .

:c_c02d4d7d dct:created "2019-12-13T23:04:41.568Z"^^xsd:dateTime .

:c_7b85eda3 dc:source :c_ca00c020 .

:c_10030a9a dct:created "2019-12-13T23:03:38.460Z"^^xsd:dateTime;
  skos:definition "The boundary of the land that belongs to a building, or, where the land abuts a road, railway, canal or river, the centre line of that road, railway, canal or river."@en;
  skos:inScheme :conceptScheme_751925ed .

:xl_en_ecb8813d a skosxl:Label .

:skosCollection_4ff8449c dct:created "2018-04-07T20:06:25.388Z"^^xsd:dateTime .

:c_0a3a129e skos:narrower :c_aab41011 .

:c_b2cab8d9 a skos:Concept;
  skos:prefLabel "perimeter (of a building)"@en .

:xl_en_74b321d9 skosxl:literalForm "pip"@en .

:c_b0f3b4fb skos:definition "(unless otherwise specified, e.g. as in the case of flats) The distance that a person would travel from any point within the floor area to the nearest storey exit, determined by the layout of walls, partitions and fittings."@en .

:c_34f295d5 rdfs:seeAlso <http://www.legislation.gov.uk/uksi/2010/2214/regulation/2>;
  skos:editorialNote "NOTE: Except for the items marked * (which are from the Building Regulations 2010), these definitions apply only to Approved Document B.<p>NOTE: The terms defined below are key terms used in this document only. Refer to BS 4422 for further guidance on the definitions of common terms used in the fire safety industry which are not listed below.</p>"@en .

:c_da6168d8 skos:editorialNote "NOTE: Except for the items marked * (which are from the Building Regulations 2010), these definitions apply only to Approved Document B.<p>NOTE: The terms defined below are key terms used in this document only. Refer to BS 4422 for further guidance on the definitions of common terms used in the fire safety industry which are not listed below.</p>"@en;
  skos:notation "*B2"@en .

:c_f70bb786 dct:created "2019-12-12T20:17:42.317Z"^^xsd:dateTime;
  skos:broader :c_13911a49;
  skos:definition "A fire resisting wall or floor to separate one fire compartment from another."@en;
  skos:exactMatch :c_4cdc3b72;
  skos:inScheme :conceptScheme_751925ed;
  skos:notation "B2"@en;
  skos:note "NOTE: Provisions relating to construction are given in Section 8."@en;
  skos:prefLabel "compartment wall or floor"@en .

:xl_en_d34f5762 skosxl:literalForm "P"@en .

:c_28e7c922 a skos:Concept;
  dct:created "2019-12-15T08:40:53.169Z"^^xsd:dateTime;
  dct:modified "2019-12-15T08:46:58.969Z"^^xsd:dateTime;
  skos:broader :c_13911a49;
  skos:definition """A room such as any of the following.
<ul><li>Oil-filled transformer room.
<li>Switch gear room.
<li>Boiler room.
<li>Storage space for fuel or other highly flammable substance(s).
<li>Room that houses a fixed internal combustion engine.</ul>"""@en;
  skos:inScheme :conceptScheme_751925ed;
  skos:prefLabel "place of special fire hazard"@en .

:c_38ba0f99 a skos:Concept;
  skos:inScheme :conceptScheme_751925ed;
  skos:prefLabel "platform floor"@en .

:xl_en_511d9a71 a skosxl:Label;
  skosxl:literalForm "basmp"@en .

:c_6cbca36f dct:created "2018-08-20T10:00:12.829Z"^^xsd:dateTime .

:xl_en_32357ece a skosxl:Label .

:c_4fe84b3b skos:prefLabel "gross internal volume"@en .

:c_7a2d826e dc:source :c_6c82c09f .

:xl_en_f38b7b49 a skosxl:Label;
  skosxl:literalForm """2.1.7
"""@en .

:xl_en_9717bf9a a skosxl:Label;
  skosxl:literalForm "plans"@en .

:c_04c52352 dc:source :c_ca00c020 .

:xl_en_cff63d0f skosxl:literalForm "tidp"@en .

:xl_en_7699a05e a skosxl:Label;
  skosxl:literalForm "part g - sanitation, hot water safety and water efficiency"@en .

:c_79a3679f a skos:Concept;
  dct:created "2019-12-13T23:25:23.779Z"^^xsd:dateTime;
  skos:broader :c_13911a49;
  skos:definition "A design of a building containing flats, in which each flat is approached via a common horizontal internal access or circulation space, which may include a common entrance hall."@en;
  skos:inScheme :conceptScheme_751925ed;
  skos:prefLabel "corridor access"@en .

:c_228ee3b0 dct:modified "2020-10-26T07:27:03.595Z"^^xsd:dateTime .

:c_b44f46e0 skos:editorialNote "NOTE: Except for the items marked * (which are from the Building Regulations 2010), these definitions apply only to Approved Document B.<p>NOTE: The terms defined below are key terms used in this document only. Refer to BS 4422 for further guidance on the definitions of common terms used in the fire safety industry which are not listed below.</p>"@en;
  skos:notation "*"@en .

:c_5724a233 a skos:Concept;
  dct:created "2019-12-21T07:05:05.556Z"^^xsd:dateTime;
  skos:broader :c_13911a49;
  skos:definition """Includes any of the following.
<ul><li>Any gallery in an assembly building (purpose group 5).
<li>Any gallery in any other type of building if its area is more than half that of the space into which it projects.
<li>A roof, unless it is accessible only for maintenance and repair.</ul>"""@en;
  skos:inScheme :conceptScheme_751925ed;
  skos:note "NOTE: The building is regarded as a multi-storey building if both of the following apply.<ul><li>There is more than one gallery. <li>The total aggregate area of all the galleries in one space is more than half the floor area of that space.</ul>"@en;
  skos:prefLabel "storey"@en .

:c_42d467db a skos:Concept;
  dct:created "2018-03-28T19:10:37.917Z"^^xsd:dateTime;
  skos:broader :c_502a871c;
  skos:inScheme :conceptScheme_751925ed;
  skos:prefLabel "part h - drainage and waste disposal"@en;
  skosxl:prefLabel :xl_en_8587f86b .

:c_73c4361e a skos:Concept;
  dct:created "2018-03-28T19:10:28.620Z"^^xsd:dateTime;
  skos:broader :c_502a871c;
  skos:inScheme :conceptScheme_751925ed;
  skos:prefLabel "part g - sanitation, hot water safety and water efficiency"@en;
  skosxl:prefLabel :xl_en_7699a05e .

:c_44c61ce8 skos:prefLabel "ventilation 2010 edition incorporating 2010 and 2013 amendments"@en .

:xl_en_8587f86b a skosxl:Label;
  skosxl:literalForm "part h - drainage and waste disposal"@en .

:c_4cdc3b72 skos:exactMatch :c_f70bb786 .

:xl_en_1333d9a7 a skosxl:Label;
  skosxl:literalForm """2.1.6
"""@en .

:c_ee10273a dc:source :c_6c82c09f;
  dct:created "2019-12-21T06:21:43.979Z"^^xsd:dateTime;
  dct:modified "2019-12-21T06:27:11.530Z"^^xsd:dateTime;
  skos:broader :c_13911a49;
  skos:definition "The boundary or notional boundary that one side of the building faces and/or coincides with, and that is parallel or at an angle of a maximum of 80 degrees to that side of the building."@en .

:c_13911a49 skos:narrower :c_cc61a0f4, :c_e7e6b110, :c_ee10273a .

:c_cc61a0f4 a skos:Concept;
  dc:source :c_6c82c09f, :c_ca00c020;
  dct:created "2019-12-21T06:23:21.636Z"^^xsd:dateTime;
  skos:broader :c_13911a49;
  skos:definition "A dome light, lantern light, skylight, ridge light, glazed barrel vault or other element to admit daylight through a roof."@en;
  skos:inScheme :conceptScheme_751925ed;
  skos:prefLabel "rooflight"@en .

:c_83464c52 skos:inScheme :conceptScheme_751925ed .

:xl_en_400b0017 skosxl:literalForm "part m - access to and use of buildings"@en .

:c_88af4873 a skos:Concept;
  dct:created "2019-12-12T20:43:47.043Z"^^xsd:dateTime;
  skos:broader :c_13911a49;
  skos:definition "A lift with additional protection and with controls that enable it to be used by the fire and rescue service when fighting a fire. (See Section 17.)"@en;
  skos:inScheme :conceptScheme_751925ed;
  skos:prefLabel "firefighting lift"@en .

:c_9b7f9eb7 a skos:Concept;
  dct:created "2019-12-12T20:43:57.040Z"^^xsd:dateTime;
  skos:broader :c_13911a49;
  skos:inScheme :conceptScheme_751925ed .

:xl_en_8715993d skosxl:literalForm "cobie"@en .

:c_7c12f560 dc:source :c_6c82c09f;
  dct:modified "2019-12-21T06:27:11.881Z"^^xsd:dateTime .

:c_46be855e dc:source :c_6c82c09f, :c_ca00c020;
  dct:modified "2019-12-21T06:27:12.018Z"^^xsd:dateTime .

:c_13543964 dc:source :c_6c82c09f, :c_ca00c020 .

:c_7400b440 dc:source :c_6c82c09f, :c_ca00c020 .

:c_7b85eda3 dc:source :c_6c82c09f .

:xl_en_bdc8faa4 a skosxl:Label;
  skosxl:literalForm """2.1.5
"""@en .

:c_5ffbc967 a skos:Concept;
  dct:created "2018-03-28T19:11:39.728Z"^^xsd:dateTime;
  skos:broader :c_502a871c;
  skos:inScheme :conceptScheme_751925ed;
  skos:prefLabel "part q - security"@en;
  skosxl:prefLabel :xl_en_93b6dba8 .

:c_679215e0 dct:created "2020-10-25T05:17:58.202Z"^^xsd:dateTime .

:c_fec1533e a skos:Concept;
  dct:created "2018-03-28T19:10:47.855Z"^^xsd:dateTime;
  skos:broader :c_502a871c;
  skos:inScheme :conceptScheme_751925ed;
  skos:prefLabel "part j - combustion appliances and fuel storage systems"@en;
  skosxl:prefLabel :xl_en_f259c22d .

:c_152c4bbc skos:narrower :c_01839084 .

:c_8cba3c82 a skos:Concept;
  dct:created "2018-03-28T19:10:07.222Z"^^xsd:dateTime;
  skos:inScheme :conceptScheme_751925ed;
  skos:prefLabel "part d - toxic substances"@en;
  skosxl:prefLabel :xl_en_6bbf3d9b .

:c_b7bccf3d a skos:Concept;
  dct:created "2018-03-28T19:11:51.452Z"^^xsd:dateTime;
  skos:broader :c_502a871c;
  skos:inScheme :conceptScheme_751925ed;
  skos:prefLabel "part r - physical infrastructure for high speed electronic communications networks"@en;
  skosxl:prefLabel :xl_en_b9ef8f0c .

:c_0109c085 skos:inScheme :conceptScheme_751925ed .

:c_a20cbb62 a skos:Concept;
  dct:created "2018-03-28T19:11:17.122Z"^^xsd:dateTime;
  skos:broader :c_502a871c;
  skos:inScheme :conceptScheme_751925ed;
  skos:prefLabel "part m - access to and use of buildings"@en;
  skosxl:prefLabel :xl_en_400b0017 .

:c_be604dfa a skos:Concept;
  dct:created "2018-03-28T19:10:59.073Z"^^xsd:dateTime;
  skos:broader :c_502a871c;
  skos:inScheme :conceptScheme_751925ed;
  skos:prefLabel "part k - protection from falling, collision and impact"@en;
  skosxl:prefLabel :xl_en_3e905d0b .

:skosCollection_50d4bd2e skos:member :c_1d89066b, :c_2ca7a450 .

:c_f68328a2 a skos:Concept;
  dct:created "2018-03-28T19:11:07.411Z"^^xsd:dateTime;
  skos:broader :c_502a871c;
  skos:inScheme :conceptScheme_751925ed;
  skos:prefLabel "part l - conservation of fuel and power"@en;
  skosxl:prefLabel :xl_en_0460024f .

:c_ae74ec82 dct:modified "2020-10-26T06:52:56.572Z"^^xsd:dateTime .

:c_e186f594 a skos:Concept;
  dct:created "2018-03-28T19:09:58.476Z"^^xsd:dateTime;
  dct:modified "2020-10-23T17:06:53.653Z"^^xsd:dateTime;
  skos:broader :c_502a871c;
  skos:inScheme :conceptScheme_751925ed;
  skos:prefLabel "part c - site preparation and resistance to contaminates and moisture"@en;
  skosxl:prefLabel :xl_en_c14ad7c7 .

:c_2a34c0b8 skos:broader :c_502a871c .

:c_835978b6 dct:modified "2020-10-27T08:47:32.078Z"^^xsd:dateTime .

:c_c66a31b4 dct:modified "2020-10-27T16:10:33.573Z"^^xsd:dateTime .

:xl_en_d2f47531 a skosxl:Label .

:c_f5536b7d a skos:Concept;
  skos:note "NOTE: The soffit of a rooflight, but not the frame, is included as part of the surface of the ceiling. An upstand below a rooflight is considered as a wall."@en .

:c_e7e6b110 a skos:Concept;
  dct:created "2019-12-13T23:13:42.083Z"^^xsd:dateTime;
  dct:modified "2020-10-26T07:20:05.119Z"^^xsd:dateTime;
  skos:broader :c_13911a49;
  skos:definition "A space (including a protected stairway) mainly used as a means of access between a room and an exit from the building or compartment."@en;
  skos:inScheme :conceptScheme_751925ed .

:c_cb3d4c10 dc:source :c_ca00c020;
  dct:created "2019-12-21T06:24:42.742Z"^^xsd:dateTime;
  dct:modified "2019-12-21T06:27:11.372Z"^^xsd:dateTime;
  skos:broader :c_13911a49;
  skos:definition "An enclosed space within a building that is not used solely as a circulation space. The term includes not only conventional rooms, but also cupboards that are not fittings and large spaces such as warehouses and auditoria. The term does not include cavities such as ducts, ceiling cavities and roof spaces."@en;
  skos:inScheme :conceptScheme_751925ed;
  skos:prefLabel "room"@en .

:c_13911a49 skos:narrower :c_61f82d61, :c_6284471b, :c_7400b440, :c_7b85eda3, :c_7c12f560,
    :c_8258611b, :c_b2cab8d9, :c_cb3d4c10, :c_d32d8045, :c_d5c15327 .

:c_ee10273a a skos:Concept;
  dc:source :c_ca00c020;
  skos:prefLabel "relevant boundary"@en .

:c_b3f65603 dct:created "2019-12-15T08:27:29.025Z"^^xsd:dateTime;
  skos:broader :c_13911a49 .

:c_9e4931f7 dc:source :c_ca00c020;
  dct:modified "2019-12-13T23:33:59.230Z"^^xsd:dateTime .

:c_56fef4b5 a skos:Concept;
  dc:source :c_ca00c020;
  dct:modified "2019-12-21T07:22:01.287Z"^^xsd:dateTime;
  skos:note "NOTE: Recessed car parking areas as shown in Diagram A1 should not be regarded as unprotected areas."@en;
  skos:prefLabel "unprotected area"@en .

:c_61f82d61 dct:created "2019-12-13T22:48:54.196Z"^^xsd:dateTime;
  dct:modified "2019-12-13T23:33:58.730Z"^^xsd:dateTime;
  skos:broader :c_13911a49;
  skos:definition "A duct to deliver combustion air to a gas appliance."@en;
  skos:inScheme :conceptScheme_751925ed;
  skos:prefLabel "appliance ventilation duct"@en .

:c_6284471b dct:created "2019-12-13T22:51:41.721Z"^^xsd:dateTime;
  dct:modified "2019-12-13T23:33:58.863Z"^^xsd:dateTime;
  skos:broader :c_13911a49;
  skos:definition "A device that normally holds a door open, but closes it automatically if any one of the following occurs.<ul><ul>Smoke is detected by an automatic device of a suitable nature and quality in a suitable location.<li>A hand-operated switch, fitted in a suitable position, is operated.<li>The electricity supply to the device, apparatus or switch fails.<li>The fire alarm system, if any, is operated.</ul>"@en;
  skos:inScheme :conceptScheme_751925ed .

:c_793b849c dct:created "2018-08-11T13:05:19.050Z"^^xsd:dateTime .

:xl_en_74b321d9 a skosxl:Label .

:c_b975b2d2 dc:source :c_ca00c020;
  dct:modified "2019-12-21T07:22:01.349Z"^^xsd:dateTime .

:c_8258611b a skos:Concept;
  dct:created "2019-12-13T22:50:02.994Z"^^xsd:dateTime;
  dct:modified "2019-12-13T23:33:58.801Z"^^xsd:dateTime;
  skos:broader :c_13911a49;
  skos:definition "A continuous space that passes through one or more structural floors within a building, not necessarily vertically."@en;
  skos:inScheme :conceptScheme_751925ed .

:skosCollection_c85ed09f dct:created "2018-03-28T14:43:50.385Z"^^xsd:dateTime .

:c_3cae7829 dc:source :c_6c82c09f .

:c_5ef03467 a skos:Concept;
  dct:created "2019-12-13T22:46:11.837Z"^^xsd:dateTime;
  skos:broader :c_13911a49;
  skos:inScheme :conceptScheme_751925ed;
  skos:prefLabel "alternative exit"@en .

:c_58df2af5 dct:created "2019-12-21T10:17:39.618Z"^^xsd:dateTime;
  skos:inScheme :conceptScheme_751925ed;
  skos:narrower :c_56aca7cf .

:c_da6168d8 dc:source :c_6c82c09f .

:xl_en_32357ece skosxl:literalForm "eir"@en .

:c_727adfdb dct:modified "2019-12-21T07:22:01.574Z"^^xsd:dateTime;
  skos:note "NOTE: If an institutional building is planned to enable progressive horizontal evacuation, a door in a compartment wall is considered a storey exit for the purposes of requirement B1."@en .

:c_a4eaf123 a skos:Concept;
  dct:created "2019-12-21T07:13:55.109Z"^^xsd:dateTime;
  skos:broader :c_13911a49;
  skos:inScheme :conceptScheme_751925ed;
  skos:prefLabel "suspended ceiling"@en .

:c_d5c15327 dc:source :c_6c82c09f, :c_ca00c020;
  dct:created "2019-12-15T08:44:56.144Z"^^xsd:dateTime;
  skos:broader :c_13911a49 .

:c_38ba0f99 dc:source :c_ca00c020 .

:c_28e7c922 dc:source :c_ca00c020 .

:c_35d3a535 dc:source :c_ca00c020 .

:c_7b85eda3 a skos:Concept;
  dct:created "2019-12-21T06:10:33.715Z"^^xsd:dateTime;
  skos:broader :c_13911a49;
  skos:inScheme :conceptScheme_751925ed;
  skos:prefLabel "protected corridor/lobby"@en .

:c_7c12f560 dct:created "2019-12-21T06:14:37.859Z"^^xsd:dateTime .

:c_0a3a129e skos:narrower :c_4867a906, :c_d55b2d04 .

:c_33c0e1b5 skos:prefLabel "common balcony"@en .

:c_f70bb786 dc:source :c_6c82c09f .

:c_9e8d26ab dct:modified "2019-12-14T08:48:47.100Z"^^xsd:dateTime .

:xl_en_d34f5762 dct:modified "2018-06-01T23:31:11.865Z"^^xsd:dateTime .

:c_6c82c09f skos:exactMatch <http://www.worldcat.org/oclc/1120217476>;
  skos:narrower :c_4f2b64be .

:c_228ee3b0 a skos:Concept .

:c_b6083e42 dct:modified "2019-12-13T23:33:58.541Z"^^xsd:dateTime .

:c_cb86c2ff dc:source :c_6c82c09f .

:c_c07e16c5 skos:prefLabel "free area"@en .

:c_d4480e31 dct:modified "2020-10-23T17:06:41.749Z"^^xsd:dateTime .

:c_ca00c020 skos:topConceptOf :c_ca00c020 .

:xl_en_f2eee9b5 a skosxl:Label .

:xl_en_d4ddf75e a skosxl:Label;
  skosxl:literalForm "bim"@en .

:c_b0f3b4fb skos:prefLabel "travel distance"@en .

:c_7400b440 dct:created "2019-12-21T06:16:01.865Z"^^xsd:dateTime;
  dct:modified "2019-12-21T06:27:11.768Z"^^xsd:dateTime;
  skos:broader :c_13911a49;
  skos:definition "A classification of a building according to the purpose to which it is intended to be put. (See Table 0.1.)"@en .

:c_d32d8045 dc:source :c_6c82c09f, :c_ca00c020;
  dct:created "2019-12-21T06:49:49.146Z"^^xsd:dateTime;
  dct:modified "2019-12-21T06:53:32.122Z"^^xsd:dateTime;
  skos:broader :c_13911a49;
  skos:definition "building A building that consists of a ground storey only. Basements are not counted as storeys in a building (see Appendix D). A separated part that consists of a ground storey only, with a roof to which access is only provided for repair or maintenance, may be treated as a single storey building."@en;
  skos:inScheme :conceptScheme_751925ed .

:c_40560ccd dc:source :c_6c82c09f, :c_ca00c020 .

:c_132d79ca a skos:Concept .

:c_f479d1cb dct:created "2018-08-11T14:26:15.280Z"^^xsd:dateTime .

:xl_en_63b1eba4 a skosxl:Label;
  skosxl:literalForm """2.1.4
"""@en .

:xl_en_93b6dba8 a skosxl:Label;
  skosxl:literalForm "part q - security"@en .

:c_cd2ba206 a skos:Concept;
  dc:source :c_6c82c09f, :c_ca00c020;
  dct:created "2019-12-14T06:21:42.550Z"^^xsd:dateTime;
  dct:modified "2019-12-14T06:53:28.582Z"^^xsd:dateTime;
  skos:broader :c_13911a49;
  skos:definition "An area from which escape is possible in one direction only."@en;
  skos:inScheme :conceptScheme_751925ed;
  skos:prefLabel "dead end"@en .

:c_13911a49 skos:narrower :c_47c790ae, :c_49a5a923, :c_7e4da283, :c_b304ed8a, :c_b4ccd5f2,
    :c_b67f0d40, :c_b98dbf2a, :c_c916e597, :c_cd2ba206, :c_f12e46ec, :c_f636fce4 .

:c_b4ccd5f2 a skos:Concept;
  dc:source :c_6c82c09f, :c_ca00c020;
  dct:created "2019-12-14T06:49:21.314Z"^^xsd:dateTime;
  rdfs:seeAlso <http://www.legislation.gov.uk/uksi/2010/2214/regulation/2>;
  skos:broader :c_13911a49;
  skos:definition """The external wall of a building includes all of the following. 
<ul><li>Anything located within any space forming part of the wall.
<li>Any decoration or other finish applied to any external (but not internal) surface forming part of the wall.
<li>Any windows and doors in the wall.
<li>Any part of a roof pitched at an angle of more than 70 degrees to the horizontal if that part of the roof adjoins a space within the building to which persons have access, but not access only for the purpose of carrying out repairs or maintenance.</ul>"""@en;
  skos:editorialNote "NOTE: Except for the items marked * (which are from the Building Regulations 2010), these definitions apply only to Approved Document B.<p>NOTE: The terms defined below are key terms used in this document only. Refer to BS 4422 for further guidance on the definitions of common terms used in the fire safety industry which are not listed below.</p>"@en;
  skos:inScheme :conceptScheme_751925ed;
  skos:notation "*"@en;
  skos:prefLabel "external wall"@en .

:c_f636fce4 a skos:Concept;
  dc:source :c_6c82c09f, :c_ca00c020;
  dct:created "2019-12-14T06:23:01.241Z"^^xsd:dateTime;
  dct:modified "2019-12-14T06:53:28.651Z"^^xsd:dateTime;
  skos:broader :c_13911a49;
  skos:definition "The shortest distance from any point within the floor area to the nearest storey exit, measured within the external enclosures of the building, and ignoring walls, partitions and fittings other than the enclosing walls and partitions to protected stairways."@en;
  skos:inScheme :conceptScheme_751925ed;
  skos:prefLabel "direct distance"@en .

:c_b304ed8a a skos:Concept;
  dc:source :c_6c82c09f, :c_ca00c020;
  dct:created "2019-12-14T06:25:02.042Z"^^xsd:dateTime;
  rdfs:seeAlso <http://www.legislation.gov.uk/uksi/2010/2214/regulation/2>;
  skos:broader :c_13911a49;
  skos:definition "Does not include a flat or a building containing a flat."@en;
  skos:editorialNote "NOTE: Except for the items marked * (which are from the Building Regulations 2010), these definitions apply only to Approved Document B.<p>NOTE: The terms defined below are key terms used in this document only. Refer to BS 4422 for further guidance on the definitions of common terms used in the fire safety industry which are not listed below.</p>"@en;
  skos:inScheme :conceptScheme_751925ed;
  skos:notation "*"@en;
  skos:prefLabel "dwellinghouse"@en .

:c_7e4da283 a skos:Concept;
  dc:source :c_6c82c09f, :c_ca00c020;
  dct:created "2019-12-14T06:31:19.918Z"^^xsd:dateTime;
  dct:modified "2019-12-14T06:53:29.065Z"^^xsd:dateTime;
  skos:broader :c_13911a49;
  skos:definition """Any of the following.
<ul><li>A member that forms part of the structural frame of a building, or any other beam or column.
<li>A loadbearing wall or loadbearing part of a wall.
<li>A floor.
<li>A gallery (but not a loading gallery, fly gallery, stage grid, lighting bridge, or any gallery provided for similar purposes or for maintenance and repair).
<li>An external wall.
<li>A compartment wall (including a wall that is common to two or more buildings).</ul>
"""@en;
  skos:inScheme :conceptScheme_751925ed;
  skos:note "NOTE: However, see the guidance to requirement B3, paragraph 7.3, for a list of structures that are not considered to be elements of structure."@en;
  skos:prefLabel "element of structure"@en .

:c_49a5a923 a skos:Concept;
  dc:source :c_6c82c09f, :c_ca00c020;
  dct:created "2019-12-14T06:34:27.645Z"^^xsd:dateTime;
  dct:modified "2019-12-14T06:53:29.138Z"^^xsd:dateTime;
  skos:broader :c_13911a49;
  skos:definition "Lighting for use when the power supply to the normal lighting fails."@en;
  skos:inScheme :conceptScheme_751925ed;
  skos:prefLabel "emergency lighting"@en .

:c_b67f0d40 a skos:Concept;
  dc:source :c_6c82c09f, :c_ca00c020;
  dct:created "2019-12-14T06:36:59.442Z"^^xsd:dateTime;
  dct:modified "2019-12-14T06:53:29.194Z"^^xsd:dateTime;
  skos:broader :c_13911a49;
  skos:definition "The part of the emergency lighting that is provided to ensure that the escape route is illuminated at all material times."@en;
  skos:inScheme :conceptScheme_751925ed;
  skos:prefLabel "escape lighting"@en .

:c_b98dbf2a a skos:Concept;
  dc:source :c_6c82c09f, :c_ca00c020;
  dct:created "2019-12-14T06:43:26.810Z"^^xsd:dateTime;
  dct:modified "2019-12-14T06:53:29.257Z"^^xsd:dateTime;
  skos:broader :c_13911a49;
  skos:definition "The route along which people can escape from any point in a building to a final exit."@en;
  skos:inScheme :conceptScheme_751925ed;
  skos:prefLabel "escape route"@en .

:c_c916e597 a skos:Concept;
  dc:source :c_6c82c09f, :c_ca00c020;
  dct:created "2019-12-14T06:44:56.922Z"^^xsd:dateTime;
  dct:modified "2019-12-14T06:53:29.333Z"^^xsd:dateTime;
  skos:broader :c_13911a49;
  skos:definition "A lift that may be used to evacuate people in a fire."@en;
  skos:inScheme :conceptScheme_751925ed;
  skos:prefLabel "evacuation lift"@en .

:c_f12e46ec a skos:Concept;
  dc:source :c_6c82c09f, :c_ca00c020;
  dct:created "2019-12-14T06:46:09.069Z"^^xsd:dateTime;
  dct:modified "2019-12-14T06:53:29.420Z"^^xsd:dateTime;
  skos:broader :c_13911a49;
  skos:definition "A protected passageway that connects a protected stairway to a final exit."@en;
  skos:inScheme :conceptScheme_751925ed;
  skos:note "NOTE: Exit passageways should be protected to the same standard as the stairway they serve."@en;
  skos:prefLabel "exit passageway"@en .

:c_da6168d8 rdfs:seeAlso <http://www.legislation.gov.uk/uksi/2010/2214/regulation/2> .

:c_ca00c020 skos:narrower :c_13911a49 .

:c_6c82c09f skos:narrower :c_13911a49 .

:c_c02d4d7d rdfs:seeAlso <http://www.legislation.gov.uk/uksi/2010/2214/regulation/2>;
  skos:editorialNote "NOTE: Except for the items marked * (which are from the Building Regulations 2010), these definitions apply only to Approved Document B.<p>NOTE: The terms defined below are key terms used in this document only. Refer to BS 4422 for further guidance on the definitions of common terms used in the fire safety industry which are not listed below.</p>"@en .

:c_47c790ae a skos:Concept;
  dc:source :c_ca00c020;
  dct:created "2019-12-14T08:08:45.280Z"^^xsd:dateTime;
  dct:modified "2019-12-14T08:48:47.736Z"^^xsd:dateTime;
  skos:broader :c_13911a49;
  skos:definition "The end of an escape route from a building that gives direct access to a street, passageway, walkway or open space, and is sited to ensure that people rapidly disperse away from the building so that they are no longer in danger from fire and/or smoke."@en;
  skos:inScheme :conceptScheme_751925ed;
  skos:note "NOTE: Windows are not acceptable as final exits."@en;
  skos:prefLabel "final exit"@en .

:c_cb86c2ff a skos:Concept;
  dct:created "2019-12-14T08:22:05.410Z"^^xsd:dateTime;
  dct:modified "2019-12-14T08:48:47.223Z"^^xsd:dateTime;
  skos:broader :c_13911a49;
  skos:definition "A door or shutter which, together with its frame and furniture as installed in a building, is intended (when closed) to resist the spread of fire and/or gaseous products of combustion and meets specified performance criteria to those ends."@en;
  skos:inScheme :conceptScheme_751925ed;
  skos:note "NOTE: A fire doorset may have one or more leaves. The term includes a cover or other form of protection to an opening in a fire resisting wall or floor, or in a structure that surrounds a protected shaft. A fire doorset is a complete door assembly, assembled on site or delivered as a completed assembly, consisting of the door frame, leaf or leaves, essential hardware, edge seals and glazing, and any integral side panels or fanlight panels in an associated door screen."@en;
  skos:prefLabel "fire doorset"@en .

:c_7804ad6c a skos:Concept;
  dc:source :c_ca00c020;
  dct:created "2019-12-14T08:10:24.678Z"^^xsd:dateTime;
  skos:broader :c_13911a49;
  skos:definition "Combination of components for giving an audible and/or other perceptible warning of fire."@en;
  skos:inScheme :conceptScheme_751925ed;
  skos:prefLabel "fire alarm system"@en .

:c_c8b52d92 a skos:Concept;
  dc:source :c_6c82c09f, :c_ca00c020;
  dct:created "2019-12-14T08:12:53.416Z"^^xsd:dateTime;
  dct:modified "2019-12-14T08:48:47.374Z"^^xsd:dateTime;
  skos:broader :c_13911a49;
  skos:definition "A fire damper which, in addition to the performance of the fire damper, resists the spread of smoke."@en;
  skos:inScheme :conceptScheme_751925ed;
  skos:prefLabel "fire and smoke damper"@en .

:c_13911a49 skos:narrower :c_14b52896, :c_1a7ea9e5, :c_362390fa, :c_3cae7829, :c_706598d3,
    :c_7804ad6c, :c_7a2d826e, :c_9a0f5e20, :c_9e8d26ab, :c_b980c88c, :c_c8b52d92, :c_cb86c2ff,
    :c_d8e990c2, :c_dd03e186 .

:c_1a7ea9e5 a skos:Concept;
  dc:source :c_6c82c09f, :c_ca00c020;
  dct:created "2019-12-14T08:11:47.430Z"^^xsd:dateTime;
  dct:modified "2019-12-14T08:48:47.468Z"^^xsd:dateTime;
  skos:broader :c_13911a49;
  skos:definition "A mechanical or intumescent device within a duct or ventilation opening that operates automatically and is designed to resist the spread of fire."@en;
  skos:inScheme :conceptScheme_751925ed;
  skos:prefLabel "fire damper"@en .

:c_9e8d26ab a skos:Concept;
  dct:created "2019-12-14T08:37:19.617Z"^^xsd:dateTime;
  skos:broader :c_13911a49;
  skos:definition "A protected lobby that provides access from a firefighting stair to the accommodation area and to any associated firefighting lift."@en;
  skos:inScheme :conceptScheme_751925ed;
  skos:prefLabel "firefighting lobby"@en .

:c_14b52896 a skos:Concept;
  dct:created "2019-12-14T08:38:57.474Z"^^xsd:dateTime;
  skos:broader :c_13911a49;
  skos:definition "A protected enclosure that contains a firefighting stair, firefighting lobbies and, if provided, a firefighting lift together with its machine room."@en;
  skos:inScheme :conceptScheme_751925ed;
  skos:prefLabel "firefighting shaft"@en .

:c_9a0f5e20 a skos:Concept;
  dc:source :c_ca00c020;
  dct:created "2019-12-14T08:40:17.510Z"^^xsd:dateTime;
  skos:broader :c_13911a49;
  skos:definition "A protected stairway that connects to the accommodation area through only a firefighting lobby."@en;
  skos:inScheme :conceptScheme_751925ed;
  skos:prefLabel "firefighting stair"@en .

:c_3cae7829 a skos:Concept;
  dc:source :c_ca00c020;
  dct:created "2019-12-14T08:41:43.182Z"^^xsd:dateTime;
  skos:broader :c_13911a49;
  skos:definition "The ability of a component or a building to satisfy, for a stated period of time, some or all of the appropriate criteria given in the relevant standard."@en;
  skos:inScheme :conceptScheme_751925ed;
  skos:prefLabel "fire resisting (Fire resistance)"@en .

:c_7a2d826e a skos:Concept;
  dc:source :c_ca00c020;
  dct:created "2019-12-14T08:43:50.303Z"^^xsd:dateTime;
  dct:modified "2020-10-26T07:31:03.576Z"^^xsd:dateTime;
  skos:broader :c_13911a49;
  skos:definition "A compartment wall, compartment floor, cavity barrier and construction that encloses a protected escape route and/or a place of special fire hazard."@en;
  skos:inScheme :conceptScheme_751925ed;
  skos:prefLabel "fire-separating element"@en .

:c_706598d3 a skos:Concept;
  dc:source :c_ca00c020;
  dct:created "2019-12-14T08:45:42.181Z"^^xsd:dateTime;
  dct:modified "2019-12-14T08:48:46.560Z"^^xsd:dateTime;
  skos:broader :c_13911a49;
  skos:definition "A seal provided to close an imperfection of fit or design tolerance between elements or components, to restrict the spread of fire and smoke."@en;
  skos:inScheme :conceptScheme_751925ed;
  skos:prefLabel "fire-stop (Fire-stopping)"@en .

:c_362390fa a skos:Concept;
  dc:rights :c_6c82c09f;
  dc:source :c_6c82c09f, :c_ca00c020;
  dct:created "2019-12-15T07:08:51.487Z"^^xsd:dateTime;
  dct:modified "2019-12-15T07:54:23.946Z"^^xsd:dateTime;
  skos:broader :c_13911a49;
  skos:definition "A flat is a separate and self-contained premises constructed or adapted for use for residential purposes and forming part of a building from some other part of which it is divided horizontally."@en;
  skos:editorialNote "NOTE: Except for the items marked * (which are from the Building Regulations 2010), these definitions apply only to Approved Document B.<p>NOTE: The terms defined below are key terms used in this document only. Refer to BS 4422 for further guidance on the definitions of common terms used in the fire safety industry which are not listed below.</p> "@en;
  skos:inScheme :conceptScheme_751925ed;
  skos:notation "*"@en;
  skos:prefLabel "flat"@en .

:c_abc6dc1e a skos:Concept;
  dc:source :c_6c82c09f, :c_ca00c020;
  dct:created "2019-12-15T07:39:20.183Z"^^xsd:dateTime;
  dct:modified "2019-12-21T06:41:26.072Z"^^xsd:dateTime;
  skos:broader :c_4f2b64be;
  skos:inScheme :conceptScheme_751925ed;
  skos:prefLabel "diagram d1 measurement of door width"@en .

:c_b980c88c a skos:Concept;
  dc:rights :c_6c82c09f;
  dc:source :c_6c82c09f, :c_ca00c020;
  dct:created "2019-12-15T07:11:52.263Z"^^xsd:dateTime;
  dct:modified "2019-12-15T07:54:23.704Z"^^xsd:dateTime;
  skos:broader :c_13911a49;
  skos:definition "A floor or balcony that does not extend across the full extent of a building’s footprint and is open to the floor below."@en;
  skos:inScheme :conceptScheme_751925ed;
  skos:prefLabel "gallery"@en .

:c_4f2b64be a skos:Concept;
  dct:created "2019-12-15T07:22:31.525Z"^^xsd:dateTime;
  dct:modified "2019-12-15T08:07:58.561Z"^^xsd:dateTime;
  skos:broader :c_6c82c09f, :c_ca00c020;
  skos:inScheme :conceptScheme_751925ed;
  skos:narrower :c_45ef22f5, :c_8d791a67, :c_abc6dc1e, :c_c1a78f4b, :c_cc92c6ff;
  skos:note "<ul><li>a. Double pitch roof<ul>b. Mansard type roof<li>c. Flat or monopitch roof</ul>"@en;
  skos:prefLabel "appendix d: methods of measurement"@en .

:c_dd03e186 a skos:Concept;
  dc:rights :c_6c82c09f;
  dc:source :c_6c82c09f, :c_ca00c020;
  dct:created "2019-12-15T07:13:02.940Z"^^xsd:dateTime;
  dct:modified "2019-12-15T07:54:23.601Z"^^xsd:dateTime;
  skos:broader :c_13911a49;
  skos:definition "A room used, or intended to be used, for people to live in (including, for the purposes of Approved Document B Volumes 1 and 2, a kitchen, but not a bathroom)."@en;
  skos:inScheme :conceptScheme_751925ed;
  skos:prefLabel "habitable room"@en .

:c_d8e990c2 a skos:Concept;
  dc:rights :c_6c82c09f;
  dc:source :c_6c82c09f, :c_ca00c020;
  dct:created "2019-12-15T07:14:31.932Z"^^xsd:dateTime;
  dct:modified "2019-12-15T07:58:00.018Z"^^xsd:dateTime;
  rdfs:seeAlso :c_c1a78f4b, :c_cc92c6ff;
  skos:broader :c_13911a49;
  skos:definition """(of a building or storey for the purposes of Approved Document B Volumes 1 and 2) 
<ul><li>Height of a building is measured as shown in Appendix D, Diagram D4. 
<li>Height of the floor of the top storey above ground level is measured as shown in Appendix D, Diagram D6.</ul>"""@en;
  skos:inScheme :conceptScheme_751925ed;
  skos:prefLabel "height"@en .

:c_cc92c6ff a skos:Concept;
  dc:source :c_6c82c09f, :c_ca00c020;
  dct:created "2019-12-15T07:24:50.211Z"^^xsd:dateTime;
  dct:modified "2019-12-21T06:53:31.807Z"^^xsd:dateTime;
  skos:broader :c_4f2b64be;
  skos:inScheme :conceptScheme_751925ed;
  skos:prefLabel "diagram d4 height of building"@en .

:c_45ef22f5 a skos:Concept;
  dc:source :c_6c82c09f, :c_ca00c020;
  dct:created "2019-12-15T07:40:59.818Z"^^xsd:dateTime;
  dct:modified "2019-12-21T06:41:36.318Z"^^xsd:dateTime;
  skos:broader :c_4f2b64be;
  skos:inScheme :conceptScheme_751925ed;
  skos:note "<ul><li>a. cubic capacity of a building<li>b. Cubic capacity of compartments or separated part of a building</ul>"@en;
  skos:prefLabel "diagram d2 cubic capacity"@en .

:c_be34e7b3 a skos:Concept;
  dc:source :c_ca00c020;
  dct:created "2019-12-15T07:42:05.586Z"^^xsd:dateTime;
  dct:modified "2019-12-21T06:53:31.745Z"^^xsd:dateTime;
  skos:broader :c_4f2b64be;
  skos:inScheme :conceptScheme_751925ed;
  skos:note """<ul><li>a. Surface area: roofs and rooflights
In each case measure the visible area<li>b. Floor area:Room, garage, conservatory or outbuilding,measure to inner surface of enclosing walls<li>c. Floor area:Storey, part or compartment measure to inner surface of enclosing walls and include internal walls and partitions</ul>"""@en;
  skos:prefLabel "diagram d3 area"@en .

:c_8d791a67 a skos:Concept;
  dc:source :c_6c82c09f, :c_ca00c020;
  dct:created "2019-12-15T07:49:01.790Z"^^xsd:dateTime;
  dct:modified "2019-12-21T06:53:31.869Z"^^xsd:dateTime;
  skos:broader :c_4f2b64be;
  skos:inScheme :conceptScheme_751925ed;
  skos:note "NOTES:<ul><li>1. In assembly buildings (purpose group 5), a galleryis included as a storey, but not if it is a loading gallery, fly gallery, stage grid, lighting bridge, or any gallery provided for similar purposes, or for maintenance and repair<li>.2. In other purpose group buildings, galleries are not counted as a storey.<li>3.For the definition of basement, see Appendix A</ul>"@en;
  skos:prefLabel "diagram d5 number of storeys"@en .

:c_c1a78f4b a skos:Concept;
  dc:source :c_ca00c020;
  dct:created "2019-12-15T07:52:39.429Z"^^xsd:dateTime;
  dct:modified "2019-12-21T06:42:53.312Z"^^xsd:dateTime;
  skos:broader :c_4f2b64be;
  skos:inScheme :conceptScheme_751925ed;
  skos:prefLabel "diagram d6 height of top storey in building"@en .

:c_13911a49 dct:modified "2019-12-21T09:26:33.488Z"^^xsd:dateTime .

:c_7d862abe dct:modified "2019-12-21T06:40:53.066Z"^^xsd:dateTime .

:c_ca00c020 skos:narrower :c_4f2b64be .

:c_056e5a0a a skos:Concept;
  skos:broader :c_13911a49;
  skos:inScheme :conceptScheme_751925ed;
  skos:prefLabel "inner room"@en .

:c_f127ef1e skos:inScheme :conceptScheme_751925ed .

:c_659ab1b8 skos:inScheme :conceptScheme_751925ed .

:c_f340cba7 skos:inScheme :conceptScheme_751925ed .

:c_3a5b7e76 skos:inScheme :conceptScheme_751925ed .

:c_daa05efb skos:inScheme :conceptScheme_751925ed .

:c_851c02b0 skos:inScheme :conceptScheme_751925ed .

:c_e756ef49 skos:inScheme :conceptScheme_751925ed .

:c_75f7c82b skos:narrower :c_1e8a7cbf, :c_5918929b, :c_c31ddac5, :c_ef1c9d78, :c_f97db0fd .

:c_007625df skos:inScheme :conceptScheme_751925ed .

:c_9d2dac79 skos:inScheme :conceptScheme_751925ed .

:c_2f92acaa skos:inScheme :conceptScheme_751925ed .

:c_a4cdd233 skos:inScheme :conceptScheme_751925ed .

:c_da079e58 skos:inScheme :conceptScheme_751925ed .

:c_fabf0784 skos:inScheme :conceptScheme_751925ed .

:c_1d287961 skos:inScheme :conceptScheme_751925ed .

:c_a86611c3 a skos:Concept;
  dct:created "2020-10-14T06:58:19.971Z"^^xsd:dateTime;
  dct:modified "2020-10-16T17:01:59.623Z"^^xsd:dateTime;
  skos:broader :c_12c47f28;
  skos:definition """The following meanings apply to terms
throughout this section:"""@en;
  skos:inScheme :conceptScheme_751925ed;
  skos:notation "2.3"@en;
  skos:prefLabel "definitions (ada)"@en .

:c_e943b612 a skos:Concept;
  dct:created "2020-10-16T16:35:40.410Z"^^xsd:dateTime;
  dct:modified "2020-10-16T16:39:48.540Z"^^xsd:dateTime;
  skos:broader :c_a86611c3;
  skos:definition """A wall designed and
constructed to afford lateral support to another
wall perpendicular to it, support being provided
from the base to the top of the wall."""@en;
  skos:inScheme :conceptScheme_751925ed;
  skos:prefLabel "buttressing wall"@en .

:c_12c47f28 a skos:Concept;
  dct:created "2020-10-16T16:31:14.686Z"^^xsd:dateTime;
  dct:modified "2020-10-25T05:32:03.824Z"^^xsd:dateTime;
  skos:broader :c_1b060096;
  skos:inScheme :conceptScheme_751925ed;
  skos:prefLabel "structure 2004 edition incorporating 2004,2010 and 2013 amendments"@en .

:c_4e975ede a skos:Concept;
  dct:created "2020-10-16T16:59:05.253Z"^^xsd:dateTime;
  skos:broader :c_e186f594;
  skos:definition """This document is one of a series that has been
approved by the First Secretary of State for the
purpose of providing practical guidance with
respect to the requirements of Schedule 1 to and
Regulation 7 of the Building Regulations 2010 (SI
2010/2214) for England and Wales."""@en;
  skos:inScheme :conceptScheme_751925ed;
  skos:prefLabel "site preparation and resistance to contaminants and moisture 2004 edition incorporating 2010 and 2013 amendments"@en .

:c_db47eea3 a skos:Concept;
  dct:created "2020-10-16T16:41:44.186Z"^^xsd:dateTime;
  dct:modified "2020-10-16T16:42:21.594Z"^^xsd:dateTime;
  skos:broader :c_a86611c3;
  skos:definition """The load assumed to be produced
by the intended occupancy or use, including
the weight of movable partitions, distributed,
concentrated, impact, inertia and snow loads,
but excluding wind loads."""@en;
  skos:inScheme :conceptScheme_751925ed;
  skos:prefLabel "imposed load"@en .

:c_cda2477f a skos:Concept;
  dct:created "2020-10-16T16:40:01.369Z"^^xsd:dateTime;
  dct:modified "2020-10-16T16:42:57.737Z"^^xsd:dateTime;
  skos:broader :c_a86611c3;
  skos:definition """The horizontal distance between
the two leaves of a cavity wall."""@en;
  skos:inScheme :conceptScheme_751925ed;
  skos:prefLabel "cavity width"@en .

:c_054f5d4e a skos:Concept;
  dct:created "2020-10-16T16:40:35.037Z"^^xsd:dateTime;
  dct:modified "2020-10-16T16:42:48.002Z"^^xsd:dateTime;
  skos:broader :c_a86611c3;
  skos:definition """A wall constructed as a
compartment wall to meet the requirements of
regulation B3(2)."""@en;
  skos:inScheme :conceptScheme_751925ed;
  skos:prefLabel "compartment wall"@en .

:c_25dbe396 a skos:Concept;
  dct:created "2020-10-16T16:41:12.480Z"^^xsd:dateTime;
  dct:modified "2020-10-16T16:42:35.513Z"^^xsd:dateTime;
  skos:broader :c_a86611c3;
  skos:definition """The load due to the weight of
all walls, permanent partitions, floors, roofs
and finishes including services, and all other
permanent construction."""@en;
  skos:inScheme :conceptScheme_751925ed;
  skos:prefLabel "dead load"@en .

:c_d44ed148 a skos:Concept;
  dct:created "2020-10-16T16:43:29.330Z"^^xsd:dateTime;
  dct:modified "2020-10-16T16:43:49.605Z"^^xsd:dateTime;
  skos:broader :c_a86611c3;
  skos:definition """A member which forms an integral part
of a wall, in the form of a thickened section at
intervals along the wall, so as to afford lateral
support to the wall to which it is bonded or
securely tied."""@en;
  skos:inScheme :conceptScheme_751925ed;
  skos:prefLabel "pier"@en .

:c_5fea650b a skos:Concept;
  dct:created "2020-10-16T16:44:07.193Z"^^xsd:dateTime;
  dct:modified "2020-10-16T16:44:28.367Z"^^xsd:dateTime;
  skos:broader :c_a86611c3;
  skos:definition """A wall or part of a wall which is
common to adjoining buildings, and constructed
to meet the requirements of regulation B3(2)."""@en;
  skos:inScheme :conceptScheme_751925ed;
  skos:prefLabel "separating wall"@en .

:c_48a520f8 a skos:Concept;
  dct:created "2020-10-16T16:44:39.652Z"^^xsd:dateTime;
  dct:modified "2020-10-16T16:45:12.189Z"^^xsd:dateTime;
  skos:broader :c_a86611c3;
  skos:definition """The distance between the longitudinal
centres of any two adjacent timber members of
the same type, measured in the plane of floor,
ceiling or roof structure."""@en;
  skos:inScheme :conceptScheme_751925ed;
  skos:prefLabel "spacing"@en .

:c_d54c6174 a skos:Concept;
  dct:created "2020-10-16T16:45:44.754Z"^^xsd:dateTime;
  dct:modified "2020-10-16T16:46:12.785Z"^^xsd:dateTime;
  skos:broader :c_a86611c3;
  skos:definition """The distance measured along the centre
line of a member between the centres of any two
adjacent bearings or supports."""@en;
  skos:inScheme :conceptScheme_751925ed;
  skos:prefLabel "span"@en .

:c_778ca063 a skos:Concept;
  dct:created "2020-10-16T16:46:30.436Z"^^xsd:dateTime;
  dct:modified "2020-10-16T16:47:04.924Z"^^xsd:dateTime;
  skos:broader :c_a86611c3;
  skos:definition """A wall to which lateral support is
afforded by a combination of buttressing walls,
piers or chimneys acting in conjunction with
floor(s) or roof."""@en;
  skos:inScheme :conceptScheme_751925ed;
  skos:prefLabel "supported wall"@en .

:c_ce403f47 a skos:Concept;
  dct:created "2020-10-16T16:47:37.008Z"^^xsd:dateTime;
  dct:modified "2020-10-16T16:48:47.813Z"^^xsd:dateTime;
  skos:broader :c_a86611c3;
  skos:definition """The load due to the effect of wind
pressure or suction."""@en;
  skos:inScheme :conceptScheme_751925ed;
  skos:prefLabel "wind load"@en .

:c_90aedbdc skos:narrower :c_0cdb0b97, :c_1aa022f8 .

:c_42d467db dct:modified "2020-10-25T05:18:33.206Z"^^xsd:dateTime;
  skos:narrower :c_679215e0 .

:c_597ee1e5 a skos:Concept;
  dct:created "2020-10-16T17:01:23.399Z"^^xsd:dateTime;
  dct:modified "2020-10-16T17:03:42.971Z"^^xsd:dateTime;
  skos:broader :c_4e975ede;
  skos:definition """The following meanings apply to terms
throughout this Approved Document:"""@en;
  skos:inScheme :conceptScheme_751925ed;
  skos:notation "0.12"@en;
  skos:prefLabel "definitions (adc)"@en .

:c_2618c4b3 a skos:Concept;
  dct:created "2020-10-16T17:04:51.739Z"^^xsd:dateTime;
  dct:modified "2020-10-16T17:05:21.774Z"^^xsd:dateTime;
  skos:broader :c_597ee1e5;
  skos:definition """Any substance13 which is or
may become harmful to persons or buildings,
including substances which are corrosive,
explosive, flammable, radioactive or toxic."""@en;
  skos:inScheme :conceptScheme_751925ed;
  skos:prefLabel "contaminant"@en .

:c_43d8f455 a skos:Concept;
  dct:created "2020-10-16T17:04:03.527Z"^^xsd:dateTime;
  dct:modified "2020-10-16T17:04:34.252Z"^^xsd:dateTime;
  skos:broader :c_597ee1e5;
  skos:definition """The building and all the land forming the site
subject to building operations which includes
land under the building and the land around it
which may have an effect on the building or its
users (see also paragraph 2.11)."""@en;
  skos:inScheme :conceptScheme_751925ed;
  skos:prefLabel "building and land associated with the building"@en .

:c_f5ae3ea1 a skos:Concept;
  dct:created "2020-10-16T17:05:42.497Z"^^xsd:dateTime;
  dct:modified "2020-10-16T17:06:10.910Z"^^xsd:dateTime;
  skos:broader :c_597ee1e5;
  skos:definition """Lower horizontal surface of any space in a
building including finishes that are laid as part of
the permanent construction."""@en;
  skos:inScheme :conceptScheme_751925ed;
  skos:prefLabel "floor"@en .

:c_3afc08f0 a skos:Concept;
  dct:created "2020-10-16T17:06:31.015Z"^^xsd:dateTime;
  dct:modified "2020-10-16T17:06:53.217Z"^^xsd:dateTime;
  skos:broader :c_597ee1e5;
  skos:definition """Water in liquid form, either as a
static water table or flowing through the ground."""@en;
  skos:inScheme :conceptScheme_751925ed;
  skos:prefLabel "groundwater"@en .

:c_586c25b3 a skos:Concept;
  dct:created "2020-10-16T17:07:11.530Z"^^xsd:dateTime;
  dct:modified "2020-10-16T17:07:34.990Z"^^xsd:dateTime;
  skos:broader :c_597ee1e5;
  skos:definition """Deposition of liquid
water from a vapour, occurring within or between
the layers of the building envelope."""@en;
  skos:inScheme :conceptScheme_751925ed;
  skos:prefLabel "interstitial condensation"@en .

:c_3736f311 a skos:Concept;
  dct:created "2020-10-16T17:07:50.007Z"^^xsd:dateTime;
  dct:modified "2020-10-16T17:08:13.940Z"^^xsd:dateTime;
  skos:broader :c_597ee1e5;
  skos:definition "Water in liquid, solid or gaseous form."@en;
  skos:inScheme :conceptScheme_751925ed;
  skos:prefLabel "moisture"@en .

:c_0c23af6b a skos:Concept;
  dct:created "2020-10-16T17:08:32.985Z"^^xsd:dateTime;
  dct:modified "2020-10-16T17:09:03.826Z"^^xsd:dateTime;
  skos:broader :c_597ee1e5;
  skos:definition """Moisture in any form falling from the
atmosphere, usually as rain, sleet, snow or hail."""@en;
  skos:inScheme :conceptScheme_751925ed;
  skos:prefLabel "precipitation"@en .

:c_774ecfdd a skos:Concept;
  dct:created "2020-10-16T17:09:21.752Z"^^xsd:dateTime;
  dct:modified "2020-10-16T17:10:04.522Z"^^xsd:dateTime;
  skos:broader :c_597ee1e5;
  skos:definition """Any part of the external envelope of a
building that is at an angle of less than 70° to
the horizontal."""@en;
  skos:inScheme :conceptScheme_751925ed;
  skos:prefLabel "roof"@en .

:c_040286d4 a skos:Concept;
  dct:created "2020-10-16T17:10:21.683Z"^^xsd:dateTime;
  dct:modified "2020-10-16T17:10:41.886Z"^^xsd:dateTime;
  skos:broader :c_597ee1e5;
  skos:definition """Water droplets driven by the wind from the
surface of the sea or other bodies of water adjacent
to buildings. Sea spray can be especially hazardous
to materials because of its salt content."""@en;
  skos:inScheme :conceptScheme_751925ed;
  skos:prefLabel "spray"@en .

:c_90ae9da8 a skos:Concept;
  dct:created "2020-10-16T17:10:59.392Z"^^xsd:dateTime;
  dct:modified "2020-10-16T17:11:23.669Z"^^xsd:dateTime;
  skos:broader :c_597ee1e5;
  skos:definition """Deposition of liquid
water from a vapour, occurring on visible
surfaces within the building."""@en;
  skos:inScheme :conceptScheme_751925ed;
  skos:prefLabel "surface condensation"@en .

:c_12c07b97 a skos:Concept;
  dct:created "2020-10-16T17:11:40.167Z"^^xsd:dateTime;
  dct:modified "2020-10-16T17:12:07.999Z"^^xsd:dateTime;
  skos:broader :c_597ee1e5;
  skos:definition """Material of construction,
usually a membrane, that substantially reduces
the water vapour transfer through any building in
which it is incorporated."""@en;
  skos:inScheme :conceptScheme_751925ed;
  skos:prefLabel "vapour control layer"@en .

:c_b7704238 a skos:Concept;
  dct:created "2020-10-16T17:12:23.157Z"^^xsd:dateTime;
  dct:modified "2020-10-16T17:12:41.379Z"^^xsd:dateTime;
  skos:broader :c_597ee1e5;
  skos:definition """Any opaque part of the external envelope
of a building that is at an angle of 70° or more to
the horizontal."""@en;
  skos:inScheme :conceptScheme_751925ed;
  skos:prefLabel "wall"@en .

:c_f6ff7c1c a skos:Concept;
  dct:created "2020-10-17T06:18:31.390Z"^^xsd:dateTime;
  skos:broader :c_8cba3c82;
  skos:inScheme :conceptScheme_751925ed;
  skos:prefLabel "toxic substances 1992 edition incorporating 2002, 2010 and 2013 amendments"@en .

:c_586b08a2 a skos:Concept;
  dct:created "2020-10-17T06:22:58.683Z"^^xsd:dateTime;
  dct:modified "2020-10-17T06:24:13.204Z"^^xsd:dateTime;
  skos:broader :c_1a6e1e92;
  skos:definition """* This Approved Document gives guidance for
compliance with the Building Regulations for
building work carried out in England. It also
applies to building work carried out on excepted
energy buildings in Wales as defined in the Welsh
Ministers (Transfer of Functions)(No 2) Order 2009."""@en;
  skos:inScheme :conceptScheme_751925ed;
  skos:prefLabel "resistance to the passage of sound 2003 edition incorporating 2004, 2010, 2013 and 2015 amendments"@en .

:c_f4cc0ec3 a skos:Concept;
  dct:created "2020-10-17T06:26:16.079Z"^^xsd:dateTime;
  skos:broader :c_586b08a2;
  skos:definition """The definitions given below are for the purposes of this document only, and are not intended to
be rigorous. Fuller definitions of the various
acoustical terms are to be found in the relevant British Standards listed in Annex D."""@en;
  skos:inScheme :conceptScheme_751925ed;
  skos:prefLabel "annex c: glossary"@en .

:c_4b4c9739 dct:modified "2020-10-24T20:01:47.685Z"^^xsd:dateTime .

:c_59a3ae21 skos:narrower :c_0319d3fa, :c_03fe243e, :c_2842eb4b, :c_3f23e147, :c_485cf2fc,
    :c_54dcd677, :c_62cc4d78, :c_76c8b363, :c_7cf13722, :c_7cf2b5eb, :c_a8de44e3, :c_c07e16c5,
    :c_dd64e423, :c_eb6a5187, :c_f3c590e2, :c_fc7ec0c8 .

:c_4d4c50dd skos:inScheme :conceptScheme_751925ed;
  skos:prefLabel "infiltration"@en .

:c_a8de44e3 dct:modified "2020-10-24T19:09:33.148Z"^^xsd:dateTime .

:c_1fa348f3 a skos:Concept;
  dct:created "2020-10-19T19:02:43.189Z"^^xsd:dateTime;
  skos:broader :c_58df2af5;
  skos:inScheme :conceptScheme_751925ed;
  skos:prefLabel "a1 loading"@en .

:c_34ab31dc a skos:Concept;
  dct:created "2020-10-19T19:02:59.575Z"^^xsd:dateTime;
  skos:broader :c_58df2af5;
  skos:inScheme :conceptScheme_751925ed;
  skos:prefLabel "a2 ground movement"@en .

:c_56aca7cf a skos:Concept;
  dct:created "2020-10-19T19:03:45.481Z"^^xsd:dateTime;
  skos:broader :c_58df2af5;
  skos:inScheme :conceptScheme_751925ed;
  skos:prefLabel "a3 disproportionate collapse"@en .

:c_bd26d581 a skos:Concept;
  dct:created "2020-10-19T19:04:13.948Z"^^xsd:dateTime;
  skos:broader :c_58df2af5;
  skos:inScheme :conceptScheme_751925ed;
  skos:prefLabel "b1 means of waring and escape"@en .

:c_926affad a skos:Concept;
  dct:created "2020-10-19T19:04:58.189Z"^^xsd:dateTime;
  skos:broader :c_58df2af5;
  skos:inScheme :conceptScheme_751925ed;
  skos:prefLabel "b2 internal fire spread linings"@en .

:c_d7714b03 a skos:Concept;
  dct:created "2020-10-19T19:05:20.709Z"^^xsd:dateTime;
  skos:broader :c_58df2af5;
  skos:inScheme :conceptScheme_751925ed;
  skos:prefLabel "b3 internal fire spread structure"@en .

:c_95a5e382 a skos:Concept;
  dct:created "2020-10-19T19:05:41.132Z"^^xsd:dateTime;
  skos:broader :c_58df2af5;
  skos:inScheme :conceptScheme_751925ed;
  skos:prefLabel "b4 external fire spread"@en .

:c_419da0ad a skos:Concept;
  dct:created "2020-10-19T19:06:06.820Z"^^xsd:dateTime;
  skos:broader :c_58df2af5;
  skos:inScheme :conceptScheme_751925ed;
  skos:prefLabel "b5 access and facilities for the fire service"@en .

:c_9d708081 a skos:Concept;
  dct:created "2020-10-19T19:07:46.203Z"^^xsd:dateTime;
  skos:inScheme :conceptScheme_751925ed;
  skos:prefLabel "regulation 38 fire safety information"@en .

:c_58df2af5 skos:narrower :c_1fa348f3, :c_34ab31dc, :c_419da0ad, :c_926affad, :c_95a5e382,
    :c_bd26d581, :c_d7714b03 .

:c_86cfaae6 skos:narrower :c_58df2af5 .

:c_6b24d6e2 skos:notation "uksi 2010 2214"@en .

:c_37246cae skos:prefLabel "managing health and safety in construction"@en .

:c_f9b32acf dct:modified "2020-11-04T20:20:47.442Z"^^xsd:dateTime .

:c_feba40b2 a skos:Concept;
  skos:broader :c_37246cae;
  skos:definition """as a file appropriate to the characteristics of
the project, containing relevant health and safety information to be taken into
account during any subsequent project"""@en;
  skos:inScheme :conceptScheme_751925ed;
  skos:prefLabel "appendix 4 the health and safety file"@en .

:skosCollection_50d4bd2e a skos:Collection;
  dct:created "2020-10-23T17:24:32.699Z"^^xsd:dateTime;
  skos:member :c_040286d4, :c_04c52352, :c_054f5d4e, :c_056e5a0a, :c_0c23af6b, :c_10030a9a,
    :c_10ea4ecc, :c_12c07b97, :c_132d79ca, :c_13543964, :c_14b52896, :c_1a7ea9e5, :c_1f1f7725,
    :c_228ee3b0, :c_25dbe396, :c_2618c4b3, :c_28013078, :c_28e7c922, :c_33c0e1b5, :c_34f295d5,
    :c_35d3a535, :c_362390fa, :c_3736f311, :c_38ba0f99, :c_3afc08f0, :c_3cae7829, :c_3d59dac9,
    :c_3e5063e6, :c_40560ccd, :c_43d8f455, :c_46be855e, :c_47c790ae, :c_48a520f8, :c_49a5a923,
    :c_4a90e0e1, :c_4aee7770, :c_4cb80404, :c_4cdc3b72, :c_56fef4b5, :c_5724a233, :c_586c25b3,
    :c_5ef03467, :c_5fea650b, :c_61f82d61, :c_6284471b, :c_706598d3, :c_727adfdb, :c_7400b440,
    :c_774ecfdd, :c_778ca063, :c_7804ad6c, :c_79a3679f, :c_7a2d826e, :c_7b85eda3, :c_7c12f560,
    :c_7d862abe, :c_7e4da283, :c_7fc5469b, :c_8258611b, :c_83464c52, :c_858351ef, :c_88af4873,
    :c_90ae9da8, :c_9a0f5e20, :c_9b7f9eb7, :c_9e4931f7, :c_9e8d26ab, :c_a4eaf123, :c_a965ecce,
    :c_ad9a7d0c, :c_b0f3b4fb, :c_b2cab8d9, :c_b304ed8a, :c_b3f65603, :c_b44f46e0, :c_b4ccd5f2,
    :c_b6083e42, :c_b67f0d40, :c_b7704238, :c_b975b2d2, :c_b980c88c, :c_b98dbf2a, :c_bed063fd,
    :c_c02d4d7d, :c_c8b52d92, :c_c916e597, :c_cb3d4c10, :c_cb86c2ff, :c_cc61a0f4, :c_cd2ba206,
    :c_cda2477f, :c_ce403f47, :c_d32d8045, :c_d44ed148, :c_d54c6174, :c_d5c15327, :c_d8e990c2,
    :c_da6168d8, :c_db47eea3, :c_dd03e186, :c_e7e6b110, :c_e943b612, :c_ee10273a, :c_f12e46ec,
    :c_f4139893, :c_f5536b7d, :c_f5ae3ea1, :c_f636fce4, :c_f70bb786;
  skos:prefLabel "building regulation key terms"@en .

:c_37246cae a skos:Concept;
  dct:created "2020-10-23T16:58:55.740Z"^^xsd:dateTime;
  skos:inScheme :conceptScheme_751925ed;
  skos:narrower :c_feba40b2 .

:c_f9b32acf skos:prefLabel "legislation"@en .

:c_0109c085 skos:broader :c_502a871c .

:c_06f29df7 rdfs:isDefinedBy "https://www.legislation.gov.uk/uksi/2010/2214/regulation/7/made"@en;
  skos:broader :c_86cfaae6 .

:c_0e0d001c dct:modified "2020-11-04T19:53:51.127Z"^^xsd:dateTime;
  skos:broader :c_f9b32acf .

:c_6b24d6e2 dct:modified "2020-11-04T18:00:53.849Z"^^xsd:dateTime .

:c_502a871c skos:narrower :c_1a6e1e92, :c_1b060096, :c_2a34c0b8, :c_2ca1576c, :c_42d467db,
    :c_5ffbc967, :c_73c4361e, :c_8cba3c82, :c_a20cbb62, :c_b7bccf3d, :c_be604dfa, :c_d4480e31,
    :c_e186f594, :c_f68328a2, :c_fec1533e .

:c_63df1a7b a skos:Concept;
  skos:broader :c_59a3ae21;
  skos:definition " (general ventilation) is nominally continuous ventilation of rooms or spaces at a relatively low rate to dilute and remove pollutants and water vapour not removed by operation of extract ventilation, purge ventilation or infiltration, as well as supplying outdoor air into the building. For an individual dwelling this is referred to as ‘whole dwelling ventilation’."@en;
  skos:inScheme :conceptScheme_751925ed;
  skos:prefLabel "whole building ventilation"@en .

:c_eb6a5187 a skos:Concept;
  dct:modified "2020-10-26T07:32:32.754Z"^^xsd:dateTime;
  skos:broader :c_59a3ae21;
  skos:definition "is where a mechanical ventilator does not run all the time, usually running only when there is a particular need to remove pollutants or water vapour (e.g. during cooking or bathing). Intermittent operation may be under either manual control or automatic control."@en;
  skos:inScheme :conceptScheme_751925ed;
  skos:prefLabel "intermittent operation"@en .

:c_373d0f37 skos:broader :c_59a3ae21;
  skos:inScheme :conceptScheme_751925ed .

:c_8dc8a4f6 a skos:Concept;
  skos:broader :c_59a3ae21;
  skos:definition "is a room containing a bath or shower and, in addition, can also include sanitary accommodation."@en;
  skos:inScheme :conceptScheme_751925ed .

:c_dd64e423 a skos:Concept;
  skos:broader :c_59a3ae21;
  skos:definition "is a space where large numbers of people are expected to gather, such as a shopping mall or cinema/theatre foyer. For the purposes of this Approved Document, a space used solely or principally for circulation (e.g. a corridor or lift lobby in an office building or blocks of flats) is not a common space."@en .

:c_7cf2b5eb skos:inScheme :conceptScheme_751925ed;
  skos:prefLabel "purge ventilation"@en .

:c_eeea044b dct:modified "2020-10-26T07:31:36.088Z"^^xsd:dateTime;
  skos:broader :c_59a3ae21;
  skos:prefLabel "bcb or building control body"@en .

:c_54dcd677 a skos:Concept;
  skos:broader :c_59a3ae21;
  skos:definition "is a measure of the aerodynamic performance of a ventilator. It is the area of a sharp-edged circular orifice which air would pass through at the same volume flow rate, under an identical applied pressure difference, as the opening under consideration."@en;
  skos:inScheme :conceptScheme_751925ed;
  skos:prefLabel "cquivalent area"@en .

:c_62cc4d78 a skos:Concept;
  dct:modified "2020-10-26T07:28:48.195Z"^^xsd:dateTime;
  skos:definition "is a ventilation opening which may be opened and closed under either manual or automatic control."@en;
  skos:inScheme :conceptScheme_751925ed;
  skos:prefLabel "closable opening"@en .

:c_0319d3fa a skos:Concept;
  dct:modified "2020-10-26T07:23:20.238Z"^^xsd:dateTime;
  skos:definition "is where a ventilation device is opened and closed, or switched on and off, or its performance is adjusted by the occupants of a room or building (see automatic control)."@en;
  skos:inScheme :conceptScheme_751925ed;
  skos:prefLabel "manual control"@en .

:c_15104e5f skos:broader :c_59a3ae21;
  skos:inScheme :conceptScheme_751925ed;
  skos:prefLabel "stack effect"@en .

:c_fc7ec0c8 a skos:Concept;
  skos:broader :c_59a3ae21;
  skos:definition "is a general descriptive term for the resistance of the building envelope to infiltration with ventilators closed. The greater the airtightness at a given pressure difference across the envelope, the lower the infiltration."@en;
  skos:inScheme :conceptScheme_751925ed;
  skos:prefLabel "airtightness"@en .

:c_485cf2fc dct:modified "2020-10-24T19:07:17.093Z"^^xsd:dateTime;
  skos:broader :c_59a3ae21;
  skos:definition "(in relation to dwellings) is a dwelling, or a usable part of a dwelling (i.e. a habitable room), that is situated partly or entirely below ground level. Note that a cellar is distinct from a basement in that it is used only for storage, heating plant or purposes other than habitation."@en;
  skos:inScheme :conceptScheme_751925ed;
  skos:prefLabel "basement"@en .

:c_830012c2 a skos:Concept;
  dct:modified "2020-10-24T19:07:36.414Z"^^xsd:dateTime;
  skos:definition "is a part of a dwelling which is situated partly or entirely below ground level, and is distinct from a basement in that it is used only for storage, heating plant or purposes other than habitation."@en;
  skos:inScheme :conceptScheme_751925ed .

:c_3f23e147 skos:broader :c_59a3ae21;
  skos:definition "is a ventilation system using ducts from terminals in the ceiling of rooms to terminals on the roof that extract air to outside by a combination of the natural stack effect and the pressure effects of wind passing over the roof of the building."@en;
  skos:inScheme :conceptScheme_751925ed;
  skos:prefLabel "passive stack ventilation (psv)"@en .

:c_7cf13722 a skos:Concept;
  skos:broader :c_59a3ae21;
  skos:definition "is a room in a building other than a dwelling that is occupied by people, such as an office, workroom, classroom or hotel bedroom, but not a bathroom, sanitary accommodation, utility room or rooms or spaces used solely or principally for circulation, building services plant or storage purposes."@en;
  skos:inScheme :conceptScheme_751925ed;
  skos:prefLabel "occupiable room"@en .

:c_9b5f7333 a skos:Concept;
  skos:broader :c_59a3ae21;
  skos:definition "is any means of purpose- provided ventilation (whether it is permanent or closable) which opens directly to external air, such as the openable parts of a window, a louvre or a background ventilator. It also includes any door which opens directly to external air."@en;
  skos:inScheme :conceptScheme_751925ed;
  skos:prefLabel "ventilation opening"@en .

:c_ac856c1e a skos:Concept;
  skos:broader :c_59a3ae21;
  skos:definition "is the physical property used to measure the airtightness of the building fabric. It is defined as air leakage rate per hour per square metre of envelope area at a test reference pressure differential across the building envelope of 50 Pascal (50 N/m2). The design air permeability is the target value set at the design stage."@en;
  skos:inScheme :conceptScheme_751925ed;
  skos:prefLabel "air permeability"@en .

:c_e7b31cc5 a skos:Concept;
  dct:modified "2020-10-26T07:36:15.983Z"^^xsd:dateTime;
  skos:broader :c_59a3ae21;
  skos:definition "is a room used for domestic activities (such as cooking, clothes washing and bathing) which give rise to significant production of airborne moisture, e.g. a kitchen, utility room or bathroom. For the purposes of Part F, sanitary accommodation is also regarded as a wet room."@en;
  skos:inScheme :conceptScheme_751925ed;
  skos:prefLabel "wet room"@en .

:c_59a3ae21 a skos:Concept;
  dct:created "2020-10-24T18:42:24.065Z"^^xsd:dateTime;
  skos:definition """The following are key terms used in this
document:"""@en;
  skos:inScheme :conceptScheme_751925ed;
  skos:narrower :c_15104e5f, :c_32d39119, :c_373d0f37, :c_4fe84b3b, :c_63df1a7b, :c_67f6207e,
    :c_8dc8a4f6, :c_92db7c07, :c_9b5f7333, :c_ac856c1e, :c_d10595f3, :c_e7b31cc5;
  skos:notation "3.1"@en;
  skos:prefLabel "key terms (adf)"@en .

:c_90aedbdc skos:narrower :c_e2afc611 .

:c_92db7c07 a skos:Concept;
  dct:modified "2020-10-26T07:20:25.585Z"^^xsd:dateTime;
  skos:broader :c_59a3ae21;
  skos:definition "is a measure of the availability of water to micro-organisms, and is determined from the ratio of the vapour pressure of the water in the substrate to that of pure water at the same temperature and pressure. This ratio is, in steady-state conditions, numerically equal to the equilibrium relative humidity of the air, except that the latter is commonly expressed as a percentage (from IEA Annex 14 source book, 1991)."@en;
  skos:inScheme :conceptScheme_751925ed;
  skos:prefLabel "surface water activity"@en .

:c_67f6207e a skos:Concept;
  dct:modified "2020-10-26T07:24:36.849Z"^^xsd:dateTime;
  skos:broader :c_59a3ae21;
  skos:definition "is a room containing a sink or other feature or equipment which may reasonably be expected to produce water vapour in significant quantities."@en;
  skos:inScheme :conceptScheme_751925ed;
  skos:prefLabel "utility room"@en .

:c_f3c590e2 a skos:Concept;
  dct:modified "2020-10-26T07:40:01.575Z"^^xsd:dateTime;
  skos:broader :c_59a3ae21;
  skos:definition "is a small ventilation opening designed to provide controllable whole building ventilation. See Diagram 1."@en;
  skos:inScheme :conceptScheme_751925ed;
  skos:prefLabel "background ventilator"@en .

:c_32d39119 a skos:Concept;
  dct:modified "2020-10-26T07:38:12.648Z"^^xsd:dateTime;
  skos:broader :c_59a3ae21;
  skos:definition "is that part of the ventilation of a building provided by ventilation devices designed into the building (e.g. via background ventilators, PSV, extract fans, mechanical ventilation or air-conditioning systems)."@en;
  skos:inScheme :conceptScheme_751925ed;
  skos:prefLabel "purpose-provided ventilation"@en .

:c_a8de44e3 a skos:Concept;
  skos:broader :c_59a3ae21;
  skos:definition "which is permanently fixed in the open position."@en;
  skos:inScheme :conceptScheme_751925ed;
  skos:prefLabel "permanent opening is a ventilation opening"@en .

:c_c07e16c5 a skos:Concept;
  dct:modified "2020-10-26T07:39:23.102Z"^^xsd:dateTime;
  skos:broader :c_59a3ae21;
  skos:definition "is the geometric open area of a ventilator."@en .

:c_4d4c50dd a skos:Concept;
  dct:modified "2020-10-26T07:44:14.675Z"^^xsd:dateTime;
  skos:broader :c_59a3ae21;
  skos:definition "is the uncontrolled exchange of air between inside a building and outside through cracks, porosity and other unintentional openings in a building, caused by pressure difference effects of the wind and/or stack effect."@en .

:c_f851b292 a skos:Concept;
  dct:modified "2020-10-26T07:37:24.648Z"^^xsd:dateTime;
  skos:broader :c_59a3ae21;
  skos:definition "is a room used for dwelling purposes but which is not solely a kitchen, utility room, bathroom, cellar or sanitary accommodation."@en;
  skos:inScheme :conceptScheme_751925ed .

:c_76c8b363 a skos:Concept;
  dct:modified "2020-10-26T07:33:24.590Z"^^xsd:dateTime;
  skos:broader :c_59a3ae21;
  skos:definition "is the removal of air directly from a space or spaces to outside. Extract ventilation may be by natural means (e.g. by passive stack ventilation) or by mechanical means (e.g. by an extract fan or central system)."@en .

:c_4fe84b3b a skos:Concept;
  dct:modified "2020-10-26T07:39:36.168Z"^^xsd:dateTime;
  skos:broader :c_59a3ae21;
  skos:definition "is the total internal volume of the heated space, including the volume of all furniture, internal walls, internal floors, etc."@en .

:c_2842eb4b a skos:Concept;
  dct:modified "2020-10-26T07:42:52.163Z"^^xsd:dateTime;
  skos:broader :c_59a3ae21;
  skos:definition "is where a mechanical ventilation device runs all the time, e.g. mechanical extract ventilation (MEV) and mechanical ventilation with heat recovery (MVHR). The air flow rate provided by the mechanical ventilation need not be constant but may be varied, under either manual or automatic control, in response to the demand for pollutant or water vapour removal."@en;
  skos:inScheme :conceptScheme_751925ed;
  skos:prefLabel "continuous operation"@en .

:c_03fe243e a skos:Concept;
  dct:modified "2020-10-26T07:41:29.432Z"^^xsd:dateTime;
  skos:broader :c_59a3ae21;
  skos:definition "is where a ventilation device is opened and closed or switched on and off or its performance is adjusted by a mechanical or electronic controller which responds to a relevant stimulus. That stimulus is usually related to the humidity of the air in a room, pollutant levels (e.g. carbon dioxide concentration in a room), occupancy of the space (e.g. using a passive infra-red motion detector) or pressure difference across the device (e.g. due to the wind outside)."@en;
  skos:inScheme :conceptScheme_751925ed;
  skos:prefLabel "automatic control"@en .

:c_d10595f3 a skos:Concept;
  skos:broader :c_59a3ae21;
  skos:definition "is the supply and removal of air (by natural and/or mechanical means) to and from a space or spaces in a building. It normally comprises a combination of purpose-provided ventilation and infiltration."@en;
  skos:prefLabel "ventilation"@en .

:c_6d6d73cd a skos:Concept;
  skos:inScheme :conceptScheme_751925ed;
  skos:prefLabel "sanitation, hot water safety and water efficiency 2015 edition with 2016 amendments"@en .

:c_373d0f37 a skos:Concept;
  dct:modified "2020-10-26T07:35:27.876Z"^^xsd:dateTime;
  skos:definition "is a space containing one or more water closets or urinals. Sanitary accommodation containing one or more cubicles counts as a single space if there is free circulation of air throughout the space."@en;
  skos:prefLabel "sanitary accommodation"@en .

:c_7cf2b5eb a skos:Concept;
  dct:modified "2020-10-26T07:27:18.364Z"^^xsd:dateTime;
  skos:broader :c_59a3ae21;
  skos:definition "is manually controlled ventilation of rooms or spaces at a relatively high rate to rapidly dilute pollutants and/or water vapour. Purge ventilation may be provided by natural means (e.g. an openable window) or by mechanical means (e.g. a fan)."@en .

:c_dd64e423 dct:modified "2020-10-26T07:37:58.283Z"^^xsd:dateTime;
  skos:inScheme :conceptScheme_751925ed;
  skos:prefLabel "common space"@en .

:c_eeea044b a skos:Concept;
  skos:definition "is a local authority or an approved inspector."@en;
  skos:inScheme :conceptScheme_751925ed .

:c_0319d3fa skos:broader :c_59a3ae21 .

:c_fc7ec0c8 dct:modified "2020-10-24T19:06:57.628Z"^^xsd:dateTime .

:c_54dcd677 dct:modified "2020-10-26T07:29:31.653Z"^^xsd:dateTime .

:c_3f23e147 a skos:Concept;
  dct:modified "2020-10-26T07:36:30.614Z"^^xsd:dateTime .

:c_485cf2fc a skos:Concept .

:c_830012c2 skos:broader :c_59a3ae21;
  skos:prefLabel "cellar"@en .

:c_8dc8a4f6 dct:modified "2020-10-24T19:07:23.555Z"^^xsd:dateTime;
  skos:prefLabel "bathroom"@en .

:c_15104e5f a skos:Concept;
  dct:modified "2020-10-26T07:26:15.736Z"^^xsd:dateTime;
  skos:definition "is the pressure differential between inside and outside a building caused by differences in the density of the air due to an indoor/outdoor temperature difference."@en .

:c_ac856c1e dct:modified "2020-10-26T07:31:51.631Z"^^xsd:dateTime .

:c_63df1a7b dct:modified "2020-10-26T07:20:56.289Z"^^xsd:dateTime .

:c_9b5f7333 dct:modified "2020-10-26T07:22:06.343Z"^^xsd:dateTime .

:c_7cf13722 dct:modified "2020-10-26T07:27:46.498Z"^^xsd:dateTime .

:c_3b5778ee a skos:Concept;
  skos:broader :c_f4cc0ec3;
  skos:definition "Sound insulation that reduces transmission of airborne sound between buildings or parts of buildings."@en;
  skos:prefLabel "airborne sound insulation"@en .

:c_438bd78a a skos:Concept;
  skos:broader :c_f4cc0ec3;
  skos:definition "A direct or indirect air passage from one side of a structure to the other."@en;
  skos:prefLabel "air path"@en .

:c_8144317d a skos:Concept;
  skos:broader :c_f4cc0ec3;
  skos:definition "Process of sealing joints"@en;
  skos:prefLabel "caulking"@en .

:c_0c33e781 a skos:Concept;
  skos:broader :c_f4cc0ec3;
  skos:definition "A proprietary product or material such as mineral wool used to close the gap in a cavity wall."@en;
  skos:prefLabel "cavity stop"@en .

:c_f213d52c a skos:Concept;
  skos:broader :c_f4cc0ec3;
  skos:definition "The correction to a sound insulation quantity (such as DnT,w) to take account of a specific sound spectrum. See BS EN ISO 717-1:1997."@en;
  skos:prefLabel "ctr"@en .

:c_61aec10c a skos:Concept;
  skos:broader :c_f4cc0ec3;
  skos:definition "(See decibel)"@en;
  skos:prefLabel "db"@en .

:c_5bb42f0e a skos:Concept;
  skos:broader :c_f4cc0ec3;
  skos:definition "The unit used for many acoustic quantities to indicate the level with respect to a reference level."@en;
  skos:prefLabel "decibel (dB)"@en .

:c_1166f883 a skos:Concept;
  skos:broader :c_f4cc0ec3;
  skos:definition "Mass per unit volume, expressed in kilograms per cubic metre (kg/m3)."@en;
  skos:prefLabel "density"@en .

:c_e85e2d31 a skos:Concept;
  skos:broader :c_f4cc0ec3;
  skos:definition "The process in which sound that is incident on one side of a building element is radiated by the other side."@en;
  skos:prefLabel "direct transmission"@en .

:c_b3eb4d7b a skos:Concept;
  skos:broader :c_f4cc0ec3;
  skos:definition "The difference in sound level between a pair of rooms, in a stated frequency band, corrected for the reverberation time. See BS EN ISO 140-4:1998."@en;
  skos:prefLabel "dnt"@en .

:c_9a21f5a2 a skos:Concept;
  skos:broader :c_f4cc0ec3;
  skos:definition "A single-number quantity which characterises the airborne sound insulation between rooms. See BS EN ISO 717-1:1997"@en;
  skos:prefLabel "dnt,w"@en .

:c_c57961a6 a skos:Concept;
  skos:broader :c_f4cc0ec3;
  skos:definition "A single-number quantity which characterises the airborne sound insulation between rooms using noise spectrum no. 2 as defined in BS EN ISO 717-1:1997. See BS EN ISO 717-1:1997."@en;
  skos:prefLabel "dnt,w + ctr"@en .

:c_cbfc0947 a skos:Concept;
  skos:broader :c_f4cc0ec3;
  skos:definition "A parameter used to describe the ability of a resilient material or wall tie to transmit vibration. Specimens with high dynamic stiffness (dynamically ‘stiff’) transmit more vibration than specimens with low dynamic stiffness (dynamically ‘soft’). See BS EN 29052-1:1992 for resilient materials. See BRE Information Paper IP 3/01 for wall ties."@en;
  skos:prefLabel "dynamic stiffness"@en .

:c_4cb28fa4 a skos:Concept;
  skos:broader :c_f4cc0ec3;
  skos:definition "Any building element that contributes to sound transmission between rooms in a building that is not a separating floor or separating wall."@en;
  skos:prefLabel "flanking element"@en .

:c_345811e8 a skos:Concept;
  skos:broader :c_f4cc0ec3;
  skos:definition "Sound transmitted between rooms via flanking elements instead of directly through separating elements or along any path other than the direct path."@en;
  skos:prefLabel "flanking transmission"@en .

:c_3262a30a a skos:Concept;
  skos:broader :c_f4cc0ec3;
  skos:definition "A floating floor consists of a floating layer and resilient layer (see also resilient layer and floating layer)."@en;
  skos:prefLabel "floating floor"@en .

:c_4f47aeea a skos:Concept;
  skos:broader :c_f4cc0ec3;
  skos:definition "A surface layer that rests on a resilient layer and is therefore isolated from the base floor and the surrounding walls (see also resilient layer)."@en;
  skos:prefLabel "floating layer"@en .

:c_d68c8ade a skos:Concept;
  skos:broader :c_f4cc0ec3;
  skos:definition "A partition consisting of board or boards connected to both sides of a wood or metal frame."@en;
  skos:prefLabel "framed wall"@en .

:c_8abc2fd9 a skos:Concept;
  skos:broader :c_f4cc0ec3;
  skos:definition "The number of pressure variations (or cycles) per second that gives a sound its distinctive tone. The unit of frequency is the Hertz (Hz)."@en;
  skos:prefLabel "frequency"@en .

:c_f40ac57b a skos:Concept;
  skos:broader :c_f4cc0ec3;
  skos:definition "A continuous range of frequencies between stated upper and lower limits (see also octave band and one-third octave band)."@en;
  skos:prefLabel "frequency band"@en .

:c_aa316632 a skos:Concept;
  skos:broader :c_f4cc0ec3;
  skos:definition "The unit of the frequency of a sound (formerly called cycles per second)."@en;
  skos:prefLabel "hertz (hz)"@en .

:c_c2902dec a skos:Concept;
  skos:broader :c_f4cc0ec3;
  skos:definition "Sound resulting from direct impact on a building element."@en;
  skos:prefLabel "impact sound"@en .

:c_588bf28f a skos:Concept;
  skos:broader :c_f4cc0ec3;
  skos:definition "Sound insulation which reduces impact sound transmission from direct impacts such as footsteps on a building element."@en;
  skos:prefLabel "impact sound insulation"@en .

:c_895306c7 a skos:Concept;
  skos:broader :c_f4cc0ec3;
  skos:definition "A ceiling which is fixed independently of a separating floor or an internal floor (see separating floor and internal floor)."@en;
  skos:prefLabel "independent ceiling"@en .

:c_07abc5c2 a skos:Concept;
  skos:broader :c_f4cc0ec3;
  skos:definition "Any floor that is not a separating floor (see separating floor)."@en;
  skos:prefLabel "internal floor"@en .

:c_c8566bf0 a skos:Concept;
  skos:broader :c_f4cc0ec3;
  skos:definition "A landing between two floors (see also landing)."@en;
  skos:prefLabel "intermediate landing"@en .

:c_3d888dc1 a skos:Concept;
  skos:broader :c_f4cc0ec3;
  skos:definition "Any wall that does not have a separating function."@en;
  skos:prefLabel "internal wall"@en .

:c_70a0403c a skos:Concept;
  skos:broader :c_f4cc0ec3;
  skos:definition "The absence of rigid connections between two or more parts of a structure."@en;
  skos:prefLabel "isolation"@en .

:c_34c7d4e3 a skos:Concept;
  skos:broader :c_f4cc0ec3;
  skos:definition "A platform or part of floor structure at the end of a flight of stairs or ramp."@en;
  skos:prefLabel "landing"@en .

:c_81482951 a skos:Concept;
  dct:modified "2020-10-25T04:25:51.418Z"^^xsd:dateTime;
  skos:broader :c_f4cc0ec3;
  skos:definition "The impact sound pressure level in a stated frequency band, corrected for the reverberation time. See BS EN ISO 140-7:1998."@en;
  skos:inScheme :conceptScheme_751925ed;
  skos:prefLabel "l’nt"@en .

:c_d26ff5d2 a skos:Concept;
  skos:broader :c_f4cc0ec3;
  skos:definition "A single-number quantity used to characterise the impact sound insulation of floors. See BS EN ISO 717-2:1997."@en;
  skos:prefLabel "l’nt,w"@en .

:c_b4273037 a skos:Concept;
  skos:broader :c_f4cc0ec3;
  skos:definition "Mass per unit area is expressed in terms of kilograms per square metre (kg/m²)."@en;
  skos:prefLabel "mass per unit area"@en .

:c_93488b6d a skos:Concept;
  dct:modified "2020-10-25T04:26:50.620Z"^^xsd:dateTime;
  skos:broader :c_f4cc0ec3;
  skos:definition "Noise is unwanted sound."@en;
  skos:inScheme :conceptScheme_751925ed;
  skos:prefLabel "noise"@en .

:c_e6d846bf a skos:Concept;
  dct:modified "2020-10-25T04:27:00.327Z"^^xsd:dateTime;
  skos:broader :c_f4cc0ec3;
  skos:definition "A frequency band in which the upper limit of the band is twice the frequency of the lower limit."@en;
  skos:inScheme :conceptScheme_751925ed;
  skos:prefLabel "octave band"@en .

:c_c13a7c46 a skos:Concept;
  skos:broader :c_f4cc0ec3;
  skos:definition "A frequency band in which the upper limit of the band is 21/3 times the frequency of the lower limit."@en;
  skos:prefLabel "one-third octave band"@en .

:c_2a1002d3 a skos:Concept;
  dct:modified "2020-10-25T04:27:58.892Z"^^xsd:dateTime;
  skos:broader :c_f4cc0ec3;
  skos:definition "A single-number quantity which characterises the airborne sound insulation of a material or building element in the laboratory. See BS EN ISO 717-1:1997."@en;
  skos:inScheme :conceptScheme_751925ed;
  skos:prefLabel "rw"@en .

:c_3fc6a13d a skos:Concept;
  dct:modified "2020-10-25T04:27:25.919Z"^^xsd:dateTime;
  skos:broader :c_f4cc0ec3;
  skos:definition "A layer that isolates a floating layer from a base floor and surrounding walls."@en;
  skos:inScheme :conceptScheme_751925ed;
  skos:prefLabel "resilient layer"@en .

:c_8f476b03 a skos:Concept;
  dct:modified "2020-10-25T04:27:37.381Z"^^xsd:dateTime;
  skos:broader :c_f4cc0ec3;
  skos:definition "The persistence of sound in a space after a sound source has been stopped."@en;
  skos:inScheme :conceptScheme_751925ed;
  skos:prefLabel "reverberation"@en .

:c_6ed11205 a skos:Concept;
  dct:modified "2020-10-25T04:27:48.773Z"^^xsd:dateTime;
  skos:broader :c_f4cc0ec3;
  skos:definition "The time, in seconds, taken for the sound to decay by 60dB after a sound source has been stopped."@en;
  skos:inScheme :conceptScheme_751925ed;
  skos:prefLabel "reverberation time"@en .

:c_fa726c7b a skos:Concept;
  dct:modified "2020-10-25T04:28:10.553Z"^^xsd:dateTime;
  skos:broader :c_f4cc0ec3;
  skos:definition "Floor that separates flats or rooms for residential purposes."@en;
  skos:inScheme :conceptScheme_751925ed;
  skos:prefLabel "separating floor"@en .

:c_e43f1fcb a skos:Concept;
  dct:modified "2020-10-25T04:28:20.895Z"^^xsd:dateTime;
  skos:broader :c_f4cc0ec3;
  skos:definition "Wall that separates adjoining dwelling-houses, flats or rooms for residential purposes."@en;
  skos:inScheme :conceptScheme_751925ed;
  skos:prefLabel "separating wall"@en .

:c_da4b364b a skos:Concept;
  dct:modified "2020-10-25T04:28:31.298Z"^^xsd:dateTime;
  skos:broader :c_f4cc0ec3;
  skos:definition "A quantity related to the physical intensity of a sound."@en;
  skos:inScheme :conceptScheme_751925ed;
  skos:prefLabel "sound pressure level"@en .

:c_95d3756f a skos:Concept;
  dct:modified "2020-10-25T04:28:53.490Z"^^xsd:dateTime;
  skos:broader :c_f4cc0ec3;
  skos:definition "A quantity, measured in a laboratory, which characterises the sound insulating properties of a material or building element in a stated frequency band. See BS EN ISO 140-3:1995."@en;
  skos:inScheme :conceptScheme_751925ed;
  skos:prefLabel "sound reduction index (r)"@en .

:c_8c6a9923 a skos:Concept;
  dct:modified "2020-10-25T04:29:06.143Z"^^xsd:dateTime;
  skos:broader :c_f4cc0ec3;
  skos:definition "The composition of a particular sound in terms of separate frequency bands."@en;
  skos:inScheme :conceptScheme_751925ed;
  skos:prefLabel "spectrum"@en .

:c_3b310e19 a skos:Concept;
  dct:modified "2020-10-25T04:29:20.043Z"^^xsd:dateTime;
  skos:broader :c_f4cc0ec3;
  skos:definition "Sound which is carried via the structure of a building."@en;
  skos:inScheme :conceptScheme_751925ed;
  skos:prefLabel "structure-borne sound"@en .

:c_5aa42901 a skos:Concept;
  dct:modified "2020-10-25T04:29:34.851Z"^^xsd:dateTime;
  skos:broader :c_f4cc0ec3;
  skos:definition "United Kingdom Accreditation Service."@en;
  skos:inScheme :conceptScheme_751925ed;
  skos:prefLabel "ukas"@en .

:c_ac95ba41 a skos:Concept;
  dct:modified "2020-10-24T20:19:52.881Z"^^xsd:dateTime;
  skos:broader :c_f4cc0ec3;
  skos:definition "The measured improvement of impact sound insulation resulting from the installation of a floor covering or floating floor on a test floor in a laboratory. See BS EN ISO 717-2:1997."@en;
  skos:inScheme :conceptScheme_751925ed;
  skos:prefLabel "dlw"@en .

:c_f40ac57b dct:modified "2020-10-24T20:24:01.793Z"^^xsd:dateTime;
  skos:inScheme :conceptScheme_751925ed .

:c_1166f883 dct:modified "2020-10-24T20:19:10.331Z"^^xsd:dateTime;
  skos:inScheme :conceptScheme_751925ed .

:c_438bd78a dct:modified "2020-10-24T20:10:42.096Z"^^xsd:dateTime;
  skos:inScheme :conceptScheme_751925ed .

:c_aa316632 dct:modified "2020-10-24T20:24:34.204Z"^^xsd:dateTime;
  skos:inScheme :conceptScheme_751925ed .

:c_4cb28fa4 dct:modified "2020-10-24T20:22:03.002Z"^^xsd:dateTime;
  skos:inScheme :conceptScheme_751925ed .

:c_07abc5c2 dct:modified "2020-10-25T04:25:09.858Z"^^xsd:dateTime;
  skos:inScheme :conceptScheme_751925ed .

:c_8abc2fd9 dct:modified "2020-10-24T20:23:35.208Z"^^xsd:dateTime;
  skos:inScheme :conceptScheme_751925ed .

:c_0c33e781 dct:modified "2020-10-24T20:11:55.304Z"^^xsd:dateTime;
  skos:inScheme :conceptScheme_751925ed .

:c_c57961a6 dct:modified "2020-10-24T20:21:01.089Z"^^xsd:dateTime;
  skos:inScheme :conceptScheme_751925ed .

:c_c2902dec dct:modified "2020-10-24T20:25:01.285Z"^^xsd:dateTime;
  skos:inScheme :conceptScheme_751925ed .

:c_3262a30a dct:modified "2020-10-24T20:22:24.209Z"^^xsd:dateTime;
  skos:inScheme :conceptScheme_751925ed .

:c_cbfc0947 dct:modified "2020-10-24T20:21:20.858Z"^^xsd:dateTime;
  skos:inScheme :conceptScheme_751925ed .

:c_5bb42f0e dct:modified "2020-10-24T20:18:46.501Z"^^xsd:dateTime;
  skos:inScheme :conceptScheme_751925ed .

:c_61aec10c dct:modified "2020-10-24T20:18:25.333Z"^^xsd:dateTime;
  skos:inScheme :conceptScheme_751925ed .

:c_3d888dc1 dct:modified "2020-10-25T04:25:22.708Z"^^xsd:dateTime;
  skos:inScheme :conceptScheme_751925ed .

:c_d68c8ade dct:modified "2020-10-24T20:23:10.718Z"^^xsd:dateTime;
  skos:inScheme :conceptScheme_751925ed .

:c_b4273037 dct:modified "2020-10-25T04:26:38.681Z"^^xsd:dateTime;
  skos:inScheme :conceptScheme_751925ed .

:c_34c7d4e3 dct:modified "2020-10-25T04:26:24.011Z"^^xsd:dateTime;
  skos:inScheme :conceptScheme_751925ed .

:c_4f47aeea dct:modified "2020-10-24T20:22:46.510Z"^^xsd:dateTime;
  skos:inScheme :conceptScheme_751925ed .

:c_9a21f5a2 dct:modified "2020-10-24T20:20:33.912Z"^^xsd:dateTime;
  skos:inScheme :conceptScheme_751925ed .

:c_588bf28f dct:modified "2020-10-25T04:24:24.550Z"^^xsd:dateTime;
  skos:inScheme :conceptScheme_751925ed .

:c_f213d52c dct:modified "2020-10-24T20:17:54.891Z"^^xsd:dateTime;
  skos:inScheme :conceptScheme_751925ed .

:c_70a0403c dct:modified "2020-10-25T04:25:34.953Z"^^xsd:dateTime;
  skos:inScheme :conceptScheme_751925ed .

:c_c8566bf0 dct:modified "2020-10-25T04:24:52.842Z"^^xsd:dateTime;
  skos:inScheme :conceptScheme_751925ed .

:c_3b5778ee dct:modified "2020-10-24T20:10:58.711Z"^^xsd:dateTime;
  skos:inScheme :conceptScheme_751925ed .

:c_895306c7 dct:modified "2020-10-25T04:24:39.232Z"^^xsd:dateTime;
  skos:inScheme :conceptScheme_751925ed .

:c_e85e2d31 dct:modified "2020-10-24T20:19:31.526Z"^^xsd:dateTime;
  skos:inScheme :conceptScheme_751925ed .

:c_345811e8 dct:modified "2020-10-26T07:19:47.127Z"^^xsd:dateTime;
  skos:inScheme :conceptScheme_751925ed .

:c_d26ff5d2 dct:modified "2020-10-25T04:26:09.753Z"^^xsd:dateTime;
  skos:inScheme :conceptScheme_751925ed .

:c_b3eb4d7b dct:modified "2020-10-24T20:20:13.014Z"^^xsd:dateTime;
  skos:inScheme :conceptScheme_751925ed .

:c_c13a7c46 dct:modified "2020-10-25T04:27:14.383Z"^^xsd:dateTime;
  skos:inScheme :conceptScheme_751925ed .

:c_8144317d dct:modified "2020-10-24T20:11:37.568Z"^^xsd:dateTime;
  skos:inScheme :conceptScheme_751925ed .

:c_f4cc0ec3 dct:modified "2020-10-24T20:07:15.383Z"^^xsd:dateTime;
  skos:narrower :c_07abc5c2, :c_0c33e781, :c_0db511ab, :c_1166f883, :c_2a1002d3, :c_3262a30a,
    :c_345811e8, :c_34c7d4e3, :c_3b310e19, :c_3b5778ee, :c_3d888dc1, :c_3fc6a13d, :c_438bd78a,
    :c_4b4c9739, :c_4cb28fa4, :c_4f47aeea, :c_588bf28f, :c_5aa42901, :c_5bb42f0e, :c_61aec10c,
    :c_6ed11205, :c_70a0403c, :c_8144317d, :c_81482951, :c_895306c7, :c_8abc2fd9, :c_8c6a9923,
    :c_8f476b03, :c_93488b6d, :c_95d3756f, :c_9a21f5a2, :c_aa316632, :c_ac95ba41, :c_b3eb4d7b,
    :c_b4273037, :c_c13a7c46, :c_c2902dec, :c_c57961a6, :c_c8566bf0, :c_c878dbda, :c_cbfc0947,
    :c_d26ff5d2, :c_d68c8ade, :c_da4b364b, :c_e43f1fcb, :c_e6d846bf, :c_e85e2d31, :c_f213d52c,
    :c_f3cee240, :c_f40ac57b, :c_fa726c7b .

:c_0db511ab a skos:Concept;
  dct:modified "2020-10-24T20:01:38.708Z"^^xsd:dateTime;
  skos:broader :c_f4cc0ec3;
  skos:definition "Conversion of sound energy to heat, often by the use of a porous material."@en;
  skos:inScheme :conceptScheme_751925ed;
  skos:prefLabel "absorption"@en .

:c_4b4c9739 a skos:Concept;
  skos:broader :c_f4cc0ec3;
  skos:definition "A quantity characterising the effectiveness of a sound absorbing surface. The proportion of sound energy absorbed is given as a number between zero (for a fully reflective surface) and one (for a fully absorptive surface). Note that sound absorption coefficients determined from laboratory measurements may have values slightly larger than one. See BS EN 20354:1993."@en;
  skos:inScheme :conceptScheme_751925ed;
  skos:prefLabel "absorption coefficient"@en .

:c_c878dbda a skos:Concept;
  dct:modified "2020-10-24T20:01:44.488Z"^^xsd:dateTime;
  skos:broader :c_f4cc0ec3;
  skos:definition "Material that absorbs sound energy."@en;
  skos:inScheme :conceptScheme_751925ed;
  skos:prefLabel "absorptive material"@en .

:c_f3cee240 a skos:Concept;
  dct:modified "2020-10-24T20:01:41.621Z"^^xsd:dateTime;
  skos:broader :c_f4cc0ec3;
  skos:definition "Sound propagating through the air."@en;
  skos:inScheme :conceptScheme_751925ed;
  skos:prefLabel "airborne sound"@en .

:c_44c61ce8 a skos:Concept;
  dct:created "2020-10-25T04:32:22.323Z"^^xsd:dateTime;
  skos:broader :c_2ca1576c;
  skos:inScheme :conceptScheme_751925ed;
  skos:narrower :c_59a3ae21 .

:c_6d6d73cd dct:created "2020-10-25T04:38:31.854Z"^^xsd:dateTime;
  skos:broader :c_73c4361e;
  skos:narrower :c_90aedbdc .

:c_d10595f3 dct:modified "2020-10-25T04:37:04.887Z"^^xsd:dateTime .

:c_73c4361e skos:narrower :c_6d6d73cd .

:c_59a3ae21 dct:modified "2020-10-25T04:34:27.571Z"^^xsd:dateTime;
  skos:broader :c_44c61ce8 .

:c_2ca1576c dct:modified "2020-10-25T04:35:01.892Z"^^xsd:dateTime;
  skos:narrower :c_44c61ce8 .

:c_90aedbdc a skos:Concept;
  dct:created "2020-10-25T04:45:46.524Z"^^xsd:dateTime;
  skos:broader :c_6d6d73cd;
  skos:inScheme :conceptScheme_751925ed;
  skos:narrower :c_316d73a9;
  skos:prefLabel "key terms (adg)"@en .

:c_679215e0 skos:definition """This document is one of a series that has been
approved and issued by the Secretary of State
for the purpose of providing practical guidance
with respect to the requirements of Schedule 1
to and Regulation 7 of the Building Regulations
2010 (SI 2010/2214) for England and Wales."""@en .

:c_0822f77e a skos:Concept;
  skos:broader :c_90aedbdc;
  skos:definition "includes the erection or extension of a building, the provision or extension of a controlled service or ﬁtting in or in connection with a building, and the material alteration of a building, or a controlled service or ﬁtting."@en;
  skos:prefLabel "building work"@en .

:c_39f68990 a skos:Concept;
  skos:broader :c_90aedbdc;
  skos:definition "means a mechanically operated valve that opens to discharge water when a ﬁxed (factory set) temperature or ﬁxed (factory set) pressure  is exceeded."@en;
  skos:prefLabel "combined temperature and pressure relief valve"@en .

:c_a1430501 a skos:Concept;
  skos:broader :c_90aedbdc;
  skos:definition "includes a service or ﬁtting subject to Schedule 1 requirements in respect of sanitation, hot water safety, water efﬁciency, drainage and waste disposal, combustion appliances and fuel storage, conservation of fuel or power, and electrical safety."@en .

:c_70908a07 skos:narrower :c_ab063a87 .

:c_62dfaa11 a skos:Concept;
  skos:broader :c_90aedbdc;
  skos:definition "means a method of heating in which the heat source is integral with the hot water vessel. Examples are an electrical immersion heater, or a gas burner with a ﬂue arrangement that passes through the vessel so that the ﬂue transfers heat to the stored water, or the circulation of water from a vessel situated near a burner with a ﬂue arrangement so that the ﬂue transfers heat to the circulating water."@en;
  skos:prefLabel "direct heating"@en .

:c_252b3da8 a skos:Concept;
  skos:broader :c_90aedbdc;
  skos:definition "means water that has been heated for cooking, food preparation, personal washing or cleaning purposes. The term is used irrespective of the type of building in which the hot water system is installed."@en;
  skos:prefLabel "domestic hot water"@en .

:c_36ceda7d a skos:Concept;
  skos:broader :c_90aedbdc;
  skos:definition "means a closet having a movable receptacle for the reception of faecal matter and its deodorisation by the use of earth, ashes or chemicals, or by other methods. This will therefore include chemical and composting toilets."@en .

:skosCollection_50d4bd2e skos:member :c_45847832, :c_4bcbd7aa, :c_e31d69a7 .

:c_8caf9cc1 a skos:Concept;
  skos:broader :c_90aedbdc;
  skos:definition "means the erection of any building or extension of a kind described in regulation 9 of and Schedule 2 to the Building Regulations 2010; or the carrying out of any work to or in connection with such a building or extension, if after the carrying out of that work it is still a building or extension of a kind described in that Schedule."@en;
  skos:prefLabel "exempt buildings and work"@en .

:c_66727700 a skos:Concept;
  skos:broader :c_90aedbdc;
  skos:definition "means a vessel to temporarily accommodate the expansion of water from the unvented hot water storage vessel as it is heated."@en;
  skos:prefLabel "expansion vessel"@en .

:c_e4d9fbd5 a skos:Concept;
  skos:broader :c_90aedbdc;
  skos:definition "is domestic wastewater excluding faecal matter and urine. When appropriately treated this may replace the use of wholesome water in WCs, urinals, irrigation or washing machines."@en;
  skos:prefLabel "greywater"@en .

:c_b1f8943d a skos:Concept;
  skos:broader :c_90aedbdc;
  skos:definition "means rainwater harvested from roofs or other suitable surfaces and collected and stored. When appropriately treated, this may replace the use of wholesome water in WCs, urinals, irrigation or washing machines."@en;
  skos:prefLabel "harvested rainwater"@en .

:c_cb024dd1 a skos:Concept;
  skos:broader :c_90aedbdc;
  skos:definition "means water that, when cold, was wholesome in accordance with the deﬁnition below and has been subjected to a heat source to increase its temperature."@en;
  skos:prefLabel "heated wholesome water"@en .

:c_3f5a9958 a skos:Concept;
  skos:broader :c_90aedbdc;
  skos:definition "means a vessel for storing: a. heated wholesome hot water or softened wholesome hot water for subsequent use b. water that is used to heat other water together with any ancillary safety devices described in paragraphs 3.10 and 3.11 of this Approved Document and all other applicable operating devices."@en;
  skos:prefLabel "hot water storage system"@en .

:c_ced9eb5e a skos:Concept;
  dct:modified "2020-10-26T07:29:02.985Z"^^xsd:dateTime;
  skos:broader :c_90aedbdc;
  skos:definition "means a hot water storage system having the safety devices described in 3.10 and 3.17 of this Approved Document factory-ﬁtted by the manufacturer, together with a kit containing other applicable devices supplied by the manufacturer to be ﬁtted by the installer."@en;
  skos:inScheme :conceptScheme_751925ed;
  skos:prefLabel "hot water storage system package"@en .

:c_86cbd31f a skos:Concept;
  skos:broader :c_90aedbdc;
  skos:definition "means a hot water storage system having the safety devices described in 3.10 and 3.17 of this Approved Document and all other applicable operating devices factory-ﬁtted by the manufacturer."@en;
  skos:prefLabel "hot water storage system unit"@en .

:c_f7036f54 a skos:Concept;
  skos:broader :c_90aedbdc;
  skos:definition "means a method of heating stored water through a heat exchanger."@en;
  skos:prefLabel "indirect heating"@en .

:c_4a4a5b61 a skos:Concept;
  skos:broader :c_90aedbdc;
  skos:definition "means a room or part of a room which contains a sink and food preparation facilities"@en;
  skos:prefLabel "kitchen"@en .

:c_47b084b0 a skos:Concept;
  dct:modified "2020-10-26T07:34:46.172Z"^^xsd:dateTime;
  skos:broader :c_90aedbdc;
  skos:definition "means an alteration which results in a building or a controlled service or ﬁtting not complying with, or being more, means of warning and escape, internal and external ﬁre spread, ﬁre service access and facilities, and access and use."@en;
  skos:inScheme :conceptScheme_751925ed;
  skos:prefLabel "material alteration"@en .

:c_ee888332 a skos:Concept;
  skos:broader :c_90aedbdc;
  skos:definition "means a device that will interrupt the supply of heat to a hot water storage vessel when a ﬁxed (factory set) temperature is exceeded. If this protective device is actuated it should only be possible to reset it manually."@en;
  skos:prefLabel "non-self-resetting energy cut-out"@en .

:c_e47ea7fb a skos:Concept;
  dct:modified "2020-10-26T07:35:00.935Z"^^xsd:dateTime;
  skos:broader :c_90aedbdc;
  skos:definition "means handling, making and cooking of food."@en;
  skos:inScheme :conceptScheme_751925ed;
  skos:prefLabel "preparation of food"@en .

:c_1aa022f8 a skos:Concept;
  dct:modified "2020-10-26T07:28:29.370Z"^^xsd:dateTime;
  skos:broader :c_90aedbdc;
  skos:definition "means a mechanically operated valve that opens to discharge water when a ﬁxed (factory set) pressure is exceeded."@en;
  skos:inScheme :conceptScheme_751925ed;
  skos:prefLabel "pressure relief valve"@en .

:c_0cdb0b97 a skos:Concept;
  dct:modified "2020-10-26T07:35:13.859Z"^^xsd:dateTime;
  skos:broader :c_90aedbdc;
  skos:definition "means a store of heat energy that can be used to heat domestic hot water by means of a heat exchanger. The thermal store can be heated by a variety of heat sources. Primary hot water thermal stores can be either vented or unvented."@en;
  skos:inScheme :conceptScheme_751925ed;
  skos:prefLabel "primary thermal store"@en .

:c_e2afc611 a skos:Concept;
  dct:modified "2020-10-26T07:32:20.075Z"^^xsd:dateTime;
  skos:broader :c_90aedbdc;
  skos:definition "for the purposes of this document means the identiﬁcation of the hazards associated with a process or activity combined with an assessment of the probability and consequences of each hazard."@en;
  skos:inScheme :conceptScheme_751925ed;
  skos:prefLabel "risk assessment"@en .

:c_fec9943e a skos:Concept;
  skos:broader :c_90aedbdc;
  skos:definition "means a room, or a suite of rooms, which is not a dwelling- house or a ﬂat and which is used by one or more persons to live and sleep in, and includes a room in a hostel, a hotel, a boarding house, a hall of residence or a residential home, but does not include a room in a hospital, or other similar establishment, used for patient accommodation.        "@en;
  skos:inScheme :conceptScheme_751925ed .

:c_316d73a9 a skos:Concept;
  dct:modified "2020-10-26T07:39:49.038Z"^^xsd:dateTime;
  skos:broader :c_90aedbdc;
  skos:definition "means a room containing a WC or urinal, whether or not it also contains other sanitary appliances. Sanitary accommodation containing one or more cubicles counts as a single space if there is free circulation of air throughout the space."@en;
  skos:inScheme :conceptScheme_751925ed;
  skos:prefLabel "sanitary accommodation"@en .

:c_f8b75f3a a skos:Concept;
  dct:modified "2020-10-26T07:36:00.668Z"^^xsd:dateTime;
  skos:broader :c_90aedbdc;
  skos:definition "means WC, urinal, bath, shower, washbasin, sink, bidet and drinking fountain. It also includes appliances that are not connected to a water supply (e.g. composting toilet) or drain (e.g. waterless urinal)."@en;
  skos:inScheme :conceptScheme_751925ed;
  skos:prefLabel "sanitary appliance"@en .

:c_1b2db6bc a skos:Concept;
  skos:broader :c_90aedbdc;
  skos:definition "means closets and urinals."@en;
  skos:inScheme :conceptScheme_751925ed .

:c_00af1bc5 a skos:Concept;
  dct:modified "2020-10-25T05:13:52.276Z"^^xsd:dateTime;
  skos:broader :c_90aedbdc;
  skos:definition "means a receptacle used for holding water (for preparation of food or washing up) supplied through a tap and having a wastepipe."@en;
  skos:inScheme :conceptScheme_751925ed;
  skos:prefLabel "sink"@en .

:c_3d59dac9 a skos:Concept;
  skos:broader :c_90aedbdc;
  skos:definition "means water which would be regarded as wholesome for the purposes of regulations made under section 67 of the Water Industry Act 1991 (standards of wholesomeness) as they apply for the purposes of Part G of Schedule 1 in accordance with paragraph (2c) but for the presence of sodium in excess of the level speciﬁed in those regulations if it is caused by a water softener or water softening process which reduces the concentrations of calcium and magnesium."@en;
  skos:inScheme :conceptScheme_751925ed .

:c_e146ab76 skos:definition "is the maximum declared energy output rate (kW) as declared on the appliance data plate."@en .

:c_e31d69a7 a skos:Concept;
  dct:modified "2020-10-25T05:14:01.936Z"^^xsd:dateTime;
  skos:broader :c_90aedbdc;
  skos:definition "means a device, installed in the discharge pipe from a valve, that provides an air break allowing discharge to be conducted safely to a place of termination. The tundish also provides a visible indication of a discharge and functions as backﬂow prevention device."@en;
  skos:inScheme :conceptScheme_751925ed;
  skos:prefLabel "tundish"@en .

:c_4bcbd7aa a skos:Concept;
  dct:modified "2020-10-26T07:40:29.959Z"^^xsd:dateTime;
  skos:broader :c_90aedbdc;
  skos:definition "means a mechanically operated valve that opens to discharge water when a ﬁxed (factory set) temperature is exceeded."@en;
  skos:inScheme :conceptScheme_751925ed;
  skos:prefLabel "temperature relief valve"@en .

:c_fbe47c16 a skos:Concept;
  dct:modified "2020-10-26T07:20:41.669Z"^^xsd:dateTime;
  skos:broader :c_90aedbdc;
  skos:definition "means a vessel fed with cold water from a supply pipe or dedicated storage cistern (without a vent pipe) and in which water is heated directly or indirectly. Expansion of the water when it is heated is accommodated either internally or externally and the system is ﬁtted with safety devices to prevent water temperatures exceeding 100˚C, and other applicable operating devices to control primary ﬂow, prevent backﬂow, control working pressure and accommodate expansion."@en;
  skos:inScheme :conceptScheme_751925ed;
  skos:prefLabel "unvented (closed) hot water storage system"@en .

:c_885de476 a skos:Concept;
  dct:modified "2020-10-25T05:14:32.439Z"^^xsd:dateTime;
  skos:broader :c_90aedbdc;
  skos:definition "means an appliance used for reception and disposal of urine."@en;
  skos:inScheme :conceptScheme_751925ed;
  skos:prefLabel "urinal"@en .

:c_a0d96205 a skos:Concept;
  dct:modified "2020-10-26T07:28:00.179Z"^^xsd:dateTime;
  skos:broader :c_90aedbdc;
  skos:definition "means a vessel fed with cold water from a dedicated storage cistern. Expansion of the water when it is heated is accommodated through the cold feed pipe. A vent pipe connecting the top of the vessel to a point open to the atmosphere above the cold water storage cistern is provided as a safety device."@en;
  skos:inScheme :conceptScheme_751925ed;
  skos:prefLabel "vented (open) hot water storage system"@en .

:c_9d5baa50 a skos:Concept;
  skos:broader :c_90aedbdc;
  skos:definition "means a closet that has a separate ﬁxed receptacle connected to a drainage system and separate provision for ﬂushing from a supply of clean water either by the operation of a mechanism or by automatic action. Water-closets are also referred to as WCs."@en;
  skos:inScheme :conceptScheme_751925ed .

:skosCollection_50d4bd2e skos:member :c_12b20158, :c_7f8af2c2, :c_885de476, :c_a0d96205,
    :c_d39bf581, :c_fbe47c16 .

:c_99150200 a skos:Concept;
  dct:modified "2020-10-26T07:30:33.748Z"^^xsd:dateTime;
  skos:broader :c_90aedbdc;
  skos:definition "means water complying  with the requirements of regulations made under Section 67 (Standards of wholesomeness) of the Water Industry Act 1991. The regulations made under this Section at the time of publication Regulations 2000 (SI 2000/3184 as amended),and, for Wales, the Water Supply (Water Quality) Regulations 2001 (SI 2001/3911 as amended)."@en;
  skos:inScheme :conceptScheme_751925ed;
  skos:prefLabel "wholesome water"@en .

:c_a1430501 skos:inScheme :conceptScheme_751925ed .

:c_70908a07 dct:modified "2020-10-26T06:59:49.089Z"^^xsd:dateTime .

:c_39f68990 dct:modified "2020-10-26T07:43:22.855Z"^^xsd:dateTime;
  skos:inScheme :conceptScheme_751925ed .

:c_8caf9cc1 dct:modified "2020-10-26T07:29:45.865Z"^^xsd:dateTime;
  skos:inScheme :conceptScheme_751925ed .

:c_3f5a9958 dct:modified "2020-10-26T07:30:48.875Z"^^xsd:dateTime;
  skos:inScheme :conceptScheme_751925ed .

:c_b1f8943d dct:modified "2020-10-26T07:27:31.748Z"^^xsd:dateTime;
  skos:inScheme :conceptScheme_751925ed .

:c_e4d9fbd5 dct:modified "2020-10-26T07:40:45.571Z"^^xsd:dateTime;
  skos:inScheme :conceptScheme_751925ed .

:c_252b3da8 dct:modified "2020-10-26T07:33:40.695Z"^^xsd:dateTime;
  skos:inScheme :conceptScheme_751925ed .

:c_62dfaa11 dct:modified "2020-10-26T07:42:24.653Z"^^xsd:dateTime;
  skos:inScheme :conceptScheme_751925ed .

:c_0822f77e skos:inScheme :conceptScheme_751925ed .

:c_152c4bbc a skos:Concept;
  dct:created "2020-10-25T05:44:27.690Z"^^xsd:dateTime;
  dct:modified "2020-10-25T06:30:47.310Z"^^xsd:dateTime;
  skos:broader :c_710680da;
  skos:definition "The following definitions have been adopted solely for the purposes of providing clarity in this Approved Document."@en;
  skos:inScheme :conceptScheme_751925ed;
  skos:narrower :c_e146ab76;
  skos:notation "1.4"@en;
  skos:prefLabel "explanation of terms used"@en .

:c_36ceda7d skos:inScheme :conceptScheme_751925ed .

:c_f7036f54 dct:modified "2020-10-26T07:26:46.645Z"^^xsd:dateTime;
  skos:inScheme :conceptScheme_751925ed .

:c_cb024dd1 dct:modified "2020-10-26T07:19:05.888Z"^^xsd:dateTime;
  skos:inScheme :conceptScheme_751925ed .

:c_4a4a5b61 dct:modified "2020-10-25T05:15:00.041Z"^^xsd:dateTime;
  skos:inScheme :conceptScheme_751925ed .

:c_66727700 dct:modified "2020-10-26T07:40:15.158Z"^^xsd:dateTime;
  skos:inScheme :conceptScheme_751925ed .

:c_86cbd31f dct:modified "2020-10-26T07:26:00.678Z"^^xsd:dateTime;
  skos:inScheme :conceptScheme_751925ed .

:c_ee888332 dct:modified "2020-10-26T07:21:33.767Z"^^xsd:dateTime;
  skos:inScheme :conceptScheme_751925ed .

:c_90aedbdc dct:modified "2020-10-25T05:16:53.211Z"^^xsd:dateTime;
  skos:narrower :c_00af1bc5, :c_0822f77e, :c_1b2db6bc, :c_252b3da8, :c_36ceda7d, :c_39f68990,
    :c_3d59dac9, :c_3f5a9958, :c_47b084b0, :c_4a4a5b61, :c_4bcbd7aa, :c_62dfaa11, :c_66727700,
    :c_86cbd31f, :c_885de476, :c_8caf9cc1, :c_99150200, :c_9d5baa50, :c_a0d96205, :c_a1430501,
    :c_b1f8943d, :c_cb024dd1, :c_ced9eb5e, :c_e31d69a7, :c_e4d9fbd5, :c_ee888332, :c_f7036f54,
    :c_f8b75f3a, :c_fbe47c16, :c_fec9943e .

:c_f6ff7c1c dct:modified "2020-10-25T05:28:02.128Z"^^xsd:dateTime;
  skos:definition """The Building Regulations 2010 (SI 2010/2214),
which came into operation on 1 October 2010,
replace the Building Regulations 2000 (SI 2000/2531)
and consolidate all subsequent revisions to those
regulations. This document is one of a series that
has been approved and issued by the Secretary
of State for the purpose of providing practical
guidance with respect to the requirements of
Schedule 1 to and Regulation 7 of the Building
Regulations 2010 for England and Wales."""@en .

:c_679215e0 a skos:Concept;
  dct:modified "2020-10-25T05:21:08.543Z"^^xsd:dateTime;
  skos:broader :c_42d467db;
  skos:inScheme :conceptScheme_751925ed;
  skos:prefLabel "drainage and waste disposal 2015 edition"@en .

:c_44c61ce8 dct:modified "2020-10-25T05:26:12.088Z"^^xsd:dateTime;
  skos:definition """This document has been approved by the
Secretary of State to provide practical guidance
on ways of complying with the requirements in
Part F of Schedule 1 to, and regulations 39, 42
and 44 (in so far as it relates to fixed systems
for mechanical ventilation) of, the Building
Regulations 2010 (SI 2010/2214) for England
and Wales, and regulations 20(1) and 20(6) (in so
far as it relates to fixed systems for mechanical
ventilation) of the Building (Approved Inspectors
etc) Regulations 2010 (SI 2010/2215) for England
and Wales. The Building Regulations 2010
and the Building (Approved Inspectors etc)
Regulations 2010 are referred to throughout
the remainder of this document as ‘the Building
Regulations’ and ‘the Approved Inspectors
Regulations’ respectively."""@en .

:c_73c4361e dct:modified "2020-10-25T05:23:12.369Z"^^xsd:dateTime .

:c_4e975ede dct:modified "2020-10-25T05:31:08.927Z"^^xsd:dateTime .

:c_6d6d73cd dct:modified "2020-10-25T05:25:19.058Z"^^xsd:dateTime;
  skos:definition """This document has been approved and issued
by the Secretary of State to provide practical
guidance on ways of complying with Requirements G1 to G6 and regulations 7 and 36 of the Building
Regulations 2010 (SI 2010/2214) for England and
Wales, as amended. The Building Regulations
2010 are referred to throughout the remainder
of this Document as ‘the Building Regulations’.
Where appropriate the Approved Document also
gives guidance on relevant requirements in the
Building (Approved Inspectors etc.) Regulations
2010 (SI 2010/2215)."""@en .

:c_12c47f28 skos:definition """This document is one of a series that has been
approved by the First Secretary of State for the
purpose of providing practical guidance with
respect to the requirements of Schedule 1 to and
Regulation 7 of the Building Regulations 2010
(SI 2010/2214) for England and Wales."""@en .

:c_710680da a skos:Concept;
  dct:created "2020-10-25T05:35:17.135Z"^^xsd:dateTime;
  dct:modified "2020-10-25T05:45:02.801Z"^^xsd:dateTime;
  skos:broader :c_fec1533e;
  skos:definition """This document has been approved and issued
by the Secretary of State to provide practical
guidance on ways of complying with Requirements
J1 to J7 and regulations 7 of the Building
Regulations 2010 (SI 2010/2214) for England
and Wales. The Building Regulations 2010 are
referred to throughout the remainder of this
Document as ‘the Building Regulations’. Where
appropriate the Approved Document also gives
guidance on relevant requirements in the Building
(Approved Inspectors etc) Regulations 2010
(SI 2010/2215)."""@en;
  skos:inScheme :conceptScheme_751925ed;
  skos:narrower :c_152c4bbc;
  skos:prefLabel "combustion appliances and fuel storage systems 2010 edition incorporating 2010 and 2013 amendments"@en .

:c_fec1533e dct:modified "2020-10-25T05:36:43.835Z"^^xsd:dateTime;
  skos:narrower :c_710680da .

:c_3b6a6b21 dct:modified "2020-10-26T07:26:32.046Z"^^xsd:dateTime;
  skos:prefLabel "solid biofuel"@en .

:c_be620037 a skos:Concept;
  skos:broader :c_152c4bbc;
  skos:definition "is an enclosure specifically constructed or adapted to accommodate one or more combustion appliances."@en;
  skos:prefLabel "appliance compartment"@en .

:c_3fa58f37 a skos:Concept;
  skos:broader :c_152c4bbc;
  skos:definition "is a method of installing an open-flued appliance into a compartment which is sealed from the remainder of the building and whose ventilation is so arranged in conjunction with the appliance flue as to achieve a balanced flue effect."@en;
  skos:prefLabel "balanced compartment"@en .

:c_2ea90bc3 a skos:Concept;
  skos:broader :c_152c4bbc;
  skos:definition "appliance is a type of room- sealed appliance which draws its combustion air from a point outside the building adjacent to the point at which the combustion products are discharged, the inlet and outlet being so disposed that wind effects are substantially balanced. Balanced flues may run vertically, but in the most common configuration they discharge horizontally through the external wall against which the appliance is situated."@en;
  skos:prefLabel "balanced flue"@en .

:c_0de6ed98 a skos:Concept;
  skos:broader :c_152c4bbc;
  skos:definition "is the boundary of the land or buildings belonging to and under the control of the building owner. Depending upon the paragraphs of this Approved Document to which it applies, it may be drawn only around the perimeter of the land in question or extended to the centreline of adjacent routes or waterways as shown in Diagram 1."@en;
  skos:prefLabel "boundary"@en .

:c_3e30efaf a skos:Concept;
  skos:broader :c_152c4bbc;
  skos:definition "is a body that carries out checks for compliance with the Building Regulations on plans of building work and on the building work itself. The Building Control Body may be either the local authority or an Approved Inspector. For further details, see the manual to the Building Regulations."@en;
  skos:prefLabel "building control body"@en .

:c_8c3e4b6f a skos:Concept;
  skos:broader :c_152c4bbc;
  skos:definition "The of an oil tank is its nominal capacity as stated by the manufacturer. It is usually 95 per cent of the volume of liquid required to fill it to the brim."@en;
  skos:prefLabel "capacity"@en .

:c_4a83bd38 a skos:Concept;
  skos:broader :c_152c4bbc;
  skos:definition " is a structure consisting of a wall or walls enclosing one or more flues (see Diagram 2). In the gas industry, the chimney for a gas appliance is commonly called the flue."@en;
  skos:prefLabel "chimney"@en .

:c_cf1e8e52 a skos:Concept;
  skos:broader :c_152c4bbc;
  skos:definition " is an apparatus where fuel is burned to generate heat for space heating, water heating, cooking or other similar purpose. The appliance does not include systems to deliver fuel to it or for the distribution of heat. Typical combustion appliances are boilers, warm air heaters, water heaters, fires, stoves and cookers."@en;
  skos:prefLabel "combustion appliance (or appliance)"@en .

:c_7390c895 a skos:Concept;
  skos:broader :c_152c4bbc;
  skos:definition "in BS EN 1443:2003 expresses the performance characteristics of a chimney or its components, as assessed in accordance with an appropriate European product standard, by means of a code such as EN 1234 – T400 N1 D1 Gxx. Further information is given in Appendix G."@en;
  skos:prefLabel "designation system"@en .

:c_ee1dbf01 a skos:Concept;
  skos:broader :c_152c4bbc;
  skos:definition "is an opening formed by a factory-made component into any part of the flue serving an open-flued appliance. Such openings may be provided to allow dilution air to be drawn into a flue or to lessen the effects of down-draught on combustion in the appliance"@en;
  skos:prefLabel "draught break"@en .

:c_119d7903 a skos:Concept;
  skos:broader :c_152c4bbc;
  skos:definition "is a form of draught break intended to prevent conditions in the main length of flue from interfering with the combustion performance of an open-flued appliance (see Diagram 3(a)). It allows the appliance to operate without interference from down- draughts that may occur in adverse wind conditions and excessive draught."@en;
  skos:prefLabel "draught diverter"@en .

:c_bfc3ac08 a skos:Concept;
  skos:broader :c_152c4bbc;
  skos:definition "is a factory-made counter-balanced flap device admitting air to the flue, from the same space as the combustion air, to prevent excessive variations in the draught (see Diagram 3(b)). It is usual for these to be in the fluepipe or chimney, but they may be located on the appliance."@en;
  skos:prefLabel "draught stabiliser"@en .

:c_d55b06b8 a skos:Concept;
  skos:broader :c_152c4bbc;
  skos:definition "is defined in BS EN 13141 -1:2004 as the area of a sharp-edged circular orifice which would pass the same air flow rate at the same applied pressure difference as the product or device being tested. The equivalent area of a simple ventilator will be less than the geometrical free area and for complex products may be significantly less."@en;
  skos:prefLabel "equivalent area"@en .

:c_0ef5294b a skos:Concept;
  skos:broader :c_152c4bbc;
  skos:definition "are prefabricated chimneys that are commonly manufactured as sets of components for assembly on site (although they can be supplied as one unit), having the performance appropriate for the intended appliance. They are available in various materials and types ranging from single-walled metal chimneys suitable for some gas appliances to twin-walled chimneys with insulation sandwiched between an inner liner and an outer metal wall which are designed for oil or solid fuel use."@en;
  skos:prefLabel "factory-made metal chimneys (also known as system chimneys)"@en .

:c_17d58c6d a skos:Concept;
  skos:broader :c_152c4bbc;
  skos:definition "the proper discharge of the flue gases depends upon the operation of a fan, which may be separately installed in the flue or may be an integral part of the combustion appliance. Fans in combustion appliances either may extract flue gases from the combustion chamber or may cause the flue gases to be displaced from the combustion chamber if the fan is supplying it with air for combustion. Appliances with fans providing the combustion air (including most oil-fired and many gas- fired boilers) are also commonly referred to as forced draught appliances (see Diagram 4). Flues in fanned draught installations run horizontally or vertically and can be at higher or lower pressures than their surroundings, dependent upon the location of the fan."@en;
  skos:prefLabel "fanned draught installation"@en .

:c_ed23b7cc a skos:Concept;
  skos:broader :c_152c4bbc;
  skos:definition "is a building or part of a building comprising one or more rooms, spaces or storeys constructed to prevent the spread of fire to or from another part of the same building or an adjoining building. (A roof-10. space above the top storey of a fire compartment is included in that fire compartment.) "@en;
  skos:prefLabel "fire compartment"@en .

:c_870f938c a skos:Concept;
  dct:modified "2020-10-26T07:21:50.256Z"^^xsd:dateTime;
  skos:broader :c_152c4bbc;
  skos:definition "of a building is a form of compartmentation in which part of a building is separated from another part of the same building by a compartment wall. Such walls run the full height of the part and are in one vertical plane. Further information on this is given in Approved Document B Vol 2 (see Section 8 Compartmentation and Appendix C Methods of Measurement)."@en;
  skos:inScheme :conceptScheme_751925ed;
  skos:prefLabel "separated part"@en .

:c_45847832 a skos:Concept;
  dct:modified "2020-10-26T07:45:06.786Z"^^xsd:dateTime;
  skos:broader :c_152c4bbc;
  skos:definition "is a structural opening (sometimes called a builder’s opening) formed in a wall or in a chimney breast, from which a chimney leads and which has a hearth at its base. Simple structural openings (Diagram 5(a)) are suitable for closed appliances such as stoves, cookers or boilers, but gathers (Diagram 5(b)) are necessary for accommodating open fires. Fireplace recesses are often lined with firebacks to accommodate inset open fires (Diagram 5(c)). Lining components and decorative treatments fitted around openings reduce the opening area. It is the finished fireplace opening area which determines the size of flue required for an open fire in such a recess."@en;
  skos:inScheme :conceptScheme_751925ed;
  skos:prefLabel "fireplace recess"@en .

:c_9ab3dc4c a skos:Concept;
  skos:broader :c_152c4bbc;
  skos:definition "of a component or construction is a measure of its ability to withstand the effects of fire in one or more ways for a stated period of time. Guidance on determination of performance in terms of fire resistance is given in Approved Document B (Fire Safety)."@en;
  skos:prefLabel "fire resistance"@en .

:c_3a3a6363 a skos:Concept;
  skos:broader :c_152c4bbc;
  skos:definition "is a means of shielding a fuel tank from the thermal radiation from a fire. For  LPG tanks, it also ensures that gas accidentally leaking from the tank or fittings must travel by a longer path and therefore disperse safely, before reaching a hazard such as an opening in a building, a boundary or other potential ignition source."@en;
  skos:prefLabel "fire wall"@en .

:c_12b20158 a skos:Concept;
  dct:modified "2020-10-25T06:27:16.350Z"^^xsd:dateTime;
  skos:broader :c_152c4bbc;
  skos:definition "is a passage that conveys the products of combustion from an appliance to the outside air (see Diagram 2)."@en;
  skos:inScheme :conceptScheme_751925ed;
  skos:prefLabel "flue"@en .

:c_3a623af3 a skos:Concept;
  skos:broader :c_152c4bbc;
  skos:definition "systems consist of a set of factory-made components, made from precast concrete, clay or other masonry units, that are designed for assembly on site to provide a complete chimney having the performance appropriate for the intended appliance. There are two types of common systems, one being solely for use with gas- burning appliances and the other, often called chimney block systems, being primarily designed for solid fuel-burning appliances."@en;
  skos:prefLabel "flueblock chimney"@en .

:c_7f8af2c2 a skos:Concept;
  skos:broader :c_152c4bbc;
  skos:definition "is a factory made unit, usually made of metal, which is similar to a prefabricated appliance chamber except that it is designed to accommodate a gas burning appliance in conjunction with a factory-made chimney."@en;
  skos:prefLabel "flue box"@en .

:c_9e940521 a skos:Concept;
  dct:modified "2020-10-26T07:41:44.182Z"^^xsd:dateTime;
  skos:broader :c_152c4bbc;
  skos:definition "is one which is designed to be used without connection to a flue. Its products of combustion mix with the surrounding room air and are eventually transported to the outside as stale air leaves the room (see Diagram 4(g))."@en;
  skos:inScheme :conceptScheme_751925ed;
  skos:prefLabel "flueless appliance"@en .

:c_e9c0c7da a skos:Concept;
  dct:modified "2020-10-26T07:31:18.401Z"^^xsd:dateTime;
  skos:broader :c_152c4bbc;
  skos:definition "is the wall of the chimney that is in contact with the products of combustion (see Diagram 2), such as a concrete flue liner, the inner liner of a factory-made chimney system or a flexible liner fitted into an existing chimney."@en;
  skos:inScheme :conceptScheme_751925ed;
  skos:prefLabel "flue liner"@en .

:c_873f1974 a skos:Concept;
  dct:modified "2020-10-26T07:43:06.458Z"^^xsd:dateTime;
  skos:broader :c_152c4bbc;
  skos:definition "is the point at which the products of combustion are discharged from the flue to the outside atmosphere, such as the top of a chimney pot or flue terminal."@en;
  skos:inScheme :conceptScheme_751925ed;
  skos:prefLabel "flue outlet"@en .

:c_dcbadafe a skos:Concept;
  dct:modified "2020-10-25T06:28:21.890Z"^^xsd:dateTime;
  skos:broader :c_152c4bbc;
  skos:definition "is a pipe, either single walled (bare or insulated) or double walled, which connects a combustion appliance to a flue in a chimney. For clarity, when used in this way, it may be called a connecting fluepipe. (Fluepipe is also used to describe the tubular components from which some factory made chimneys for gas and oil appliances are made or from which plastic flue systems are made)."@en;
  skos:inScheme :conceptScheme_751925ed;
  skos:prefLabel "fluepipe"@en .

:c_229f83e8 a skos:Concept;
  dct:modified "2020-10-26T07:24:13.103Z"^^xsd:dateTime;
  skos:broader :c_152c4bbc;
  skos:definition "is a base intended to safely isolate a combustion appliance from people, combustible parts of the building fabric and soft furnishings. The exposed surface of the hearth provides a region around the appliance which can be kept clear of anything at risk of fire. The body of the hearth may be thin insulating board, a substantial thickness of material such as concrete or some intermediate provision dependent upon the weight and downward heat emission characteristics of the appliance(s) upon it (see Diagram 6)."@en;
  skos:inScheme :conceptScheme_751925ed;
  skos:prefLabel "hearth"@en .

:c_22c38d73 a skos:Concept;
  dct:modified "2020-10-26T07:22:24.968Z"^^xsd:dateTime;
  skos:broader :c_152c4bbc;
  skos:definition "is the maximum rate of energy flow into an appliance. It is calculated as the rate of fuel flow to the appliance multiplied by either the fuel’s gross or net calorific value."@en;
  skos:inScheme :conceptScheme_751925ed;
  skos:prefLabel "heat input rate"@en .

:c_53d35017 a skos:Concept;
  dct:modified "2020-10-26T07:35:44.265Z"^^xsd:dateTime;
  skos:broader :c_152c4bbc;
  skos:definition "are those instructions produced by manufacturers to enable installers to correctly install and test appliances and flues and to commission them into service."@en;
  skos:inScheme :conceptScheme_751925ed;
  skos:prefLabel "installation instructions"@en .

:c_41ebf78a a skos:Concept;
  dct:modified "2020-10-25T06:28:31.179Z"^^xsd:dateTime;
  skos:broader :c_152c4bbc;
  skos:definition "the combustion products flow into the flue as a result of the draught produced due to the difference between the temperature of the gases within the flue and the temperature of the ambient air. Taller flues produce a greater draught at their base. Except for those balanced flue appliances which are designed to discharge directly through the wall adjacent to the appliance, a satisfactory natural draught requires an essentially vertical run of flue (see Diagram 4 (a) and (b))."@en;
  skos:inScheme :conceptScheme_751925ed;
  skos:prefLabel "natural draught flue"@en .

:c_ad9a7d0c a skos:Concept;
  dct:modified "2020-10-25T06:28:05.847Z"^^xsd:dateTime;
  skos:broader :c_152c4bbc;
  skos:definition "This is the highest level of reaction to fire performance. Non-combustible materials include: a. any material which when tested to BS 476-11:1982 (2007) does not flame nor cause any rise in temperature on either the centre (specimen) or furnace thermocouples; and b. products classified as non-combustible in tests following the procedures in BS 476-4:1970 (2007); c. any material classified as class A1 in accordance with BS EN 13501-1:2002 Fire classification of construction products and building elements. Classification using data from reaction to fire tests. Typical examples of such materials to be found in buildings include totally inorganic materials such as concrete, fired clay, ceramics, metals, plaster and masonry containing not more than 1 per cent by weight or volume of organic material. (Use in buildings of combustible metals such as magnesium–aluminium alloys should be assessed in each individual case.) More detailed information is given in Approved Document B (Fire Safety)."@en;
  skos:inScheme :conceptScheme_751925ed;
  skos:prefLabel "non-combustible material"@en .

:c_d39bf581 a skos:Concept;
  dct:modified "2020-10-25T06:27:28.765Z"^^xsd:dateTime;
  skos:broader :c_152c4bbc;
  skos:definition "for the purposes of the Gas Appliances (Safety) Regulations (1995), means: a. a. a body which is approved by the Secretary of State for Trade and Industry as being competent to carry out the required Attestation procedures for gas appliances and whose name and identification number has been notified by him/her to the Commission of the European Community and to other member States in accordance with the Gas Appliances (Safety) Regulations (1995); b. b. a body which has been similarly approved for the purposes of the Gas Appliances Directive by another member State and whose name and identification number has been notified to the Commission and to other member States pursuant to the Gas Appliances Directive."@en;
  skos:inScheme :conceptScheme_751925ed;
  skos:prefLabel "notified body"@en .

:c_22764bab a skos:Concept;
  dct:modified "2020-10-26T07:24:24.540Z"^^xsd:dateTime;
  skos:broader :c_152c4bbc;
  skos:definition "is one which draws its combustion air from the room or space within which it is installed and which requires a flue to discharge its products of combustion to the outside air (see Diagram 4 (a), (c) and (e))."@en;
  skos:inScheme :conceptScheme_751925ed;
  skos:prefLabel "open-flued appliance"@en .

:c_d67339c2 a skos:Concept;
  dct:modified "2020-10-26T07:34:19.568Z"^^xsd:dateTime;
  skos:broader :c_152c4bbc;
  skos:definition "is a set of factory-made precast concrete components designed to provide a fireplace recess to accommodate an appliance such as a stove, and incorporates a gather when used with an open fire. The chamber is normally positioned against a wall and may be designed to support a chimney. The chamber and chimney are often enclosed to create a false chimney breast (see also ‘flue box’)."@en;
  skos:inScheme :conceptScheme_751925ed;
  skos:prefLabel "prefabricated appliance chamber"@en .

:c_a794f4c0 a skos:Concept;
  dct:modified "2020-10-26T07:21:19.736Z"^^xsd:dateTime;
  skos:broader :c_152c4bbc;
  skos:definition "(sometimes shortened to rated input) for a gas appliance is the maximum heat input rate at which it can be operated, as declared on the appliance data plate. (See also heat input rate.)"@en;
  skos:inScheme :conceptScheme_751925ed;
  skos:prefLabel "rated heat input"@en .

:c_e146ab76 a skos:Concept;
  skos:broader :c_152c4bbc;
  skos:inScheme :conceptScheme_751925ed;
  skos:prefLabel "rated heat output for an oil appliance"@en .

:skosCollection_50d4bd2e skos:member :c_0ab83009, :c_2d35a0e4, :c_9d5baa50 .

:c_75f221c0 a skos:Concept;
  dct:modified "2020-10-26T07:32:58.549Z"^^xsd:dateTime;
  skos:broader :c_152c4bbc;
  skos:definition "for a solid fuel appliance is the manufacturer’s declared nominal energy output rate (kW) for the appliance. This may be different for different fuels."@en;
  skos:inScheme :conceptScheme_751925ed;
  skos:prefLabel "rated heat output for a solid fuel appliance"@en .

:c_0ab83009 a skos:Concept;
  dct:modified "2020-10-26T07:19:27.005Z"^^xsd:dateTime;
  skos:broader :c_152c4bbc;
  skos:definition "means an appliance whose combustion system is sealed from the room in which the appliance is located and which obtains air for combustion from a ventilated uninhabited space within the building or directly from the open air outside the building and which vents the products of combustion directly to open air outside the building (see Diagram 4 (b), (d) and (f))."@en;
  skos:inScheme :conceptScheme_751925ed;
  skos:prefLabel "room-sealed appliance"@en .

:c_3b6a6b21 a skos:Concept;
  skos:broader :c_152c4bbc;
  skos:definition "means, for the purpose of this Approved Document, a solid fuel derived from plants and trees. It can include logs, wood chips, wood pellets and other processed plant material."@en;
  skos:inScheme :conceptScheme_751925ed .

:c_152c4bbc skos:narrower :c_0ab83009, :c_0de6ed98, :c_0ef5294b, :c_119d7903, :c_12b20158,
    :c_17d58c6d, :c_22764bab, :c_229f83e8, :c_22c38d73, :c_2ea90bc3, :c_3a3a6363, :c_3a623af3,
    :c_3b6a6b21, :c_3e30efaf, :c_3fa58f37, :c_41ebf78a, :c_45847832, :c_4a83bd38, :c_53d35017,
    :c_7390c895, :c_75f221c0, :c_7f8af2c2, :c_870f938c, :c_873f1974, :c_8c3e4b6f, :c_9ab3dc4c,
    :c_9e940521, :c_a794f4c0, :c_ad9a7d0c, :c_be620037, :c_bfc3ac08, :c_cf1e8e52, :c_d39bf581,
    :c_d55b06b8, :c_d67339c2, :c_dcbadafe, :c_e9c0c7da, :c_ed23b7cc, :c_ee1dbf01 .

:c_01839084 a skos:Concept;
  dct:modified "2020-10-25T06:27:56.486Z"^^xsd:dateTime;
  skos:broader :c_152c4bbc;
  skos:definition "is a contracted part of the flue between a fireplace recess and its chimney (see Diagram 22). Throats are usually formed from prefabricated components as shown in Diagram 29."@en;
  skos:inScheme :conceptScheme_751925ed;
  skos:prefLabel "throat"@en .

:c_cf1e8e52 dct:modified "2020-10-26T07:43:35.566Z"^^xsd:dateTime;
  skos:inScheme :conceptScheme_751925ed .

:c_bfc3ac08 dct:modified "2020-10-26T07:33:53.775Z"^^xsd:dateTime;
  skos:inScheme :conceptScheme_751925ed .

:c_0de6ed98 dct:modified "2020-10-25T06:27:22.230Z"^^xsd:dateTime;
  skos:inScheme :conceptScheme_751925ed .

:c_2ea90bc3 dct:modified "2020-10-26T07:18:32.123Z"^^xsd:dateTime;
  skos:inScheme :conceptScheme_751925ed .

:c_17d58c6d dct:modified "2020-10-25T06:27:31.963Z"^^xsd:dateTime;
  skos:inScheme :conceptScheme_751925ed .

:c_0ef5294b dct:modified "2020-10-26T07:39:08.805Z"^^xsd:dateTime;
  skos:inScheme :conceptScheme_751925ed .

:c_3a3a6363 dct:modified "2020-10-26T07:30:00.294Z"^^xsd:dateTime;
  skos:inScheme :conceptScheme_751925ed .

:c_3fa58f37 dct:modified "2020-10-26T07:32:06.808Z"^^xsd:dateTime;
  skos:inScheme :conceptScheme_751925ed .

:c_ee1dbf01 dct:modified "2020-10-26T07:38:24.827Z"^^xsd:dateTime;
  skos:inScheme :conceptScheme_751925ed .

:c_119d7903 dct:modified "2020-10-26T07:37:41.839Z"^^xsd:dateTime;
  skos:inScheme :conceptScheme_751925ed .

:c_9ab3dc4c dct:modified "2020-10-26T07:29:18.306Z"^^xsd:dateTime;
  skos:inScheme :conceptScheme_751925ed .

:c_d55b06b8 dct:modified "2020-10-26T07:34:33.284Z"^^xsd:dateTime;
  skos:inScheme :conceptScheme_751925ed .

:c_be620037 dct:modified "2020-10-26T07:42:11.041Z"^^xsd:dateTime;
  skos:inScheme :conceptScheme_751925ed .

:c_8c3e4b6f dct:modified "2020-10-25T06:28:38.650Z"^^xsd:dateTime;
  skos:inScheme :conceptScheme_751925ed .

:c_4a83bd38 dct:modified "2020-10-26T07:42:36.954Z"^^xsd:dateTime;
  skos:inScheme :conceptScheme_751925ed .

:c_7390c895 dct:modified "2020-10-26T07:23:55.969Z"^^xsd:dateTime;
  skos:inScheme :conceptScheme_751925ed .

:c_3a623af3 dct:modified "2020-10-26T07:34:07.183Z"^^xsd:dateTime;
  skos:inScheme :conceptScheme_751925ed .

:c_7f8af2c2 dct:modified "2020-10-26T07:41:01.784Z"^^xsd:dateTime;
  skos:inScheme :conceptScheme_751925ed .

:c_3e30efaf dct:modified "2020-10-25T07:06:05.116Z"^^xsd:dateTime;
  skos:inScheme :conceptScheme_751925ed .

:c_ed23b7cc dct:modified "2020-10-26T07:43:47.723Z"^^xsd:dateTime;
  skos:inScheme :conceptScheme_751925ed .

:c_0822f77e dct:modified "2020-10-26T07:32:45.968Z"^^xsd:dateTime;
  skos:editorialNote """Note: Terms shown with * are defined in
legislation, either in the Building Act 1984 or the
Building Regulations 2010, where the definition
may be fuller than the definition given here."""@en;
  skos:notation "*"@en .

:c_36ceda7d dct:modified "2020-10-26T07:44:45.155Z"^^xsd:dateTime;
  skos:editorialNote """Note: Terms shown with * are defined in
legislation, either in the Building Act 1984 or the
Building Regulations 2010, where the definition
may be fuller than the definition given here."""@en;
  skos:notation "*"@en;
  skos:prefLabel "earth-closet"@en .

:skosCollection_50d4bd2e skos:member :c_00af1bc5, :c_01839084, :c_0822f77e, :c_0cdb0b97,
    :c_0de6ed98, :c_0ef5294b, :c_119d7903, :c_17d58c6d, :c_1aa022f8, :c_1b2db6bc, :c_22764bab,
    :c_229f83e8, :c_22c38d73, :c_252b3da8, :c_2ea90bc3, :c_316d73a9, :c_36ceda7d, :c_39f68990,
    :c_3a3a6363, :c_3a623af3, :c_3b6a6b21, :c_3e30efaf, :c_3f5a9958, :c_3fa58f37, :c_41ebf78a,
    :c_47b084b0, :c_4a4a5b61, :c_4a83bd38, :c_53d35017, :c_62dfaa11, :c_66727700, :c_7390c895,
    :c_75f221c0, :c_86cbd31f, :c_870f938c, :c_873f1974, :c_8c3e4b6f, :c_8caf9cc1, :c_99150200,
    :c_9ab3dc4c, :c_9e940521, :c_a1430501, :c_a5feab63, :c_a794f4c0, :c_b1f8943d, :c_be620037,
    :c_bfc3ac08, :c_cb024dd1, :c_ced9eb5e, :c_cf1e8e52, :c_d55b06b8, :c_d67339c2, :c_dcbadafe,
    :c_e146ab76, :c_e2afc611, :c_e47ea7fb, :c_e4d9fbd5, :c_e9c0c7da, :c_ed23b7cc, :c_ee1dbf01,
    :c_ee888332, :c_f7036f54, :c_f8b75f3a, :c_fec9943e .

:c_fec9943e dct:modified "2020-10-26T07:24:49.568Z"^^xsd:dateTime;
  skos:editorialNote """Note: Terms shown with * are defined in
legislation, either in the Building Act 1984 or the
Building Regulations 2010, where the definition
may be fuller than the definition given here."""@en;
  skos:notation "*"@en;
  skos:prefLabel "room for residential purposes"@en .

:c_1b2db6bc dct:modified "2020-10-26T07:28:14.032Z"^^xsd:dateTime;
  skos:editorialNote """Note: Terms shown with * are defined in
legislation, either in the Building Act 1984 or the
Building Regulations 2010, where the definition
may be fuller than the definition given here."""@en;
  skos:notation "*"@en;
  skos:prefLabel "sanitary convenience"@en .

:c_3d59dac9 dct:modified "2020-10-26T07:41:15.460Z"^^xsd:dateTime;
  skos:editorialNote """Note: Terms shown with * are defined in
legislation, either in the Building Act 1984 or the
Building Regulations 2010, where the definition
may be fuller than the definition given here."""@en;
  skos:notation "*"@en;
  skos:prefLabel "softened wholesome water"@en .

:c_9d5baa50 dct:modified "2020-10-26T07:37:00.801Z"^^xsd:dateTime;
  skos:editorialNote """Note: Terms shown with * are defined in
legislation, either in the Building Act 1984 or the
Building Regulations 2010, where the definition
may be fuller than the definition given here."""@en;
  skos:notation "*"@en;
  skos:prefLabel "water-closet (wc)"@en .

:c_e146ab76 dct:modified "2020-10-25T07:03:16.838Z"^^xsd:dateTime .

:c_16ea33d2 a skos:Concept;
  dct:created "2020-10-25T08:38:05.473Z"^^xsd:dateTime;
  dct:modified "2020-10-25T08:41:26.894Z"^^xsd:dateTime;
  skos:broader :c_be604dfa;
  skos:definition """* This approved document gives guidance for compliance with the Building Regulations for building
work carried out in England. It also applies to building work carried out on excepted energy
buildings in Wales as defined in the Welsh Ministers (Transfer of Functions) (No. 2) Order 2009."""@en;
  skos:inScheme :conceptScheme_751925ed;
  skos:narrower :c_b7d8c7ee;
  skos:prefLabel "protection from falling, collision and impact 2013 edition – for use in England*"@en .

:c_be604dfa dct:modified "2020-10-25T08:38:34.390Z"^^xsd:dateTime;
  skos:narrower :c_16ea33d2 .

:c_b7d8c7ee a skos:Concept;
  dct:created "2020-10-25T08:40:53.062Z"^^xsd:dateTime;
  skos:broader :c_16ea33d2;
  skos:definition "The following are key terms used in this document:"@en;
  skos:inScheme :conceptScheme_751925ed;
  skos:prefLabel "appendix a: key terms (adk)"@en .

:c_2d35a0e4 a skos:Concept;
  skos:broader :c_b7d8c7ee;
  skos:definition "An entrance which is accessible to people regardless of disability, age or gender."@en;
  skos:prefLabel "accessible entrance"@en .

:c_d3c63474 a skos:Concept;
  skos:broader :c_b7d8c7ee;
  skos:definition "A stair with paddle-shaped treads where the wide portion is on alternate sides on consecutive treads (see paragraphs 1.29 and 1.30)."@en;
  skos:prefLabel "alternating tread stair"@en .

:c_c9535965 a skos:Concept;
  skos:broader :c_b7d8c7ee;
  skos:definition "A structure – either a raised rail or a solid wall – that denies access to another area."@en;
  skos:prefLabel "barrier"@en .

:c_bf5868a2 a skos:Concept;
  skos:broader :c_b7d8c7ee;
  skos:definition "Serving more than one dwelling. "@en;
  skos:prefLabel "common stair"@en .

:c_22ca257a a skos:Concept;
  skos:broader :c_b7d8c7ee;
  skos:definition "The perception of a visual difference between two elements of the building, or fittings within the building, so that the difference in light reflectance value is of sufficient points to distinguish between the two elements."@en;
  skos:prefLabel "contrast visually"@en .

:c_b93c6e7e a skos:Concept;
  skos:broader :c_b7d8c7ee;
  skos:definition "A continuous series of steps or a continuous slope (ramp) between landings. (For the widths and lengths of flights see paragraphs 1.14–1.24.)"@en;
  skos:prefLabel "flight"@en .

:c_a9d47a76 a skos:Concept;
  dct:modified "2020-10-25T09:02:18.402Z"^^xsd:dateTime;
  skos:broader :c_b7d8c7ee;
  skos:definition "A stair intended for all users of a building on a day-to-day basis, as a normal route between levels."@en;
  skos:inScheme :conceptScheme_751925ed;
  skos:prefLabel "general access stair"@en .

:c_28dbd28f a skos:Concept;
  dct:modified "2020-10-25T09:02:27.555Z"^^xsd:dateTime;
  skos:broader :c_b7d8c7ee;
  skos:definition "For stairs: the depth from front to back of a tread, less any overlap with the next tread above (see paragraphs 1.2 and 1.3). (For the measurement of the going on tapered treads see paragraphs 1.25– 1.27.) For ramps: the length of the ramp between landings."@en;
  skos:inScheme :conceptScheme_751925ed;
  skos:prefLabel "going"@en .

:c_5d93d9fd a skos:Concept;
  skos:broader :c_b7d8c7ee;
  skos:definition "A barrier that denies pedestrians or vehicles access to another area, for example the floor below (see Diagrams 3.1 and 3.2)."@en;
  skos:prefLabel "guarding"@en .

:c_f902cb9b a skos:Concept;
  dct:modified "2020-10-25T09:02:12.811Z"^^xsd:dateTime;
  skos:broader :c_b7d8c7ee;
  skos:definition "A rail, at hand height or a little higher, for people to hold for support. (For handrails for stairs, see paragraphs 1.34–1.37; for handrails for ramps, see paragraphs 2.11–2.12.)"@en;
  skos:inScheme :conceptScheme_751925ed;
  skos:prefLabel "handrail"@en .

:c_c412c788 a skos:Concept;
  dct:modified "2020-10-25T09:02:56.193Z"^^xsd:dateTime;
  skos:broader :c_b7d8c7ee;
  skos:definition "A stair in a helix around a central void (see paragraph 1.28)."@en;
  skos:inScheme :conceptScheme_751925ed;
  skos:prefLabel "helical stair"@en .

:c_4bf44d19 a skos:Concept;
  dct:modified "2020-10-25T09:02:30.316Z"^^xsd:dateTime;
  skos:broader :c_b7d8c7ee;
  skos:definition "A means of access to another level, formed by a series of rungs or narrow treads. People normally ascend or descend facing the ladder. (See paragraphs 1.31–1.33.)"@en;
  skos:inScheme :conceptScheme_751925ed;
  skos:prefLabel "ladder"@en .

:c_3c4ca936 a skos:Concept;
  dct:modified "2020-10-25T09:03:18.170Z"^^xsd:dateTime;
  skos:broader :c_b7d8c7ee;
  skos:definition "The total quantity of visible light reflected by a surface at all wavelengths and directions when illuminated by a light source."@en;
  skos:inScheme :conceptScheme_751925ed;
  skos:prefLabel "light reflectance value (lrv)"@en .

:c_b21555ba a skos:Concept;
  dct:modified "2020-10-25T09:02:45.116Z"^^xsd:dateTime;
  skos:broader :c_b7d8c7ee;
  skos:definition "The leading edge of a stair tread. "@en;
  skos:inScheme :conceptScheme_751925ed;
  skos:prefLabel "nosing"@en .

:c_d287c321 a skos:Concept;
  dct:modified "2020-10-25T09:03:02.179Z"^^xsd:dateTime;
  skos:broader :c_b7d8c7ee;
  skos:definition "The angle of inclination (slope) between the horizontal and a line connecting the nosings of a stair."@en;
  skos:inScheme :conceptScheme_751925ed;
  skos:prefLabel "pitch"@en .

:c_c67b07d9 a skos:Concept;
  dct:modified "2020-10-25T09:02:09.354Z"^^xsd:dateTime;
  skos:broader :c_b7d8c7ee;
  skos:definition "A stair intended to be used for only one dwelling. "@en;
  skos:inScheme :conceptScheme_751925ed;
  skos:prefLabel "private stair"@en .

:c_4c4cb482 a skos:Concept;
  dct:modified "2020-10-25T09:02:36.919Z"^^xsd:dateTime;
  skos:broader :c_b7d8c7ee;
  skos:definition "An entrance which a visitor not familiar with the building would normally expect to approach. "@en;
  skos:inScheme :conceptScheme_751925ed;
  skos:prefLabel "principal entrance"@en .

:c_b45c8cb2 a skos:Concept;
  dct:modified "2020-10-25T09:02:21.630Z"^^xsd:dateTime;
  skos:broader :c_b7d8c7ee;
  skos:definition "A gangway at an angle to the rows of seats/wheelchair spaces or a stepped gangway in tiered seating."@en;
  skos:inScheme :conceptScheme_751925ed;
  skos:prefLabel "radial gangway"@en .

:c_49fde689 a skos:Concept;
  dct:modified "2020-10-25T09:02:39.736Z"^^xsd:dateTime;
  skos:broader :c_b7d8c7ee;
  skos:definition "A slope steeper than 1:20, on which a pedestrian or wheelchair user can move from one level to another (see Section 2)."@en;
  skos:inScheme :conceptScheme_751925ed;
  skos:prefLabel "ramp"@en .

:c_5e6f602a a skos:Concept;
  dct:modified "2020-10-25T09:02:33.682Z"^^xsd:dateTime;
  skos:broader :c_b7d8c7ee;
  skos:definition "The height between consecutive treads (see paragraphs 1.2 and 1.3). For ramps: the vertical distance between each end of the ramp flight."@en;
  skos:inScheme :conceptScheme_751925ed;
  skos:prefLabel "rise"@en .

:c_a5feab63 a skos:Concept;
  dct:modified "2020-10-25T09:02:15.606Z"^^xsd:dateTime;
  skos:broader :c_b7d8c7ee;
  skos:definition "A stair in a helix around a central column (see paragraph 1.28)."@en;
  skos:inScheme :conceptScheme_751925ed;
  skos:prefLabel "spiral stair"@en .

:c_78459267 a skos:Concept;
  dct:modified "2020-10-25T09:02:05.570Z"^^xsd:dateTime;
  skos:broader :c_b7d8c7ee;
  skos:definition "The clear width between the walls or balustrades. "@en;
  skos:inScheme :conceptScheme_751925ed;
  skos:prefLabel "stair width"@en .

:c_272d3c0a a skos:Concept;
  dct:modified "2020-10-25T09:02:59.137Z"^^xsd:dateTime;
  skos:broader :c_b7d8c7ee;
  skos:definition "A step in which the going reduces from one side to the other (see paragraphs 1.25–1.27). "@en;
  skos:inScheme :conceptScheme_751925ed;
  skos:prefLabel "tapered tread"@en .

:c_4010d5b9 a skos:Concept;
  dct:modified "2020-10-25T09:02:02.615Z"^^xsd:dateTime;
  skos:broader :c_b7d8c7ee;
  skos:definition "A flat gangway parallel to the rows of seating/wheelchair spaces."@en;
  skos:inScheme :conceptScheme_751925ed;
  skos:prefLabel "transverse gangway"@en .

:c_f2f44aa9 a skos:Concept;
  dct:modified "2020-10-25T09:02:24.856Z"^^xsd:dateTime;
  skos:broader :c_b7d8c7ee;
  skos:definition "A stair used for escape, access for maintenance, or purposes other than as the usual route for moving between levels on a day-to-day basis."@en;
  skos:inScheme :conceptScheme_751925ed;
  skos:prefLabel "utility stair"@en .

:c_2ca7a450 a skos:Concept;
  dct:modified "2020-10-25T09:03:11.860Z"^^xsd:dateTime;
  skos:broader :c_b7d8c7ee;
  skos:definition "Storey exits provided within the body of a seating layout."@en;
  skos:inScheme :conceptScheme_751925ed;
  skos:prefLabel "vomitory exits"@en .

:c_b93c6e7e dct:modified "2020-10-25T09:02:42.445Z"^^xsd:dateTime;
  skos:inScheme :conceptScheme_751925ed .

:c_c9535965 dct:modified "2020-10-25T09:02:47.854Z"^^xsd:dateTime;
  skos:inScheme :conceptScheme_751925ed .

:c_22ca257a dct:modified "2020-10-25T09:02:50.221Z"^^xsd:dateTime;
  skos:inScheme :conceptScheme_751925ed .

:c_bf5868a2 dct:modified "2020-10-25T09:02:52.810Z"^^xsd:dateTime;
  skos:inScheme :conceptScheme_751925ed .

:c_2d35a0e4 dct:modified "2020-10-26T07:30:16.215Z"^^xsd:dateTime;
  skos:inScheme :conceptScheme_751925ed .

:c_d3c63474 dct:modified "2020-10-25T09:03:07.980Z"^^xsd:dateTime;
  skos:inScheme :conceptScheme_751925ed .

:c_5d93d9fd dct:modified "2020-10-25T09:03:15.218Z"^^xsd:dateTime;
  skos:inScheme :conceptScheme_751925ed .

:c_b7d8c7ee dct:modified "2020-10-25T09:04:42.246Z"^^xsd:dateTime;
  skos:narrower :c_22ca257a, :c_272d3c0a, :c_28dbd28f, :c_2ca7a450, :c_2d35a0e4, :c_3c4ca936,
    :c_4010d5b9, :c_49fde689, :c_4bf44d19, :c_4c4cb482, :c_5d93d9fd, :c_5e6f602a, :c_78459267,
    :c_a5feab63, :c_a9d47a76, :c_b21555ba, :c_b45c8cb2, :c_b93c6e7e, :c_bf5868a2, :c_c412c788,
    :c_c67b07d9, :c_c9535965, :c_d287c321, :c_d3c63474, :c_f2f44aa9, :c_f902cb9b .

:skosCollection_50d4bd2e skos:member :c_07abc5c2, :c_0c33e781, :c_0db511ab, :c_1166f883,
    :c_22ca257a, :c_272d3c0a, :c_28dbd28f, :c_2a1002d3, :c_2bb3748c, :c_3262a30a, :c_345811e8,
    :c_34c7d4e3, :c_3b310e19, :c_3b5778ee, :c_3c4ca936, :c_3d888dc1, :c_3fc6a13d, :c_4010d5b9,
    :c_438bd78a, :c_49fde689, :c_4b4c9739, :c_4bf44d19, :c_4c4cb482, :c_4cb28fa4, :c_4f47aeea,
    :c_588bf28f, :c_5aa42901, :c_5bb42f0e, :c_5d93d9fd, :c_5e6f602a, :c_61aec10c, :c_6badbeaf,
    :c_6ed11205, :c_70a0403c, :c_78459267, :c_8144317d, :c_81482951, :c_895306c7, :c_8abc2fd9,
    :c_8c6a9923, :c_8f476b03, :c_93488b6d, :c_95d3756f, :c_9a21f5a2, :c_a9d47a76, :c_aa316632,
    :c_ac95ba41, :c_b21555ba, :c_b3eb4d7b, :c_b4273037, :c_b45c8cb2, :c_b93c6e7e, :c_bf5868a2,
    :c_c13a7c46, :c_c2902dec, :c_c412c788, :c_c57961a6, :c_c67b07d9, :c_c8566bf0, :c_c878dbda,
    :c_c9535965, :c_cbfc0947, :c_d26ff5d2, :c_d287c321, :c_d3c63474, :c_d68c8ade, :c_da4b364b,
    :c_e43f1fcb, :c_e6d846bf, :c_e85e2d31, :c_f213d52c, :c_f2f44aa9, :c_f3cee240, :c_f40ac57b,
    :c_f902cb9b, :c_fa726c7b .

:c_e7aee361 a skos:Concept;
  dct:created "2020-10-26T05:33:49.239Z"^^xsd:dateTime;
  dct:modified "2020-10-26T07:04:15.510Z"^^xsd:dateTime;
  skos:broader :c_f68328a2;
  skos:inScheme :conceptScheme_751925ed;
  skos:narrower :c_70908a07, :c_ae74ec82 .

:c_29cf7b46 dct:modified "2020-10-26T07:00:50.727Z"^^xsd:dateTime;
  skos:inScheme :conceptScheme_751925ed;
  skos:note """Note: Sub-paragraph c means that, for example, the presence of a small flat for a manager in a large non-domestic building does not result in the whole building being treated as a dwelling.
Similarly, if a room is used as an office or utility space within a dwelling, that does not mean that the building should not be treated as a dwelling."""@en .

:c_f68328a2 skos:definition """* This approved document gives guidance for compliance with the Building Regulations for
building work carried out in England. It also applies to building work carried out on excepted
energy buildings in Wales as defined in the Welsh Ministers (Transfer of Functions) (No.2) Order
2009. This approved document also gives guidance applying to buildings of statutory undertakers
and of the Crown or carried out by Crown authorities in both England and Wales in respect of
regulations 25, 25A, 25B and 26."""@en;
  skos:narrower :c_e7aee361 .

:c_ae74ec82 a skos:Concept;
  dct:created "2020-10-26T05:36:13.809Z"^^xsd:dateTime;
  skos:broader :c_e7aee361;
  skos:inScheme :conceptScheme_751925ed;
  skos:narrower :c_2bb3748c, :c_4487e3fd, :c_4e2f4fd0;
  skos:note "The following are key terms used in this document:"@en;
  skos:prefLabel "appendix a: key terms and abbreviations"@en .

:c_70908a07 a skos:Concept;
  dct:created "2020-10-26T06:10:39.834Z"^^xsd:dateTime;
  skos:broader :c_e7aee361;
  skos:inScheme :conceptScheme_751925ed;
  skos:note "This approved document gives guidance on what, in ordinary circumstances, may be considered reasonable provision to comply with the requirements of regulations 26, 26A and 40 of, and Part L of Schedule 1 to, the Building Regulations for those creating new dwellings. In addition, this approved document gives guidance on how to comply with regulations 25A, 27, 27A, 43 and 44 of the Building Regulations and regulation 20 of the Building (Approved Inspectors etc.) Regulations 2010 where an approved inspector is the BCB."@en;
  skos:prefLabel "appendix b: types of work covered by this approved document"@en .

:c_9397feee a skos:Concept;
  dct:modified "2020-10-26T07:41:56.725Z"^^xsd:dateTime;
  skos:broader :c_ae74ec82;
  skos:definition "is the physical property used to measure airtightness of the building fabric. It is defined as air leakage rate per hour per square metre of envelope area at the test reference pressure differential of 50 pascals (50 N/m2). The envelope area, or measured part of the building, is the total area of all floors, walls and ceilings bordering the internal volume that is the subject of the pressure test. This includes walls and floors below external ground level. Overall internal dimensions are used to calculate this envelope area and no subtractions are made for the area of the junctions of internal walls, floors and ceilings with exterior walls, floors and ceilings."@en;
  skos:inScheme :conceptScheme_751925ed;
  skos:prefLabel "air permeability"@en .

:c_21b61df0 a skos:Concept;
  dct:modified "2020-10-26T07:18:47.233Z"^^xsd:dateTime;
  skos:broader :c_ae74ec82;
  skos:definition "is the worst allowable air permeability."@en;
  skos:inScheme :conceptScheme_751925ed;
  skos:prefLabel "limiting air permeability"@en .

:c_75d877dd a skos:Concept;
  skos:broader :c_ae74ec82;
  skos:definition "is the target value set at the design stage, and must always be no worse than the limiting value."@en;
  skos:prefLabel "design air permeability"@en .

:c_c65780e9 a skos:Concept;
  dct:modified "2020-10-26T07:22:42.768Z"^^xsd:dateTime;
  skos:broader :c_ae74ec82;
  skos:definition "is the value used in establishing the DER and the DFEE rate, and is based on a specific measurement of the dwelling concerned or on measurements of other dwellings of the same dwelling type."@en;
  skos:inScheme :conceptScheme_751925ed;
  skos:note "NOTE: The envelope area of a terraced house includes the party wall(s). The envelope area of a flat in a multiple-storey building includes the floors, walls and ceilings which are shared with adjacent flats."@en;
  skos:prefLabel "assessed air permeability"@en .

:c_e3217f0c a skos:Concept;
  dct:modified "2020-10-26T06:50:06.671Z"^^xsd:dateTime;
  skos:broader :c_ae74ec82;
  skos:definition "is the advancement of a fixed building service after all or part of the system has been installed, replaced or altered. The system is taken from a state of static completion to working order. Testing and adjusting, as necessary, ensure that the whole system uses no more fuel and power than  is reasonable in the circumstances, without compromising the need to comply with health and safety requirements. For each system, commissioning includes the following: setting-to-work; regulation (that is, testing and adjusting repetitively) to achieve the specified performance; calibration, setting up and testing of the associated automatic control systems; and recording of the system settings and the performance test results that have been accepted as satisfactory."@en;
  skos:inScheme :conceptScheme_751925ed;
  skos:prefLabel "commissioning"@en .

:c_13c7985e a skos:Concept;
  dct:modified "2020-10-26T06:49:56.942Z"^^xsd:dateTime;
  skos:broader :c_ae74ec82;
  skos:definition "is the Dwelling CO2 Emission Rate expressed as kgCO2/(m2 year)."@en;
  skos:inScheme :conceptScheme_751925ed;
  skos:prefLabel "der"@en .

:c_96f4329c a skos:Concept;
  dct:modified "2020-10-26T07:21:08.623Z"^^xsd:dateTime;
  skos:broader :c_ae74ec82;
  skos:definition "is the dwelling fabric energy efficiency rate expressed as kWh/(m2.year). Dwelling means a self-contained unit designed to accommodate a single household."@en;
  skos:inScheme :conceptScheme_751925ed;
  skos:note "NOTE: Buildings exclusively containing rooms for residential purposes, such as nursing homes, student accommodation and similar, are not dwellings, and in such cases, Approved Document L2A applies."@en;
  skos:prefLabel "dfee rate"@en .

:c_63561321 a skos:Concept;
  dct:modified "2020-10-26T06:49:15.510Z"^^xsd:dateTime;
  skos:broader :c_ae74ec82;
  skos:definition "is the particular group allocated to each dwelling on a development to provide the basis for assessing the pressure testing regime. The allocation of each dwelling to a dwelling type should be the responsibility of the person carrying out the pressure testing. To be classed as of the same type, dwellings should: i. be of the same generic form (i.e. detached, semi-detached, end terrace, mid-terrace, ground- floor flat (including ground-floor maisonette), mid-floor flat, top-floor flat (including top-floor maisonette); iii. include the same number of storeys; iii have the same design air permeability; iiii have similar adjacency to unheated spaces such as stairwells, integral garages etc. v. have the same principal construction details vi. have a similar (i.e. 1) number of significant penetrations, i.e. for windows, doors, flues/ chimneys, supply/exhaust terminals, waste water pipes; vii. have envelope areas that do not differ by more than 10 per cent (see air permeability for a definition of envelope area)."@en;
  skos:inScheme :conceptScheme_751925ed;
  skos:prefLabel "dwelling type"@en .

:c_e382854e a skos:Concept;
  dct:modified "2020-10-26T06:49:53.674Z"^^xsd:dateTime;
  skos:broader :c_ae74ec82;
  skos:definition "is the Target CO2 Emission Rate expressed as kgCO2/(m2 year)."@en;
  skos:inScheme :conceptScheme_751925ed;
  skos:prefLabel "ter"@en .

:c_4487e3fd a skos:Concept;
  dct:modified "2020-10-26T06:49:12.580Z"^^xsd:dateTime;
  skos:broader :c_ae74ec82;
  skos:definition " is the Target Fabric Energy Efficiency rate expressed as kWh/(m2.year)."@en;
  skos:inScheme :conceptScheme_751925ed;
  skos:prefLabel "tfee"@en .

:c_42f32053 a skos:Concept;
  dct:modified "2020-10-26T06:50:15.968Z"^^xsd:dateTime;
  skos:broader :c_ae74ec82;
  skos:inScheme :conceptScheme_751925ed;
  skos:notation "brukl"@en;
  skos:prefLabel "building regulations uk part l"@en .

:c_63f653cb a skos:Concept;
  dct:modified "2020-10-26T06:49:36.714Z"^^xsd:dateTime;
  skos:broader :c_ae74ec82;
  skos:inScheme :conceptScheme_751925ed;
  skos:notation "ukas"@en;
  skos:prefLabel "united kingdom accreditation service"@en .

:c_2bb3748c a skos:Concept;
  dct:modified "2020-10-26T06:49:39.743Z"^^xsd:dateTime;
  skos:broader :c_ae74ec82;
  skos:inScheme :conceptScheme_751925ed;
  skos:notation "tfa"@en;
  skos:prefLabel "total floor area"@en .

:c_4e2f4fd0 a skos:Concept;
  dct:modified "2020-10-26T06:50:12.992Z"^^xsd:dateTime;
  skos:broader :c_ae74ec82;
  skos:inScheme :conceptScheme_751925ed;
  skos:notation "tmp"@en;
  skos:prefLabel "thermal mass parameter"@en .

:c_5ecea38f a skos:Concept;
  dct:modified "2020-10-26T07:25:43.946Z"^^xsd:dateTime;
  skos:broader :c_ae74ec82;
  skos:inScheme :conceptScheme_751925ed;
  skos:notation "sedbuk"@en;
  skos:prefLabel "seasonal efficiency of domestic boilers in the uk"@en .

:c_716e9379 a skos:Concept;
  dct:modified "2020-10-26T06:49:18.591Z"^^xsd:dateTime;
  skos:broader :c_ae74ec82;
  skos:inScheme :conceptScheme_751925ed;
  skos:notation "co2"@en;
  skos:prefLabel "carbon dioxide"@en .

:c_b9d06847 a skos:Concept;
  dct:modified "2020-10-26T06:56:19.370Z"^^xsd:dateTime;
  skos:broader :c_ae74ec82;
  skos:definition "The act of erecting a new dwelling is not a material change of use. Approved Document L1B applies where a dwelling is being created in an existing building as the result of a material change of use of all or part of the building."@en;
  skos:inScheme :conceptScheme_751925ed;
  skos:prefLabel "material changes of use"@en .

:c_ab063a87 a skos:Concept;
  dct:modified "2020-10-26T06:58:33.948Z"^^xsd:dateTime;
  skos:broader :c_70908a07;
  skos:definition "When constructing a dwelling as part of a larger building that contains other types of accommodation, sometimes called a mixed-use development, use this Approved Document L1A for guidance in relation to each individual dwelling. Approved Document L2A gives guidance relating to the non-dwelling parts of such buildings, such as heated common areas, and in the case of mixed-use developments, the commercial or retail space."@en;
  skos:inScheme :conceptScheme_751925ed;
  skos:prefLabel "mixed-use developments"@en .

:c_1c9c5904 a skos:Concept;
  dct:modified "2020-10-26T06:58:50.851Z"^^xsd:dateTime;
  skos:broader :c_70908a07;
  skos:definition "The act of erecting a new dwelling is not a material change of use. Approved Document L1B applies where a dwelling is being created in an existing building as the result of a material change of use of all or part of the building."@en;
  skos:inScheme :conceptScheme_751925ed;
  skos:prefLabel "material changes of use"@en .

:c_29cf7b46 a skos:Concept;
  skos:broader :c_70908a07;
  skos:definition "If a unit contains both living accommodation and space to be used for commercial purposes (e.g. as a workshop or office), the whole unit should be treated as a dwelling, as long as the commercial part can revert to domestic use. This can be the case if, for example: a. there is direct access between the commercial space and the living accommodation; and b. both are contained within the same thermal envelope; and c. the living accommodation occupies a substantial proportion of the total area of the unit."@en;
  skos:prefLabel "live–work units"@en .

:c_75d877dd dct:modified "2020-10-26T07:44:00.398Z"^^xsd:dateTime;
  skos:inScheme :conceptScheme_751925ed .

:c_ae74ec82 skos:narrower :c_13c7985e, :c_1c9c5904, :c_21b61df0, :c_42f32053, :c_5ecea38f,
    :c_63561321, :c_63f653cb, :c_716e9379, :c_75d877dd, :c_9397feee, :c_96f4329c, :c_ab063a87,
    :c_c65780e9, :c_e3217f0c, :c_e382854e .

:c_e7aee361 skos:prefLabel "l1a conservation of fuel and power 2013 edition incorporating 2016 amendments – for use in England*"@en .

:c_70908a07 skos:narrower :c_1c9c5904, :c_29cf7b46 .

:c_a1430501 dct:modified "2020-10-26T07:17:54.434Z"^^xsd:dateTime;
  skos:prefLabel "controlled service or ﬁtting"@en .

:c_454526b8 skos:inScheme :conceptScheme_751925ed .

:c_4161794e a skos:Concept;
  dct:created "2020-10-27T06:04:22.445Z"^^xsd:dateTime;
  skos:broader :c_f68328a2;
  skos:inScheme :conceptScheme_751925ed;
  skos:note """This Approved Document, which takes
effect on 1 October 2010, has been approved
and issued by the Secretary of State to provide
practical guidance on ways of complying with the
energy efficiency requirements (see Section 2)
and regulation 7 of the Building Regulations 2010
(SI 2010/2214) for England and Wales. Regulation
2(1) of the Building Regulations defines the energy
efficiency requirements as the requirements of
regulations 23, 25A, 25B, 26, 28 and 40 and Part
L of Schedule 1. The Building Regulations 2010
are referred to throughout the remainder of this
Document as ‘the Building Regulations’."""@en;
  skos:prefLabel "l2b conservation of fuel and power in existing buildings other than dwellings 2010 edition incorporating 2010, 2011, 2013 and 2016 amendments"@en .

:c_f68328a2 skos:narrower :c_4161794e .

:c_aca129a3 a skos:Concept;
  dct:created "2020-10-27T06:08:52.145Z"^^xsd:dateTime;
  skos:inScheme :conceptScheme_751925ed;
  skos:prefLabel "appendix a: key terms and abbreviations (l2a)"@en .

:skosCollection_50d4bd2e skos:member :c_5ecea38f, :c_e382854e, :c_f31dbf5c .

:c_13c34a40 a skos:Concept;
  dct:modified "2020-10-27T06:29:13.400Z"^^xsd:dateTime;
  skos:broader :c_aca129a3;
  skos:definition "is the worst allowable air permeability."@en;
  skos:inScheme :conceptScheme_751925ed;
  skos:prefLabel "limiting air permeability"@en .

:c_d64e2e84 a skos:Concept;
  dct:modified "2020-10-27T06:28:36.780Z"^^xsd:dateTime;
  skos:broader :c_aca129a3;
  skos:definition "is the Building CO2 Emission Rate expressed as kgCO2/(m2 year)."@en;
  skos:inScheme :conceptScheme_751925ed;
  skos:prefLabel "ber"@en .

:c_baf59db7 a skos:Concept;
  dct:modified "2020-10-27T06:28:48.281Z"^^xsd:dateTime;
  skos:broader :c_aca129a3;
  skos:definition "means an area of glazing, including glazed doors, intended for the display of products or services on offer within the building, positioned: a.at the external perimeter of the building; and b. at an access level; and c. immediately adjacent to a pedestrian thoroughfare. There should be no permanent workspace within one glazing height of the perimeter. Glazing more than 3 m above such an access level should not be considered part of a display window except: a. where the products on display require a greater height of glazing; b. in cases where building work involving changes to the façade and glazing requiring planning consent, where planners require a greater height of glazing, e.g. to fit with surrounding buildings or to match the character of the existing façade. It is expected that display windows will be found in planning Use Classes A1, A2, A3 and D2 as detailed in the table below."@en;
  skos:inScheme :conceptScheme_751925ed;
  skos:prefLabel "display window"@en .

:c_a6ddbdac a skos:Concept;
  dct:modified "2020-10-27T06:29:10.530Z"^^xsd:dateTime;
  skos:broader :c_aca129a3;
  skos:definition "means lighting intended to highlight displays of exhibits or merchandise, or lighting used in spaces for public leisure and entertainment such as dance halls, auditoria, conference halls, restaurants and cinemas"@en;
  skos:inScheme :conceptScheme_751925ed;
  skos:prefLabel "display lighting"@en .

:c_e85468f5 a skos:Concept;
  dct:modified "2020-10-27T06:28:58.203Z"^^xsd:dateTime;
  skos:broader :c_aca129a3;
  skos:definition "includes a dwelling-house and a flat and means a self-contained unit designed to accommodate a single household. Buildings exclusively containing rooms for residential purposes such as nursing homes, student accommodation and similar are not dwellings, and in such cases, this Approved Document L2A applies."@en;
  skos:inScheme :conceptScheme_751925ed;
  skos:prefLabel "dwelling (l2a)"@en .

:c_b468fcc4 a skos:Concept;
  dct:modified "2020-10-27T06:28:39.478Z"^^xsd:dateTime;
  skos:broader :c_aca129a3;
  skos:definition "means that part of emergency lighting that provides illumination for  the safety of people leaving an area or attempting to terminate a dangerous process before leaving an area"@en;
  skos:inScheme :conceptScheme_751925ed;
  skos:note "NOTE: In respect of new buildings other than dwellings, the applicable requirements are those of Part L and regulations 25A and 26"@en;
  skos:prefLabel "emergency escape lighting"@en .

:c_7e8f8302 a skos:Concept;
  dct:modified "2020-10-27T06:29:01.259Z"^^xsd:dateTime;
  skos:broader :c_aca129a3;
  skos:definition "means that work needed to complete the partitioning and building services within the external fabric of the building (the shell) to meet the specific needs of incoming occupiers. fit-out work can be carried out in whole or in parts: a. a. in the same project and time frame as the construction of the building shell; or b. a. at some time after the shell has been completed."@en;
  skos:inScheme :conceptScheme_751925ed;
  skos:prefLabel "fit-out work"@en .

:c_74e681f9 a skos:Concept;
  dct:modified "2020-10-27T06:28:55.440Z"^^xsd:dateTime;
  skos:broader :c_aca129a3;
  skos:definition "means a door to an entrance primarily for the use of people that is expected to experience large volumes of traffic, and where robustness and/or powered operation is the main performance requirement. To qualify as a high-usage entrance door, the door should be equipped with automatic closers and, except where operational requirements preclude it, be protected by a lobby."@en;
  skos:inScheme :conceptScheme_751925ed;
  skos:prefLabel "high-usage entrance door"@en .

:c_3350a84a a skos:Concept;
  dct:modified "2020-10-27T06:28:42.277Z"^^xsd:dateTime;
  skos:broader :c_aca129a3;
  skos:definition "means lighting intended to illuminate specialist tasks within a space, rather than the space itself. It could include theatre spotlights, projection equipment, lighting in TV and photographic studios, medical lighting in operating theatres and doctors’ and dentists’ surgeries, illuminated signs, coloured or stroboscopic lighting, and art objects with integral lighting such as sculptures, decorative fountains and chandeliers."@en;
  skos:inScheme :conceptScheme_751925ed;
  skos:prefLabel "specialist process lighting"@en .

:c_06d9104f a skos:Concept;
  dct:modified "2020-10-27T06:28:51.460Z"^^xsd:dateTime;
  skos:broader :c_aca129a3;
  skos:definition "is the total area of all enclosed spaces measured to the internal face of the external walls. In this convention: a. a. the area of sloping surfaces such as staircases, galleries, raked auditoria and tiered terraces should be taken as their area on plan; and b. a. areas that are not enclosed such as open floors, covered ways and balconies are excluded."@en;
  skos:inScheme :conceptScheme_751925ed;
  skos:note "NOTE: This area is the gross floor area as measured in accordance with the guidance issued to surveyors by the Royal Institution of Chartered Surveyors (RICS)."@en;
  skos:prefLabel "total useful floor area"@en .

:c_9e56cd49 a skos:Concept;
  dct:modified "2020-10-27T06:29:27.009Z"^^xsd:dateTime;
  skos:broader :c_aca129a3;
  skos:inScheme :conceptScheme_751925ed;
  skos:notation "HVAC"@en;
  skos:prefLabel "heating, ventilation and air-conditioning"@en .

:c_2a4fc22e a skos:Concept;
  dct:modified "2020-10-27T06:29:04.683Z"^^xsd:dateTime;
  skos:broader :c_aca129a3;
  skos:inScheme :conceptScheme_751925ed;
  skos:notation "LZC"@en;
  skos:prefLabel "low and zero carbon"@en .

:c_6badbeaf a skos:Concept;
  dct:modified "2020-10-27T06:29:23.993Z"^^xsd:dateTime;
  skos:broader :c_aca129a3;
  skos:inScheme :conceptScheme_751925ed;
  skos:notation "SFP"@en;
  skos:prefLabel "specific fan power"@en .

:c_5d579e20 a skos:Concept;
  dct:modified "2020-10-27T06:29:16.391Z"^^xsd:dateTime;
  skos:broader :c_aca129a3;
  skos:inScheme :conceptScheme_751925ed;
  skos:notation "SEER"@en;
  skos:prefLabel "seasonal energy efficiency ratio"@en .

:c_f31dbf5c a skos:Concept;
  dct:modified "2020-10-27T08:35:50.450Z"^^xsd:dateTime;
  skos:broader :c_aca129a3;
  skos:inScheme :conceptScheme_751925ed;
  skos:notation "SSEER"@en .

:c_5e92bf81 a skos:Concept;
  dct:modified "2020-10-27T06:29:07.605Z"^^xsd:dateTime;
  skos:broader :c_aca129a3;
  skos:inScheme :conceptScheme_751925ed;
  skos:notation "FF"@en;
  skos:prefLabel "frame factor"@en .

:c_ba365c10 a skos:Concept;
  dct:modified "2020-10-27T06:28:45.149Z"^^xsd:dateTime;
  skos:broader :c_aca129a3;
  skos:inScheme :conceptScheme_751925ed;
  skos:notation "DX"@en;
  skos:prefLabel "direct exchange"@en .

:c_e41ef2d9 skos:narrower :c_563fcfe6 .

:c_aca129a3 dct:modified "2020-10-27T06:43:09.984Z"^^xsd:dateTime;
  skos:broader :c_8f28ad6e;
  skos:narrower :c_06d9104f, :c_13c34a40, :c_2a4fc22e, :c_3350a84a, :c_5d579e20, :c_5e92bf81,
    :c_6badbeaf, :c_74e681f9, :c_7e8f8302, :c_9e56cd49, :c_a6ddbdac, :c_b468fcc4, :c_ba365c10,
    :c_baf59db7, :c_d64e2e84, :c_e85468f5, :c_f31dbf5c .

:skosCollection_50d4bd2e skos:member :c_06d9104f, :c_13c34a40, :c_13c7985e, :c_1c9c5904,
    :c_1cfc2b23, :c_21b61df0, :c_247e4247, :c_2a4fc22e, :c_3350a84a, :c_352a7ba0, :c_42f32053,
    :c_4487e3fd, :c_4e2f4fd0, :c_5d579e20, :c_5e92bf81, :c_63561321, :c_63f653cb, :c_716e9379,
    :c_74e681f9, :c_75d877dd, :c_7e8f8302, :c_9397feee, :c_96f4329c, :c_9e56cd49, :c_a6ddbdac,
    :c_ab063a87, :c_b468fcc4, :c_b9d06847, :c_ba365c10, :c_baf59db7, :c_bb0d6dd0, :c_c65780e9,
    :c_d64e2e84, :c_e3217f0c, :c_e448e5c3, :c_e85468f5 .

:c_8f28ad6e a skos:Concept;
  dct:created "2020-10-27T06:38:09.688Z"^^xsd:dateTime;
  skos:broader :c_f68328a2;
  skos:inScheme :conceptScheme_751925ed;
  skos:prefLabel "l2a Conservation of fuel and power in new buildings other than dwellings 2013 edition incorporating 2016 amendments – for use in england*"@en .

:c_4161794e dct:modified "2020-10-27T06:48:26.172Z"^^xsd:dateTime;
  skos:narrowMatch :c_0aaf684b .

:c_f68328a2 dct:modified "2020-10-27T06:38:32.899Z"^^xsd:dateTime;
  skos:narrower :c_8f28ad6e .

:c_0aaf684b a skos:Concept;
  dct:created "2020-10-27T06:47:51.399Z"^^xsd:dateTime;
  skos:broader :c_4161794e;
  skos:inScheme :conceptScheme_751925ed;
  skos:prefLabel "key terms (l2b)"@en .

:c_247e4247 a skos:Concept;
  dct:modified "2020-10-27T07:01:19.763Z"^^xsd:dateTime;
  skos:broader :c_0aaf684b;
  skos:definition "means those energy efficiency improvements required by regulation 28."@en;
  skos:inScheme :conceptScheme_751925ed;
  skos:prefLabel "consequential improvements"@en .

:c_1cfc2b23 a skos:Concept;
  dct:modified "2020-10-27T08:36:16.565Z"^^xsd:dateTime;
  skos:broader :c_0aaf684b;
  skos:definition "means the amount of time it  will take to recover the initial investment through energy savings, and is calculated by dividing the marginal additional cost of implementing an energy efficiency measure by the value of the annual energy savings achieved by that measure taking no account of VAT. When making this calculation, the following guidance should be used:"@en;
  skos:inScheme :conceptScheme_751925ed;
  skos:prefLabel "simple payback"@en .

:c_352a7ba0 a skos:Concept;
  dct:modified "2020-10-27T08:36:43.215Z"^^xsd:dateTime;
  skos:broader :c_0aaf684b;
  skos:definition "means the work necessary to achieve the client’s purposes in extending the building and/or increasing the installed capacity of any fixed building services. The value of the principal works is the basis for determining a reasonable provision of consequential improvements. a. The marginal additional cost is the additional cost (materials and labour) of incorporating (e.g.) additional insulation, not the whole cost of the work. b. The cost of implementing the measure should be based on prices current at the date the proposals are made known to the BCB and be confirmed in a report signed by a suitably qualified person. c. The annual energy savings should be estimated using an energy calculation tool approved by the Secretary of State pursuant to regulation 24. d. For the purposes of this Approved Document, the energy prices that are current at the time of the application to building control should be used when evaluating the annual energy savings. Current energy prices can be obtained from the DECC website1."@en;
  skos:inScheme :conceptScheme_751925ed;
  skos:prefLabel "principal works"@en .

:c_e448e5c3 a skos:Concept;
  dct:modified "2020-10-27T08:36:03.272Z"^^xsd:dateTime;
  skos:broader :c_0aaf684b;
  skos:definition "is the total area of all enclosed spaces measured to the internal face  of the external walls, that is to say it is the gross floor area as measured in accordance with the guidance issued to surveyors by the RICS. In this convention: a. a. the area of sloping surfaces such as staircases, galleries, raked auditoria, and tiered terraces should be taken as their area on plan; and b. b. areas that are not enclosed such as open floors, covered ways and balconies are excluded. This equates to the gross floor area as measured in accordance with the guidance issued to surveyors by the RICS."@en;
  skos:inScheme :conceptScheme_751925ed;
  skos:note "Note that this definition encompasses the walls and floor of a swimming pool basin where this is part of an existing building"@en;
  skos:prefLabel "total useful floor area"@en .

:c_6a1a3775 a skos:Concept;
  dct:created "2020-10-27T07:03:59.856Z"^^xsd:dateTime;
  dct:modified "2020-10-27T07:58:25.743Z"^^xsd:dateTime;
  skos:broader :c_a20cbb62;
  skos:inScheme :conceptScheme_751925ed;
  skos:narrower :c_3cf43794;
  skos:prefLabel "access to and use of buildings volume 1: dwellings 2015 edition incorporating 2016 amendments for use in england*"@en .

:c_a20cbb62 skos:narrower :c_6a1a3775 .

:c_0109c085 dct:created "2020-10-27T16:36:09.588Z"^^xsd:dateTime .

:c_3cf43794 a skos:Concept;
  dct:created "2020-10-27T07:15:01.792Z"^^xsd:dateTime;
  skos:broader :c_6a1a3775;
  skos:inScheme :conceptScheme_751925ed;
  skos:note "Note: Terms shown with * are definition legislation, either in the Building Act 1984 or the Building Regulations 2010, where the definition may be fuller than the  definition given here."@en;
  skos:prefLabel "appendix a: key terms (adm1)"@en .

:c_7003e65c a skos:Concept;
  skos:broader :c_3cf43794;
  skos:definition "A threshold that is level or, if raised, has a total height of not more than 15mm, a minimum number of upstands and slopes and with any upstands higher than 5mm chamfered. Other acceptable solutions are described in Accessible thresholds in new housing – Guidance for house builders and developers, The Stationery Offi e Ltd. ISBN 0 11 702333 3. 1999."@en;
  skos:note "Note: Terms shown with * are definition legislation, either in the Building Act 1984 or the Building Regulations 2010, where the definition may be fuller than the  definition given here."@en;
  skos:prefLabel "accessible threshold"@en .

:c_6bf8d62f a skos:Concept;
  skos:broader :c_3cf43794;
  skos:definition "Internal or external path or corridor usually leading to the principal private entrance of a dwelling from a defined starting point (typically the pavement immediately outside of the curtilage or plot boundary)."@en;
  skos:prefLabel "approach route"@en .

:c_b630c168 a skos:Concept;
  skos:broader :c_3cf43794;
  skos:definition "A suitable sleeping area for one person. (A single bedroom provides one bedspace and a double or twin bedroom provides two bedspaces where these rooms also meet any other requirements for the relevant category of dwelling)."@en;
  skos:prefLabel "bedspace"@en .

:c_1d89066b a skos:Concept;
  skos:broader :c_3cf43794;
  skos:definition "Clear, unobstructed ‘pathway’ to access a window or other feature. Localised obstructions are not permitted unless specifically stated."@en;
  skos:prefLabel "clear access route"@en .

:c_f21d57e8 a skos:Concept;
  skos:broader :c_3cf43794;
  skos:definition "Clear, unobstructed space for access or manoeuvring. Localised obstructions are not permitted unless specifically stated."@en;
  skos:prefLabel "clear access zone"@en .

:c_7d70a254 a skos:Concept;
  skos:broader :c_3cf43794;
  skos:definition "Clear distance measured between the inside face of the doorframe (or door stop) and the face of the door when open at 90 degrees. Door furniture and ironmongery may be disregarded when measuring the clear opening width."@en;
  skos:prefLabel "clear opening width"@en .

:c_08556adc a skos:Concept;
  skos:broader :c_3cf43794;
  skos:definition "Clear floor space, represented by a circle, or an ellipse, that allows a wheelchair user to turn independently in a single movement. A door swing is permitted within a clear turning space unless stated otherwise."@en;
  skos:prefLabel "clear turning circle"@en .

:c_fcd25267 a skos:Concept;
  skos:broader :c_3cf43794;
  skos:definition "Clear distance measured between walls or other fixed obstructions (except permitted localised obstructions) or across a path. Skirtings totalling up to 50mm total thickness and shallow projecting ducts or casings above 1800mm may be discounted when measuring clear width."@en;
  skos:prefLabel "clear width"@en .

:c_09ab5f8e a skos:Concept;
  skos:broader :c_3cf43794;
  skos:definition "Shared area accessed by, or intended for the use of, more than one dwelling."@en;
  skos:prefLabel "communal or common (area, facilities or entrances)"@en .

:c_3d9928e0 a skos:Concept;
  skos:broader :c_3cf43794;
  skos:definition "The floor level (of the dwelling) on which the principal private entrance is located."@en;
  skos:prefLabel "entrance storey"@en .

:c_6dcae9b3 a skos:Concept;
  skos:broader :c_3cf43794;
  skos:definition "A house or flat. Student accommodation is treated as hotel/motel accommodation."@en;
  skos:notation "*"@en;
  skos:prefLabel "dwelling (adm1)"@en .

:c_5fcbc183 a skos:Concept;
  skos:broader :c_3cf43794;
  skos:definition "The surface of a door which follows into (or faces away from) the room or space into which the door is being opened – sometimes referred to as ‘the push side’."@en;
  skos:prefLabel "following edge (of door)"@en .

:c_00b6a69e a skos:Concept;
  skos:broader :c_3cf43794;
  skos:definition "Gradient between 1:60 and 1:20"@en;
  skos:prefLabel "gently sloping"@en .

:c_44e39791 a skos:Concept;
  dct:modified "2020-10-27T07:40:41.627Z"^^xsd:dateTime;
  skos:broader :c_3cf43794;
  skos:definition "Step-free area with no lips or upstands, suitable for showering, with a floor laid to shallow falls towards a floor gulley connected to the drainage system."@en;
  skos:inScheme :conceptScheme_751925ed;
  skos:prefLabel "installed level access shower"@en .

:c_283297ae a skos:Concept;
  skos:broader :c_3cf43794;
  skos:definition "The surface of a door which leads into (or faces) the room or space into which the door is being opened – sometimes referred to as ‘the pull side’"@en;
  skos:prefLabel "leading edge (of door)"@en .

:c_728f0bd1 a skos:Concept;
  dct:modified "2020-10-27T07:40:54.077Z"^^xsd:dateTime;
  skos:broader :c_3cf43794;
  skos:definition "Gradient not exceeding 1:60"@en;
  skos:inScheme :conceptScheme_751925ed;
  skos:prefLabel "level"@en .

:c_a5ffe780 a skos:Concept;
  skos:broader :c_3cf43794;
  skos:definition "Vertical route linking all floors of a dwelling accommodating (or capable of accommodating) a lift or lifting platform."@en;
  skos:prefLabel "liftway"@en .

:c_572989c8 a skos:Concept;
  dct:modified "2020-10-27T07:40:57.316Z"^^xsd:dateTime;
  skos:broader :c_3cf43794;
  skos:definition "Short, fixed element, such as a bollard lighting column or radiator, not more than 150mm deep that may intrude into a path, route, or corridor, that does not unduly restrict the passage of a wheelchair user."@en;
  skos:inScheme :conceptScheme_751925ed;
  skos:prefLabel "localised obstruction"@en .

:c_e0b7bab3 a skos:Concept;
  dct:modified "2020-10-27T07:41:00.019Z"^^xsd:dateTime;
  skos:broader :c_3cf43794;
  skos:definition "Clear floor space, represented by a rectangle which allows a wheelchair user to turn independently in a series of manoeuvres. A door swing is permitted within a clear manoeuvring space unless stated otherwise"@en;
  skos:inScheme :conceptScheme_751925ed;
  skos:prefLabel "manoeuvring space"@en .

:c_a3306811 a skos:Concept;
  skos:broader :c_3cf43794;
  skos:definition "A line that connects the nosing of the treads of a stair."@en;
  skos:prefLabel "pitch line"@en .

:c_8bff5d6c a skos:Concept;
  dct:modified "2020-10-27T07:40:38.057Z"^^xsd:dateTime;
  skos:broader :c_3cf43794;
  skos:definition "The gradient measured between the entrance storey finished floor level of the dwelling and the point of access."@en;
  skos:inScheme :conceptScheme_751925ed;
  skos:prefLabel "plot gradient"@en .

:c_cb235281 a skos:Concept;
  dct:modified "2020-10-27T07:41:03.084Z"^^xsd:dateTime;
  skos:broader :c_3cf43794;
  skos:definition "The point at which a person visiting a dwelling would normally get out of a car before approaching the dwelling. The point of access may be within or outside the plot."@en;
  skos:inScheme :conceptScheme_751925ed;
  skos:prefLabel "point of access"@en .

:c_917ae1af a skos:Concept;
  dct:modified "2020-10-27T07:41:23.006Z"^^xsd:dateTime;
  skos:broader :c_3cf43794;
  skos:definition "Space capable of providing a level access shower without the need to move walls, remove screed  or other solid flooring. It should include a capped- off floor gulley, set at an appropriate level and connected to the drainage system. (Usually provided within a wet room)."@en;
  skos:inScheme :conceptScheme_751925ed;
  skos:prefLabel "potential level access shower"@en .

:c_bb0d6dd0 a skos:Concept;
  dct:modified "2020-10-27T07:41:53.346Z"^^xsd:dateTime;
  skos:broader :c_3cf43794;
  skos:definition "The communal entrance (to the core of the building containing the dwelling) which a visitor not familiar with the building would normally expect to approach (usually the common entrance to the core of a block of flats)."@en;
  skos:inScheme :conceptScheme_751925ed;
  skos:prefLabel "principal communal entrance"@en .

:c_f90cac15 a skos:Concept;
  dct:modified "2020-10-27T07:41:29.163Z"^^xsd:dateTime;
  skos:broader :c_3cf43794;
  skos:definition "The entrance to the individual dwelling that a visitor not familiar with the dwelling would normally approach (usually the ‘front door’ to a house or ground floor flat)."@en;
  skos:inScheme :conceptScheme_751925ed;
  skos:prefLabel "principal private entrance"@en .

:c_b9882564 a skos:Concept;
  dct:modified "2020-10-27T07:41:37.993Z"^^xsd:dateTime;
  skos:broader :c_3cf43794;
  skos:definition "The floor level (of the dwelling) on which the main living space is located, where this is not the entrance storey."@en;
  skos:inScheme :conceptScheme_751925ed;
  skos:prefLabel "principal storey"@en .

:c_8a096c20 a skos:Concept;
  dct:modified "2020-10-27T07:42:06.138Z"^^xsd:dateTime;
  skos:broader :c_3cf43794;
  skos:definition "Area belonging to an individual dwelling."@en;
  skos:inScheme :conceptScheme_751925ed;
  skos:prefLabel "private (area, facilities or entrances)"@en .

:c_c12dc11d a skos:Concept;
  dct:modified "2020-10-27T07:40:29.092Z"^^xsd:dateTime;
  skos:broader :c_3cf43794;
  skos:definition "Gradient between 1:20 and 1:12"@en;
  skos:inScheme :conceptScheme_751925ed;
  skos:prefLabel "ramped"@en .

:c_089706ad a skos:Concept;
  dct:modified "2020-10-27T07:42:15.960Z"^^xsd:dateTime;
  skos:broader :c_3cf43794;
  skos:definition "A parking bay 2.4m wide x 4.8m long"@en;
  skos:inScheme :conceptScheme_751925ed;
  skos:prefLabel "standard parking bay"@en .

:c_d4fd4da6 a skos:Concept;
  dct:modified "2020-10-27T07:41:09.137Z"^^xsd:dateTime;
  skos:broader :c_3cf43794;
  skos:definition "A plot where the gradient exceeds 1:15."@en;
  skos:inScheme :conceptScheme_751925ed;
  skos:prefLabel "steeply sloping plot"@en .

:c_4eca6bbf a skos:Concept;
  dct:modified "2020-10-27T07:40:47.779Z"^^xsd:dateTime;
  skos:broader :c_3cf43794;
  skos:definition "Route without steps but that may include a ramp or a lift suitable for a wheelchair user."@en;
  skos:inScheme :conceptScheme_751925ed;
  skos:prefLabel "step-free"@en .

:c_0bf85e96 a skos:Concept;
  dct:modified "2020-10-27T07:41:17.160Z"^^xsd:dateTime;
  skos:broader :c_3cf43794;
  skos:definition "External ground surface that is firm, even, smooth enough to be wheeled over, is not covered with loose laid materials such as gravel and shingle, and has a maximum crossfall of 1:40."@en;
  skos:inScheme :conceptScheme_751925ed;
  skos:prefLabel "suitable ground surface"@en .

:c_1ca5a508 a skos:Concept;
  dct:modified "2020-10-27T07:41:34.935Z"^^xsd:dateTime;
  skos:broader :c_3cf43794;
  skos:definition "Nosings that conform with one of the options shown in Diagram 1.2 of Approved Document K"@en;
  skos:inScheme :conceptScheme_751925ed;
  skos:prefLabel "suitable tread nosings"@en .

:c_9797ec63 a skos:Concept;
  dct:modified "2020-10-27T07:42:09.634Z"^^xsd:dateTime;
  skos:broader :c_3cf43794;
  skos:definition "Category 3 dwelling constructed to be suitable for immediate occupation by a wheelchair user where the planning authority specifies that optional requirement M4(3)(2)(b) applies."@en;
  skos:inScheme :conceptScheme_751925ed;
  skos:prefLabel "wheelchair accessible"@en .

:c_2eabf3c7 a skos:Concept;
  dct:modified "2020-10-27T07:42:12.922Z"^^xsd:dateTime;
  skos:broader :c_3cf43794;
  skos:definition "Category 3 dwelling constructed with the potential to be adapted for occupation by a wheelchair user where optional requirement M4(3)(2)(a) applies."@en;
  skos:inScheme :conceptScheme_751925ed;
  skos:prefLabel "wheelchair adaptable"@en .

:c_db39fc1a a skos:Concept;
  dct:modified "2020-10-27T07:41:32.232Z"^^xsd:dateTime;
  skos:broader :c_3cf43794;
  skos:definition "WC or bathroom compartment with tanking and drainage laid to fall to a connected gulley capable of draining the floor area when used as a shower."@en;
  skos:inScheme :conceptScheme_751925ed;
  skos:prefLabel "wet room"@en .

:c_b630c168 dct:modified "2020-10-27T07:40:31.921Z"^^xsd:dateTime;
  skos:inScheme :conceptScheme_751925ed .

:c_6dcae9b3 dct:modified "2020-10-27T07:40:35.360Z"^^xsd:dateTime;
  skos:inScheme :conceptScheme_751925ed .

:c_1d89066b dct:modified "2020-10-27T07:40:45.038Z"^^xsd:dateTime;
  skos:inScheme :conceptScheme_751925ed .

:c_fcd25267 dct:modified "2020-10-27T07:40:51.011Z"^^xsd:dateTime;
  skos:inScheme :conceptScheme_751925ed .

:c_09ab5f8e dct:modified "2020-10-27T07:41:06.232Z"^^xsd:dateTime;
  skos:inScheme :conceptScheme_751925ed .

:c_5fcbc183 dct:modified "2020-10-27T07:41:11.850Z"^^xsd:dateTime;
  skos:inScheme :conceptScheme_751925ed .

:c_7003e65c dct:modified "2020-10-27T07:41:14.583Z"^^xsd:dateTime;
  skos:inScheme :conceptScheme_751925ed .

:c_6bf8d62f dct:modified "2020-10-27T07:41:20.070Z"^^xsd:dateTime;
  skos:inScheme :conceptScheme_751925ed .

:c_3d9928e0 dct:modified "2020-10-27T07:41:25.887Z"^^xsd:dateTime;
  skos:inScheme :conceptScheme_751925ed .

:c_08556adc dct:modified "2020-10-27T07:41:40.864Z"^^xsd:dateTime;
  skos:inScheme :conceptScheme_751925ed .

:c_00b6a69e dct:modified "2020-10-27T07:41:43.644Z"^^xsd:dateTime;
  skos:inScheme :conceptScheme_751925ed .

:c_7d70a254 dct:modified "2020-10-27T07:41:47.023Z"^^xsd:dateTime;
  skos:inScheme :conceptScheme_751925ed .

:c_a3306811 dct:modified "2020-10-27T07:41:49.761Z"^^xsd:dateTime;
  skos:inScheme :conceptScheme_751925ed .

:c_a5ffe780 dct:modified "2020-10-27T07:41:56.380Z"^^xsd:dateTime;
  skos:inScheme :conceptScheme_751925ed .

:c_f21d57e8 dct:modified "2020-10-27T07:41:59.665Z"^^xsd:dateTime;
  skos:inScheme :conceptScheme_751925ed .

:c_283297ae dct:modified "2020-10-27T07:42:02.710Z"^^xsd:dateTime;
  skos:inScheme :conceptScheme_751925ed .

:c_3cf43794 dct:modified "2020-10-27T07:44:07.827Z"^^xsd:dateTime;
  skos:narrower :c_00b6a69e, :c_08556adc, :c_089706ad, :c_09ab5f8e, :c_0bf85e96, :c_1ca5a508,
    :c_1d89066b, :c_283297ae, :c_2eabf3c7, :c_3d9928e0, :c_44e39791, :c_4eca6bbf, :c_572989c8,
    :c_5fcbc183, :c_6bf8d62f, :c_6dcae9b3, :c_7003e65c, :c_728f0bd1, :c_7d70a254, :c_8a096c20,
    :c_8bff5d6c, :c_917ae1af, :c_9797ec63, :c_a3306811, :c_a5ffe780, :c_b630c168, :c_b9882564,
    :c_bb0d6dd0, :c_c12dc11d, :c_cb235281, :c_d4fd4da6, :c_db39fc1a, :c_e0b7bab3, :c_f21d57e8,
    :c_f90cac15, :c_fcd25267 .

:skosCollection_50d4bd2e skos:member :c_00b6a69e, :c_084501a5, :c_08556adc, :c_089706ad,
    :c_09ab5f8e, :c_0bf85e96, :c_1ca5a508, :c_283297ae, :c_2eabf3c7, :c_3d9928e0, :c_44e39791,
    :c_4eca6bbf, :c_563fcfe6, :c_572989c8, :c_5fcbc183, :c_64811e49, :c_6bf8d62f, :c_6dcae9b3,
    :c_7003e65c, :c_728f0bd1, :c_7d70a254, :c_8a096c20, :c_8bff5d6c, :c_917ae1af, :c_9491fb8a,
    :c_9726335f, :c_9797ec63, :c_a3306811, :c_a5ffe780, :c_add7f88a, :c_b630c168, :c_b9882564,
    :c_ba5ca672, :c_c12dc11d, :c_c21e6883, :c_cb235281, :c_d4fd4da6, :c_db39fc1a, :c_dc50eeef,
    :c_e0b7bab3, :c_f21d57e8, :c_f90cac15, :c_fcd25267 .

:c_a20cbb62 dct:modified "2020-10-27T07:57:16.414Z"^^xsd:dateTime;
  skos:narrower :c_781b2410 .

:c_781b2410 a skos:Concept;
  dct:created "2020-10-27T07:56:56.364Z"^^xsd:dateTime;
  dct:modified "2020-10-27T08:02:27.391Z"^^xsd:dateTime;
  skos:broader :c_a20cbb62;
  skos:inScheme :conceptScheme_751925ed;
  skos:narrower :c_e41ef2d9;
  skos:prefLabel "access to and use of buildings volume 2 – buildings other than dwellings 2015 edition for use in england*"@en .

:c_e41ef2d9 a skos:Concept;
  dct:created "2020-10-27T08:01:59.653Z"^^xsd:dateTime;
  dct:modified "2020-10-27T08:28:37.886Z"^^xsd:dateTime;
  skos:broader :c_781b2410;
  skos:definition "The following meanings apply to terms throughout this Approved Document."@en;
  skos:inScheme :conceptScheme_751925ed;
  skos:narrower :c_084501a5, :c_64811e49, :c_9491fb8a, :c_9726335f, :c_add7f88a, :c_ba5ca672,
    :c_c21e6883, :c_dc50eeef;
  skos:notation "1.26"@en;
  skos:prefLabel "definitions"@en .

:c_64811e49 a skos:Concept;
  dct:modified "2020-10-27T08:25:48.066Z"^^xsd:dateTime;
  skos:broader :c_e41ef2d9;
  skos:definition "approach, entry or exit."@en;
  skos:inScheme :conceptScheme_751925ed;
  skos:prefLabel "access"@en .

:c_dc50eeef a skos:Concept;
  dct:modified "2020-10-27T08:25:29.835Z"^^xsd:dateTime;
  skos:broader :c_e41ef2d9;
  skos:definition "with respect to buildings or parts of buildings, means that people, regardless of disability, age or gender, are able to gain access."@en;
  skos:inScheme :conceptScheme_751925ed;
  skos:prefLabel "accessible"@en .

:c_9726335f a skos:Concept;
  dct:modified "2020-10-27T08:25:26.584Z"^^xsd:dateTime;
  skos:broader :c_e41ef2d9;
  skos:definition "when used to indicate the visual perception of one element of the building, or fitting within the building, against another means that the difference in light reflectance value between the two surfaces is greater than 30 points. Where illuminance on surfaces is greater than 200 lux, a difference in light reflectance value should be a minimum of 20 points. Where door opening furniture projects beyond the face of the door or otherwise creates enhanced differentiation and shade, a minimum difference in light reflectance value of 15 points is considered adequate. For further information, reference should be made to Colour, contrast and perception – Design guidance for internal built environments – Reading University."@en;
  skos:inScheme :conceptScheme_751925ed;
  skos:prefLabel "contrast visually"@en .

:c_ba5ca672 a skos:Concept;
  dct:modified "2020-10-27T08:25:38.305Z"^^xsd:dateTime;
  skos:broader :c_e41ef2d9;
  skos:definition "a stair intended for all users of a building on a day-to day- basis, as a normal route between levels."@en;
  skos:inScheme :conceptScheme_751925ed;
  skos:prefLabel "general access stair"@en .

:c_9491fb8a a skos:Concept;
  dct:modified "2020-10-27T08:25:32.723Z"^^xsd:dateTime;
  skos:broader :c_e41ef2d9;
  skos:definition "the amount of light falling on a surface, measured in lumens per square metre (lm/m2) or lux (lx)."@en;
  skos:inScheme :conceptScheme_751925ed;
  skos:prefLabel "illuminance"@en .

:c_563fcfe6 a skos:Concept;
  dct:modified "2020-10-27T08:25:44.114Z"^^xsd:dateTime;
  skos:broader :c_e41ef2d9;
  skos:definition "the total quantity of visible light reflected by a surface at all wavelengths and directions when illuminated by a light source."@en;
  skos:inScheme :conceptScheme_751925ed;
  skos:prefLabel "light reflectance value (lrv)"@en .

:c_add7f88a a skos:Concept;
  dct:modified "2020-10-27T08:25:35.781Z"^^xsd:dateTime;
  skos:broader :c_e41ef2d9;
  skos:definition "with respect to means of access and facilities, means that they are designed for use by people regardless of disability, age or gender, but subject to the usual gender-related conventions regarding sanitary accommodation."@en;
  skos:inScheme :conceptScheme_751925ed;
  skos:prefLabel "suitable"@en .

:c_c21e6883 a skos:Concept;
  dct:modified "2020-10-27T08:25:41.309Z"^^xsd:dateTime;
  skos:broader :c_e41ef2d9;
  skos:definition "with respect to buildings or parts of buildings, means that they are convenient for independent use."@en;
  skos:inScheme :conceptScheme_751925ed;
  skos:prefLabel "usable"@en .

:c_084501a5 a skos:Concept;
  dct:modified "2020-10-27T08:25:23.800Z"^^xsd:dateTime;
  skos:broader :c_e41ef2d9;
  skos:definition "a stair used for escape, access for maintenance, or purposes other than as a usual route for moving between levels on a day-to-day basis."@en;
  skos:inScheme :conceptScheme_751925ed;
  skos:prefLabel "utility stair"@en .

:c_f31dbf5c skos:prefLabel "seasonal system energy efficiency ratio"@en .

:c_8100dcd2 a skos:Concept;
  dct:created "2020-10-27T08:39:03.287Z"^^xsd:dateTime;
  dct:modified "2020-10-27T08:42:10.485Z"^^xsd:dateTime;
  skos:broader :c_2a34c0b8;
  skos:inScheme :conceptScheme_751925ed;
  skos:narrower :c_63f863a5;
  skos:prefLabel "p1 design and installation of electrical installations2013 edition – for use in england*"@en .

:c_2a34c0b8 dct:modified "2020-10-27T08:39:29.824Z"^^xsd:dateTime;
  skos:narrower :c_8100dcd2 .

:c_63f863a5 a skos:Concept;
  dct:created "2020-10-27T08:41:20.704Z"^^xsd:dateTime;
  dct:modified "2020-10-27T08:49:12.146Z"^^xsd:dateTime;
  skos:broader :c_8100dcd2;
  skos:inScheme :conceptScheme_751925ed;
  skos:narrower :c_1361b988, :c_7c734287, :c_82b1caf3, :c_835978b6, :c_9f89ffaf, :c_cca40edf;
  skos:prefLabel "appendix a: key terms (adp)"@en .

:c_0a3a129e skos:narrower :c_e4fa13e0 .

:c_cca40edf a skos:Concept;
  dct:modified "2020-10-27T08:47:18.121Z"^^xsd:dateTime;
  skos:broader :c_63f863a5;
  skos:definition "A certificate issued by an installer registered with an authorised competent person self-certification scheme, or by a certifier registered with an authorised third-party certification scheme stating that the work described in the certificate complies with regulations 4 and 7 of the Building Regulations 2010 (that is, the work complies with all applicable requirements in the Building Regulations)"@en;
  skos:inScheme :conceptScheme_751925ed;
  skos:prefLabel "building regulations compliance certificate"@en .

:c_82b1caf3 a skos:Concept;
  dct:modified "2020-10-27T08:47:21.041Z"^^xsd:dateTime;
  skos:broader :c_63f863a5;
  skos:definition "Fixed electric cables or fixed electrical equipment located on the consumer’s side of the electricity supply meter"@en;
  skos:inScheme :conceptScheme_751925ed;
  skos:note "NOTE: *Terms defined in regulation 2 of the Building Regulations 2010"@en;
  skos:prefLabel "electrical installation*"@en .

:c_9f89ffaf a skos:Concept;
  dct:modified "2020-10-27T08:47:26.374Z"^^xsd:dateTime;
  skos:broader :c_63f863a5;
  skos:definition "A voltage not exceeding 50V ac or 120V ripple-free dc, whether between conductors or to earth"@en;
  skos:inScheme :conceptScheme_751925ed;
  skos:note "NOTE: *Terms defined in regulation 2 of the Building Regulations 2010"@en;
  skos:prefLabel "extra-low voltage*"@en .

:c_1361b988 a skos:Concept;
  dct:modified "2020-10-27T08:47:29.156Z"^^xsd:dateTime;
  skos:broader :c_63f863a5;
  skos:definition "A voltage exceeding extra-low voltage but not exceeding 1000V ac or 1500V dc between conductors, or 600V ac or 900V dc between conductors and earth"@en;
  skos:inScheme :conceptScheme_751925ed;
  skos:note "NOTE: *Terms defined in regulation 2 of the Building Regulations 2010"@en;
  skos:prefLabel "low voltage*"@en .

:c_7c734287 a skos:Concept;
  dct:modified "2020-10-27T08:47:23.814Z"^^xsd:dateTime;
  skos:broader :c_63f863a5;
  skos:definition "A competent person registered with a Part P competent person self-certification scheme"@en;
  skos:inScheme :conceptScheme_751925ed;
  skos:prefLabel "registered competent person"@en .

:c_835978b6 a skos:Concept;
  skos:broader :c_63f863a5;
  skos:definition "A competent person registered with a Part P competent person third-party certification scheme"@en;
  skos:inScheme :conceptScheme_751925ed;
  skos:prefLabel "registered third-party certifier"@en .

:skosCollection_50d4bd2e skos:member :c_1361b988, :c_15b9d927, :c_33cf3a6e, :c_33f8635d,
    :c_4e5f287b, :c_63f863a5, :c_67243ba7, :c_6eb9d2c5, :c_7c734287, :c_7f8ff8de, :c_82b1caf3,
    :c_835978b6, :c_9f89ffaf, :c_ae0f295c, :c_c46bfd51, :c_cca40edf .

:c_c66a31b4 a skos:Concept;
  dct:created "2020-10-27T16:08:22.110Z"^^xsd:dateTime;
  skos:broader :c_5ffbc967;
  skos:inScheme :conceptScheme_751925ed;
  skos:narrower :c_6eb9d2c5;
  skos:prefLabel "q1 unauthorised access 2015 edition – for use in england*"@en .

:c_5ffbc967 dct:modified "2020-10-27T16:08:50.227Z"^^xsd:dateTime;
  skos:narrower :c_c66a31b4 .

:c_6eb9d2c5 a skos:Concept;
  dct:created "2020-10-27T16:10:02.767Z"^^xsd:dateTime;
  dct:modified "2020-10-27T16:21:33.349Z"^^xsd:dateTime;
  skos:broader :c_c66a31b4;
  skos:inScheme :conceptScheme_751925ed;
  skos:narrower :c_15b9d927, :c_33f8635d, :c_67243ba7, :c_7f8ff8de, :c_ae0f295c, :c_c46bfd51;
  skos:prefLabel "appendix a: key terms (adq)"@en .

:c_c46bfd51 a skos:Concept;
  dct:modified "2020-10-27T16:20:05.217Z"^^xsd:dateTime;
  skos:broader :c_6eb9d2c5;
  skos:definition "A complete door assembly, assembled on site or delivered as a completed assembly, consisting of the door frame, door leaf or leaves, essential hardware and any integral side panel or fanlight (but excluding coupled assemblies)."@en;
  skos:inScheme :conceptScheme_751925ed;
  skos:prefLabel "doorset"@en .

:c_7f8ff8de a skos:Concept;
  dct:modified "2020-10-27T16:19:51.515Z"^^xsd:dateTime;
  skos:broader :c_6eb9d2c5;
  skos:definition "Windows, rooflights, roof windows and similar."@en;
  skos:inScheme :conceptScheme_751925ed;
  skos:prefLabel "window"@en .

:c_4e5f287b a skos:Concept;
  dct:modified "2020-10-27T16:19:56.873Z"^^xsd:dateTime;
  skos:broader :c_c66a31b4;
  skos:definition "Either: a doorset that is proven to resist physical attack by a casual or opportunist burglar, or a bespoke doorset incorporating construction features that are proven to reduce crime."@en;
  skos:inScheme :conceptScheme_751925ed;
  skos:prefLabel "secure doorset"@en .

:c_15b9d927 a skos:Concept;
  dct:modified "2020-10-27T16:20:07.951Z"^^xsd:dateTime;
  skos:broader :c_6eb9d2c5;
  skos:definition "Either: a window that is proven to resist criminal attack, or • a bespoke window incorporating construction features that are proven to reduce crime."@en;
  skos:inScheme :conceptScheme_751925ed;
  skos:prefLabel "secure window"@en .

:c_67243ba7 a skos:Concept;
  dct:modified "2020-10-27T16:19:59.664Z"^^xsd:dateTime;
  skos:broader :c_63f863a5;
  skos:definition "Either: a window or doorway, any part of which is within 2m vertically of an accessible level surface  such as the ground or basement level, or an access balcony, or a window within 2m vertically of a flat or sloping roof (with a pitch of less than 30°) that is within 3.5m of ground level."@en;
  skos:inScheme :conceptScheme_751925ed;
  skos:prefLabel "easily accessible"@en .

:c_33f8635d a skos:Concept;
  dct:modified "2020-10-27T16:20:02.506Z"^^xsd:dateTime;
  skos:broader :c_6eb9d2c5;
  skos:definition "A doorset and window that are supplied as separate self-contained frames and fixed together on site."@en;
  skos:inScheme :conceptScheme_751925ed;
  skos:prefLabel "coupled assembly"@en .

:c_ae0f295c a skos:Concept;
  dct:modified "2020-10-27T16:19:54.140Z"^^xsd:dateTime;
  skos:broader :c_6eb9d2c5;
  skos:definition "(In the context of secure doorsets and secure windows) – a product designed and constructed in accordance with a specification or design shown by test to be capable of meeting the required performance. Further information on materials and workmanship is given in Approved Document 7."@en;
  skos:inScheme :conceptScheme_751925ed;
  skos:note "NOTE 1: Laboratories accredited by the United Kingdom Accreditation Service (UKAS) or an equivalent European national accreditation body should have the necessary expertise to conduct the relevant tests NOTE 2: Any test evidence used to confirm the security of a construction should be carefully checked to ensure that it demonstrates compliance that is adequate and that applies to the intended use. Evidence passed from one organisation to another can become unreliable if important details are lost. Small differences in construction can significantly affect the performance of a doorset or window. NOTE 3: Schemes that certify compliance with PAS 24:2012 or other standards that offer similar or better performance may be acceptable for demonstrating compliance. A list of UKAS-accredited certification bodies is given on the UKAS website. Many recognised schemes are also listed in Secured by Design’s New Homes 2014, Section 2."@en;
  skos:prefLabel "proven"@en .

:c_502a871c dct:modified "2020-10-27T16:36:44.176Z"^^xsd:dateTime;
  skos:narrower :c_0109c085 .

:c_a9fc7032 a skos:Concept;
  dct:created "2020-10-27T16:38:04.682Z"^^xsd:dateTime;
  skos:broader :c_0109c085;
  skos:inScheme :conceptScheme_751925ed;
  skos:prefLabel "appendix i key terms"@en .

:c_63242aeb a skos:Concept;
  dct:created "2020-10-27T16:22:40.546Z"^^xsd:dateTime;
  dct:modified "2020-10-27T16:25:51.039Z"^^xsd:dateTime;
  skos:broader :c_b7bccf3d;
  skos:inScheme :conceptScheme_751925ed;
  skos:narrower :c_0e4cfb77;
  skos:prefLabel "r1 In-building physical infrastructure 2016 edition – for use in england*"@en .

:c_b7bccf3d dct:modified "2020-10-27T16:23:06.700Z"^^xsd:dateTime;
  skos:narrower :c_63242aeb .

:c_0e4cfb77 a skos:Concept;
  dct:created "2020-10-27T16:25:11.673Z"^^xsd:dateTime;
  dct:modified "2020-10-27T16:27:35.347Z"^^xsd:dateTime;
  skos:broader :c_63242aeb;
  skos:definition "The following are key terms used in this document and defined in regulation 44C of the Building Regulations 2010 (as amended):"@en;
  skos:inScheme :conceptScheme_751925ed;
  skos:prefLabel "appendix a: key terms (adr)"@en .

:c_67b341f4 a skos:Concept;
  dct:modified "2020-10-27T16:31:48.821Z"^^xsd:dateTime;
  skos:broader :c_0e4cfb77;
  skos:definition "A physical point, located inside or outside the building, accessible to undertakings providing or authorised to provide public communications networks, where connection to the high-speed- ready in-building physical infrastructure is made available."@en;
  skos:inScheme :conceptScheme_751925ed;
  skos:prefLabel "access point"@en .

:c_26e1919c a skos:Concept;
  dct:modified "2020-10-27T16:31:52.607Z"^^xsd:dateTime;
  skos:broader :c_0e4cfb77;
  skos:definition "An electronic communications network which is capable of delivering broadband access services at speeds of at least 30 Mbps."@en;
  skos:inScheme :conceptScheme_751925ed;
  skos:prefLabel "high-speed electronic communications network"@en .

:c_5e7bed84 a skos:Concept;
  dct:modified "2020-10-27T16:31:45.812Z"^^xsd:dateTime;
  skos:broader :c_0e4cfb77;
  skos:definition "In-building physical infrastructure intended to host elements, or enable delivery, of high-speed electronic communications networks."@en;
  skos:inScheme :conceptScheme_751925ed;
  skos:prefLabel "high-speed-ready in-building physical infrastructure"@en .

:c_99119e22 a skos:Concept;
  dct:modified "2020-10-27T16:31:58.708Z"^^xsd:dateTime;
  skos:broader :c_0e4cfb77;
  skos:definition "Physical infrastructure or installations at the end- user’s location, including elements under joint ownership, intended to host wired or wireless access networks, where such access networks are capable of delivering electronic communications services and connecting the building access point with the network termination point."@en;
  skos:inScheme :conceptScheme_751925ed;
  skos:prefLabel "in-building physical infrastructure"@en .

:c_af28f591 a skos:Concept;
  dct:modified "2020-10-27T16:31:55.572Z"^^xsd:dateTime;
  skos:broader :c_0e4cfb77;
  skos:definition "Works at the end-user’s location encompassing structural modifications of the entire in-building physical infrastructure, or of a significant part of it."@en;
  skos:inScheme :conceptScheme_751925ed;
  skos:prefLabel "major renovation works"@en .

:c_2a5aa469 a skos:Concept;
  skos:broader :c_0e4cfb77;
  skos:definition "A physical point at which an occupier is provided with access to high-speed electronic communications networks."@en;
  skos:inScheme :conceptScheme_751925ed;
  skos:note "NOTE: The ‘occupier’ is the subscriber to the broadband service. The termination point is typically inside the building, but may be outside the building for wireless connections."@en;
  skos:prefLabel "network termination point"@en .

:skosCollection_50d4bd2e skos:member :c_26e1919c, :c_2a5aa469, :c_5e7bed84, :c_67b341f4,
    :c_99119e22, :c_af28f591 .

:c_0109c085 a skos:Concept;
  dct:modified "2020-10-27T16:38:34.982Z"^^xsd:dateTime;
  skos:narrower :c_a9fc7032;
  skos:prefLabel "manual to the building regulations"@en .

:c_d4970b41 a skos:Concept;
  skos:broader :c_a9fc7032;
  skos:definition "followed by a number refers to a regulation in the Building Regulations 2010."@en;
  skos:note "Terms relating to the structure of legislation:"@en;
  skos:prefLabel "regulation"@en .

:c_89c887d6 a skos:Concept;
  skos:broader :c_a9fc7032;
  skos:definition "refers to a schedule contained in the Building Regulations 2010, for example Schedule 1 to the Building Regulations."@en;
  skos:note "Terms relating to the structure of legislation:"@en;
  skos:prefLabel "schedule"@en .

:c_325fa285 a skos:Concept;
  skos:broader :c_a9fc7032;
  skos:definition "refers to a section of the Building Act 1984."@en;
  skos:note "Terms relating to the structure of legislation:"@en;
  skos:prefLabel "section"@en .

:c_345c095e a skos:Concept;
  skos:broader :c_a9fc7032;
  skos:definition "refers to a change of the scope of an initial notice. For further information see Chapter E."@en;
  skos:prefLabel "amendment notice"@en .

:c_66d06a87 a skos:Concept;
  skos:broader :c_a9fc7032;
  skos:definition "refers to a document approved by government that provides practical guidance on how the Building Regulations can be satisfied in some common situations. Approved documents are given legal status by the Building Act 1984."@en;
  skos:prefLabel "approved document"@en .

:c_9e9fac9d a skos:Concept;
  skos:broader :c_a9fc7032;
  skos:definition "are companies or individuals authorised under the Building Act 1984 to carry out building control work in England and Wales. They must be registered with the Construction Industry Council Approved Inspectors Register (CICAIR), which provides a list of approved inspectors. https://www.cicair.org.uk/approved-inspectors-register/"@en;
  skos:prefLabel "approved inspectors"@en .

:c_4aee7770 a skos:Concept;
  skos:broader :c_a9fc7032;
  skos:definition "refers to the Building (Approved Inspectors etc.) Regulations 2010."@en;
  skos:prefLabel "approved inspectors regulations"@en .

:c_33cf3a6e a skos:Concept;
  skos:broader :c_a9fc7032;
  skos:definition "is generally any permanent or temporary building. A reference to a building includes a reference to part of a building. Buildings include dwellings (houses, flats) and public buildings."@en;
  skos:inScheme :conceptScheme_751925ed;
  skos:prefLabel "building"@en .

:c_77212558 a skos:Concept;
  skos:broader :c_a9fc7032;
  skos:definition "refers to the Building Act 1984."@en;
  skos:inScheme :conceptScheme_751925ed;
  skos:prefLabel "building act"@en .

:c_0775280b a skos:Concept;
  skos:broader :c_a9fc7032;
  skos:definition "is a local authority building control department or an approved inspector."@en;
  skos:inScheme :conceptScheme_751925ed;
  skos:prefLabel "building control body"@en .

:c_616fbf78 a skos:Concept;
  skos:broader :c_a9fc7032;
  skos:definition "is a route to Building Regulations approval using local authority building control. Refer to Chapter D for details."@en;
  skos:inScheme :conceptScheme_751925ed;
  skos:prefLabel "building notice"@en .

:c_d4486d47 a skos:Concept;
  skos:broader :c_a9fc7032;
  skos:definition "refers to the Building Regulations 2010."@en;
  skos:inScheme :conceptScheme_751925ed;
  skos:prefLabel "building regulations"@en .

:c_a00c11cf a skos:Concept;
  skos:broader :c_a9fc7032;
  skos:definition "includes erecting or extending a building, providing or extending a controlled service or fitting in or in connection with a building, and the material alteration of a building or a controlled service or fitting."@en;
  skos:inScheme :conceptScheme_751925ed;
  skos:prefLabel "building work"@en .

:c_22a21142 a skos:Concept;
  skos:broader :c_a9fc7032;
  skos:definition "under the Construction Products Regulation (305/2011/EU-CPR). The Construction Products Regulation requires that construction products on the EU market covered by a harmonised European product standard normally have a CE marking. Refer to Chapter F for details."@en;
  skos:inScheme :conceptScheme_751925ed;
  skos:prefLabel "ce marking"@en .

:c_0f6ef18a a skos:Concept;
  skos:broader :c_a9fc7032;
  skos:definition "allow tradespeople to demonstrate their ability to carry out certain work to required standards instead of the work going through a building control body approval process. Refer to Chapter 5 and Chapter C."@en;
  skos:inScheme :conceptScheme_751925ed;
  skos:prefLabel "competent person schemes"@en .

:c_e8d281dd a skos:Concept;
  skos:broader :c_a9fc7032;
  skos:definition "are issued by the local authority to confirm that it has taken reasonable steps to ensure that there is evidence, but not necessarily conclusive evidence, that the work complies with the relevant requirements of the Building Regulations."@en;
  skos:inScheme :conceptScheme_751925ed;
  skos:prefLabel "completion certificates"@en .

:c_6b4d8aa6 a skos:Concept;
  skos:broader :c_a9fc7032;
  skos:definition "include a service or fitting subject to Schedule 1 (to the Building Regulations) requirements in respect of sanitation, hot water safety, water efficiency, drainage and waste disposal, combustion appliances and fuel storage, conservation of fuel or power, and electrical safety."@en;
  skos:inScheme :conceptScheme_751925ed;
  skos:prefLabel "controlled services or fittings"@en .

:c_24fd49d7 a skos:Concept;
  skos:broader :c_a9fc7032;
  skos:definition "refers to the certificate issued by the approved inspector to the person carrying out the work and the local authority and confirms that the work in the initial notice is complete and that the approved inspector is satisfied that it complies with the relevant requirements of the Building Regulations."@en;
  skos:inScheme :conceptScheme_751925ed;
  skos:prefLabel "final certificate"@en .

:c_43607495 a skos:Concept;
  skos:broader :c_a9fc7032;
  skos:definition "refers to the route to Building Regulations approval using local authority building control. Refer to Chapter D for details."@en;
  skos:inScheme :conceptScheme_751925ed;
  skos:prefLabel "full plans"@en .

:c_7a693319 a skos:Concept;
  skos:broader :c_a9fc7032;
  skos:definition "refers to the notice served on the local authority jointly by the client and the approved inspector when an approved inspector is selected as the building control body."@en;
  skos:inScheme :conceptScheme_751925ed;
  skos:prefLabel "initial notice"@en .

:c_ab86b8aa a skos:Concept;
  skos:broader :c_a9fc7032;
  skos:definition "operates in addition to normal planning controls under the  Planning (Listed Buildings and Conservation Areas) Act 1990. Listed building consent is likely to be required for any alteration to a listed building."@en;
  skos:inScheme :conceptScheme_751925ed;
  skos:prefLabel "listed building consent"@en .

:c_3f20a780 a skos:Concept;
  skos:broader :c_a9fc7032;
  skos:definition "is the building control department of the local authority."@en;
  skos:inScheme :conceptScheme_751925ed;
  skos:prefLabel "local authority building control"@en .

:c_8eaab627 a skos:Concept;
  skos:broader :c_a9fc7032;
  skos:definition "is defined in Approved Document L1B, 5.6A and L2B, 3.1."@en;
  skos:inScheme :conceptScheme_751925ed;
  skos:prefLabel "major renovation"@en .

:c_58d3c1e1 a skos:Concept;
  skos:broader :c_a9fc7032;
  skos:definition "is defined under Regulation 3 of the Building Regulations. An alteration is a material alteration if the proposed building work would make a building less safe structurally, more at risk from fire or less accessible for disabled people."@en;
  skos:inScheme :conceptScheme_751925ed;
  skos:prefLabel "material alteration"@en .

:c_fd257378 a skos:Concept;
  skos:broader :c_a9fc7032;
  skos:definition "include: manufactured products, such as components, fittings, items of equipment and systems; naturally occurring materials, such as stone, timber and thatch; and    backfilling for excavations in connection with building work."@en;
  skos:inScheme :conceptScheme_751925ed;
  skos:prefLabel "materials"@en .

:c_2da98c6b a skos:Concept;
  skos:broader :c_a9fc7032;
  skos:definition "is approval to carry out building work from a town and country planning point of view. It is typically required to construct or extend a building or change the use of a building. The local planning authority decides whether a project will need planning permission."@en;
  skos:inScheme :conceptScheme_751925ed;
  skos:prefLabel "planning permission"@en .

:c_6c87e49d a skos:Concept;
  skos:broader :c_a9fc7032;
  skos:definition "can be used to demonstrate that detailed plans of the work or a part of it comply with the Building Regulations. They are described in Regulations 14 and 15 of the Approved Inspectors Regulations and Section 50 of the Building Act."@en;
  skos:inScheme :conceptScheme_751925ed;
  skos:prefLabel "plans certificates"@en .

:c_c463b9ee a skos:Concept;
  skos:broader :c_a9fc7032;
  skos:definition "can be issued by local authorities retrospectively to indicate that work started after 11 November 1985 which has been completed complies with the Building Regulations which applied at the time the works were done."@en;
  skos:inScheme :conceptScheme_751925ed;
  skos:prefLabel "regularisation certificates"@en .

:c_646e9bae a skos:Concept;
  skos:broader :c_a9fc7032;
  skos:definition "(in relation to a thermal element) is defined in Approved Document L1B, 5.6A and L2B, 3.1."@en;
  skos:inScheme :conceptScheme_751925ed;
  skos:prefLabel "renovation"@en .

:c_a9823a22 a skos:Concept;
  skos:broader :c_a9fc7032;
  skos:definition "is the person defined in article 3 of the Regulatory Reform (Fire Safety) Order 2005 and having the duties for compliance with the Order as prescribed in article 5."@en;
  skos:inScheme :conceptScheme_751925ed;
  skos:prefLabel "responsible person"@en .

:c_fad4ccd1 a skos:Concept;
  skos:broader :c_a9fc7032;
  skos:definition "is a material that contributes to the thermal performance of a building’s thermal envelope, such as any element of a wall, floor or roof but not a door or window. Thermal element is defined in Regulation 2(3) of the Building Regulations."@en;
  skos:inScheme :conceptScheme_751925ed;
  skos:prefLabel "thermal element"@en .

:c_d4970b41 skos:inScheme :conceptScheme_751925ed .

:c_89c887d6 skos:inScheme :conceptScheme_751925ed .

:c_325fa285 skos:inScheme :conceptScheme_751925ed .

:c_345c095e skos:inScheme :conceptScheme_751925ed .

:c_66d06a87 skos:inScheme :conceptScheme_751925ed .

:c_9e9fac9d skos:inScheme :conceptScheme_751925ed .

:c_4aee7770 skos:inScheme :conceptScheme_751925ed .

:c_a9fc7032 dct:modified "2020-10-27T16:54:37.631Z"^^xsd:dateTime;
  skos:narrower :c_0775280b, :c_0f6ef18a, :c_1b060096, :c_22a21142, :c_24fd49d7, :c_2da98c6b,
    :c_325fa285, :c_33cf3a6e, :c_345c095e, :c_3f20a780, :c_43607495, :c_4aee7770, :c_58d3c1e1,
    :c_616fbf78, :c_646e9bae, :c_66d06a87, :c_6b4d8aa6, :c_6c87e49d, :c_77212558, :c_7a693319,
    :c_89c887d6, :c_8eaab627, :c_9e9fac9d, :c_a00c11cf, :c_a9823a22, :c_ab86b8aa, :c_c463b9ee,
    :c_d4486d47, :c_d4970b41, :c_e8d281dd, :c_fad4ccd1, :c_fd257378 .

:skosCollection_50d4bd2e skos:member :c_0775280b, :c_0f6ef18a, :c_22a21142, :c_24fd49d7,
    :c_2da98c6b, :c_325fa285, :c_345c095e, :c_3f20a780, :c_43607495, :c_58d3c1e1, :c_616fbf78,
    :c_646e9bae, :c_66d06a87, :c_6b4d8aa6, :c_6c87e49d, :c_77212558, :c_7a693319, :c_89c887d6,
    :c_8eaab627, :c_9e9fac9d, :c_a00c11cf, :c_a9823a22, :c_ab86b8aa, :c_c463b9ee, :c_d4486d47,
    :c_d4970b41, :c_e8d281dd, :c_fad4ccd1, :c_fd257378 .

:c_37246cae skos:broader :c_502a871c;
  skos:narrower :c_3da44764;
  skos:notation " L153"@en .

:c_3da44764 a skos:Concept;
  dct:created "2020-10-27T17:03:12.864Z"^^xsd:dateTime;
  dct:modified "2020-10-27T17:16:15.520Z"^^xsd:dateTime;
  skos:broader :c_37246cae;
  skos:inScheme :conceptScheme_751925ed;
  skos:narrower :c_08eb88d2, :c_0af8118b, :c_2689a172, :c_3454d214, :c_366cf430, :c_4775ba65,
    :c_547611a3, :c_58bdb729, :c_7abc215a, :c_8883ce73, :c_9243074f, :c_aae4241b, :c_c53e946f,
    :c_c984b189, :c_cf85f340, :c_d996e4f9, :c_da4c39b1, :c_fe309bb8;
  skos:prefLabel "glossary of acronyms and terms"@en .

:c_fe309bb8 a skos:Concept;
  skos:broader :c_3da44764;
  skos:inScheme :conceptScheme_751925ed;
  skos:notation "ACOP"@en;
  skos:prefLabel "approved code of practice"@en .

:c_6e741d9b a skos:Concept;
  skos:broader :c_3da44764;
  skos:inScheme :conceptScheme_751925ed;
  skos:notation "AOGBO 2013 "@en;
  skos:prefLabel "application to areas outside great britain order 2013"@en .

:c_547611a3 a skos:Concept;
  skos:broader :c_3da44764;
  skos:inScheme :conceptScheme_751925ed;
  skos:notation "CDM 2007 "@en;
  skos:prefLabel "construction (design and management) regulations 2007"@en .

:c_4775ba65 a skos:Concept;
  skos:broader :c_3da44764;
  skos:inScheme :conceptScheme_751925ed;
  skos:notation "CITB"@en;
  skos:prefLabel "construction industry training board"@en .

:c_0af8118b a skos:Concept;
  skos:broader :c_3da44764;
  skos:inScheme :conceptScheme_751925ed;
  skos:notation "HSE"@en;
  skos:prefLabel "health and safety executive"@en .

:c_c984b189 a skos:Concept;
  skos:broader :c_3da44764;
  skos:inScheme :conceptScheme_751925ed;
  skos:notation "HSWA"@en;
  skos:prefLabel "health and safety at work etc act 1974"@en .

:c_58bdb729 a skos:Concept;
  skos:broader :c_3da44764;
  skos:inScheme :conceptScheme_751925ed;
  skos:notation "LWIT"@en;
  skos:prefLabel "leadership and worker involvement toolkit"@en .

:c_aae4241b a skos:Concept;
  skos:broader :c_3da44764;
  skos:definition "management of health and safety at work regulations 1999"@en;
  skos:inScheme :conceptScheme_751925ed;
  skos:prefLabel "the management regulations"@en .

:c_3454d214 a skos:Concept;
  skos:broader :c_3da44764;
  skos:definition "‘must’ is used only where there is an absolute duty, ie an explicit legal requirement to take a certain action which is not qualified by terms such as ‘so far as reasonably practicable’"@en;
  skos:inScheme :conceptScheme_751925ed;
  skos:prefLabel "must"@en .

:c_d996e4f9 a skos:Concept;
  skos:broader :c_3da44764;
  skos:inScheme :conceptScheme_751925ed;
  skos:notation "ONR"@en;
  skos:prefLabel "office for nuclear regulation"@en .

:c_da4c39b1 a skos:Concept;
  skos:broader :c_3da44764;
  skos:inScheme :conceptScheme_751925ed;
  skos:notation "ORR"@en;
  skos:prefLabel "office of rail regulation"@en .

:c_9243074f a skos:Concept;
  skos:broader :c_3da44764;
  skos:inScheme :conceptScheme_751925ed;
  skos:notation "PAS 91 "@en;
  skos:prefLabel "publicly available specification 91"@en .

:c_366cf430 a skos:Concept;
  skos:broader :c_3da44764;
  skos:definition "balancing the level of risk against the measures needed to control the real risk in terms of money, time or trouble. However, you do not need to take action if it would be grossly disproportionate to the level of risk (see www.gov.uk/risk/faq.htm for the most up-to-date explanation of what ‘reasonably practicable’ means.)"@en;
  skos:inScheme :conceptScheme_751925ed;
  skos:prefLabel "reasonably practicable"@en .

:c_8883ce73 a skos:Concept;
  skos:broader :c_3da44764;
  skos:definition "areas outside the territorial sea designated for the exploration or exploitation of energy from water or winds (see section 84 of the Energy Act 2004)."@en;
  skos:inScheme :conceptScheme_751925ed;
  skos:prefLabel "renewable energy zone"@en .

:c_7abc215a a skos:Concept;
  skos:broader :c_3da44764;
  skos:definition "‘should’ is used to indicate what to do to comply with legal requirements which are qualified by terms such as ‘so far as reasonably practicable’."@en;
  skos:inScheme :conceptScheme_751925ed;
  skos:prefLabel "should"@en .

:c_c53e946f a skos:Concept;
  skos:broader :c_3da44764;
  skos:definition "not necessarily those that involve the greatest risks, but those (including health risks) that are not likely to be obvious, are unusual, or likely to be difficult to manage effectively."@en;
  skos:inScheme :conceptScheme_751925ed;
  skos:prefLabel "significant risks"@en .

:c_2689a172 a skos:Concept;
  skos:broader :c_3da44764;
  skos:definition "SSIP"@en;
  skos:inScheme :conceptScheme_751925ed;
  skos:prefLabel "safety schemes in procurement"@en .

:c_08eb88d2 a skos:Concept;
  skos:broader :c_3da44764;
  skos:definition "means the belt of waters extending from the coast of Great Britain up to 12 nautical miles."@en;
  skos:inScheme :conceptScheme_751925ed;
  skos:prefLabel "territorial sea"@en .

:c_cf85f340 a skos:Concept;
  skos:broader :c_3da44764;
  skos:definition "Workplace (Health, Safety and Welfare) Regulations 1992."@en;
  skos:inScheme :conceptScheme_751925ed;
  skos:prefLabel "workplace regulations"@en .

:skosCollection_50d4bd2e dct:modified "2020-10-27T17:17:05.529Z"^^xsd:dateTime;
  skos:member :c_08eb88d2, :c_0af8118b, :c_2689a172, :c_3454d214, :c_366cf430, :c_4775ba65,
    :c_547611a3, :c_58bdb729, :c_6e741d9b, :c_7abc215a, :c_8883ce73, :c_9243074f, :c_aae4241b,
    :c_c53e946f, :c_c984b189, :c_cf85f340, :c_d996e4f9, :c_da4c39b1, :c_fe309bb8 .

:c_58df2af5 rdfs:isDefinedBy "https://www.legislation.gov.uk/uksi/2010/2214/schedule/1/made"@en .

:c_1fa348f3 dct:modified "2020-11-04T19:36:58.191Z"^^xsd:dateTime;
  rdfs:isDefinedBy "https://www.legislation.gov.uk/uksi/2010/2214/schedule/1/made"@en;
  skos:definition """The building shall be constructed so that the combined dead,
imposed and wind loads are sustained and transmitted by it to the
ground: (a) safely; and (b) without causing such deflection or deformation of any
part of the building, or such movement of the ground, as will impair
the stability of any part of another building. (2) In assessing whether a building complies with sub-paragraph
(1) regard shall be had to the imposed and wind loads to which it is
likely to be subjected in the ordinary course of its use for the purpose
for which it is intended."""@en;
  skos:notation "uksi 2010 2214"@en .

:c_56aca7cf dct:modified "2020-11-04T19:35:46.767Z"^^xsd:dateTime;
  rdfs:isDefinedBy "https://www.legislation.gov.uk/uksi/2010/2214/schedule/1/made"@en;
  skos:definition """The building shall be constructed so that in the event of an accident
the building will not suffer collapse to an extent disproportionate to
the cause."""@en;
  skos:notation "uksi 2010 2214"@en .

:c_34ab31dc dct:modified "2020-11-04T19:46:53.950Z"^^xsd:dateTime;
  rdfs:isDefinedBy "https://www.legislation.gov.uk/uksi/2010/2214/schedule/1/made"@en;
  skos:definition "The building shall be constructed so that ground movement\\\\ncaused by: (a) swelling, shrinkage or freezing of the subsoil; or (b) land-slip or subsidence (other than subsidence arising\\\\nfrom shrinkage), in so far as the risk can be reasonably foreseen,will not impair the stability of any part of the building."@en;
  skos:notation "uksi 2010 2214"@en .

:c_bd26d581 dct:modified "2020-11-04T19:40:29.581Z"^^xsd:dateTime;
  rdfs:isDefinedBy "https://www.legislation.gov.uk/uksi/2010/2214/schedule/1/made"@en;
  skos:definition """The building shall be designed and constructed so that
there are appropriate provisions for the early warning
of fire, and appropriate means of escape in case of
fire from the building to a place of safety outside the
building capable of being safely and effectively used
at all material times."""@en;
  skos:notation "uksi 2010 2214"@en .

:c_926affad dct:modified "2020-11-04T19:49:53.201Z"^^xsd:dateTime;
  rdfs:isDefinedBy "https://www.legislation.gov.uk/uksi/2010/2214/schedule/1/made"@en;
  skos:definition """(1) To inhibit the spread of fire within the building,
the internal linings shall
(a) adequately resist the spread of flame over
their surfaces; and
(b) have, if ignited, either a rate of heat release
or a rate of fire growth, which is reasonable in
the circumstances.
(2) In this paragraph internal linings means the
materials or products used in lining any partition,
wall, ceiling or other internal structure."""@en;
  skos:notation "uksi 2010 2214"@en .

:c_419da0ad dct:modified "2020-11-04T19:46:15.575Z"^^xsd:dateTime;
  rdfs:isDefinedBy "https://www.legislation.gov.uk/uksi/2010/2214/schedule/1/made"@en;
  skos:definition """(1) The building shall be designed and constructed
so as to provide reasonable facilities to assist fire
fighters in the protection of life.
(2) Reasonable provision shall be made within the site of the building to enable fire appliances to gain
access to the building."""@en;
  skos:notation "uksi 2010 2214"@en .

:c_d7714b03 dct:modified "2020-11-04T19:43:36.245Z"^^xsd:dateTime;
  rdfs:isDefinedBy "https://www.legislation.gov.uk/uksi/2010/2214/schedule/1/made"@en;
  skos:definition """1) The building shall be designed and constructed
so that, in the event of fire, its stability will be
maintained for a reasonable period
(2) A wall common to two or more buildings shall be
designed and constructed so that it adequately
resists the spread of fire between those buildings.
For the purposes of this sub-paragraph a house in
a terrace and a semi-detached house are each to
be treated as a separate building.
(3) Where reasonably necessary to inhibit the spread
of fire within the building, measures shall be
taken, to an extent appropriate to the size and
intended use of the building, comprising either or
both of the following
(a) sub-division of the building with fire-resisting
construction;
(b) installation of suitable automatic fire
suppression systems.
(4) The building shall be designed and constructed so that
the unseen spread of fire and smoke within concealed
spaces in its structure and fabric is inhibited."""@en;
  skos:notation "uksi 2010 2214"@en .

:c_95a5e382 dct:modified "2020-11-04T19:44:22.103Z"^^xsd:dateTime;
  rdfs:isDefinedBy "https://www.legislation.gov.uk/uksi/2010/2214/schedule/1/made"@en;
  skos:definition """(1) The external walls of the building shall adequately
resist the spread of fire over the walls and from
one building to another, having regard to the
height, use and position of the building.
(2) The roof of the building shall adequately resist
the spread of fire over the roof and from one
building to another, having regard to the use and
position of the building."""@en;
  skos:notation "uksi 2010 2214"@en .

:c_86cfaae6 dct:modified "2020-11-04T18:00:49.243Z"^^xsd:dateTime .

:c_06f29df7 skos:definition """(1) Building work shall be carried out
(a) with adequate and proper materials which
(i) are appropriate for the circumstances in which
they are used,
(ii) are adequately mixed or prepared, and
(iii) are applied, used or fixed so as adequately
to perform the functions for which they are
designed; and
(b) in a workmanlike manner.
(2) Subject to paragraph (3), building work shall be
carried out so that materials which become part
of an external wall, or specified attachment, of a
relevant building are of European Classification
A2-s1, d0 or A1, classified in accordance with BS EN
13501-1:2007+A1:2009 entitled Fire classification
of construction products and building elements.
Classification using test data from reaction to fire
tests (ISBN 978 0 580 59861 6) published by the
British Standards Institution on 30th March 2007 and
amended in November 2009."""@en .

:c_0e0d001c skos:notation "uksi 2005 1541"@en .

:c_3360da6c a skos:Concept;
  dct:created "2020-11-04T20:20:33.430Z"^^xsd:dateTime;
  dct:modified "2020-11-04T20:35:53.626Z"^^xsd:dateTime;
  rdfs:isDefinedBy "https://www.legislation.gov.uk/uksi/2015/51/contents"@en;
  skos:broader :c_f9b32acf;
  skos:inScheme :conceptScheme_751925ed;
  skos:notation "uksi 2015 51"@en;
  skos:prefLabel "construction design and management regulations 2015"@en .

:c_968e7c1f a skos:Concept;
  skos:broader :c_0a3a129e;
  skos:definition "The relevant RIBA Workplan stage(s)"@en;
  skos:prefLabel "stage"@en .

:c_f9b32acf skos:narrower :c_3360da6c .

:c_0a3a129e skos:narrower :c_018a1d30, :c_0210074d, :c_05c76d2d, :c_07a8e657, :c_0802aff2,
    :c_137f7ffc, :c_139d2f2a, :c_18e998f8, :c_1c903d67, :c_26743597, :c_2ac99285, :c_2c07ff89,
    :c_2cb7906e, :c_318fb161, :c_3349c2e1, :c_35c247b9, :c_39577f6f, :c_3b05bfb8, :c_484e0930,
    :c_4a67ba9b, :c_4a8dcdc9, :c_4f742433, :c_52a85821, :c_53038005, :c_534d35d7, :c_58bdc056,
    :c_59b11797, :c_5b9a650d, :c_5c48bbaa, :c_5fdb1f6a, :c_63926bce, :c_64bab517, :c_65324c7f,
    :c_6a5b3011, :c_6b2833fd, :c_6eef78b8, :c_72b73e69, :c_770bb6fb, :c_77832b8d, :c_81a8092b,
    :c_89cf2365, :c_8c631147, :c_9335950c, :c_9662f5a5, :c_a036fe97, :c_b29f9b08, :c_b5c5e19b,
    :c_bca7cb38, :c_bd0800cd, :c_be148bd6, :c_bf4f2585, :c_bfc76e2b, :c_c19f24b3, :c_cc8f5bda,
    :c_cd1c45db, :c_cecb1246, :c_d2d64e35, :c_da70f5e9, :c_dcca2002, :c_e20e91e9, :c_e5e64950,
    :c_e7e7700c, :c_e902bfa9, :c_ecc476c8, :c_ee0a8125, :c_eff2c5e0, :c_f329d120, :c_f91ecc12 .

:c_2cb7906e skos:inScheme :conceptScheme_751925ed .

:c_d2d64e35 skos:inScheme :conceptScheme_751925ed .

:c_07a8e657 skos:inScheme :conceptScheme_751925ed .

:c_9335950c skos:inScheme :conceptScheme_751925ed .

:c_a7557993 a skos:Concept;
  skos:broader :c_0a3a129e;
  skos:definition "The Contracting Authority aspirations for sustainability, which may include additional objectives, measures or specific levels of performance in relation to international standards, as well as details of specific demands in relation to operational or facilities management issues."@en;
  skos:prefLabel "sustainability aspirations"@en .

:c_9662f5a5 skos:inScheme :conceptScheme_751925ed .

:c_39577f6f skos:inScheme :conceptScheme_751925ed .

:c_4867a906 skos:prefLabel "value engineering"@en .

:c_e5e64950 skos:inScheme :conceptScheme_751925ed .

:c_cd1c45db skos:inScheme :conceptScheme_751925ed .

:c_4f742433 skos:inScheme :conceptScheme_751925ed .

:c_9480d322 a skos:Concept;
  skos:broader :c_0a3a129e;
  skos:definition "The Sustainability Strategy will be prepared in response to the Sustainability Aspirations and will include specific additional items, such as an energy plan and ecology plan and the design life of the building, as appropriate."@en;
  skos:prefLabel "sustainability strategy"@en .

:c_aab41011 a skos:Concept;
  skos:broader :c_0a3a129e;
  skos:definition """The strategy established at the outset of a project that sets out technologies, including Building Information Modelling (BIM) and any supporting processes (including the Project BIM Protocol, Project Information Plan and the BIM documents), and the specific software packages that each member of the Project Team will use. Any interoperability issues can then be addressed before the design phases commence.
This strategy also establishes how information is to be communicated and managed by the use of a Common Data Environment and all information, non-graphical and graphical, and the file formats for such information that the Project Team is required to provide into the Information Model for the purpose of delivering Project Outputs. The Project Execution Plan records agreements made."""@en;
  skos:prefLabel "technology strategy"@en .

:c_cecb1246 skos:inScheme :conceptScheme_751925ed .

:c_d55b2d04 a skos:Concept;
  skos:broader :c_0a3a129e;
  skos:definition "Shall include as a minimum the consideration of issues and provision information and advice as to life cycle costs, including costs in use, appropriate sources of energy, thermal modelling, energy conservation, solar gain, environmental impact issues, water consumption, maintenance and renewal requirements, any potential benefits of long term maintenance agreements in relation to specific equipment and plant etc."@en;
  skos:prefLabel "sustainability checkpoint"@en .

:c_bd0800cd skos:inScheme :conceptScheme_751925ed .

:c_534d35d7 skos:inScheme :conceptScheme_751925ed .

:c_3b05bfb8 skos:inScheme :conceptScheme_751925ed .

:c_cc8f5bda skos:inScheme :conceptScheme_751925ed .

:c_75f7c82b a skos:Concept;
  skos:broader :c_3360da6c;
  skos:inScheme :conceptScheme_751925ed;
  skos:notation "uksi 2015 51"@en;
  skos:prefLabel "introduction"@en .

:c_3360da6c skos:narrower :c_75f7c82b .

:c_139d3767 skos:inScheme :conceptScheme_751925ed .

:c_1e8a7cbf a skos:Concept;
  skos:broader :c_75f7c82b;
  skos:definition "means a trade, business or other undertaking (whether for profit or not)"@en;
  skos:notation "uksi 2015 51"@en;
  skos:prefLabel "business"@en .

:c_c31ddac5 a skos:Concept;
  skos:broader :c_75f7c82b;
  skos:definition "means any person for whom a project is carried out"@en;
  skos:notation "uksi 2015 51"@en;
  skos:prefLabel "client"@en .

:c_ef1c9d78 a skos:Concept;
  skos:broader :c_75f7c82b;
  skos:definition "means the period of time beginning when construction work in a project starts and ending when construction work in that project is completed"@en;
  skos:notation "uksi 2015 51"@en;
  skos:prefLabel "construction phase"@en .

:c_f97db0fd a skos:Concept;
  skos:broader :c_75f7c82b;
  skos:definition "means a plan drawn up under regulations 12 or 15"@en;
  skos:notation "uksi 2015 51"@en;
  skos:prefLabel "construction phase plan"@en .

:c_5918929b a skos:Concept;
  skos:broader :c_75f7c82b;
  skos:definition "includes any place where construction work is being carried out or to which the workers have access, but does not include a workplace within the site which is set aside for purposes other than construction work"@en;
  skos:notation "uksi 2015 51"@en;
  skos:prefLabel "construction site"@en .

:c_1dfadb92 a skos:Concept;
  skos:broader :c_75f7c82b;
  skos:definition "means any person (including a non-domestic client) who, in the course or furtherance of a business, carries out, manages or controls construction work"@en;
  skos:notation "uksi 2015 51"@en;
  skos:prefLabel "contractor"@en .

:c_f127ef1e a skos:Concept;
  skos:broader :c_75f7c82b;
  skos:definition "includes drawings, design details, specifications and bills of quantities (including specification of articles or substances) relating to a structure, and calculations prepared for the purpose of a design"@en;
  skos:notation "uksi 2015 51"@en;
  skos:prefLabel "design"@en .

:c_659ab1b8 a skos:Concept;
  skos:broader :c_75f7c82b;
  skos:definition "means any person (including a client, contractor or other person referred to in these Regulations) who in the course or furtherance of a business (a) prepares or modifies a design or (b) arranges for, or instructs, any person under their control to do so, relating to a structure, or to a product or mechanical or electrical system intended for a particular structure, and a person is deemed to prepare a design where a design is prepared by a person under their control"@en;
  skos:notation "uksi 2015 51"@en;
  skos:prefLabel "designer"@en .

:c_f340cba7 a skos:Concept;
  skos:broader :c_75f7c82b;
  skos:definition "means the carrying out of any building, civil engineering or engineering construction work and includes (a) the construction, alteration, conversion, fitting out, commissioning, renovation, repair, upkeep, redecoration or other maintenance (including cleaning which involves the use of water or an abrasive at high pressure, or the use of corrosive or toxic substances), decommissioning, demolition or dismantling of a structure (b) the preparation for an intended structure, including site clearance, exploration, investigation (but not site survey) and excavation (but not pre-construction archaeological investigations), and the clearance or preparation of the site or structure for use or occupation at its conclusion (c) the assembly on site of prefabricated elements to form a structure or the disassembly on site of the prefabricated elements which, immediately before such disassembly, formed a structure (d) the removal of a structure, or of any product or waste resulting from demolition or dismantling of a structure, or from disassembly of prefabricated elements which immediately before such disassembly formed such a structure (e) the installation, commissioning, maintenance, repair or removal of mechanical, electrical, gas, compressed air, hydraulic, telecommunications, computer or similar services which are normally fixed within or to a structure"@en;
  skos:notation "uksi 2015 51"@en;
  skos:prefLabel "construction work"@en .

:c_3a5b7e76 a skos:Concept;
  skos:broader :c_75f7c82b;
  skos:definition "means a client for whom a project is being carried out which is not in the course or furtherance of a business of that client"@en;
  skos:notation "uksi 2015 51"@en;
  skos:prefLabel "domestic client"@en .

:c_daa05efb a skos:Concept;
  skos:broader :c_75f7c82b;
  skos:definition "includes any earthwork, trench, well, shaft, tunnel or underground working the general principles of prevention means the general principles of prevention specified in Schedule 1 to the Management Regulations"@en;
  skos:notation "uksi 2015 51"@en;
  skos:prefLabel "excavation"@en .

:c_454526b8 a skos:Concept;
  skos:broader :c_75f7c82b;
  skos:definition "means a file prepared under regulation 12(5)inspector for the Executive means an inspector within the meaning given in section 53(1) of the 1974 Act(a)"@en;
  skos:notation "uksi 2015 51"@en;
  skos:prefLabel "health and safety file (cdm)"@en .

:c_007625df a skos:Concept;
  skos:broader :c_75f7c82b;
  skos:definition "means any facility for loading or unloading place of work means any place which is used by any person at work for the purposes of construction work or for the purposes of any activity arising out of or in connection with construction work"@en;
  skos:notation "uksi 2015 51"@en;
  skos:prefLabel "loading bay"@en .

:c_9d2dac79 a skos:Concept;
  skos:broader :c_75f7c82b;
  skos:definition " means information in the client’s possession or which is reasonably obtainable by or on behalf of the client, which is relevant to the construction work and is of an appropriate level of detail and proportionate to the risks involved, including (a) information about—(i) the project(ii) planning and management of the project(iii) health and safety hazards, including design and construction hazards and how they will be addressed and(b) information in any existing health and safety file"@en;
  skos:notation "uksi 2015 51"@en;
  skos:prefLabel "pre-construction information"@en .

:c_2f92acaa a skos:Concept;
  skos:broader :c_75f7c82b;
  skos:definition "means any period of time during which design or preparatory work is carried out for a project and may continue during the construction phase"@en;
  skos:notation "uksi 2015 51"@en;
  skos:prefLabel "pre-construction phase"@en .

:c_a4cdd233 a skos:Concept;
  skos:broader :c_75f7c82b;
  skos:definition " means the contractor appointed under regulation 5(1)(b) to perform the specified duties in regulations 12 to 14"@en;
  skos:notation "uksi 2015 51"@en;
  skos:prefLabel "principal contractor"@en .

:c_da079e58 a skos:Concept;
  skos:broader :c_75f7c82b;
  skos:definition "means the designer appointed under regulation 5(1)(a) to perform the specified duties in regulations 11 and 12"@en;
  skos:notation "uksi 2015 51"@en;
  skos:prefLabel "principal designer"@en .

:c_fabf0784 a skos:Concept;
  skos:broader :c_75f7c82b;
  skos:definition "means a project which includes or is intended to include construction work and includes all planning, design, management or other work involved in a project until the end of the construction phase"@en;
  skos:notation "uksi 2015 51"@en;
  skos:prefLabel "project"@en .

:c_1d287961 a skos:Concept;
  skos:broader :c_75f7c82b;
  skos:definition " means rules which are drawn up for a particular construction site and are necessary for health or safety purposes structure means (a) any building, timber, masonry, metal or reinforced concrete structure, railway line or siding, tramway line, dock, harbour, inland navigation, tunnel, shaft, bridge, viaduct, waterworks, reservoir, pipe or pipeline, cable, aqueduct, sewer, sewage works, gasholder, road, airfield, sea defence works, river works, drainage works, earthworks, lagoon, dam, wall, caisson, mast, tower, pylon, underground tank, earth retaining structure or structure designed to preserve or alter any natural feature and fixed plant (b) any structure similar to anything specified in paragraph (a) (c) any formwork, falsework, scaffold or other structure designed or used to provide support or means of access during construction work, and any reference to a structure includes part of a structure"@en;
  skos:notation "uksi 2015 51"@en;
  skos:prefLabel "site rules"@en .

:c_851c02b0 a skos:Concept;
  skos:broader :c_75f7c82b;
  skos:definition "means a route for pedestrian traffic or for vehicles and includes any doorway,gateway, loading bay or ramp"@en;
  skos:notation "uksi 2015 51"@en .

:c_0a3a129e a skos:Concept;
  skos:broader :c_502a871c;
  skos:inScheme :conceptScheme_751925ed;
  skos:prefLabel "related"@en .

:c_502a871c skos:narrower :c_0a3a129e .

:c_0802aff2 a skos:Concept;
  skos:broader :c_0a3a129e;
  skos:definition "A scheme authorised under the Building Act 1984 by which registered installers are able to self-certify certain types of building work without the involvement of a building control body."@en;
  skos:prefLabel "competent person scheme"@en;
  skos:inScheme :conceptScheme_751925ed .

:c_ecc476c8 a skos:Concept;
  skos:broader :c_0a3a129e;
  skos:definition "The point at the end of the construction process when building work is completed and needs to be assessed prior to occupation."@en;
  skos:inScheme :conceptScheme_751925ed;
  skos:prefLabel "completion stage"@en .

:c_318fb161 a skos:Concept;
  skos:broader :c_0a3a129e;
  skos:definition "One of the core information products that dutyholders must produce during the design and construction phase – it describes how building safety and Building Regulations compliance will be maintained during the construction phase and how any changes to the Full Plans signed off at Gateway Point 2 will be controlled and recorded."@en;
  skos:inScheme :conceptScheme_751925ed;
  skos:prefLabel "construction control plan"@en .

:c_59b11797 a skos:Concept;
  skos:broader :c_0a3a129e;
  skos:definition "A term describing a procurement route in which the main contractor is appointed to design and construct the works, as opposed to a traditional contract, where the client appoints consultants to design the development and then a contractor is appointed to construct the works."@en;
  skos:inScheme :conceptScheme_751925ed;
  skos:prefLabel "design and build"@en .

:c_a036fe97 a skos:Concept;
  skos:broader :c_0a3a129e;
  skos:definition "An assessment carried out in lieu of a physical test. The term is particularly associated with cladding systems and is also referred to as an ‘assessment in lieu of test’."@en;
  skos:inScheme :conceptScheme_751925ed;
  skos:prefLabel "desktop study"@en .

:c_77832b8d a skos:Concept;
  skos:broader :c_0a3a129e;
  skos:definition "Those key roles (whether fulfilled by individuals or organisations) that are assigned specific responsibilities at particular phases of the building life cycle."@en;
  skos:inScheme :conceptScheme_751925ed;
  skos:prefLabel "dutyholders"@en .

:c_72b73e69 a skos:Concept;
  skos:broader :c_0a3a129e;
  skos:definition "One of the core information products that dutyholders must produce during the design and construction phase and it must be handed over to the building owner on occupation. This file will contain specified information and will help the building owner to better understand how to effectively manage their building in respect to fire/emergency situation."@en;
  skos:inScheme :conceptScheme_751925ed;
  skos:prefLabel "fire and emergency file"@en .

:c_2c07ff89 skos:inScheme :conceptScheme_751925ed .

:c_6b2833fd skos:inScheme :conceptScheme_751925ed .

:c_89cf2365 skos:inScheme :conceptScheme_751925ed .

:c_b29f9b08 skos:broader :c_0a3a129e;
  skos:definition "Guidance approved under section 6 of the Building Act 1984 to provide practical guidance on ways to comply with the requirements in the building regulations."@en .

:c_bfc76e2b a skos:Concept;
  skos:broader :c_0a3a129e;
  skos:definition "A systematic examination of the building structure, fabric and services to assess the likelihood of fire and the impact to those who may be affected if a fire occurs. Under the Regulatory Reform (Fire Safety) Order 2005, a fire risk assessment must evaluate the risk from fire to relevant persons (persons lawfully on the premises and/or persons in the immediate vicinity who are at risk from fire on the premises) for the purpose of identifying the general fire precautions needed to comply with the provisions of the Order."@en;
  skos:inScheme :conceptScheme_751925ed;
  skos:prefLabel "fire risk assessment"@en .

:c_8c631147 a skos:Concept;
  skos:broader :c_0a3a129e;
  skos:definition "Under the new regulatory framework building work to create/refurbish an HRRB will require dutyholders to submit detailed design plans that will be subject to assessment by the Joint Competent Authority (JCA). Until the JCA approve these detailed plans as properly managing the building safety risks (and meeting other Building Regulations requirements) then building work will not be allowed to commence."@en;
  skos:inScheme :conceptScheme_751925ed;
  skos:prefLabel "full plans approval"@en .

:c_3349c2e1 a skos:Concept;
  skos:broader :c_0a3a129e;
  skos:definition "This is the key stages in the building life-cycle of which the dutyholder has to satisfy the Joint Competent Authority (JCA) that their plans are robust; that their understanding and management of risk is appropriately detailed; and that they can properly account for the safety of the as-built building."@en;
  skos:inScheme :conceptScheme_751925ed;
  skos:prefLabel "gateway points"@en .

:c_5b9a650d a skos:Concept;
  skos:broader :c_0a3a129e;
  skos:definition "This is a file prepared under regulation 12 (5) of the Construction (Design and Management) Regulations 2015."@en;
  skos:inScheme :conceptScheme_751925ed;
  skos:prefLabel "health and safety file"@en .

:c_e7e7700c a skos:Concept;
  skos:broader :c_0a3a129e;
  skos:definition "Multi-occupancy higher risk residential buildings (that are 10 storeys or more in height. They are the primary focus of the new regulatory framework set out in this report."@en;
  skos:inScheme :conceptScheme_751925ed;
  skos:prefLabel "higher risk residential building (hrrb)"@en .

:c_eff2c5e0 a skos:Concept;
  skos:broader :c_0a3a129e;
  skos:definition "The proposed new combined regulatory oversight body for HRRBs, comprising the Health and Safety Executive, Local Authority Building Standards and fire and rescue authorities."@en;
  skos:inScheme :conceptScheme_751925ed;
  skos:prefLabel "joint competent authority (jca)"@en .

:c_be148bd6 a skos:Concept;
  skos:broader :c_0a3a129e;
  skos:definition "The life of a building covering procurement, design, construction, occupation, maintenance and refurbishment."@en;
  skos:inScheme :conceptScheme_751925ed;
  skos:prefLabel "life cycle of building"@en .

:c_4a8dcdc9 a skos:Concept;
  skos:definition "A statutory process of assessing plans for building work and building work on site to decide whether the plans and work comply with the requirements in the building regulations."@en;
  skos:inScheme :conceptScheme_751925ed;
  skos:prefLabel "building control"@en .

:c_e20e91e9 skos:broader :c_0a3a129e;
  skos:definition "An assessment carried out in lieu of a physical test. The term is particularly associated with cladding systems and is also referred to as a �desktop study�."@en;
  skos:inScheme :conceptScheme_751925ed .

:c_35c247b9 a skos:Concept;
  skos:broader :c_0a3a129e;
  skos:definition "Reporting of any safety-related event which, if not corrected or addressed, could endanger residents or employees."@en;
  skos:inScheme :conceptScheme_751925ed;
  skos:prefLabel "mandatory occurrence reporting"@en .

:c_65324c7f a skos:Concept;
  skos:broader :c_0a3a129e;
  skos:definition "A requirement in regulation 4(3) of the Building Regulations 2010 that building work must be carried out so that, after it has been completed, the building or controlled service or fitting complies with all relevant requirements or, where it did not previously comply, is no more unsatisfactory in relation to that requirement than before the work was carried out."@en;
  skos:inScheme :conceptScheme_751925ed;
  skos:prefLabel "non-worsening (of compliance)"@en .

:c_58bdc056 a skos:Concept;
  skos:broader :c_0a3a129e;
  skos:definition "The system defines the outcomes or performance level to be achieved not the way those outcomes must be met"@en;
  skos:inScheme :conceptScheme_751925ed;
  skos:prefLabel "outcomes-based system"@en .

:c_26743597 a skos:Concept;
  skos:broader :c_0a3a129e;
  skos:definition "The system defines the prescribed criteria to be met not the outcome to be achieved. Meeting a desired outcome or performance level is presumed if the prescribed criteria are met."@en;
  skos:inScheme :conceptScheme_751925ed;
  skos:prefLabel "prescriptive system"@en .

:c_1c903d67 a skos:Concept;
  skos:broader :c_0a3a129e;
  skos:definition "The Committee (appointed under the Building Act 1984 Part 1 Section 14) advises the Secretary of State in England on proposals to make or change building regulations and the system in which they operate. The Committee also provides expert advice to the Secretary of State on related matters such as the health and safety, welfare and convenience of people in and around buildings; energy conservation and the sustainability of buildings."@en .

:c_cecb1246 skos:broader :c_0a3a129e;
  skos:definition "A statutory enforcement notice which would include timescales for completion of any works."@en;
  skos:prefLabel "building improvement/ correction notices"@en .

:c_53038005 a skos:Concept;
  skos:inScheme :conceptScheme_751925ed .

:c_05c76d2d a skos:Concept;
  skos:prefLabel "building safety"@en .

:c_5fdb1f6a a skos:Concept;
  skos:broader :c_0a3a129e;
  skos:definition "Public Interest Disclosure Act 1998 protects workers from detrimental treatment or victimisation from their employer if, in the public interest, they make certain types of protected disclosures."@en;
  skos:inScheme :conceptScheme_751925ed;
  skos:prefLabel "public interest disclosure act"@en .

:c_17ac084f a skos:Concept;
  skos:broader :c_0a3a129e;
  skos:definition "A new sanction so that where the JCA/Local Authority Building Standards are of the opinion that the building work (or supporting processes) has serious deficiencies then work can be stopped until resolved to the satisfaction of the JCA."@en;
  skos:inScheme :conceptScheme_751925ed;
  skos:prefLabel "stop notices"@en .

:c_c19f24b3 a skos:Concept;
  skos:broader :c_0a3a129e;
  skos:definition "A plan for delivering resident engagement, outlining how the dutyholder will share information with residents, how they inform them of their rights and responsibilities, and how they consult residents on changes to the building which could impact on safety."@en;
  skos:inScheme :conceptScheme_751925ed;
  skos:prefLabel "resident engagement strategy"@en .

:c_6a5b3011 a skos:Concept;
  skos:broader :c_0a3a129e;
  skos:definition "Under the Regulatory Reform (Fire Safety) Order 2005, a responsible person is generally an employer or, in premises which is not a workplace, the owner or other person who has control of the premises in connection with carrying on of a trade, business or other undertaking (whether for profit or not)."@en;
  skos:inScheme :conceptScheme_751925ed;
  skos:prefLabel "responsible person"@en .

:c_e902bfa9 a skos:Concept;
  skos:broader :c_0a3a129e;
  skos:definition "The roles identified in the RIBA 2013 Plan of Work.  The roles and responsibilities for each of the Core Service Disciplines are provided in Framework Schedule 2: Services and Key Performance Indicators Annex A � Schedule of Services."@en;
  skos:inScheme :conceptScheme_751925ed;
  skos:prefLabel "core service disciplines"@en .

:c_6eef78b8 skos:inScheme :conceptScheme_751925ed;
  skos:prefLabel "approved inspector (ai)"@en;
  a skos:Concept .

:c_968e7c1f skos:inScheme :conceptScheme_751925ed .

:c_e4fa13e0 skos:inScheme :conceptScheme_751925ed .

:c_58b42d76 skos:inScheme :conceptScheme_751925ed .

:c_6f581d4d skos:inScheme :conceptScheme_751925ed .

:c_484e0930 skos:inScheme :conceptScheme_751925ed .

:c_dcca2002 skos:inScheme :conceptScheme_751925ed .

:c_139d2f2a skos:inScheme :conceptScheme_751925ed .

:c_5c48bbaa skos:inScheme :conceptScheme_751925ed .

:c_81a8092b skos:inScheme :conceptScheme_751925ed .

:c_bf4f2585 skos:inScheme :conceptScheme_751925ed .

:c_770bb6fb skos:inScheme :conceptScheme_751925ed .

:c_f91ecc12 skos:inScheme :conceptScheme_751925ed .

:c_64bab517 skos:inScheme :conceptScheme_751925ed .

:c_18e998f8 skos:inScheme :conceptScheme_751925ed .

:c_0210074d skos:inScheme :conceptScheme_751925ed .

:c_4a67ba9b skos:inScheme :conceptScheme_751925ed .

:c_da70f5e9 a skos:Concept;
  skos:broader :c_0a3a129e;
  skos:inScheme :conceptScheme_751925ed .

:c_f329d120 skos:inScheme :conceptScheme_751925ed .

:c_137f7ffc skos:broader :c_0a3a129e .

:c_018a1d30 skos:inScheme :conceptScheme_751925ed .

:c_bca7cb38 skos:inScheme :conceptScheme_751925ed .

:c_ee0a8125 skos:inScheme :conceptScheme_751925ed .

:c_2ac99285 skos:inScheme :conceptScheme_751925ed .

:c_a7557993 skos:inScheme :conceptScheme_751925ed .

:c_d55b2d04 skos:inScheme :conceptScheme_751925ed .

:c_9480d322 skos:inScheme :conceptScheme_751925ed .

:c_aab41011 skos:inScheme :conceptScheme_751925ed .

:c_63926bce a skos:Concept;
  skos:broader :c_0a3a129e;
  skos:definition "Architects Registration Board was established by section 1 of the Architects Act 1997 to regulate the architects� profession in the UK. Registration with the Board allows the use of the protected title architect."@en;
  skos:inScheme :conceptScheme_751925ed;
  skos:prefLabel "architects registration board"@en .

:c_bd0800cd a skos:Concept;
  skos:broader :c_0a3a129e;
  skos:definition "Information produced at the end of a project to represent what has been constructed. This will comprise a mixture of as-built information from specialist Sub-Contractors and the final construction issue from design team members. A Contracting Authority may also wish to undertake as-built surveys using new surveying technologies, to bring a further degree of accuracy to this information."@en;
  skos:prefLabel "as constructed information"@en .

:c_3b05bfb8 a skos:Concept;
  skos:broader :c_0a3a129e;
  skos:definition "The contract between the Contracting Authority, and the contractor for the design and construction of the project, or the construction of the project only. In some instances, the Building Contract may contain design duties for specialist Sub- Contractors and/or design team members. On some projects, more than one Building Contract may be required; for example, one for shell and core works and another for furniture, fitting and equipment aspects."@en;
  skos:prefLabel "building contract"@en .

:c_da334512 a skos:Concept;
  skos:broader :c_0a3a129e;
  skos:definition "An evidence based approach in which the dutyholder identifies the hazards and risks, describes how risks are controlled and describes the safety management system in place for a HRRB. The safety case file is then assessed by the JCA."@en;
  skos:prefLabel "safety case"@en .

:c_9662f5a5 a skos:Concept;
  skos:broader :c_0a3a129e;
  skos:definition "The rationale behind the initiation of a new building project. It may consist solely of a reasoned argument. It may contain supporting information, financial appraisals or other background information. It should also highlight initial considerations for the Project Outcomes. In summary, it is a combination of objective and subjective considerations.  The Business Case might be prepared in relation to a number of sites or in relation to assessing refurbishment against new build option."@en;
  skos:prefLabel "business case"@en .

:c_39577f6f a skos:Concept;
  skos:broader :c_0a3a129e;
  skos:definition """Procedures for controlling changes to the design and construction, following the sign-off of the Stage 2 Concept Design and the
Final Project Brief."""@en;
  skos:prefLabel "change control procedures"@en .

:c_b29f9b08 a skos:Concept;
  skos:inScheme :conceptScheme_751925ed;
  skos:prefLabel "approved document"@en .

:c_4867a906 a skos:Concept;
  skos:broader :c_0a3a129e;
  skos:definition "Value engineering is a systematic and organised approach to providing the necessary functions in a project at the lowest cost. Value engineering promotes the substitution of materials and methods with less expensive alternatives."@en;
  skos:inScheme :conceptScheme_751925ed .

:c_e5e64950 a skos:Concept;
  skos:broader :c_0a3a129e;
  skos:definition "The strategy that sets out when the Project Team will meet, how they will communicate effectively and the protocols for issuing information between the various parties, both informally and at Information Exchanges."@en;
  skos:prefLabel "communication strategy"@en .

:c_cd1c45db a skos:Concept;
  skos:broader :c_0a3a129e;
  skos:definition "The period in the Project Programme and the Building Contract for the construction of the project, commencing at the start of the site mobilisation date and ending at Practical Completion."@en;
  skos:prefLabel "construction programme"@en .

:c_4f742433 a skos:Concept;
  skos:broader :c_0a3a129e;
  skos:definition "A strategy that addresses specific aspects of the design that may affect the buildability or logistics of constructing a project, or may affect health and safety aspects and comprises items such as cranage, site access and accommodation locations, reviews of the supply chain and sources of materials, and specific buildability items, such as the choice of frame (steel or concrete) or the installation of larger items of plant. On a smaller project, the strategy may be restricted to the location of site cabins and storage, and the ability to transport materials up an existing staircase."@en;
  skos:prefLabel "construction strategy"@en .

:c_534d35d7 a skos:Concept;
  skos:broader :c_0a3a129e;
  skos:definition "Proposals presented by a contractor to the Contracting Authority in response to a tender that includes the Employers Requirements. The Contractors Proposals may match the Employers Requirements, although certain aspects may be varied based on value engineered solutions, and additional information may be submitted to clarify what is included in the Tender. The Contractors Proposals form an integral component of the Building Contract documentation."@en;
  skos:prefLabel "contractors proposals"@en .

:c_b5c5e19b a skos:Concept;
  skos:broader :c_0a3a129e;
  skos:definition "A diagram that clarifies the contractual relationship between the Contracting Authority and the parties undertaking the roles required on a project."@en;
  skos:inScheme :conceptScheme_751925ed;
  skos:prefLabel "contractual tree"@en .

:c_4a8dcdc9 skos:broader :c_0a3a129e .

:c_05c76d2d skos:broader :c_0a3a129e;
  skos:definition "building safety refers to fire safety and structural safety. This may also apply to other disciplines such as electrical and gas safety, where these could impact on the fire safety of the building."@en;
  skos:inScheme :conceptScheme_751925ed .

:c_1c903d67 skos:inScheme :conceptScheme_751925ed;
  skos:prefLabel "building regulations advisory committee (brac)"@en .

:c_89cf2365 a skos:Concept;
  skos:broader :c_0a3a129e;
  skos:definition "The timetable for the delivery of the outputs by each Project Team Member for one or more of the RIBA Workplan Stages;"@en;
  skos:prefLabel "delivery timetable"@en .

:c_2c07ff89 a skos:Concept;
  skos:broader :c_0a3a129e;
  skos:definition "A programme setting out the strategic dates in relation to the design process. It is aligned with the Project Programme."@en;
  skos:prefLabel "design programme"@en .

:c_52a85821 a skos:Concept;
  skos:broader :c_0a3a129e;
  skos:definition "Queries relating to the design arising from the site, typically managed using a contractors in-house request for information or technical query process."@en;
  skos:inScheme :conceptScheme_751925ed;
  skos:prefLabel "design queries"@en .

:c_cc8f5bda a skos:Concept;
  skos:broader :c_0a3a129e;
  skos:definition "A matrix that sets out who is responsible for designing each aspect of the project and when. This document sets out the extent of any performance specified design.  The Design Responsibility Matrix is created at a strategic level at Stage 1 and fine-tuned in response to the Concept Design at the end of Stage 2, and reviewed and updated at Stages 3, 4 and 5 in order to ensure that there are no design responsibility ambiguities at Stages 3, 4 and 5."@en;
  skos:prefLabel "design responsibility matrix"@en .

:c_6b2833fd a skos:Concept;
  skos:broader :c_0a3a129e;
  skos:definition "A system whereby the member of a Project Team notifies the Contracting Authority and other suppliers as soon as the member is aware of a matter adversely affecting the project, its own performance or the performance of another member of the Project Team. The notification shall include proposals (within the scope of its agreed role, responsibilities and expertise) for avoiding or remedying the matter."@en;
  skos:prefLabel "early warning system"@en .

:c_cecb1246 a skos:Concept .

:c_2cb7906e a skos:Concept;
  skos:broader :c_0a3a129e;
  skos:definition "Studies undertaken to test the feasibility of the Initial Project Brief on a specific site or in a specific context and to consider how site-wide issues will be addressed."@en;
  skos:prefLabel "feasibility study"@en .

:c_d2d64e35 a skos:Concept;
  skos:broader :c_0a3a129e;
  skos:definition "Feedback from the Project Team and the end users, following completion of a project."@en;
  skos:prefLabel "feedback"@en .

:c_07a8e657 a skos:Concept;
  skos:broader :c_0a3a129e;
  skos:definition "The Initial Project Brief amended so that it is aligned with the Concept Design and any briefing decisions made during Stage 2. (Both the Concept Design and Initial Project Brief are Information Exchanges at the end of Stage 2)."@en;
  skos:prefLabel "final project brief"@en .

:c_9335950c a skos:Concept;
  skos:broader :c_0a3a129e;
  skos:definition "The strategy for handing over a building, including the requirements for phased handovers, commissioning, training of staff or other factors crucial to the successful occupation of a building. The Government Soft Landings process shall be used as the basis for formulating the strategy and undertaking a Post-Occupancy Evaluation."@en;
  skos:prefLabel "handover strategy"@en .

:c_0210074d a skos:Concept;
  skos:broader :c_0a3a129e;
  skos:definition "The strategy covering all aspects of health and safety on the project, outlining legislative requirements as well as other project initiatives, including the Maintenance and Operational Strategy."@en;
  skos:prefLabel "health & safety strategy"@en .

:c_6eef78b8 skos:broader :c_0a3a129e;
  skos:definition "Bodies approved under Part 2 section 49 of the Building Act 1984 to carry out building control functions as an alternative to local authority building control. Almost all are private sector bodies."@en .

:c_e20e91e9 a skos:Concept;
  skos:prefLabel "assessment in lieu of test"@en .

:c_2ac99285 a skos:Concept;
  skos:broader :c_0a3a129e;
  skos:definition "The brief prepared following discussions with the Contracting Authority to ascertain the Project Objectives, the Contracting Authority Business Case and, in certain instances, in response to site Feasibility Studies."@en;
  skos:prefLabel "initial project brief"@en .

:c_ee0a8125 a skos:Concept;
  skos:broader :c_0a3a129e;
  skos:definition "The strategy for the maintenance and operation of a building, including details of any specific plant required to replace components."@en;
  skos:prefLabel "maintenance and operational strategy"@en .

:c_bca7cb38 a skos:Concept;
  skos:broader :c_0a3a129e;
  skos:definition "The Non-Core Service Disciplines comprise roles which may be required in addition to the Core Service Disciplines for a project. Examples (which are not an exhaustive list) of the Non-Core Service Disciplines that may be required are provided in Framework Schedule 2: Services and Key Performance Indicators."@en;
  skos:prefLabel "non-core service disciplines"@en .

:c_018a1d30 a skos:Concept;
  skos:broader :c_0a3a129e;
  skos:definition "Evaluation undertaken post-occupancy to determine whether the Project Outcomes, both subjective and objective, set out in the Final Project Brief have been achieved."@en;
  skos:prefLabel "post-occupancy evaluation"@en .

:c_137f7ffc a skos:Concept;
  skos:definition "A local authority or an Approved Inspector who assess conformity with the building regulations."@en;
  skos:inScheme :conceptScheme_751925ed;
  skos:prefLabel "building control bodies"@en .

:c_da334512 skos:inScheme :conceptScheme_751925ed .

:c_f329d120 a skos:Concept;
  skos:broader :c_0a3a129e;
  skos:definition "The Contracting Authority budget for the Project, which may include the construction cost as well as the cost of certain items required post completion and during its operational use."@en;
  skos:prefLabel "project budget"@en .

:c_53038005 skos:broader :c_0a3a129e;
  skos:definition "Those parts of a domestic property (such as a block of flats) which is used in common by the occupants of more than one flat (such as the corridors and fire-escape routes)."@en;
  skos:prefLabel "common parts"@en .

:c_4a67ba9b a skos:Concept;
  skos:broader :c_0a3a129e;
  skos:definition "Information, including models, documents, specifications, schedules and spreadsheets, issued between parties during each stage and, in formal Information Exchanges, at the end of each Stage."@en;
  skos:prefLabel "project information"@en .

:c_da70f5e9 skos:definition "Construction provided to prevent the spread of fire to or from another part of the same building or an adjoining building. For example, compartment walls and floors with a rated period of fire resistance are provided to separate individual flats."@en;
  skos:prefLabel "compartmentation"@en .

:c_18e998f8 a skos:Concept;
  skos:broader :c_0a3a129e;
  skos:definition "The Contracting Authority key objectives as set out in the Initial Project Brief. The document includes, where appropriate, the Contracting Authority Business Case, Sustainability Aspirations or other aspects that may influence the preparation of the brief and, in turn, the Concept Design stage. For example, Feasibility Studies may be required in order to test the Initial Project Brief against a given site, allowing certain high-level briefing issues to be considered before design work commences in earnest."@en;
  skos:prefLabel "project objectives"@en .

:c_64bab517 a skos:Concept;
  skos:broader :c_0a3a129e;
  skos:definition "The desired outcomes for the project (for example, in the case of a hospital this might be a reduction in recovery times). The outcomes may include operational aspects and a mixture of subjective and objective criteria."@en;
  skos:prefLabel "project outcomes"@en .

:c_f91ecc12 a skos:Concept;
  skos:broader :c_0a3a129e;
  skos:definition "Configured information delivered from the Information Model for a specific permitted purpose e.g. stage outputs, Information Exchanges, submissions for planning, procurement, construction etc."@en;
  skos:prefLabel "project outputs"@en .

:c_770bb6fb a skos:Concept;
  skos:broader :c_0a3a129e;
  skos:definition "The performance of the project, determined using Feedback, including about the performance of the Project Team and the performance of the building against the desired Project Outcomes."@en;
  skos:prefLabel "project performance"@en .

:c_bf4f2585 a skos:Concept;
  skos:broader :c_0a3a129e;
  skos:definition "The overall period for the briefing, design, construction and post-completion activities of a project."@en;
  skos:prefLabel "project programme"@en .

:c_81a8092b a skos:Concept;
  skos:broader :c_0a3a129e;
  skos:definition "A table that sets out the roles required on a project as well as defining the stages during which those roles are required and the parties responsible for carrying out the roles. The strategies developed in parallel with the Concept Design to support the design and, in certain instances, to respond to the Final Project Brief as it is concluded. These strategies will typically include:-          acoustic strategy -          fire engineering strategy -          Maintenance and Operational Strategy-          Sustainability Strategy -          building control strategy -          Technology Strategy These strategies are usually prepared in outline at Stage 2 and in detail at Stage 3, with the recommendations absorbed into the Stage 4 outputs and Information Exchanges. The intention is that they should be transferred into the various models or drawn information."@en;
  skos:prefLabel "project roles table"@en .

:c_5c48bbaa a skos:Concept;
  skos:broader :c_0a3a129e;
  skos:definition "The participants involved in the delivery of a project as identified in the Project Execution Plan."@en;
  skos:prefLabel "project team"@en .

:c_139d2f2a a skos:Concept;
  skos:broader :c_0a3a129e;
  skos:definition """Any person having responsibilities in relation to the production, delivery and/or use of the content of the Information Model
and appointed by the Contracting Authority in relation to a project."""@en;
  skos:prefLabel "project team member"@en .

:c_dcca2002 a skos:Concept;
  skos:broader :c_0a3a129e;
  skos:definition "The objectives that set out the quality aspects of a project. The objectives may comprise both subjective and objective aspects, although subjective aspects may be subject to a design quality indicator (DQI) benchmark review during the Feedback period."@en;
  skos:prefLabel "quality objectives"@en .

:c_484e0930 a skos:Concept;
  skos:broader :c_0a3a129e;
  skos:definition "Project specific research and development responding to the Initial Project Brief or in response to the Concept Design, as it is developed."@en;
  skos:prefLabel "research and development"@en .

:c_6f581d4d a skos:Concept;
  skos:broader :c_0a3a129e;
  skos:definition "The Risk Assessments consider the various design and other risks on a project and how each risk will be managed and the party responsible for managing each risk."@en;
  skos:prefLabel "risk assessments"@en .

:c_58b42d76 a skos:Concept;
  skos:broader :c_0a3a129e;
  skos:definition """A list of specific services and tasks (duties) to be undertaken by a party involved in the project which is incorporated into their
Call Off Agreement."""@en;
  skos:prefLabel "schedule of services"@en .

:c_e4fa13e0 a skos:Concept;
  skos:broader :c_0a3a129e;
  skos:definition "Specific Project Information in the form of specialist surveys or reports relating to the project or site specific context."@en;
  skos:prefLabel "site information"@en .

:c_6e741d9b skos:notation " L153"@en .

:c_fe309bb8 skos:notation " L153"@en .

:c_547611a3 skos:notation " L153"@en .

:c_4775ba65 skos:notation " L153"@en .

:c_c984b189 skos:notation " L153"@en .

:c_0af8118b skos:notation " L153"@en .

:c_58bdb729 skos:notation " L153"@en .

:c_3454d214 skos:notation " L153"@en .

:c_d996e4f9 skos:notation " L153"@en .

:c_da4c39b1 skos:notation " L153"@en .

:c_9243074f skos:notation " L153"@en .

:c_366cf430 skos:notation " L153"@en .

:c_8883ce73 skos:notation " L153"@en .

:c_2689a172 skos:notation " L153"@en .

:c_7abc215a skos:notation " L153"@en .

:c_c53e946f skos:notation " L153"@en .

:c_08eb88d2 skos:notation " L153"@en .

:c_aae4241b skos:notation " L153"@en .

:c_cf85f340 skos:notation " L153"@en .

:c_5db451a3 a skos:Concept;
  skos:broader :c_0a3a129e;
  skos:inScheme :conceptScheme_751925ed;
  skos:prefLabel "residual risk"@en .

:c_0a3a129e skos:narrower :c_5db451a3 .

:skosCollection_f8d24590 dct:modified "2019-11-30T10:51:04.187Z"^^xsd:dateTime .

:c_00420f4a a skos:Concept;
  dct:created "2018-04-21T07:45:14.755Z"^^xsd:dateTime;
  skos:broader :c_2425ea08;
  skos:inScheme :conceptScheme_751925ed;
  skos:prefLabel "building services designer"@en;
  skosxl:prefLabel :xl_en_7d34f8d2 .

:c_2425ea08 a skos:Concept;
  dct:created "2018-04-21T07:02:55.604Z"^^xsd:dateTime;
  dct:modified "2018-08-22T15:55:39.762Z"^^xsd:dateTime;
  skos:broader :c_ca2b1c80;
  skos:inScheme :conceptScheme_751925ed;
  skos:narrower :c_00420f4a, :c_05837165, :c_0d539813, :c_1258140e, :c_162b9e61, :c_1e174ca8,
    :c_20cde89c, :c_324b2ef1, :c_32b1f026, :c_36f0ebbb, :c_386bb74f, :c_49e95986, :c_4a31c73a,
    :c_4de09d2e, :c_4e68f3f9, :c_500dee4e, :c_5060b718, :c_55d219f9, :c_782fa318, :c_9260f33c,
    :c_92b99561, :c_97ba48a0, :c_ad02e5d9, :c_b03db527, :c_b3c41b17, :c_bbc32497, :c_bd6073c7,
    :c_c048d0a8, :c_c4f5d4fc, :c_c58c00ba, :c_d1fb700d, :c_e7195c13, :c_edaf8450;
  skos:prefLabel "engineering roles"@en;
  skosxl:prefLabel :xl_en_1a7bc156 .

:conceptScheme_751925ed a skos:ConceptScheme;
  dc:contributor "British Standards Institution"@en;
  dc:creator "P Stacey"@en;
  dct:created "2018-04-07T19:41:18.052Z"^^xsd:dateTime;
  dct:license <http://creativecommons.org/licenses/by/4.0/>;
  dct:modified "2019-11-30T10:41:58.827Z"^^xsd:dateTime;
  skos:prefLabel "Drawing information"@en, "General"@en, "Information and communication"@en,
    "Labour"@en, "Legislation"@en, "Materials"@en, "Phases of development (construction)"@en .

:xl_en_7d34f8d2 a skosxl:Label;
  skosxl:literalForm "building services designer"@en .

:c_026699d9 a skos:Concept;
  dct:created "2018-05-12T17:09:06.273Z"^^xsd:dateTime;
  dct:modified "2020-10-31T05:49:08.950Z"^^xsd:dateTime;
  skos:broader :c_a314e31f;
  skos:inScheme :conceptScheme_751925ed;
  skosxl:prefLabel :xl_en_9535d806 .

:c_a314e31f a skos:Concept;
  dc:source "BS ISO 6707-2-2017-Buildings and civil engineering works. Vocabulary. Contract and communication terms"@en;
  dct:created "2018-04-21T15:43:52.266Z"^^xsd:dateTime;
  dct:modified "2018-07-24T16:54:07.965Z"^^xsd:dateTime;
  skos:inScheme :conceptScheme_751925ed;
  skos:prefLabel "knowledge management related"@en;
  skos:topConceptOf :conceptScheme_751925ed .

:xl_en_9535d806 a skosxl:Label;
  skosxl:literalForm "inconsistency "@en .

:c_02705d6a a skos:Concept;
  dct:created "2018-05-26T09:21:04.004Z"^^xsd:dateTime;
  dct:modified "2018-05-26T09:23:19.776Z"^^xsd:dateTime;
  skos:broader :c_aca16e26;
  skos:definition "minded building information modelling, digital built environments and smart asset management"@en;
  skos:inScheme :conceptScheme_751925ed;
  skos:prefLabel "pas 1192-5:2015 specification for security"@en;
  skos:related :c_a2512527;
  skosxl:prefLabel :xl_en_e367b77f .

:c_aca16e26 a skos:Concept;
  dct:created "2018-03-28T19:31:12.323Z"^^xsd:dateTime;
  dct:modified "2018-08-11T09:26:27.621Z"^^xsd:dateTime;
  skos:inScheme :conceptScheme_751925ed;
  skos:narrower :c_02705d6a, :c_075ae9b8, :c_263f8b4d, :c_3a3d92ab, :c_42ccc536, :c_4a209fca,
    :c_4de604ce, :c_50aeabe6, :c_556714cc, :c_5de8e729, :c_6666c1fb, :c_773411de, :c_89607d24,
    :c_8cff7d88, :c_9e9b604b, :c_a2512527, :c_a6870cbf, :c_b80b8cad, :c_b95acbc8, :c_bcaf43b0,
    :c_df0a0804;
  skos:prefLabel "technical standards"@en;
  skos:topConceptOf :conceptScheme_751925ed;
  skosxl:prefLabel :xl_en_97e8ae77 .

:c_a2512527 a skos:Concept;
  dc:rights "British Standards Institution"@en;
  dct:created "2018-05-26T08:44:40.016Z"^^xsd:dateTime;
  dct:isReferencedBy :c_df0a0804;
  dct:modified "2020-10-31T06:05:45.955Z"^^xsd:dateTime;
  rdfs:seeAlso :c_075ae9b8, :c_08498a44, :c_0d6f0660, :c_19a61f73, :c_1efc9178, :c_28df75da,
    :c_2a55a494, :c_2a84910f, :c_2e6cd3a6, :c_31175b54, :c_3a3d92ab, :c_3f128faf, :c_3fdd4da0,
    :c_42ccc536, :c_4dd7fd6a, :c_50aeabe6, :c_556714cc, :c_5bc1704c, :c_5de8e729, :c_6666c1fb,
    :c_7d508f5e, :c_800d8fbb, :c_818585d8, :c_8cff7d88, :c_8f194b82, :c_9e9b604b, :c_9f1a47e2,
    :c_a6870cbf, :c_b046bfd7, :c_b80b8cad, :c_b95acbc8, :c_bcaf43b0, :c_bd21cb81, :c_c7b03ed3,
    :c_d0fec206, :c_df0a0804, :c_ff860f3e;
  skos:broader :c_aca16e26;
  skos:definition "toFollow"@en;
  skos:example <https://page.bsigroup.com/l/73472/2020-06-12/rhflqh>;
  skos:inScheme :conceptScheme_751925ed;
  skos:prefLabel "little book of bim"@en;
  skosxl:prefLabel :xl_en_479835d3 .

:xl_en_e367b77f a skosxl:Label;
  dct:modified "2018-05-26T09:22:07.717Z"^^xsd:dateTime;
  skosxl:literalForm "pas 1192-5:2015 specification for security"@en .

:c_03d0de39 a skos:Concept;
  dct:created "2018-03-28T14:43:10.502Z"^^xsd:dateTime;
  dct:modified "2018-07-20T19:46:08.284Z"^^xsd:dateTime;
  skos:broader :c_a314e31f;
  skos:hiddenLabel """2.1.1
"""@en;
  skos:inScheme :conceptScheme_751925ed;
  skos:prefLabel "Authorize Design; Provide Design Funding"@en;
  skosxl:hiddenLabel :xl_en_76bd2153;
  skosxl:prefLabel :xl_en_f47d9c96 .

:xl_en_76bd2153 a skosxl:Label;
  skosxl:literalForm """2.1.1
"""@en .

:xl_en_f47d9c96 a skosxl:Label;
  skosxl:literalForm "Authorize Design; Provide Design Funding"@en .

:c_05837165 a skos:Concept;
  dct:created "2018-04-21T07:44:52.690Z"^^xsd:dateTime;
  skos:broader :c_2425ea08;
  skos:inScheme :conceptScheme_751925ed;
  skos:prefLabel "acoustic consultant"@en;
  skosxl:prefLabel :xl_en_87b1def0 .

:xl_en_87b1def0 a skosxl:Label;
  skosxl:literalForm "acoustic consultant"@en .

:c_075ae9b8 a skos:Concept;
  dct:created "2018-05-26T09:50:15.263Z"^^xsd:dateTime;
  dct:modified "2018-05-26T09:51:31.249Z"^^xsd:dateTime;
  skos:broader :c_aca16e26;
  skos:definition "Attributes for specification and assessment, code of practice"@en;
  skos:inScheme :conceptScheme_751925ed;
  skos:prefLabel "bs 8541-4:2012 library objects for architecture, engineering and construction"@en;
  skos:related :c_a2512527;
  skosxl:prefLabel :xl_en_d1574160 .

:xl_en_d1574160 a skosxl:Label;
  skosxl:literalForm "bs 8541-4:2012 library objects for architecture, engineering and construction"@en .

:c_08498a44 a skos:Concept;
  dct:created "2018-06-02T14:17:18.327Z"^^xsd:dateTime;
  dct:modified "2020-10-31T05:16:49.678Z"^^xsd:dateTime;
  skos:broader :c_fb07c266;
  skos:definition """2D CAD drafting utilised
– no collaboration.
"""@en;
  skos:inScheme :conceptScheme_751925ed;
  skosxl:prefLabel :xl_en_5447d7e0 .

:xl_en_5447d7e0 a skosxl:Label;
  skosxl:literalForm "bim level 0"@en .

:c_09f6c52a a skos:Concept;
  dct:created "2018-05-12T17:13:53.590Z"^^xsd:dateTime;
  dct:modified "2020-11-01T10:22:22.832Z"^^xsd:dateTime;
  skos:broader :c_fb07c266;
  skos:inScheme :conceptScheme_751925ed;
  skos:prefLabel "bim protocol"@en;
  skos:related :c_0d543967;
  skosxl:prefLabel :xl_en_e9e3334d .

:xl_en_260474f3 skosxl:literalForm "bs 8536-2 briefing for design and construction. code of practice for asset management"@en .

:c_fb07c266 a skos:Concept;
  dc:source "buildingSMART Data Dictionary";
  dct:created "2018-04-20T19:12:31.991Z"^^xsd:dateTime;
  dct:modified "2018-07-20T22:12:17.282Z"^^xsd:dateTime;
  skos:broader :c_f6f95a83;
  skos:definition "A digital representation of physical and functional characteristics of a facility. As such it serves as a shared knowledge resource for information about a facility forming a reliable basis for decisions during its life cycle from inception onward.";
  skos:exactMatch <http://bsdd.buildingsmart.org/#concept/details/02GOHsd5P8QuCLyrqO__FT>;
  skos:inScheme :conceptScheme_751925ed;
  skos:narrower :c_08498a44, :c_09f6c52a, :c_0d6f0660, :c_19a61f73, :c_1efc9178, :c_28df75da,
    :c_2a55a494, :c_2a84910f, :c_2e6cd3a6, :c_31175b54, :c_3f128faf, :c_3fdd4da0, :c_5bc1704c,
    :c_7d508f5e, :c_800d8fbb, :c_818585d8, :c_8f194b82, :c_9f1a47e2, :c_b046bfd7, :c_c7b03ed3,
    :c_d0fec206, :c_ff860f3e;
  skos:prefLabel "building information modeling"@en;
  skosxl:altLabel :xl_en_d4ddf75e;
  skosxl:prefLabel :xl_en_eb6c78c3 .

:c_0d543967 a skos:Concept;
  dct:created "2018-05-12T20:37:43.793Z"^^xsd:dateTime;
  dct:modified "2018-05-12T20:41:22.761Z"^^xsd:dateTime;
  skos:broader :c_a314e31f;
  skos:exactMatch <http://skos.um.es/unescothes/C00797>;
  skos:inScheme :conceptScheme_751925ed;
  skos:prefLabel "contract law"@en;
  skosxl:prefLabel :xl_en_0788d2fb .

:xl_en_e9e3334d a skosxl:Label;
  dct:modified "2018-06-02T15:19:12.911Z"^^xsd:dateTime;
  skosxl:literalForm "bim protocol"@en .

:xl_en_0788d2fb a skosxl:Label;
  skosxl:literalForm "contract law"@en .

:c_0d6f0660 a skos:Concept;
  dct:created "2018-06-02T11:13:14.968Z"^^xsd:dateTime;
  skos:broader :c_fb07c266;
  skos:definition """Following on from the BASMP, the Built Asset Security Information Requirements shall be defined which identifies what specific information is needed to be produced and managed in order to meet the holistic approach defined within the BASMP. Details on the requirements on how information for a specific built asset should be generated, stored, disseminated and used should also be outlined. This should inform any
AIRs (PAS 1192-3) and/or EIRs (PAS 1192-2) developed.
"""@en;
  skos:inScheme :conceptScheme_751925ed;
  skos:notation "basir";
  skos:prefLabel "built asset security information requirements"@en;
  skos:related :c_2a84910f, :c_3f128faf, :c_8cff7d88, :c_9e9b604b;
  skosxl:prefLabel :xl_en_18bdd59e .

:c_2a84910f a skos:Concept;
  dct:created "2018-06-02T11:01:55.999Z"^^xsd:dateTime;
  dct:modified "2020-10-31T05:13:20.151Z"^^xsd:dateTime;
  skos:broader :c_fb07c266;
  skos:definition "This defines all of the data/information that is needed to manage the in-use phase of an asset’s lifecycle. It  is equivalent to the EIR which defines the information needed for the design and contraction phase of the lifecycle."@en;
  skos:inScheme :conceptScheme_751925ed;
  skosxl:altLabel :xl_en_42f4c7a1;
  skosxl:prefLabel :xl_en_cad85c74 .

:c_3f128faf a skos:Concept;
  dct:created "2018-05-12T17:07:10.299Z"^^xsd:dateTime;
  skos:broader :c_fb07c266;
  skos:definition """This is the document which determines what the client (the ‘Employer’) wants from the project, as delivered
by the project  team. It  identifies what the client would expect to be delivered during both the delivery and handover phases including responsibility, timescales, format and level of detail of the delivery of such information. It also includes any other project-specific requirements such procedures to be adopted, the plan of work to be used or any format restrictions.
"""@en;
  skos:inScheme :conceptScheme_751925ed;
  skos:prefLabel "employers information requirements"@en;
  skosxl:altLabel :xl_en_32357ece;
  skosxl:prefLabel :xl_en_98ded33c .

:c_8cff7d88 a skos:Concept;
  dct:created "2018-05-12T22:10:07.615Z"^^xsd:dateTime;
  dct:modified "2018-05-26T11:00:36.320Z"^^xsd:dateTime;
  skos:broader :c_aca16e26;
  skos:definition "pas 1192-2:2013 specification for information management for the capital/delivery phase of construction projects using building information modelling"@en;
  skos:inScheme :conceptScheme_751925ed;
  skos:note "Due to be replaced by ISO 19650 in late 2018"@en;
  skos:prefLabel "pas 1192-2:2013 capital/delivery"@en;
  skos:related :c_a2512527;
  skosxl:prefLabel :xl_en_aaba830f .

:c_9e9b604b a skos:Concept;
  dct:created "2018-05-26T10:56:53.876Z"^^xsd:dateTime;
  dct:modified "2018-05-26T11:12:02.704Z"^^xsd:dateTime;
  skos:broader :c_aca16e26;
  skos:definition "specification for information management for the operational phase of assets using building information modelling"@en;
  skos:inScheme :conceptScheme_751925ed;
  skos:prefLabel "pas 1192-3:2014"@en;
  skosxl:prefLabel :xl_en_ca45a339 .

:xl_en_18bdd59e a skosxl:Label;
  dct:modified "2018-07-20T21:59:35.828Z"^^xsd:dateTime;
  skosxl:literalForm "built asset security information requirements"@en .

:c_0ff3aa9f a skos:Concept;
  dct:created "2018-04-21T14:49:47.403Z"^^xsd:dateTime;
  skos:broader :c_2fb1c062;
  skos:inScheme :conceptScheme_751925ed;
  skos:prefLabel "project lead"@en;
  skosxl:prefLabel :xl_en_911d4809 .

:c_2fb1c062 a skos:Concept;
  dct:created "2018-04-21T07:04:11.037Z"^^xsd:dateTime;
  dct:modified "2018-04-21T14:51:35.768Z"^^xsd:dateTime;
  skos:broader :c_ca2b1c80;
  skos:inScheme :conceptScheme_751925ed;
  skos:narrower :c_0ff3aa9f, :c_2f23ff83, :c_4015bbab, :c_55cb6f4a, :c_974b12d0, :c_978f163b,
    :c_a4f58741;
  skos:prefLabel "team lead roles"@en;
  skosxl:prefLabel :xl_en_e476bd2c .

:xl_en_911d4809 a skosxl:Label;
  skosxl:literalForm "project lead"@en .

:c_105811e3 a skos:Concept;
  dct:created "2018-04-21T07:40:31.658Z"^^xsd:dateTime;
  dct:modified "2018-07-22T07:48:22.785Z"^^xsd:dateTime;
  skos:broader :c_b67efcfb;
  skos:inScheme :conceptScheme_751925ed;
  skos:notation "SU"@en;
  skos:prefLabel "supplier"@en;
  skosxl:prefLabel :xl_en_13907a93 .

:c_b67efcfb a skos:Concept;
  dc:source "BS ISO 6707-2-2017-Buildings and civil engineering works. Vocabulary. Contract and communication terms"@en;
  dct:created "2018-04-21T07:02:43.335Z"^^xsd:dateTime;
  dct:modified "2018-07-24T17:22:17.876Z"^^xsd:dateTime;
  skos:broader :c_ca2b1c80;
  skos:inScheme :conceptScheme_751925ed;
  skos:narrower :c_105811e3, :c_3073e948, :c_69e09153, :c_7b22749d, :c_803a74ef, :c_901951db,
    :c_b0503f89, :c_b06dcd33, :c_b50dc769, :c_be22475b, :c_cbae9e17, :c_e94e8717;
  skos:prefLabel "contractor and supplier roles"@en;
  skosxl:prefLabel :xl_en_5d8c071f .

:xl_en_13907a93 a skosxl:Label;
  skosxl:literalForm "supplier"@en .

:c_10e7ff42 a skos:Concept;
  dct:created "2018-04-21T14:35:20.939Z"^^xsd:dateTime;
  dct:modified "2018-07-22T07:50:08.902Z"^^xsd:dateTime;
  skos:broader :c_ba4a8cbb;
  skos:inScheme :conceptScheme_751925ed;
  skos:prefLabel "energy consultant"@en;
  skosxl:prefLabel :xl_en_e6a1b13e .

:c_ba4a8cbb a skos:Concept;
  dct:created "2018-04-21T07:03:39.272Z"^^xsd:dateTime;
  dct:modified "2018-07-22T07:26:11.288Z"^^xsd:dateTime;
  skos:broader :c_ca2b1c80;
  skos:inScheme :conceptScheme_751925ed;
  skos:narrower :c_10e7ff42, :c_54c8ace8, :c_bcd787cb, :c_db8a3f56, :c_fcba3610;
  skos:prefLabel "specialist roles"@en;
  skosxl:prefLabel :xl_en_7ac09f7e .

:xl_en_e6a1b13e a skosxl:Label;
  skosxl:literalForm "energy consultant"@en .

:c_13f7c864 a skos:Concept;
  dct:created "2018-04-21T14:28:39.078Z"^^xsd:dateTime;
  skos:broader :c_fbcae061;
  skos:inScheme :conceptScheme_751925ed;
  skos:prefLabel "non-executive director"@en;
  skosxl:prefLabel :xl_en_86a7e9ad .

:c_fbcae061 a skos:Concept;
  dct:created "2018-04-21T07:03:25.214Z"^^xsd:dateTime;
  dct:modified "2018-04-21T14:34:12.520Z"^^xsd:dateTime;
  skos:broader :c_ca2b1c80;
  skos:inScheme :conceptScheme_751925ed;
  skos:narrower :c_13f7c864, :c_2d052cdb, :c_51080e49, :c_6843a9be, :c_91cd7cb5, :c_9f86fc42,
    :c_a1903547, :c_c03abf22, :c_c6f08cf1, :c_e8b12fa7, :c_e9100418, :c_e9b3a976, :c_fa6f2225,
    :c_fc8d6da5;
  skos:prefLabel "organization roles"@en;
  skosxl:prefLabel :xl_en_610d53f7 .

:xl_en_86a7e9ad a skosxl:Label;
  skosxl:literalForm "non-executive director"@en .

:c_15a4664d a skos:Concept;
  dct:created "2018-04-21T15:10:57.603Z"^^xsd:dateTime;
  dct:modified "2018-07-20T19:48:44.833Z"^^xsd:dateTime;
  skos:broader :c_a314e31f;
  skos:inScheme :conceptScheme_751925ed;
  skos:narrower :c_03d0de39, :c_81a0559f, :c_c26a3327;
  skos:prefLabel "definition"@en;
  skosxl:prefLabel :xl_en_30a0e258 .

:c_43a1e1f6 a skos:Concept;
  dct:created "2018-04-21T15:07:38.605Z"^^xsd:dateTime;
  dct:modified "2018-10-25T13:30:03.748Z"^^xsd:dateTime;
  skos:inScheme :conceptScheme_751925ed;
  skos:narrower :c_10975b72, :c_1fbd8b11, :c_72030014, :c_85a522a2, :c_8d825e3a, :c_91ece774,
    :c_c02e3a4e, :c_c7d2ad4d, :c_e85c9613;
  skos:prefLabel "development stages"@en;
  skos:topConceptOf :conceptScheme_751925ed;
  skosxl:prefLabel :xl_en_8ff272ff .

:xl_en_30a0e258 a skosxl:Label;
  skosxl:literalForm "definition"@en .

:c_162b9e61 a skos:Concept;
  dct:created "2018-04-21T07:46:24.432Z"^^xsd:dateTime;
  dct:modified "2018-07-22T07:04:31.583Z"^^xsd:dateTime;
  skos:broader :c_2425ea08;
  skos:inScheme :conceptScheme_751925ed;
  skos:notation "D"@en;
  skos:prefLabel "drainage highways engineer"@en;
  skosxl:prefLabel :xl_en_2a510ed4 .

:xl_en_2a510ed4 a skosxl:Label;
  dct:modified "2018-07-22T07:04:03.501Z"^^xsd:dateTime;
  skosxl:literalForm "drainage highways engineer"@en .

:c_17a6c3cc a skos:Concept;
  dct:created "2018-04-21T15:46:17.412Z"^^xsd:dateTime;
  dct:modified "2018-07-20T18:15:11.201Z"^^xsd:dateTime;
  skos:broader :c_a314e31f;
  skos:inScheme :conceptScheme_751925ed;
  skos:prefLabel "fire protection"@en;
  skosxl:prefLabel :xl_en_07911b6c .

:xl_en_07911b6c a skosxl:Label;
  skosxl:literalForm "fire protection"@en .

:c_1808813e a skos:Concept;
  dct:created "2018-04-21T07:30:37.039Z"^^xsd:dateTime;
  skos:broader :c_54bbebe2;
  skos:inScheme :conceptScheme_751925ed;
  skos:prefLabel "client representative"@en;
  skosxl:prefLabel :xl_en_83f05d4c .

:c_54bbebe2 a skos:Concept;
  dct:created "2018-04-21T07:02:26.965Z"^^xsd:dateTime;
  dct:modified "2018-08-22T16:03:54.046Z"^^xsd:dateTime;
  skos:broader :c_ca2b1c80;
  skos:inScheme :conceptScheme_751925ed;
  skos:narrower :c_1808813e, :c_3c62e145, :c_3e1a5fff, :c_5b6f2370, :c_6be94e63, :c_86ba3858,
    :c_934dba80, :c_b0c264b4, :c_d0f52b80, :c_e92dd4bd, :c_f479b450, :c_f569343b;
  skos:prefLabel "client roles"@en;
  skosxl:prefLabel :xl_en_61a52c37 .

:xl_en_83f05d4c a skosxl:Label;
  skosxl:literalForm "client representative"@en .

:c_19203ba1 a skos:Concept;
  dct:created "2018-04-07T19:41:29.658Z"^^xsd:dateTime;
  dct:modified "2018-08-19T09:09:58.347Z"^^xsd:dateTime;
  skos:exactMatch <http://www.yso.fi/onto/yso/p689>;
  skos:inScheme :conceptScheme_751925ed;
  skos:narrower :c_281f6d96, :c_3f7d46c0, :c_618864b7, :c_73619d2a, :c_b7ef2137, :c_c76077ab,
    :c_e5b1b611, :c_f29587ff;
  skos:prefLabel "naming convention"@en;
  skos:topConceptOf :conceptScheme_751925ed;
  skosxl:prefLabel :xl_en_638c20a3 .

:c_c76077ab a skos:Concept;
  dct:created "2018-04-21T15:31:51.728Z"^^xsd:dateTime;
  dct:modified "2018-08-11T12:22:50.367Z"^^xsd:dateTime;
  skos:broader :c_19203ba1;
  skos:inScheme :conceptScheme_751925ed;
  skos:narrower :c_24506d00, :c_32da9577, :c_3c4ef6f5, :c_5ae807c5, :c_6c460406, :c_9c1d7995,
    :c_9d3f953f, :c_af7e5693, :c_b470c6f5, :c_b4f95391, :c_c4204198, :c_d837a7ac, :c_da9ab00d;
  skos:prefLabel "drawing building"@en;
  skosxl:prefLabel :xl_en_4a44a158 .

:xl_en_638c20a3 a skosxl:Label;
  dct:modified "2018-08-11T11:49:09.823Z"^^xsd:dateTime;
  skosxl:literalForm "naming convention"@en .

:c_19a61f73 a skos:Concept;
  dct:created "2018-06-02T10:10:34.225Z"^^xsd:dateTime;
  dct:modified "2020-10-31T05:15:39.224Z"^^xsd:dateTime;
  skos:broader :c_fb07c266;
  skos:definition "This describes the amount of non-graphical information a model contains."@en;
  skos:inScheme :conceptScheme_751925ed;
  skosxl:altLabel :xl_en_96c8608e;
  skosxl:prefLabel :xl_en_371750e7 .

:xl_en_371750e7 a skosxl:Label;
  dct:modified "2018-07-20T22:22:33.610Z"^^xsd:dateTime;
  skosxl:literalForm "level of information"@en .

:c_1a6a26ea a skos:Concept;
  dct:created "2018-04-21T14:44:11.714Z"^^xsd:dateTime;
  skos:broader :c_d7f03766;
  skos:inScheme :conceptScheme_751925ed;
  skos:prefLabel "planning consultant"@en;
  skosxl:prefLabel :xl_en_f17d80f7 .

:c_d7f03766 a skos:Concept;
  dct:created "2018-04-21T07:04:00.622Z"^^xsd:dateTime;
  dct:modified "2018-08-22T16:01:27.524Z"^^xsd:dateTime;
  skos:broader :c_ca2b1c80;
  skos:inScheme :conceptScheme_751925ed;
  skos:narrower :c_1a6a26ea, :c_1ae27dc8, :c_2363e9c3, :c_517519ce, :c_5dc9194d, :c_87ff7e6c,
    :c_96391878, :c_9ce01e2d, :c_ab14190c, :c_b7c13cf0, :c_be027528, :c_f74d9794;
  skos:prefLabel "surveyor and planner roles"@en;
  skosxl:prefLabel :xl_en_7d7cec2b .

:xl_en_f17d80f7 a skosxl:Label;
  skosxl:literalForm "planning consultant"@en .

:c_1ae27dc8 a skos:Concept;
  dct:created "2018-04-21T14:44:49.977Z"^^xsd:dateTime;
  skos:broader :c_d7f03766;
  skos:inScheme :conceptScheme_751925ed;
  skos:prefLabel "survey specialist"@en;
  skosxl:prefLabel :xl_en_d75fa915 .

:xl_en_d75fa915 a skosxl:Label;
  skosxl:literalForm "survey specialist"@en .

:c_1e174ca8 a skos:Concept;
  dct:created "2018-04-21T07:46:55.943Z"^^xsd:dateTime;
  skos:broader :c_2425ea08;
  skos:inScheme :conceptScheme_751925ed;
  skos:prefLabel "marine engineer"@en;
  skosxl:prefLabel :xl_en_22117e20 .

:xl_en_22117e20 a skosxl:Label;
  skosxl:literalForm "marine engineer"@en .

:c_1efc9178 a skos:Concept;
  dct:created "2018-06-02T11:11:23.104Z"^^xsd:dateTime;
  dct:modified "2020-10-31T05:41:50.138Z"^^xsd:dateTime;
  skos:broader :c_fb07c266;
  skos:definition """The Security Breach / Incident Management Plan forms part of the BASMP and should provide detail on
 
how and the impact of failure and / or disruption is minimised ensuring business continuity is maintained and the security is upheld.
"""@en;
  skos:inScheme :conceptScheme_751925ed;
  skosxl:altLabel :xl_en_2de5ebbe;
  skosxl:prefLabel :xl_en_a36af88a .

:xl_en_a36af88a a skosxl:Label;
  dct:modified "2018-07-20T22:07:44.817Z"^^xsd:dateTime;
  skosxl:literalForm "security breach / incident management plan"@en .

:c_1f36603b a skos:Concept;
  dct:created "2018-04-21T14:36:02.694Z"^^xsd:dateTime;
  dct:modified "2018-04-21T14:38:01.686Z"^^xsd:dateTime;
  skos:broader :c_2664d806;
  skos:inScheme :conceptScheme_751925ed;
  skos:prefLabel "insurance consultant"@en;
  skosxl:prefLabel :xl_en_d5033a46 .

:c_2664d806 a skos:Concept;
  dct:created "2018-04-21T07:03:50.421Z"^^xsd:dateTime;
  dct:modified "2018-08-22T16:08:44.080Z"^^xsd:dateTime;
  skos:broader :c_ca2b1c80;
  skos:inScheme :conceptScheme_751925ed;
  skos:narrower :c_01bda236, :c_11f27c78, :c_1f36603b, :c_359e3f51, :c_46f20ab0, :c_717bb7fd,
    :c_77a0c277, :c_77ee92ee, :c_9509873f, :c_9a568eaa, :c_b781cfae, :c_dcdc5d7e;
  skos:prefLabel "support roles"@en;
  skosxl:prefLabel :xl_en_7322e074 .

:xl_en_d5033a46 a skosxl:Label;
  skosxl:literalForm "insurance consultant"@en .

:c_1fbd8b11 a skos:Concept;
  dct:created "2018-04-21T15:11:22.473Z"^^xsd:dateTime;
  dct:modified "2018-10-25T12:27:13.484Z"^^xsd:dateTime;
  olo:index "4"^^xsd:positiveInteger;
  skos:broader :c_43a1e1f6;
  skos:inScheme :conceptScheme_751925ed;
  skos:notation "4"@en;
  skos:prefLabel "technical design"@en;
  skosxl:prefLabel :xl_en_a2b1c3d9 .

:xl_en_a2b1c3d9 a skosxl:Label;
  dct:modified "2018-05-12T21:36:30.008Z"^^xsd:dateTime;
  skosxl:literalForm "technical design"@en .

:c_20cde89c a skos:Concept;
  dc:source "Building a Safer Future – Independent Review of Building Regulations and Fire Safety: Final Report"@en;
  dct:created "2018-04-21T07:46:46.388Z"^^xsd:dateTime;
  dct:modified "2018-07-28T16:38:30.267Z"^^xsd:dateTime;
  skos:broader :c_2425ea08;
  skos:definition "A person with the ability to apply scientific and engineering principles, rules and expert judgement, based on an understanding of the phenomena and effects of fire and of the reaction and behaviour of people to fire, to protect people, property and the environment from the destructive effects of fire"@en;
  skos:inScheme :conceptScheme_751925ed;
  skos:notation "FEng"@en;
  skos:prefLabel "fire engineering consultant"@en;
  skosxl:prefLabel :xl_en_baef5ad9 .

:xl_en_baef5ad9 a skosxl:Label;
  skosxl:literalForm "fire engineering consultant"@en .

:c_22fa7b92 a skos:Concept;
  dct:created "2018-03-28T18:08:31.327Z"^^xsd:dateTime;
  dct:modified "2018-04-21T16:13:10.746Z"^^xsd:dateTime;
  skos:broader :c_8d825e3a;
  skos:inScheme :conceptScheme_751925ed;
  skos:prefLabel "agree sales mix"@en;
  skosxl:prefLabel :xl_en_717c6377 .

:c_8d825e3a a skos:Concept;
  dct:created "2018-04-21T15:08:46.281Z"^^xsd:dateTime;
  dct:modified "2018-10-25T12:26:04.386Z"^^xsd:dateTime;
  olo:index "2"^^xsd:positiveInteger;
  skos:broader :c_43a1e1f6;
  skos:inScheme :conceptScheme_751925ed;
  skos:narrower :c_22fa7b92, :c_499e656c, :c_4bbe2792, :c_4d537a54, :c_581128f4, :c_583a056d,
    :c_86013584, :c_96da4523, :c_b9523fc1, :c_cdf35a77, :c_d9801b1d;
  skos:notation "2"@en;
  skos:prefLabel "concept design"@en;
  skosxl:prefLabel :xl_en_47240b6a .

:xl_en_717c6377 a skosxl:Label;
  dct:modified "2018-04-07T19:31:22.595Z"^^xsd:dateTime;
  skosxl:literalForm "agree sales mix"@en .

:c_2361a039 a skos:Concept;
  dct:created "2018-04-21T14:23:48.547Z"^^xsd:dateTime;
  skos:broader :c_b8f9acb4;
  skos:inScheme :conceptScheme_751925ed;
  skos:prefLabel "sustainability consultant"@en;
  skosxl:prefLabel :xl_en_e6554c56 .

:c_b8f9acb4 a skos:Concept;
  dct:created "2018-04-21T07:03:07.899Z"^^xsd:dateTime;
  dct:modified "2018-08-22T15:52:27.403Z"^^xsd:dateTime;
  skos:broader :c_ca2b1c80;
  skos:inScheme :conceptScheme_751925ed;
  skos:narrower :c_1e86ab1c, :c_2361a039, :c_369e4bb6, :c_4a5391b1, :c_70159d2c, :c_d9ac339e,
    :c_dca128d9, :c_de6816aa, :c_ed68836f, :c_fb85aed5;
  skos:prefLabel "environmental and geological roles"@en;
  skosxl:prefLabel :xl_en_c531fffd .

:xl_en_e6554c56 a skosxl:Label;
  skosxl:literalForm "sustainability consultant"@en .

:c_2363e9c3 a skos:Concept;
  dct:created "2018-04-21T14:43:26.202Z"^^xsd:dateTime;
  skos:broader :c_d7f03766;
  skos:inScheme :conceptScheme_751925ed;
  skos:prefLabel "building inspector"@en;
  skosxl:prefLabel :xl_en_e3093885 .

:xl_en_e3093885 a skosxl:Label;
  skosxl:literalForm "building inspector"@en .

:c_ca2b1c80 a skos:Concept;
  dct:created "2018-04-07T19:38:06.796Z"^^xsd:dateTime;
  dct:modified "2018-04-21T07:24:04.613Z"^^xsd:dateTime;
  skos:inScheme :conceptScheme_751925ed;
  skos:narrower :c_2425ea08, :c_2664d806, :c_2fb1c062, :c_54bbebe2, :c_b67efcfb, :c_b8f9acb4,
    :c_ba4a8cbb, :c_d63bf876, :c_d7f03766, :c_da75b83b, :c_fbcae061;
  skos:prefLabel "occupational groups"@en;
  skos:topConceptOf :conceptScheme_751925ed;
  skosxl:prefLabel :xl_en_f97f9a08 .

:c_324b2ef1 a skos:Concept;
  dct:created "2018-04-21T07:46:13.541Z"^^xsd:dateTime;
  dct:modified "2018-07-22T07:52:07.347Z"^^xsd:dateTime;
  skos:broader :c_2425ea08;
  skos:inScheme :conceptScheme_751925ed;
  skos:notation "DEM"@en;
  skos:prefLabel "demolition engineer"@en;
  skosxl:prefLabel :xl_en_4092cafc .

:c_32b1f026 a skos:Concept;
  dct:created "2018-04-21T07:46:03.326Z"^^xsd:dateTime;
  skos:broader :c_2425ea08;
  skos:inScheme :conceptScheme_751925ed;
  skos:prefLabel "commissioning specialist"@en;
  skosxl:prefLabel :xl_en_9783936d .

:c_4a31c73a a skos:Concept;
  dct:created "2018-04-21T07:45:35.041Z"^^xsd:dateTime;
  dct:modified "2018-07-22T07:02:58.787Z"^^xsd:dateTime;
  skos:broader :c_2425ea08;
  skos:inScheme :conceptScheme_751925ed;
  skos:notation "C"@en;
  skos:prefLabel "civil engineer"@en;
  skosxl:prefLabel :xl_en_5b75f095 .

:c_4de09d2e a skos:Concept;
  dct:created "2018-04-21T07:45:44.421Z"^^xsd:dateTime;
  skos:broader :c_2425ea08;
  skos:inScheme :conceptScheme_751925ed;
  skos:prefLabel "civil engineering designer"@en;
  skosxl:prefLabel :xl_en_551b4be5 .

:c_4e68f3f9 a skos:Concept;
  dct:created "2018-04-21T07:47:35.010Z"^^xsd:dateTime;
  skos:broader :c_2425ea08;
  skos:inScheme :conceptScheme_751925ed;
  skos:prefLabel "network modeller"@en;
  skosxl:prefLabel :xl_en_6938f5ab .

:c_500dee4e a skos:Concept;
  dct:created "2018-04-21T07:48:33.877Z"^^xsd:dateTime;
  skos:broader :c_2425ea08;
  skos:inScheme :conceptScheme_751925ed;
  skos:prefLabel "telecommunication engineer"@en;
  skosxl:prefLabel :xl_en_98f6ec45 .

:c_55d219f9 a skos:Concept;
  dct:created "2018-04-21T07:47:58.356Z"^^xsd:dateTime;
  dct:modified "2018-07-22T07:18:19.781Z"^^xsd:dateTime;
  skos:broader :c_2425ea08;
  skos:inScheme :conceptScheme_751925ed;
  skos:notation "P"@en;
  skos:prefLabel "public health engineer"@en;
  skosxl:prefLabel :xl_en_c059ec62 .

:c_92b99561 a skos:Concept;
  dct:created "2018-04-21T07:48:17.862Z"^^xsd:dateTime;
  skos:broader :c_2425ea08;
  skos:inScheme :conceptScheme_751925ed;
  skos:prefLabel "structural engineering designer"@en;
  skosxl:prefLabel :xl_en_0024b5e7 .

:c_97ba48a0 a skos:Concept;
  dct:created "2018-04-21T07:48:08.016Z"^^xsd:dateTime;
  dct:modified "2018-07-22T07:20:32.028Z"^^xsd:dateTime;
  skos:broader :c_2425ea08;
  skos:inScheme :conceptScheme_751925ed;
  skos:notation "S"@en;
  skos:prefLabel "structural engineer"@en;
  skosxl:prefLabel :xl_en_afa6b17f .

:c_ad02e5d9 a skos:Concept;
  dct:created "2018-04-21T07:47:46.031Z"^^xsd:dateTime;
  skos:broader :c_2425ea08;
  skos:inScheme :conceptScheme_751925ed;
  skos:prefLabel "process engineer"@en;
  skosxl:prefLabel :xl_en_1f8ea7d8 .

:c_b03db527 a skos:Concept;
  dct:created "2018-04-21T07:45:24.669Z"^^xsd:dateTime;
  skos:broader :c_2425ea08;
  skos:inScheme :conceptScheme_751925ed;
  skos:prefLabel "building services engineer"@en;
  skosxl:prefLabel :xl_en_73e4d0b6 .

:c_b3c41b17 a skos:Concept;
  dct:created "2018-04-21T07:47:22.895Z"^^xsd:dateTime;
  skos:broader :c_2425ea08;
  skos:inScheme :conceptScheme_751925ed;
  skos:prefLabel "mechanical, electrical, instrumentation, control and automation (MEICA) consultant"@en;
  skosxl:prefLabel :xl_en_68c040b3 .

:c_bbc32497 a skos:Concept;
  dct:created "2018-04-21T07:48:44.576Z"^^xsd:dateTime;
  dct:modified "2018-07-21T16:08:43.887Z"^^xsd:dateTime;
  skos:broader :c_2425ea08;
  skos:inScheme :conceptScheme_751925ed;
  skos:notation "water"@en;
  skos:prefLabel "water engineer"@en;
  skosxl:prefLabel :xl_en_8640cb95 .

:c_c048d0a8 a skos:Concept;
  dct:created "2018-04-21T07:46:36.811Z"^^xsd:dateTime;
  dct:modified "2018-07-22T07:05:40.707Z"^^xsd:dateTime;
  skos:broader :c_2425ea08;
  skos:inScheme :conceptScheme_751925ed;
  skos:notation "E"@en;
  skos:prefLabel "electrical engineer"@en;
  skosxl:prefLabel :xl_en_de124a5c .

:c_c58c00ba a skos:Concept;
  dct:created "2018-04-21T07:45:04.609Z"^^xsd:dateTime;
  skos:broader :c_2425ea08;
  skos:inScheme :conceptScheme_751925ed;
  skos:prefLabel "acoustic engineers"@en;
  skosxl:prefLabel :xl_en_865b7696 .

:c_d1fb700d a skos:Concept;
  dct:created "2018-04-21T07:45:53.739Z"^^xsd:dateTime;
  skos:broader :c_2425ea08;
  skos:inScheme :conceptScheme_751925ed;
  skos:prefLabel "commissioning engineer"@en;
  skosxl:prefLabel :xl_en_d1442c80 .

:c_e7195c13 a skos:Concept;
  dct:created "2018-04-21T07:47:06.758Z"^^xsd:dateTime;
  dct:modified "2018-07-22T07:17:43.942Z"^^xsd:dateTime;
  skos:broader :c_2425ea08;
  skos:inScheme :conceptScheme_751925ed;
  skos:notation "M"@en;
  skos:prefLabel "mechanical engineer"@en;
  skosxl:prefLabel :xl_en_ac6bbf19 .

:xl_en_1a7bc156 a skosxl:Label;
  skosxl:literalForm "engineering roles"@en .

:c_359e3f51 a skos:Concept;
  dct:created "2018-04-21T14:37:06.947Z"^^xsd:dateTime;
  dct:modified "2018-04-21T14:39:04.282Z"^^xsd:dateTime;
  skos:broader :c_2664d806;
  skos:inScheme :conceptScheme_751925ed;
  skos:prefLabel "procurement consultant"@en;
  skosxl:prefLabel :xl_en_e618ab4f .

:c_717bb7fd a skos:Concept;
  dct:created "2018-04-21T14:35:40.172Z"^^xsd:dateTime;
  dct:modified "2020-10-31T05:32:16.482Z"^^xsd:dateTime;
  skos:broader :c_2664d806;
  skos:inScheme :conceptScheme_751925ed;
  skos:notation "HS"@en;
  skosxl:prefLabel :xl_en_59685d3e .

:c_77a0c277 a skos:Concept;
  dct:created "2018-04-21T14:36:31.268Z"^^xsd:dateTime;
  dct:modified "2018-04-21T14:38:37.201Z"^^xsd:dateTime;
  skos:broader :c_2664d806;
  skos:inScheme :conceptScheme_751925ed;
  skos:prefLabel "management consultant"@en;
  skosxl:prefLabel :xl_en_62778564 .

:c_77ee92ee a skos:Concept;
  dct:created "2018-04-21T14:36:21.148Z"^^xsd:dateTime;
  dct:modified "2018-04-21T14:38:19.809Z"^^xsd:dateTime;
  skos:broader :c_2664d806;
  skos:inScheme :conceptScheme_751925ed;
  skos:prefLabel "maintenance provider"@en;
  skosxl:prefLabel :xl_en_5d78835d .

:c_9a568eaa a skos:Concept;
  dc:source "Interim Advice Note 184/16 Highways England CAD and Data Standard"@en;
  dct:created "2018-04-21T14:36:12.121Z"^^xsd:dateTime;
  dct:modified "2018-08-22T16:06:39.068Z"^^xsd:dateTime;
  skos:broader :c_2664d806;
  skos:inScheme :conceptScheme_751925ed;
  skos:notation "ZL"@en;
  skos:prefLabel "lawyer"@en;
  skosxl:altLabel :xl_en_1b847882;
  skosxl:prefLabel :xl_en_66ebdf30 .

:c_dcdc5d7e a skos:Concept;
  dct:created "2018-04-21T14:35:49.549Z"^^xsd:dateTime;
  dct:modified "2018-07-21T13:16:11.354Z"^^xsd:dateTime;
  skos:broader :c_2664d806;
  skos:inScheme :conceptScheme_751925ed;
  skos:prefLabel "health and safety consultant"@en;
  skosxl:altLabel :xl_en_ecb8813d;
  skosxl:prefLabel :xl_en_f6592c32 .

:xl_en_7322e074 a skosxl:Label;
  skosxl:literalForm "support roles"@en .

:c_28df75da a skos:Concept;
  dct:created "2018-06-02T11:03:32.959Z"^^xsd:dateTime;
  dct:modified "2020-10-31T05:33:27.422Z"^^xsd:dateTime;
  skos:broader :c_fb07c266;
  skos:definition "The Built Asset Security Strategy should be developed for the lifecycle of a given built asset and should determine the relevant security requirements and associated risks as well as the strategy to mitigate these risks through a Built Asset Risk Management Plan.    This should inform any OIRs (PAS 1192-3) and/or PLQs (PAS 1192-2) developed."@en;
  skos:inScheme :conceptScheme_751925ed;
  skos:related :c_8cff7d88, :c_8f194b82, :c_9e9b604b, :c_d0fec206;
  skosxl:altLabel :xl_en_0049082b;
  skosxl:prefLabel :xl_en_83d0a7a6 .

:c_8f194b82 a skos:Concept;
  dct:created "2018-06-02T10:20:45.003Z"^^xsd:dateTime;
  dct:modified "2020-10-30T20:31:02.280Z"^^xsd:dateTime;
  skos:broader :c_fb07c266;
  skos:definition "Questions asked of the supply chain by the employer to inform decision-making at key stages of an asset lifecycle or project."@en;
  skos:inScheme :conceptScheme_751925ed;
  skosxl:altLabel :xl_en_913b3693;
  skosxl:prefLabel :xl_en_33c481b3 .

:c_d0fec206 a skos:Concept;
  dct:created "2018-06-02T11:00:04.465Z"^^xsd:dateTime;
  skos:broader :c_fb07c266;
  skos:definition """This defines what data/information is required to achieve an organization’s strategic objectives. The
OIR may be developed from an ISO 55001, Asset
management system.
"""@en;
  skos:inScheme :conceptScheme_751925ed;
  skos:prefLabel "organization information requirements"@en;
  skosxl:altLabel :xl_en_1ec12f25;
  skosxl:prefLabel :xl_en_3f00a2dd .

:xl_en_83d0a7a6 a skosxl:Label;
  dct:modified "2018-07-20T22:00:48.659Z"^^xsd:dateTime;
  skosxl:literalForm "built asset security strategy"@en .

:c_295c3f50 a skos:Concept;
  dct:created "2018-05-12T17:15:08.235Z"^^xsd:dateTime;
  skos:broader :c_f6f95a83;
  skos:inScheme :conceptScheme_751925ed;
  skos:prefLabel "information model"@en;
  skosxl:prefLabel :xl_en_c85a3575 .

:c_084a4f3a dct:created "2020-10-31T08:33:53.497Z"^^xsd:dateTime;
  skos:inScheme :conceptScheme_751925ed;
  skos:prefLabel "information management"@en .

:c_f6f95a83 a skos:Concept;
  dct:created "2018-04-20T19:10:01.144Z"^^xsd:dateTime;
  dct:modified "2018-06-02T00:29:32.610Z"^^xsd:dateTime;
  skos:exactMatch <http://urn.fi/URN:NBN:fi:au:tt:t117>;
  skos:inScheme :conceptScheme_751925ed;
  skos:narrower :c_295c3f50, :c_fb07c266;
  skos:prefLabel "knowledge, information and data"@en;
  skos:topConceptOf :conceptScheme_751925ed;
  skosxl:prefLabel :xl_en_5728ead4 .

:c_4dd7fd6a a skos:Concept;
  dct:created "2018-05-12T17:09:36.685Z"^^xsd:dateTime;
  dct:modified "2020-10-31T08:46:02.052Z"^^xsd:dateTime;
  skos:broader :c_084a4f3a;
  skos:definition "All the information that is needed to support the management and operation of the built asset (infrastructure or building). This can be formed partly from the PIM at the handover stage of a project. It differs from the PIM in that it consists only of the information that is needed to support the management   and operation of the asset. The AIM will continually be updated and developed throughout the life of the asset as information is fed into the model during the asset’s management."@en;
  skos:inScheme :conceptScheme_751925ed;
  skos:prefLabel "asset information model"@en;
  skosxl:altLabel :xl_en_44ca1675;
  skosxl:prefLabel :xl_en_8f8bcdd8 .

:c_bd21cb81 a skos:Concept;
  dct:created "2018-05-12T17:15:46.670Z"^^xsd:dateTime;
  dct:modified "2020-10-31T08:47:43.988Z"^^xsd:dateTime;
  skos:broader :c_084a4f3a;
  skos:definition "The single source of information for any given project, used to collect, manage and disseminate all relevant approved project information. Stored digitally, this is where information is shared collaboratively in a logical, accessible way to help all key parties gain access to information."@en;
  skos:inScheme :conceptScheme_751925ed;
  skos:prefLabel "common data environment"@en;
  skosxl:altLabel :xl_en_f2eee9b5;
  skosxl:prefLabel :xl_en_68bbe786 .

:xl_en_c85a3575 a skosxl:Label;
  skosxl:literalForm "information model"@en .

:c_2a55a494 a skos:Concept;
  dct:created "2018-06-02T10:08:31.063Z"^^xsd:dateTime;
  dct:modified "2020-10-30T20:28:30.447Z"^^xsd:dateTime;
  skos:broader :c_fb07c266;
  skos:definition "The Level of Detail defines the amount of graphical information a model contains."@en;
  skos:inScheme :conceptScheme_751925ed;
  skosxl:altLabel :xl_en_3c41ea90;
  skosxl:prefLabel :xl_en_372c946e .

:xl_en_372c946e a skosxl:Label;
  dct:modified "2018-07-20T22:03:14.217Z"^^xsd:dateTime;
  skosxl:literalForm "level of detail"@en .

:xl_en_cad85c74 a skosxl:Label;
  dct:modified "2018-07-20T21:58:12.758Z"^^xsd:dateTime;
  skosxl:literalForm "asset information requirements"@en .

:c_2bffe0d4 a skos:Concept;
  dct:created "2018-03-28T14:42:58.118Z"^^xsd:dateTime;
  dct:modified "2020-10-31T05:47:25.223Z"^^xsd:dateTime;
  skos:broader :c_a314e31f;
  skos:definition "From Disposal Process See Figure A-9"@en;
  skos:inScheme :conceptScheme_751925ed;
  skos:notation "A";
  skos:prefLabel "Disposal Process See Figure A-9"@en;
  skosxl:hiddenLabel :xl_en_74ce780a;
  skosxl:prefLabel :xl_en_42a2e79e .

:xl_en_74ce780a a skosxl:Label;
  skosxl:literalForm """2
"""@en .

:xl_en_42a2e79e a skosxl:Label;
  dct:modified "2020-10-31T05:47:33.932Z"^^xsd:dateTime;
  skosxl:literalForm "Disposal Process See Figure A-9"@en .

:c_2d052cdb a skos:Concept;
  dct:created "2018-04-21T14:29:00.655Z"^^xsd:dateTime;
  skos:broader :c_fbcae061;
  skos:inScheme :conceptScheme_751925ed;
  skos:prefLabel "president"@en;
  skosxl:prefLabel :xl_en_ad75ab37 .

:xl_en_ad75ab37 a skosxl:Label;
  skosxl:literalForm "president"@en .

:c_2e6cd3a6 a skos:Concept;
  dct:created "2018-06-02T10:06:09.221Z"^^xsd:dateTime;
  dct:modified "2020-10-31T05:38:16.102Z"^^xsd:dateTime;
  skos:broader :c_fb07c266;
  skos:definition "This defines the rules of how the information within the CDE is managed, for example, naming conventions and status codes adopted in the project."@en;
  skos:inScheme :conceptScheme_751925ed;
  skosxl:altLabel :xl_en_f987d3fd;
  skosxl:prefLabel :xl_en_7ffdd613 .

:xl_en_7ffdd613 a skosxl:Label;
  dct:modified "2018-07-20T22:09:02.536Z"^^xsd:dateTime;
  skosxl:literalForm "standard methods and procedures"@en .

:c_2eb971b3 a skos:Concept;
  dct:created "2018-04-07T19:39:04.118Z"^^xsd:dateTime;
  dct:modified "2018-07-22T07:00:53.059Z"^^xsd:dateTime;
  skos:broader :c_d63bf876;
  skos:inScheme :conceptScheme_751925ed;
  skos:notation "A"@en;
  skos:prefLabel "architect"@en;
  skosxl:prefLabel :xl_en_36eecb52 .

:c_d63bf876 a skos:Concept;
  dct:created "2018-04-21T07:02:10.941Z"^^xsd:dateTime;
  dct:modified "2018-08-20T10:21:01.515Z"^^xsd:dateTime;
  skos:broader :c_ca2b1c80;
  skos:inScheme :conceptScheme_751925ed;
  skos:narrower :c_2eb971b3, :c_40fcae48, :c_503d9a20, :c_68a58f6d, :c_9e715393, :c_b1c5511d,
    :c_d19fc7a3, :c_e231ef90, :c_e8742734;
  skos:prefLabel "architectural roles"@en;
  skosxl:prefLabel :xl_en_aa53329a .

:xl_en_36eecb52 a skosxl:Label;
  skosxl:literalForm "architect"@en .

:c_2f23ff83 a skos:Concept;
  dct:created "2018-04-21T14:48:43.814Z"^^xsd:dateTime;
  skos:broader :c_2fb1c062;
  skos:inScheme :conceptScheme_751925ed;
  skos:prefLabel "asset management lead"@en;
  skosxl:prefLabel :xl_en_4a2241c9 .

:xl_en_4a2241c9 a skosxl:Label;
  skosxl:literalForm "asset management lead"@en .

:c_4015bbab a skos:Concept;
  dct:created "2018-04-21T14:49:14.447Z"^^xsd:dateTime;
  skos:broader :c_2fb1c062;
  skos:inScheme :conceptScheme_751925ed;
  skos:prefLabel "operation lead"@en;
  skosxl:prefLabel :xl_en_68051b88 .

:c_55cb6f4a a skos:Concept;
  dct:created "2018-04-21T14:49:02.862Z"^^xsd:dateTime;
  skos:broader :c_2fb1c062;
  skos:inScheme :conceptScheme_751925ed;
  skos:prefLabel "design lead"@en;
  skosxl:prefLabel :xl_en_1d3b7898 .

:c_974b12d0 a skos:Concept;
  dc:source "Building a Safer Future – Independent Review of Building Regulations and Fire Safety: Final Report"@en;
  dct:created "2018-04-21T14:49:24.409Z"^^xsd:dateTime;
  dct:modified "2018-07-28T16:43:03.595Z"^^xsd:dateTime;
  skos:broader :c_2fb1c062;
  skos:definition "Under the Construction (Design and Management) Regulations 2015 a principal designer is a designer who is an organisation (or, in some cases, an individual) appointed by the client to take lead control of the pre construction phase of any project where there is more than one designer involved"@en;
  skos:inScheme :conceptScheme_751925ed;
  skos:notation "PD"@en;
  skos:prefLabel "principal designer"@en;
  skosxl:prefLabel :xl_en_8ebaea43 .

:c_978f163b a skos:Concept;
  dct:created "2018-04-21T14:49:35.218Z"^^xsd:dateTime;
  skos:broader :c_2fb1c062;
  skos:inScheme :conceptScheme_751925ed;
  skos:prefLabel "programme lead"@en;
  skosxl:prefLabel :xl_en_fefa5cfb .

:c_a4f58741 a skos:Concept;
  dct:created "2018-04-21T14:48:53.663Z"^^xsd:dateTime;
  skos:broader :c_2fb1c062;
  skos:inScheme :conceptScheme_751925ed;
  skos:prefLabel "construction lead"@en;
  skosxl:prefLabel :xl_en_7071a06a .

:xl_en_e476bd2c a skosxl:Label;
  skosxl:literalForm "team lead roles"@en .

:c_3073e948 a skos:Concept;
  dct:created "2018-04-21T07:39:02.119Z"^^xsd:dateTime;
  skos:broader :c_b67efcfb;
  skos:inScheme :conceptScheme_751925ed;
  skos:prefLabel "importer"@en;
  skosxl:prefLabel :xl_en_82db6084 .

:xl_en_82db6084 a skosxl:Label;
  skosxl:literalForm "importer"@en .

:c_31175b54 a skos:Concept;
  dct:created "2018-06-02T11:09:39.039Z"^^xsd:dateTime;
  dct:modified "2020-10-31T05:37:42.191Z"^^xsd:dateTime;
  skos:broader :c_fb07c266;
  skos:definition """Following on from the BASS, the Built Asset Security Management Plan should be developed which
identifies how a holistic approach is to be implemented
in practice against the specific security risks, or combinations of risks, identified within the BASS.
"""@en;
  skos:inScheme :conceptScheme_751925ed;
  skosxl:altLabel :xl_en_511d9a71;
  skosxl:prefLabel :xl_en_a9364bf1 .

:xl_en_a9364bf1 a skosxl:Label;
  dct:modified "2018-07-20T22:00:11.379Z"^^xsd:dateTime;
  skosxl:literalForm "built asset security management plan"@en .

:xl_en_4092cafc a skosxl:Label;
  skosxl:literalForm "demolition engineer"@en .

:xl_en_9783936d a skosxl:Label;
  skosxl:literalForm "commissioning specialist"@en .

:xl_en_e618ab4f a skosxl:Label;
  skosxl:literalForm "procurement consultant"@en .

:c_3a3d92ab a skos:Concept;
  dct:created "2018-05-26T09:33:42.703Z"^^xsd:dateTime;
  dct:modified "2018-05-26T09:35:11.117Z"^^xsd:dateTime;
  skos:broader :c_aca16e26;
  skos:definition "Security techniques,Information Security Management system requirements"@en;
  skos:inScheme :conceptScheme_751925ed;
  skos:prefLabel "iso/iec/27001:2013 information technology"@en;
  skos:related :c_a2512527;
  skosxl:prefLabel :xl_en_4eeadaa5 .

:xl_en_4eeadaa5 a skosxl:Label;
  skosxl:literalForm "iso/iec/27001:2013 information technology"@en .

:c_3c62e145 a skos:Concept;
  dct:created "2018-04-21T07:31:10.106Z"^^xsd:dateTime;
  dct:modified "2018-07-22T07:39:12.255Z"^^xsd:dateTime;
  skos:broader :c_54bbebe2;
  skos:inScheme :conceptScheme_751925ed;
  skos:notation "EA"@en;
  skos:prefLabel "employers agent"@en;
  skosxl:prefLabel :xl_en_3ed7d3a2 .

:xl_en_3ed7d3a2 a skosxl:Label;
  skosxl:literalForm "employers agent"@en .

:c_3d3ab4cb a skos:Concept;
  dct:created "2018-03-28T15:54:02.561Z"^^xsd:dateTime;
  dct:modified "2018-07-20T19:47:27.751Z"^^xsd:dateTime;
  skos:broader :c_a314e31f;
  skos:hiddenLabel """2.1.7
"""@en;
  skos:inScheme :conceptScheme_751925ed;
  skos:prefLabel "Study Potential Alternatives; Develop Conceptual Plans and Costs"@en;
  skosxl:hiddenLabel :xl_en_f38b7b49;
  skosxl:prefLabel :xl_en_8ececd4f .

:xl_en_f38b7b49 a skosxl:Label;
  skosxl:literalForm """2.1.7
"""@en .

:xl_en_8ececd4f a skosxl:Label;
  skosxl:literalForm "Study Potential Alternatives; Develop Conceptual Plans and Costs"@en .

:c_3e1a5fff a skos:Concept;
  dct:created "2018-04-21T07:30:26.958Z"^^xsd:dateTime;
  skos:broader :c_54bbebe2;
  skos:inScheme :conceptScheme_751925ed;
  skos:prefLabel "client advisor"@en;
  skosxl:prefLabel :xl_en_fd1f5489 .

:xl_en_fd1f5489 a skosxl:Label;
  skosxl:literalForm "client advisor"@en .

:c_3fdd4da0 a skos:Concept;
  dct:created "2018-06-02T10:27:38.157Z"^^xsd:dateTime;
  dct:modified "2020-10-31T05:27:46.171Z"^^xsd:dateTime;
  skos:broader :c_fb07c266;
  skos:definition """Developed from the BIM Execution plan, this forms part of the (post-contract) BEP and is the primary plan for when information is going to be prepared, by whom and when. It also sets out the format and the timescales. This is developed from the BIM Execution Plan.
Each information deliverable will be aligned to a defined project stage and so the MIDP serves as a tool to define information delivery throughout the project.
"""@en;
  skos:inScheme :conceptScheme_751925ed;
  skosxl:altLabel :xl_en_0a7cb84d;
  skosxl:prefLabel :xl_en_5245a829 .

:xl_en_5245a829 a skosxl:Label;
  dct:modified "2018-07-20T22:05:03.112Z"^^xsd:dateTime;
  skosxl:literalForm "master information delivery plan"@en .

:xl_en_68051b88 a skosxl:Label;
  skosxl:literalForm "operation lead"@en .

:c_40fcae48 a skos:Concept;
  dct:created "2018-04-21T07:06:00.896Z"^^xsd:dateTime;
  skos:broader :c_d63bf876;
  skos:inScheme :conceptScheme_751925ed;
  skos:prefLabel "cladding consultant"@en;
  skosxl:prefLabel :xl_en_700446c9 .

:xl_en_700446c9 a skosxl:Label;
  skosxl:literalForm "cladding consultant"@en .

:c_42ccc536 a skos:Concept;
  dct:created "2018-05-26T09:17:02.170Z"^^xsd:dateTime;
  dct:modified "2018-05-26T09:19:28.331Z"^^xsd:dateTime;
  skos:broader :c_aca16e26;
  skos:definition "Code of practice for facilities management (Buildings infrastructure). Collaborative production of information. Fulfil employer’s information exchange requirements using COBie. Code of practice."@en;
  skos:inScheme :conceptScheme_751925ed;
  skos:prefLabel "bs 1192-4:2014 briefing for design and construction"@en;
  skos:related :c_a2512527;
  skosxl:prefLabel :xl_en_c860af68 .

:xl_en_c860af68 a skosxl:Label;
  dct:modified "2018-05-26T09:21:56.992Z"^^xsd:dateTime;
  skosxl:literalForm "bs 1192-4:2014 briefing for design and construction"@en .

:c_72030014 a skos:Concept;
  dct:created "2018-04-21T15:09:13.612Z"^^xsd:dateTime;
  dct:modified "2018-10-13T05:15:27.457Z"^^xsd:dateTime;
  skos:broader :c_43a1e1f6;
  skos:definition "Stage 0 is a new stage in which a project is strategically appraised and defined before a detailed brief is created. This is particularly relevant in the context of sustainability, when a refurbishment or extension, or indeed a rationalised space plan, may be more appropriate than a new building. Certain activities in Stage 0 are derived from the former (RIBA Outline Plan of Work 2007) Stage A."@en;
  skos:inScheme :conceptScheme_751925ed;
  skos:notation "0"@en;
  skos:prefLabel "strategic definition"@en;
  skosxl:prefLabel :xl_en_07b46ca0 .

:c_85a522a2 a skos:Concept;
  dct:created "2018-04-21T15:09:08.367Z"^^xsd:dateTime;
  dct:modified "2018-05-12T21:52:55.861Z"^^xsd:dateTime;
  skos:broader :c_43a1e1f6;
  skos:inScheme :conceptScheme_751925ed;
  skos:narrower :c_65a0a8d1, :c_9b31f808;
  skos:notation "7"@en;
  skos:prefLabel "in use"@en;
  skosxl:prefLabel :xl_en_f28f8018 .

:c_91ece774 a skos:Concept;
  dct:created "2018-04-21T15:09:02.896Z"^^xsd:dateTime;
  dct:modified "2018-10-25T12:27:35.353Z"^^xsd:dateTime;
  olo:index "5"^^xsd:positiveInteger;
  skos:broader :c_43a1e1f6;
  skos:inScheme :conceptScheme_751925ed;
  skos:narrower :c_129a5ec6, :c_2df70b84, :c_447a9eee, :c_4d73ba7d, :c_52608161, :c_86ec4f8f,
    :c_876afb3f, :c_9d7853dc, :c_b39bb643;
  skos:notation "5"@en;
  skos:prefLabel "construction"@en;
  skosxl:prefLabel :xl_en_40f29c99 .

:c_c02e3a4e a skos:Concept;
  dct:created "2018-04-21T15:08:57.117Z"^^xsd:dateTime;
  dct:modified "2018-07-20T21:49:49.963Z"^^xsd:dateTime;
  skos:broader :c_43a1e1f6;
  skos:inScheme :conceptScheme_751925ed;
  skos:narrower :c_86ec4f8f;
  skos:notation "6"@en;
  skos:prefLabel "handover and close out"@en;
  skosxl:prefLabel :xl_en_ccbbc2c1 .

:c_c7d2ad4d a skos:Concept;
  dct:created "2018-04-21T15:08:52.143Z"^^xsd:dateTime;
  dct:modified "2018-10-25T12:25:20.485Z"^^xsd:dateTime;
  olo:index "1"^^xsd:positiveInteger;
  skos:broader :c_43a1e1f6;
  skos:inScheme :conceptScheme_751925ed;
  skos:narrower :c_e2623996;
  skos:notation "1"@en;
  skos:prefLabel "preparation and brief"@en;
  skos:related :c_8cff7d88;
  skosxl:prefLabel :xl_en_e4618c12 .

:c_e85c9613 a skos:Concept;
  dct:created "2018-04-21T15:08:40.619Z"^^xsd:dateTime;
  dct:modified "2018-10-25T12:26:47.787Z"^^xsd:dateTime;
  olo:index "3"^^xsd:positiveInteger;
  skos:broader :c_43a1e1f6;
  skos:inScheme :conceptScheme_751925ed;
  skos:notation "3"@en;
  skos:prefLabel "developed design"@en;
  skosxl:prefLabel :xl_en_111e4da6 .

:xl_en_8ff272ff a skosxl:Label;
  skosxl:literalForm "development stages"@en .

:xl_en_1333d9a7 a skosxl:Label;
  skosxl:literalForm """2.1.6
"""@en .

:c_499e656c a skos:Concept;
  dct:created "2018-04-07T19:32:14.935Z"^^xsd:dateTime;
  dct:modified "2018-04-21T16:13:46.736Z"^^xsd:dateTime;
  skos:broader :c_8d825e3a;
  skos:inScheme :conceptScheme_751925ed;
  skos:prefLabel "infrastructure"@en;
  skosxl:prefLabel :xl_en_a1352f11 .

:xl_en_a1352f11 a skosxl:Label;
  skosxl:literalForm "infrastructure"@en .

:c_4a209fca a skos:Concept;
  dct:created "2018-03-28T19:32:00.633Z"^^xsd:dateTime;
  dct:modified "2020-10-31T06:00:03.127Z"^^xsd:dateTime;
  skos:broader :c_aca16e26;
  skos:definition """BS ISO 15686-5:2008 Buildings & Constructed assets - Service life planning - Part 5 - Life Cycle Costings ISO 15686-5:2008 gives guidelines for performing life cycle cost (LCC) analyses of buildings and constructed assets and their parts.
"""@en;
  skos:inScheme :conceptScheme_751925ed;
  skos:prefLabel "bs iso 15686-5:2008 constructed assets"@en;
  skos:related :c_85a522a2;
  skosxl:prefLabel :xl_en_2996f0d8 .

:xl_en_7ae952d6 skosxl:literalForm "bs 8536-1:2016 briefing for design and construction. code of practice for facilities management"@en .

:xl_en_2996f0d8 a skosxl:Label;
  dct:modified "2018-05-12T22:03:40.946Z"^^xsd:dateTime;
  skosxl:literalForm "bs iso 15686-5:2008 constructed assets"@en .

:xl_en_5b75f095 a skosxl:Label;
  skosxl:literalForm "civil engineer"@en .

:c_4a5391b1 a skos:Concept;
  dct:created "2018-04-21T14:23:37.837Z"^^xsd:dateTime;
  skos:broader :c_b8f9acb4;
  skos:inScheme :conceptScheme_751925ed;
  skos:prefLabel "geotechnical consultant"@en;
  skosxl:prefLabel :xl_en_d4111ccd .

:xl_en_d4111ccd a skosxl:Label;
  skosxl:literalForm "geotechnical consultant"@en .

:c_4bbe2792 a skos:Concept;
  dct:created "2018-04-07T19:32:20.545Z"^^xsd:dateTime;
  dct:modified "2018-04-21T16:14:02.125Z"^^xsd:dateTime;
  skos:broader :c_8d825e3a;
  skos:inScheme :conceptScheme_751925ed;
  skos:prefLabel "risk management"@en;
  skosxl:prefLabel :xl_en_d7ffc6cd .

:xl_en_d7ffc6cd a skosxl:Label;
  skosxl:literalForm "risk management"@en .

:c_4d537a54 a skos:Concept;
  dct:created "2018-04-07T19:32:32.839Z"^^xsd:dateTime;
  dct:modified "2018-04-21T16:13:20.276Z"^^xsd:dateTime;
  skos:broader :c_8d825e3a;
  skos:inScheme :conceptScheme_751925ed;
  skos:prefLabel "community engagement"@en;
  skosxl:prefLabel :xl_en_050cbfe1 .

:xl_en_050cbfe1 a skosxl:Label;
  skosxl:literalForm "community engagement"@en .

:xl_en_8f8bcdd8 a skosxl:Label;
  dct:modified "2018-07-20T21:35:16.500Z"^^xsd:dateTime;
  skosxl:literalForm "asset information model"@en .

:xl_en_551b4be5 a skosxl:Label;
  skosxl:literalForm "civil engineering designer"@en .

:c_4de604ce a skos:Concept;
  dct:created "2018-05-02T17:37:09.762Z"^^xsd:dateTime;
  dct:modified "2018-05-02T17:39:38.275Z"^^xsd:dateTime;
  skos:broader :c_aca16e26;
  skos:definition """BS 8895-2:2015 Designing for material efficiency in building projects. Code of Practice for concept and developed design The second part of BS 8895 series is a code of practice for designing for material efficiency, which is a key part to achieve higher levels of resource efficiency in a building project. This is an important standard in matters of waste management, in the construction area.BS 8895-2 gives recommendations for the processes, information exchanges and responsibilities for design teams to incorporate into projects at the Concept Design and Developed Design Stages of a building project. These recommendations are accepted as a good practice by industry leaders and practitioners.
"""@en;
  skos:inScheme :conceptScheme_751925ed;
  skos:prefLabel "bs 8895-2:2015 material"@en;
  skos:related :c_8d825e3a;
  skosxl:prefLabel :xl_en_55676187 .

:xl_en_55676187 a skosxl:Label;
  dct:modified "2018-05-12T22:03:10.660Z"^^xsd:dateTime;
  skosxl:literalForm "bs 8895-2:2015 material"@en .

:xl_en_6938f5ab a skosxl:Label;
  skosxl:literalForm "network modeller"@en .

:xl_en_98f6ec45 a skosxl:Label;
  skosxl:literalForm "telecommunication engineer"@en .

:c_503d9a20 a skos:Concept;
  dct:created "2018-04-21T07:06:33.407Z"^^xsd:dateTime;
  skos:broader :c_d63bf876;
  skos:inScheme :conceptScheme_751925ed;
  skos:prefLabel "landscape designer"@en;
  skosxl:prefLabel :xl_en_91630035 .

:xl_en_91630035 a skosxl:Label;
  skosxl:literalForm "landscape designer"@en .

:c_50aeabe6 a skos:Concept;
  dct:created "2018-05-26T09:35:49.759Z"^^xsd:dateTime;
  dct:modified "2018-05-26T09:37:18.949Z"^^xsd:dateTime;
  skos:broader :c_aca16e26;
  skos:definition "Customer satisfaction,guidelines for monitoring and measuring"@en;
  skos:inScheme :conceptScheme_751925ed;
  skos:prefLabel "bs iso 10004:2012 quality management"@en;
  skos:related :c_a2512527;
  skosxl:prefLabel :xl_en_1a5a9d4c .

:xl_en_1a5a9d4c a skosxl:Label;
  skosxl:literalForm "bs iso 10004:2012 quality management"@en .

:c_51080e49 a skos:Concept;
  dct:created "2018-04-21T14:28:50.535Z"^^xsd:dateTime;
  skos:broader :c_fbcae061;
  skos:inScheme :conceptScheme_751925ed;
  skos:prefLabel "partner"@en;
  skosxl:prefLabel :xl_en_d38b75fa .

:xl_en_d38b75fa a skosxl:Label;
  skosxl:literalForm "partner"@en .

:c_5b6f2370 a skos:Concept;
  dct:created "2018-04-21T07:30:05.439Z"^^xsd:dateTime;
  skos:broader :c_54bbebe2;
  skos:inScheme :conceptScheme_751925ed;
  skos:prefLabel "clerk of works"@en;
  skosxl:prefLabel :xl_en_8c623f12 .

:c_6be94e63 a skos:Concept;
  dct:created "2018-04-21T07:29:42.795Z"^^xsd:dateTime;
  skos:broader :c_54bbebe2;
  skos:inScheme :conceptScheme_751925ed;
  skos:prefLabel "asset management advisor"@en;
  skosxl:prefLabel :xl_en_e97ef744 .

:c_934dba80 a skos:Concept;
  dct:created "2018-04-21T07:31:27.937Z"^^xsd:dateTime;
  skos:broader :c_54bbebe2;
  skos:inScheme :conceptScheme_751925ed;
  skos:prefLabel "employers project manager"@en;
  skosxl:prefLabel :xl_en_da8246de .

:c_b0c264b4 a skos:Concept;
  dct:created "2018-04-21T07:29:54.098Z"^^xsd:dateTime;
  skos:broader :c_54bbebe2;
  skos:inScheme :conceptScheme_751925ed;
  skos:prefLabel "asset manager"@en;
  skosxl:prefLabel :xl_en_69c06b3c .

:c_d0f52b80 a skos:Concept;
  dct:created "2018-04-21T07:30:16.084Z"^^xsd:dateTime;
  dct:modified "2018-07-22T07:16:12.570Z"^^xsd:dateTime;
  skos:broader :c_54bbebe2;
  skos:inScheme :conceptScheme_751925ed;
  skos:notation "K"@en;
  skos:prefLabel "client"@en;
  skosxl:prefLabel :xl_en_8b493f51 .

:c_e92dd4bd a skos:Concept;
  dct:created "2018-04-21T07:30:52.903Z"^^xsd:dateTime;
  skos:broader :c_54bbebe2;
  skos:inScheme :conceptScheme_751925ed;
  skos:prefLabel "employer"@en;
  skosxl:prefLabel :xl_en_6a8a0f84 .

:c_f479b450 a skos:Concept;
  dct:created "2018-04-21T07:31:42.160Z"^^xsd:dateTime;
  dct:modified "2018-07-22T07:07:28.066Z"^^xsd:dateTime;
  skos:broader :c_54bbebe2;
  skos:inScheme :conceptScheme_751925ed;
  skos:notation "F"@en;
  skos:prefLabel "facilities engineer"@en;
  skosxl:prefLabel :xl_en_638d7b83 .

:xl_en_61a52c37 a skosxl:Label;
  skosxl:literalForm "client roles"@en .

:c_54c8ace8 a skos:Concept;
  dct:created "2018-04-21T14:35:30.828Z"^^xsd:dateTime;
  skos:broader :c_ba4a8cbb;
  skos:inScheme :conceptScheme_751925ed;
  skos:prefLabel "security consultant"@en;
  skosxl:prefLabel :xl_en_ab967b5b .

:xl_en_ab967b5b a skosxl:Label;
  skosxl:literalForm "security consultant"@en .

:c_556714cc a skos:Concept;
  dct:created "2018-05-26T09:29:08.764Z"^^xsd:dateTime;
  dct:modified "2018-05-26T09:30:19.239Z"^^xsd:dateTime;
  skos:broader :c_aca16e26;
  skos:definition "Requirements"@en;
  skos:inScheme :conceptScheme_751925ed;
  skos:prefLabel "iso 9001:2015 – quality management systems"@en;
  skos:related :c_a2512527;
  skosxl:prefLabel :xl_en_986849d5 .

:xl_en_986849d5 a skosxl:Label;
  skosxl:literalForm "iso 9001:2015 – quality management systems"@en .

:xl_en_1d3b7898 a skosxl:Label;
  skosxl:literalForm "design lead"@en .

:xl_en_c059ec62 a skosxl:Label;
  skosxl:literalForm "public health engineer"@en .

:c_581128f4 a skos:Concept;
  dct:created "2018-04-07T19:32:09.183Z"^^xsd:dateTime;
  dct:modified "2018-04-21T16:13:30.325Z"^^xsd:dateTime;
  skos:broader :c_8d825e3a;
  skos:inScheme :conceptScheme_751925ed;
  skos:prefLabel "constraints"@en;
  skosxl:prefLabel :xl_en_08fb6d0e .

:xl_en_08fb6d0e a skosxl:Label;
  skosxl:literalForm "constraints"@en .

:c_583a056d a skos:Concept;
  dct:created "2018-04-07T19:32:58.411Z"^^xsd:dateTime;
  dct:modified "2018-04-21T16:13:38.730Z"^^xsd:dateTime;
  skos:broader :c_8d825e3a;
  skos:inScheme :conceptScheme_751925ed;
  skos:prefLabel "discuss house type elevations"@en;
  skosxl:prefLabel :xl_en_524d7efa .

:xl_en_524d7efa a skosxl:Label;
  skosxl:literalForm "discuss house type elevations"@en .

:c_597e7267 a skos:Concept;
  dct:created "2018-04-21T16:06:31.771Z"^^xsd:dateTime;
  dct:modified "2018-04-21T16:08:04.572Z"^^xsd:dateTime;
  skos:broader :c_a314e31f;
  skos:inScheme :conceptScheme_751925ed;
  skos:prefLabel "availability"@en;
  skos:related :c_ca2b1c80;
  skosxl:prefLabel :xl_en_95170438 .

:xl_en_95170438 a skosxl:Label;
  skosxl:literalForm "availability"@en .

:c_5ae807c5 a skos:Concept;
  dc:source "zero carbon hub appendices - closing the gap between design and as-built performance - appendix c";
  dct:created "2018-04-07T19:43:05.418Z"^^xsd:dateTime;
  dct:modified "2018-08-22T16:26:54.736Z"^^xsd:dateTime;
  skos:broader :c_c76077ab;
  skos:inScheme :conceptScheme_751925ed;
  skos:notation "DET"@en;
  skos:prefLabel "junction detail"@en;
  skosxl:prefLabel :xl_en_5f1c929c .

:xl_en_5f1c929c a skosxl:Label;
  skosxl:literalForm "junction detail"@en .

:xl_en_8c623f12 a skosxl:Label;
  skosxl:literalForm "clerk of works"@en .

:c_5bc1704c a skos:Concept;
  dct:created "2018-06-02T10:29:38.780Z"^^xsd:dateTime;
  dct:modified "2020-10-31T05:37:13.352Z"^^xsd:dateTime;
  skos:broader :c_fb07c266;
  skos:definition "Task Information Delivery Plans are produced for/by each supply chain member from their viewpoint. They are collated into the Master Information Delivery Plan and are based on the deliverables as agreed within their contract."@en;
  skos:inScheme :conceptScheme_751925ed;
  skosxl:altLabel :xl_en_cff63d0f;
  skosxl:prefLabel :xl_en_6070e5f9 .

:xl_en_6070e5f9 a skosxl:Label;
  dct:modified "2018-07-20T22:09:35.677Z"^^xsd:dateTime;
  skosxl:literalForm "task information delivery plan"@en .

:c_5c66c27c a skos:Concept;
  dct:created "2018-04-17T18:52:40.251Z"^^xsd:dateTime;
  dct:modified "2018-04-21T15:44:38.553Z"^^xsd:dateTime;
  skos:broader :c_a314e31f;
  skos:inScheme :conceptScheme_751925ed;
  skos:prefLabel "project"@en;
  skosxl:prefLabel :xl_en_1d5e7066 .

:xl_en_1d5e7066 a skosxl:Label;
  skosxl:literalForm "project"@en .

:c_5dc9194d a skos:Concept;
  dct:created "2018-04-21T14:43:44.570Z"^^xsd:dateTime;
  skos:broader :c_d7f03766;
  skos:inScheme :conceptScheme_751925ed;
  skos:prefLabel "land surveyor"@en;
  skosxl:prefLabel :xl_en_07cbe557 .

:xl_en_07cbe557 a skosxl:Label;
  skosxl:literalForm "land surveyor"@en .

:c_5de8e729 a skos:Concept;
  dct:created "2018-05-26T09:43:47.183Z"^^xsd:dateTime;
  dct:modified "2020-10-31T05:55:28.517Z"^^xsd:dateTime;
  skos:broader :c_aca16e26;
  skos:definition "Linear and geographical infrastructure"@en;
  skos:inScheme :conceptScheme_751925ed;
  skos:prefLabel "bs 8536-2 briefing for design and construction. code of practice for asset management"@en;
  skos:related :c_a2512527;
  skosxl:prefLabel :xl_en_260474f3 .

:xl_en_260474f3 a skosxl:Label;
  dct:modified "2020-10-31T05:55:35.955Z"^^xsd:dateTime .

:c_5e1dcd56 a skos:Concept;
  dct:created "2018-03-28T15:48:07.134Z"^^xsd:dateTime;
  dct:modified "2018-07-20T19:47:34.606Z"^^xsd:dateTime;
  skos:broader :c_a314e31f;
  skos:hiddenLabel """2.1.4
"""@en;
  skos:inScheme :conceptScheme_751925ed;
  skos:prefLabel "Use Facilities : Identify Customer Needs and Requirements"@en;
  skosxl:hiddenLabel :xl_en_63b1eba4;
  skosxl:prefLabel :xl_en_9d737a67 .

:xl_en_63b1eba4 a skosxl:Label;
  skosxl:literalForm """2.1.4
"""@en .

:xl_en_9d737a67 a skosxl:Label;
  skosxl:literalForm "Use Facilities : Identify Customer Needs and Requirements"@en .

:c_6385917d a skos:Concept;
  dct:created "2018-04-17T18:53:39.607Z"^^xsd:dateTime;
  dct:modified "2018-04-21T06:51:27.516Z"^^xsd:dateTime;
  rdfs:seeAlso <http://eprints.bimcoordinator.co.uk/id/publication/ext-9b8c1a779fc843219ba2f1b4a6a5c188>;
  skos:broader :c_5c66c27c;
  skos:inScheme :conceptScheme_751925ed;
  skos:prefLabel "Construction-Project"@en;
  skosxl:prefLabel :xl_en_f92fa336 .

:xl_en_f92fa336 a skosxl:Label;
  skosxl:literalForm "Construction-Project"@en .

:c_65a0a8d1 a skos:Concept;
  dct:created "2018-04-21T15:10:51.765Z"^^xsd:dateTime;
  dct:modified "2018-10-13T05:17:26.581Z"^^xsd:dateTime;
  skos:broader :c_85a522a2;
  skos:inScheme :conceptScheme_751925ed;
  skos:notation "71"@en;
  skos:prefLabel "end of life"@en;
  skosxl:prefLabel :xl_en_1f70c43c .

:xl_en_1f70c43c a skosxl:Label;
  skosxl:literalForm "end of life"@en .

:c_6666c1fb a skos:Concept;
  dct:created "2018-05-26T09:48:40.744Z"^^xsd:dateTime;
  dct:modified "2018-05-26T09:49:50.257Z"^^xsd:dateTime;
  skos:broader :c_aca16e26;
  skos:definition "Shape and measurement, code of practice"@en;
  skos:inScheme :conceptScheme_751925ed;
  skos:prefLabel "bs 8541-3:2012 library objects for architecture, engineering and construction"@en;
  skos:related :c_a2512527;
  skosxl:prefLabel :xl_en_bd2d2587 .

:xl_en_bd2d2587 a skosxl:Label;
  skosxl:literalForm "bs 8541-3:2012 library objects for architecture, engineering and construction"@en .

:c_67cf7604 a skos:Concept;
  dct:created "2018-03-28T15:48:54.575Z"^^xsd:dateTime;
  dct:modified "2018-07-20T19:46:51.443Z"^^xsd:dateTime;
  skos:broader :c_a314e31f;
  skos:hiddenLabel """2.1.5
"""@en;
  skos:inScheme :conceptScheme_751925ed;
  skos:prefLabel "Establish Funding Priorities; Program Resources"@en;
  skosxl:hiddenLabel :xl_en_bdc8faa4;
  skosxl:prefLabel :xl_en_8799e7f2 .

:xl_en_bdc8faa4 a skosxl:Label;
  skosxl:literalForm """2.1.5
"""@en .

:xl_en_8799e7f2 a skosxl:Label;
  skosxl:literalForm "Establish Funding Priorities; Program Resources"@en .

:c_6843a9be a skos:Concept;
  dct:created "2018-04-21T14:27:57.692Z"^^xsd:dateTime;
  skos:broader :c_fbcae061;
  skos:inScheme :conceptScheme_751925ed;
  skos:prefLabel "director"@en;
  skosxl:prefLabel :xl_en_b57455dc .

:xl_en_b57455dc a skosxl:Label;
  skosxl:literalForm "director"@en .

:c_68a58f6d a skos:Concept;
  dct:created "2018-04-21T07:07:00.501Z"^^xsd:dateTime;
  skos:broader :c_d63bf876;
  skos:inScheme :conceptScheme_751925ed;
  skos:prefLabel "signage designer"@en;
  skosxl:prefLabel :xl_en_fd9d5696 .

:xl_en_fd9d5696 a skosxl:Label;
  skosxl:literalForm "signage designer"@en .

:c_69e09153 a skos:Concept;
  dc:source "Building a Safer Future – Independent Review of Building Regulations and Fire Safety: Final Report"@en;
  dct:created "2018-04-21T07:39:43.282Z"^^xsd:dateTime;
  dct:modified "2018-07-28T16:42:11.788Z"^^xsd:dateTime;
  skos:broader :c_b67efcfb;
  skos:definition "Under the Construction (Design and Management) Regulations 2015 a principal contractor is a contractor appointed by the client to take lead control during the construction phase of any project where there is more than one contractor involved"@en;
  skos:inScheme :conceptScheme_751925ed;
  skos:notation "PC"@en;
  skos:prefLabel "principal contractor"@en;
  skosxl:prefLabel :xl_en_ad5d671e .

:xl_en_ad5d671e a skosxl:Label;
  skosxl:literalForm "principal contractor"@en .

:xl_en_e97ef744 a skosxl:Label;
  skosxl:literalForm "asset management advisor"@en .

:c_6fdebefd a skos:Concept;
  dct:created "2018-03-28T15:42:44.763Z"^^xsd:dateTime;
  dct:modified "2018-07-20T19:47:10.563Z"^^xsd:dateTime;
  skos:broader :c_a314e31f;
  skos:definition """\"Also include Risk Assessment Acquisition Plan
Include;
Acquisition Strategy
Scope Schedule
Cost
Quality
Risk Assessment
Project team roles
And responsibilities
Project budget\"
"""@en;
  skos:hiddenLabel """2.1.11
"""@en;
  skos:inScheme :conceptScheme_751925ed;
  skos:prefLabel "K"@en;
  skosxl:hiddenLabel :xl_en_8c98a903;
  skosxl:prefLabel :xl_en_11947509 .

:xl_en_8c98a903 a skosxl:Label;
  skosxl:literalForm """2.1.11
"""@en .

:xl_en_11947509 a skosxl:Label;
  skosxl:literalForm "K"@en .

:c_70159d2c a skos:Concept;
  dct:created "2018-04-21T14:22:42.074Z"^^xsd:dateTime;
  skos:broader :c_b8f9acb4;
  skos:inScheme :conceptScheme_751925ed;
  skos:prefLabel "archaeological consultant"@en;
  skosxl:prefLabel :xl_en_93e32c2b .

:xl_en_93e32c2b a skosxl:Label;
  skosxl:literalForm "archaeological consultant"@en .

:xl_en_59685d3e a skosxl:Label;
  skosxl:literalForm "health and safety adviser"@en .

:xl_en_07b46ca0 a skosxl:Label;
  skosxl:literalForm "strategic definition"@en .

:c_75ffd205 dct:created "2018-04-21T15:09:31.302Z"^^xsd:dateTime .

:c_773411de a skos:Concept;
  dct:created "2018-05-12T22:04:38.007Z"^^xsd:dateTime;
  dct:modified "2020-10-31T05:43:58.480Z"^^xsd:dateTime;
  skos:broader :c_aca16e26;
  skos:definition """BIM - A standard Framework & Guide to BS1192 This book is a guide to BS 1192:2007 Collaborative production of architectural, engineering and construction information, the British Standard that is the code of practice that provides a best practice method for the development, organization and management of production information for the construction industry
"""@en;
  skos:inScheme :conceptScheme_751925ed;
  skos:prefLabel "guide to bs1192"@en;
  skos:related :c_c7d2ad4d;
  skosxl:prefLabel :xl_en_5e0bcc99 .

:xl_en_5e0bcc99 a skosxl:Label;
  dct:modified "2020-10-31T05:43:25.047Z"^^xsd:dateTime .

:xl_en_62778564 a skosxl:Label;
  skosxl:literalForm "management consultant"@en .

:xl_en_5d78835d a skosxl:Label;
  skosxl:literalForm "maintenance provider"@en .

:c_7b22749d a skos:Concept;
  dct:created "2018-04-21T07:38:41.256Z"^^xsd:dateTime;
  dct:modified "2020-10-30T20:38:03.862Z"^^xsd:dateTime;
  skos:broader :c_b67efcfb;
  skos:inScheme :conceptScheme_751925ed;
  skos:notation "W"@en;
  skosxl:prefLabel :xl_en_c86fdb9f .

:xl_en_c86fdb9f a skosxl:Label;
  skosxl:literalForm "contractor"@en .

:c_7d508f5e a skos:Concept;
  dct:created "2018-06-02T14:20:10.063Z"^^xsd:dateTime;
  dct:modified "2020-10-30T20:31:25.198Z"^^xsd:dateTime;
  skos:broader :c_fb07c266;
  skos:definition """All parties use their own 3D CAD
models, not necessarily working on a single, shared model
– Collaboration is used. Data is exchanged between parties and design information is shared in a single file format
– Federated BIM model is created. Each party can combine data with their own in order to make checks.
"""@en;
  skos:inScheme :conceptScheme_751925ed;
  skosxl:prefLabel :xl_en_55df4fd9 .

:xl_en_55df4fd9 a skosxl:Label;
  skosxl:literalForm "bim level 2"@en .

:c_800d8fbb a skos:Concept;
  dct:created "2018-06-02T10:32:35.705Z"^^xsd:dateTime;
  dct:modified "2020-10-30T21:00:26.451Z"^^xsd:dateTime;
  skos:broader :c_fb07c266;
  skos:definition """This is the term for the information (graphical, non-graphical, documentation) which is developed
during the design/construction phase of the project. Information that forms the PIM is created by the project team and sits within the CDE. As the project develops so too will the PIM, which will increase in both size and accuracy; starting as a design intent model progressing to an as-built model after construction is complete
"""@en;
  skos:inScheme :conceptScheme_751925ed;
  skosxl:altLabel :xl_en_7274bb0f;
  skosxl:prefLabel :xl_en_a1ae2cbd .

:xl_en_a1ae2cbd a skosxl:Label;
  dct:modified "2018-07-20T22:07:09.133Z"^^xsd:dateTime;
  skosxl:literalForm "project information model"@en .

:c_803a74ef a skos:Concept;
  dct:created "2018-04-21T07:38:30.565Z"^^xsd:dateTime;
  skos:broader :c_b67efcfb;
  skos:inScheme :conceptScheme_751925ed;
  skos:prefLabel "contract administrator"@en;
  skosxl:prefLabel :xl_en_c501e9dc .

:xl_en_c501e9dc a skosxl:Label;
  skosxl:literalForm "contract administrator"@en .

:c_818585d8 a skos:Concept;
  dct:created "2018-06-02T10:38:33.987Z"^^xsd:dateTime;
  skos:broader :c_fb07c266;
  skos:definition "A spreadsheet data format that contains digital information about an maintainable assets in as complete and as useful a form as possible. This spreadsheet has a has a pre-defined structure that is used to both store and index information transferred within the CDE.   A COBie file contains only information that is needed and is stored in such a way that the recipient knows exactly where to find any given information (allowing automation of this process)."@en;
  skos:inScheme :conceptScheme_751925ed;
  skos:prefLabel "construction operation building information exchange"@en;
  skosxl:altLabel :xl_en_8715993d;
  skosxl:prefLabel :xl_en_b9505ad1 .

:xl_en_b9505ad1 a skosxl:Label;
  dct:modified "2018-07-20T22:01:25.028Z"^^xsd:dateTime;
  skosxl:literalForm "construction operation building information exchange"@en .

:c_81a0559f a skos:Concept;
  dct:created "2018-03-28T15:56:11.217Z"^^xsd:dateTime;
  dct:modified "2018-07-20T19:46:24.119Z"^^xsd:dateTime;
  skos:broader :c_a314e31f;
  skos:hiddenLabel """2.1.8
"""@en;
  skos:inScheme :conceptScheme_751925ed;
  skos:prefLabel "Conduct Required Technical Studies (Structural, Geotech, Real Estate, etc.)"@en;
  skosxl:hiddenLabel :xl_en_718751b0;
  skosxl:prefLabel :xl_en_016f7a26 .

:xl_en_718751b0 a skosxl:Label;
  skosxl:literalForm """2.1.8
"""@en .

:xl_en_016f7a26 a skosxl:Label;
  skosxl:literalForm "Conduct Required Technical Studies (Structural, Geotech, Real Estate, etc.)"@en .

:c_9b31f808 a skos:Concept;
  dct:created "2018-04-21T15:11:12.110Z"^^xsd:dateTime;
  dct:modified "2018-10-13T05:17:37.402Z"^^xsd:dateTime;
  skos:broader :c_85a522a2;
  skos:inScheme :conceptScheme_751925ed;
  skos:notation "70"@en;
  skos:prefLabel "operation"@en;
  skosxl:prefLabel :xl_en_e4cd89c9 .

:xl_en_f28f8018 a skosxl:Label;
  skosxl:literalForm "in use"@en .

:c_86013584 a skos:Concept;
  dct:created "2018-03-28T18:07:31.253Z"^^xsd:dateTime;
  dct:modified "2018-07-20T19:54:38.089Z"^^xsd:dateTime;
  skos:broader :c_a314e31f;
  skos:inScheme :conceptScheme_751925ed;
  skos:prefLabel "concept and planning"@en;
  skosxl:prefLabel :xl_en_43071ad2 .

:xl_en_43071ad2 a skosxl:Label;
  dct:modified "2018-04-07T19:29:43.531Z"^^xsd:dateTime;
  skosxl:literalForm "concept and planning"@en .

:c_87ff7e6c a skos:Concept;
  dc:source "Interim Advice Note 184/16 Highways England CAD and Data Standard"@en;
  dct:created "2018-04-21T14:44:30.348Z"^^xsd:dateTime;
  dct:modified "2018-08-22T15:54:26.804Z"^^xsd:dateTime;
  skos:broader :c_d7f03766;
  skos:inScheme :conceptScheme_751925ed;
  skos:notation "QS"@en;
  skos:prefLabel "quantity surveyor"@en;
  skosxl:prefLabel :xl_en_f6e34ffe .

:xl_en_f6e34ffe a skosxl:Label;
  skosxl:literalForm "quantity surveyor"@en .

:c_89607d24 a skos:Concept;
  dct:created "2018-05-02T17:34:52.951Z"^^xsd:dateTime;
  dct:modified "2018-05-02T17:38:20.381Z"^^xsd:dateTime;
  skos:broader :c_aca16e26;
  skos:definition """BS ISO 29481-1-2010 BIM - Information Delivery Manual - Part 1 - Methodology & Format ISO 29481-1:2016 is intended to facilitate interoperability between software applications used during all stages of the life cycle of construction works, including briefing, design, documentation, construction, operation and maintenance, and demolition. It promotes digital collaboration between actors in the construction process and provides a basis for accurate, reliable, repeatable and high-quality information exchange.
"""@en;
  skos:inScheme :conceptScheme_751925ed;
  skos:prefLabel "bs iso 29481-1-2010 delivery manual"@en;
  skos:related :c_8d825e3a;
  skosxl:prefLabel :xl_en_ae306c51 .

:xl_en_ae306c51 a skosxl:Label;
  dct:modified "2018-05-12T22:04:06.105Z"^^xsd:dateTime;
  skosxl:literalForm "bs iso 29481-1-2010 delivery manual"@en .

:c_89628798 a skos:Concept;
  dct:created "2018-03-28T15:58:05.289Z"^^xsd:dateTime;
  dct:modified "2018-07-20T19:46:38.079Z"^^xsd:dateTime;
  skos:broader :c_a314e31f;
  skos:hiddenLabel """2.1.9
"""@en;
  skos:inScheme :conceptScheme_751925ed;
  skos:prefLabel "Develop Facility Master Plan, Identify Specific Project Requirements"@en;
  skosxl:hiddenLabel :xl_en_24febe8b;
  skosxl:prefLabel :xl_en_e593ba6c .

:xl_en_24febe8b a skosxl:Label;
  skosxl:literalForm """2.1.9
"""@en .

:xl_en_e593ba6c a skosxl:Label;
  skosxl:literalForm "Develop Facility Master Plan, Identify Specific Project Requirements"@en .

:xl_en_aaba830f a skosxl:Label;
  skosxl:literalForm "pas 1192-2:2013 capital/delivery"@en .

:c_96da4523 a skos:Concept;
  dct:created "2018-04-07T19:32:38.865Z"^^xsd:dateTime;
  dct:modified "2018-04-21T16:14:09.898Z"^^xsd:dateTime;
  skos:broader :c_8d825e3a;
  skos:inScheme :conceptScheme_751925ed;
  skos:prefLabel "submit for planning"@en;
  skosxl:prefLabel :xl_en_e381dbbb .

:c_b9523fc1 a skos:Concept;
  dct:created "2018-04-07T19:32:48.179Z"^^xsd:dateTime;
  dct:modified "2018-04-21T16:13:00.697Z"^^xsd:dateTime;
  skos:broader :c_8d825e3a;
  skos:inScheme :conceptScheme_751925ed;
  skos:prefLabel "agree design brief"@en;
  skosxl:prefLabel :xl_en_f799f626 .

:c_cdf35a77 a skos:Concept;
  dct:created "2018-04-07T19:32:26.709Z"^^xsd:dateTime;
  dct:modified "2018-04-21T16:14:17.567Z"^^xsd:dateTime;
  skos:broader :c_8d825e3a;
  skos:inScheme :conceptScheme_751925ed;
  skos:prefLabel "viability"@en;
  skosxl:prefLabel :xl_en_859d9d06 .

:c_d9801b1d a skos:Concept;
  dct:created "2018-04-07T19:32:01.941Z"^^xsd:dateTime;
  dct:modified "2018-04-21T16:13:54.869Z"^^xsd:dateTime;
  skos:broader :c_8d825e3a;
  skos:inScheme :conceptScheme_751925ed;
  skos:prefLabel "local authority policy"@en;
  skosxl:prefLabel :xl_en_328696a6 .

:xl_en_47240b6a a skosxl:Label;
  dct:modified "2018-05-12T21:37:22.989Z"^^xsd:dateTime;
  skosxl:literalForm "concept design"@en .

:xl_en_33c481b3 a skosxl:Label;
  dct:modified "2018-07-20T22:06:11.243Z"^^xsd:dateTime;
  skosxl:literalForm "plain language questions"@en .

:c_901951db a skos:Concept;
  dct:created "2018-04-21T07:40:04.310Z"^^xsd:dateTime;
  dct:modified "2018-07-22T07:53:38.126Z"^^xsd:dateTime;
  skos:broader :c_b67efcfb;
  skos:inScheme :conceptScheme_751925ed;
  skos:notation "PM"@en;
  skos:prefLabel "project manager"@en;
  skosxl:prefLabel :xl_en_234a93ca .

:xl_en_234a93ca a skosxl:Label;
  skosxl:literalForm "project manager"@en .

:c_91cd7cb5 a skos:Concept;
  dct:created "2018-04-21T14:27:07.077Z"^^xsd:dateTime;
  skos:broader :c_fbcae061;
  skos:inScheme :conceptScheme_751925ed;
  skos:prefLabel "associate"@en;
  skosxl:prefLabel :xl_en_1ecf0af8 .

:xl_en_1ecf0af8 a skosxl:Label;
  skosxl:literalForm "associate"@en .

:xl_en_40f29c99 a skosxl:Label;
  skosxl:literalForm "construction"@en .

:xl_en_0024b5e7 a skosxl:Label;
  skosxl:literalForm "structural engineering designer"@en .

:xl_en_da8246de a skosxl:Label;
  skosxl:literalForm "employers project manager"@en .

:c_96391878 a skos:Concept;
  dct:created "2018-04-21T14:44:41.135Z"^^xsd:dateTime;
  skos:broader :c_d7f03766;
  skos:inScheme :conceptScheme_751925ed;
  skos:prefLabel "site investigation consultant"@en;
  skosxl:prefLabel :xl_en_a0fa1b37 .

:xl_en_a0fa1b37 a skosxl:Label;
  skosxl:literalForm "site investigation consultant"@en .

:xl_en_e381dbbb a skosxl:Label;
  skosxl:literalForm "submit for planning"@en .

:xl_en_8ebaea43 a skosxl:Label;
  skosxl:literalForm "principal designer"@en .

:xl_en_fefa5cfb a skosxl:Label;
  skosxl:literalForm "programme lead"@en .

:xl_en_afa6b17f a skosxl:Label;
  skosxl:literalForm "structural engineer"@en .

:c_98637c9e a skos:Concept;
  dct:created "2018-04-21T14:52:41.343Z"^^xsd:dateTime;
  skos:broader :c_da75b83b;
  skos:inScheme :conceptScheme_751925ed;
  skos:prefLabel "traffic consultant"@en;
  skosxl:prefLabel :xl_en_9cde4079 .

:c_da75b83b a skos:Concept;
  dct:created "2018-04-21T07:04:22.986Z"^^xsd:dateTime;
  dct:modified "2018-04-21T14:54:07.273Z"^^xsd:dateTime;
  skos:broader :c_ca2b1c80;
  skos:inScheme :conceptScheme_751925ed;
  skos:narrower :c_98637c9e, :c_b548d0ff, :c_d63e56d7, :c_dddfdc05, :c_ed7dd1f7, :c_fcea3a25;
  skos:prefLabel "transport roles"@en;
  skosxl:prefLabel :xl_en_f1e3fb75 .

:xl_en_9cde4079 a skosxl:Label;
  skosxl:literalForm "traffic consultant"@en .

:xl_en_66ebdf30 a skosxl:Label;
  skosxl:literalForm "lawyer"@en .

:xl_en_e4cd89c9 a skosxl:Label;
  skosxl:literalForm "operation"@en .

:c_9c1d7995 a skos:Concept;
  dc:source " zero carbon hub appendices - closing the gap between design and as-built performance - appendix c";
  dct:created "2018-04-07T19:42:48.089Z"^^xsd:dateTime;
  dct:modified "2018-08-22T16:27:40.104Z"^^xsd:dateTime;
  skos:broader :c_c76077ab;
  skos:inScheme :conceptScheme_751925ed;
  skos:notation "ELEV"@en;
  skos:prefLabel "elevation"@en;
  skosxl:prefLabel :xl_en_22e9afe1 .

:xl_en_22e9afe1 a skosxl:Label;
  skosxl:literalForm "elevation"@en .

:c_9ce01e2d a skos:Concept;
  dct:created "2018-04-21T14:44:02.377Z"^^xsd:dateTime;
  skos:broader :c_d7f03766;
  skos:inScheme :conceptScheme_751925ed;
  skos:prefLabel "party wall surveyor"@en;
  skosxl:prefLabel :xl_en_be0aed0c .

:xl_en_be0aed0c a skosxl:Label;
  skosxl:literalForm "party wall surveyor"@en .

:c_9d3f953f a skos:Concept;
  dct:created "2018-04-07T19:42:42.062Z"^^xsd:dateTime;
  dct:modified "2018-07-22T08:26:59.633Z"^^xsd:dateTime;
  skos:broader :c_c76077ab;
  skos:inScheme :conceptScheme_751925ed;
  skos:notation "SECT"@en;
  skos:prefLabel "section"@en;
  skosxl:prefLabel :xl_en_23dba009 .

:xl_en_23dba009 a skosxl:Label;
  skosxl:literalForm "section"@en .

:c_9e715393 a skos:Concept;
  dct:created "2018-04-21T07:06:11.396Z"^^xsd:dateTime;
  dct:modified "2018-07-22T07:15:15.476Z"^^xsd:dateTime;
  skos:broader :c_d63bf876;
  skos:inScheme :conceptScheme_751925ed;
  skos:notation "I"@en;
  skos:prefLabel "interior designer"@en;
  skosxl:prefLabel :xl_en_f8e5da57 .

:xl_en_f8e5da57 a skosxl:Label;
  skosxl:literalForm "interior designer"@en .

:xl_en_ca45a339 a skosxl:Label;
  dct:modified "2018-05-26T11:11:06.275Z"^^xsd:dateTime;
  skosxl:literalForm "pas 1192-3:2014"@en .

:c_9f1a47e2 a skos:Concept;
  dct:created "2018-06-02T14:21:05.057Z"^^xsd:dateTime;
  skos:broader :c_fb07c266;
  skos:definition """Full collaboration between all
disciplines by means of using a single, shared project model which is held in a centralized  repository.
"""@en;
  skos:inScheme :conceptScheme_751925ed;
  skos:prefLabel "bim level 3"@en;
  skosxl:prefLabel :xl_en_f7dedf38 .

:xl_en_f7dedf38 a skosxl:Label;
  skosxl:literalForm "bim level 3"@en .

:c_9f44b691 a skos:Concept;
  dct:created "2018-03-28T15:45:05.441Z"^^xsd:dateTime;
  dct:modified "2020-10-31T05:52:54.344Z"^^xsd:dateTime;
  skos:broader :c_a314e31f;
  skos:hiddenLabel """2.1.2
"""@en;
  skos:inScheme :conceptScheme_751925ed;
  skos:prefLabel "initiate feasibility study"@en;
  skosxl:hiddenLabel :xl_en_fd21eb9e;
  skosxl:prefLabel :xl_en_7589e5ba .

:xl_en_fd21eb9e a skosxl:Label;
  skosxl:literalForm """2.1.2
"""@en .

:xl_en_7589e5ba a skosxl:Label;
  dct:modified "2020-10-31T05:51:35.986Z"^^xsd:dateTime .

:c_9f86fc42 a skos:Concept;
  dct:created "2018-04-21T14:28:30.069Z"^^xsd:dateTime;
  skos:broader :c_fbcae061;
  skos:inScheme :conceptScheme_751925ed;
  skos:prefLabel "managing director"@en;
  skosxl:prefLabel :xl_en_cd6aec65 .

:xl_en_cd6aec65 a skosxl:Label;
  skosxl:literalForm "managing director"@en .

:c_a1903547 a skos:Concept;
  dct:created "2018-04-21T14:29:10.706Z"^^xsd:dateTime;
  skos:broader :c_fbcae061;
  skos:inScheme :conceptScheme_751925ed;
  skos:prefLabel "vice chairman"@en;
  skosxl:prefLabel :xl_en_94e5c8a0 .

:xl_en_94e5c8a0 a skosxl:Label;
  skosxl:literalForm "vice chairman"@en .

:c_df0a0804 a skos:Concept;
  dct:created "2018-05-12T22:08:56.537Z"^^xsd:dateTime;
  dct:modified "2018-05-26T09:14:58.362Z"^^xsd:dateTime;
  skos:broader :c_aca16e26;
  skos:definition "Collaborative production of architectural, engineering and construction information. Code of practice."@en;
  skos:inScheme :conceptScheme_751925ed;
  skos:prefLabel "bs 1192-1 2007 + a2:2016 collaborative production"@en;
  skos:related :c_a2512527, :c_c7d2ad4d;
  skosxl:prefLabel :xl_en_a3c9f952 .

:c_a6870cbf a skos:Concept;
  dct:created "2018-05-26T09:45:52.812Z"^^xsd:dateTime;
  dct:modified "2018-05-26T09:47:39.373Z"^^xsd:dateTime;
  skos:broader :c_aca16e26;
  skos:definition " Identification and classification, code of practice"@en;
  skos:inScheme :conceptScheme_751925ed;
  skos:prefLabel "bs 8541-1:2012 library objects for architecture, engineering and construction"@en;
  skos:related :c_a2512527;
  skosxl:prefLabel :xl_en_a88bc42e .

:c_b046bfd7 a skos:Concept;
  dct:created "2018-06-02T10:16:29.928Z"^^xsd:dateTime;
  skos:broader :c_fb07c266;
  skos:definition """Broken up into pre and post-contract outputs, this document defines how the project will be carried out relates directly to the EIR. It includes, amongst other things, who is responsible for providing information,
 
what the processes will be, and provides common terminology to be adopted as well as job titles and responsibilities.
"""@en;
  skos:inScheme :conceptScheme_751925ed;
  skos:prefLabel "bim execution plan"@en;
  skosxl:altLabel :xl_en_ca2d0e57;
  skosxl:prefLabel :xl_en_a55d07c4 .

:c_b80b8cad a skos:Concept;
  dct:created "2018-05-26T09:41:08.070Z"^^xsd:dateTime;
  dct:modified "2020-10-31T05:58:19.292Z"^^xsd:dateTime;
  skos:broader :c_aca16e26;
  skos:definition "Buildings infrastructure"@en;
  skos:inScheme :conceptScheme_751925ed;
  skos:prefLabel "bs 8536-1:2016 briefing for design and construction. code of practice for facilities management"@en;
  skos:related :c_a2512527;
  skosxl:prefLabel :xl_en_7ae952d6 .

:c_b95acbc8 a skos:Concept;
  dct:created "2018-05-26T09:31:13.104Z"^^xsd:dateTime;
  dct:modified "2018-05-26T09:33:05.608Z"^^xsd:dateTime;
  skos:broader :c_aca16e26;
  skos:definition "Management systems requirements"@en;
  skos:inScheme :conceptScheme_751925ed;
  skos:prefLabel "iso 55001:2014 asset management"@en;
  skos:related :c_a2512527;
  skosxl:prefLabel :xl_en_bcefd2db .

:c_bcaf43b0 a skos:Concept;
  dct:created "2018-05-26T09:25:48.836Z"^^xsd:dateTime;
  dct:modified "2018-05-26T09:28:01.893Z"^^xsd:dateTime;
  skos:broader :c_aca16e26;
  skos:definition "A framework specification"@en;
  skos:inScheme :conceptScheme_751925ed;
  skos:prefLabel "bs 11000-1:2010 collaborative business relationships"@en;
  skos:related :c_a2512527;
  skosxl:prefLabel :xl_en_436338f3 .

:c_c7b03ed3 a skos:Concept;
  dct:created "2018-06-02T14:19:07.023Z"^^xsd:dateTime;
  skos:broader :c_fb07c266;
  skos:definition """Mixture of 3D concept work and 2D
for drafting of statutory approval documentation
– Electronic sharing of data using a common data environment (CDE)
– No collaboration between parties but data is shared.
"""@en;
  skos:inScheme :conceptScheme_751925ed;
  skos:prefLabel "bim level 1"@en;
  skosxl:prefLabel :xl_en_d0c4090d .

:c_ff860f3e a skos:Concept;
  dct:created "2018-06-02T10:31:06.126Z"^^xsd:dateTime;
  dct:modified "2020-10-31T05:26:53.672Z"^^xsd:dateTime;
  skos:broader :c_fb07c266;
  skos:definition """This forms part of the BEP and is a series of documents used to prove the supply chain’s overall capability to deliver the project, as defined by the EIR. This includes
 
a supply chain member’s current BIM knowledge and experience as well as the capability of both their IT and human resource. This will lead to an overall picture of the entire project team’s BIM capability.
"""@en;
  skos:inScheme :conceptScheme_751925ed;
  skosxl:altLabel :xl_en_74b321d9;
  skosxl:prefLabel :xl_en_8f54ec97 .

:xl_en_479835d3 a skosxl:Label;
  skosxl:literalForm "little book of bim"@en .

:xl_en_7071a06a a skosxl:Label;
  skosxl:literalForm "construction lead"@en .

:xl_en_a88bc42e a skosxl:Label;
  skosxl:literalForm "bs 8541-1:2012 library objects for architecture, engineering and construction"@en .

:c_ab14190c a skos:Concept;
  dct:created "2018-04-21T14:43:15.846Z"^^xsd:dateTime;
  skos:broader :c_d7f03766;
  skos:inScheme :conceptScheme_751925ed;
  skos:prefLabel "building control officer"@en;
  skosxl:prefLabel :xl_en_dc281a20 .

:xl_en_dc281a20 a skosxl:Label;
  skosxl:literalForm "building control officer"@en .

:xl_en_97e8ae77 a skosxl:Label;
  skosxl:literalForm "technical standards"@en .

:xl_en_1f8ea7d8 a skosxl:Label;
  skosxl:literalForm "process engineer"@en .

:c_af7e5693 a skos:Concept;
  dc:source " zero carbon hub appendices - closing the gap between design and as-built performance - appendix c";
  dct:created "2018-04-07T19:42:32.984Z"^^xsd:dateTime;
  dct:modified "2018-07-22T08:02:39.245Z"^^xsd:dateTime;
  skos:broader :c_c76077ab;
  skos:inScheme :conceptScheme_751925ed;
  skos:notation "FFP"@en;
  skos:prefLabel "floor plan"@en;
  skosxl:altLabel :xl_en_9717bf9a;
  skosxl:prefLabel :xl_en_8e62d1a9 .

:xl_en_8e62d1a9 a skosxl:Label;
  skosxl:literalForm "floor plan"@en .

:xl_en_73e4d0b6 a skosxl:Label;
  skosxl:literalForm "building services engineer"@en .

:xl_en_a55d07c4 a skosxl:Label;
  dct:modified "2018-07-20T21:58:48.407Z"^^xsd:dateTime;
  skosxl:literalForm "bim execution plan"@en .

:c_b0503f89 a skos:Concept;
  dc:source "Interim Advice Note 184/16 Highways England CAD and Data Standard"@en;
  dct:created "2018-04-21T07:40:17.129Z"^^xsd:dateTime;
  dct:modified "2020-10-31T05:30:04.404Z"^^xsd:dateTime;
  skos:broader :c_b67efcfb;
  skos:inScheme :conceptScheme_751925ed;
  skos:notation "XX"@en;
  skosxl:prefLabel :xl_en_9bd95c8b .

:xl_en_9bd95c8b a skosxl:Label;
  skosxl:literalForm "sub-contractor"@en .

:c_b06dcd33 a skos:Concept;
  dct:created "2018-04-21T07:39:28.404Z"^^xsd:dateTime;
  skos:broader :c_b67efcfb;
  skos:inScheme :conceptScheme_751925ed;
  skos:prefLabel "manufacturer"@en;
  skosxl:prefLabel :xl_en_49689d76 .

:xl_en_49689d76 a skosxl:Label;
  skosxl:literalForm "manufacturer"@en .

:xl_en_69c06b3c a skosxl:Label;
  skosxl:literalForm "asset manager"@en .

:c_b1c5511d a skos:Concept;
  dct:created "2018-04-21T07:05:47.546Z"^^xsd:dateTime;
  skos:broader :c_d63bf876;
  skos:inScheme :conceptScheme_751925ed;
  skos:prefLabel "architectural designer"@en;
  skosxl:prefLabel :xl_en_e93defbd .

:xl_en_e93defbd a skosxl:Label;
  skosxl:literalForm "architectural designer"@en .

:xl_en_68c040b3 a skosxl:Label;
  skosxl:literalForm "mechanical, electrical, instrumentation, control and automation (MEICA) consultant"@en .

:c_b50dc769 a skos:Concept;
  dct:created "2018-04-21T07:39:15.089Z"^^xsd:dateTime;
  skos:broader :c_b67efcfb;
  skos:inScheme :conceptScheme_751925ed;
  skos:prefLabel "information manager"@en;
  skosxl:prefLabel :xl_en_5e998f85 .

:xl_en_5e998f85 a skosxl:Label;
  skosxl:literalForm "information manager"@en .

:c_b548d0ff a skos:Concept;
  dct:created "2018-04-21T14:52:53.634Z"^^xsd:dateTime;
  skos:broader :c_da75b83b;
  skos:inScheme :conceptScheme_751925ed;
  skos:prefLabel "transportation planner"@en;
  skosxl:prefLabel :xl_en_ceef313c .

:xl_en_ceef313c a skosxl:Label;
  skosxl:literalForm "transportation planner"@en .

:c_cbae9e17 a skos:Concept;
  dct:created "2018-04-21T07:38:51.891Z"^^xsd:dateTime;
  skos:broader :c_b67efcfb;
  skos:inScheme :conceptScheme_751925ed;
  skos:prefLabel "cost consultant"@en;
  skosxl:prefLabel :xl_en_0d4f3cf5 .

:c_e94e8717 a skos:Concept;
  dct:created "2018-04-21T07:38:17.012Z"^^xsd:dateTime;
  skos:broader :c_b67efcfb;
  skos:inScheme :conceptScheme_751925ed;
  skos:prefLabel "construction operative"@en;
  skosxl:prefLabel :xl_en_c5d7135d .

:xl_en_5d8c071f a skosxl:Label;
  skosxl:literalForm "contractor and supplier roles"@en .

:c_b7c13cf0 a skos:Concept;
  dct:created "2018-04-21T14:43:34.934Z"^^xsd:dateTime;
  dct:modified "2018-07-22T07:01:35.003Z"^^xsd:dateTime;
  skos:broader :c_d7f03766;
  skos:inScheme :conceptScheme_751925ed;
  skos:notation "B"@en;
  skos:prefLabel "building surveyor"@en;
  skosxl:prefLabel :xl_en_a384b7e0 .

:xl_en_a384b7e0 a skosxl:Label;
  skosxl:literalForm "building surveyor"@en .

:xl_en_7ae952d6 a skosxl:Label;
  dct:modified "2020-10-31T05:58:27.613Z"^^xsd:dateTime .

:c_d9ac339e a skos:Concept;
  dct:created "2018-04-21T14:23:15.677Z"^^xsd:dateTime;
  skos:broader :c_b8f9acb4;
  skos:inScheme :conceptScheme_751925ed;
  skos:prefLabel "environmental consultant"@en;
  skosxl:prefLabel :xl_en_9f70c651 .

:c_dca128d9 a skos:Concept;
  dc:source "Interim Advice Note 184/16 Highways England CAD and Data Standard"@en;
  dct:created "2018-04-21T14:23:26.808Z"^^xsd:dateTime;
  dct:modified "2020-10-31T05:40:09.920Z"^^xsd:dateTime;
  skos:broader :c_b8f9acb4;
  skos:inScheme :conceptScheme_751925ed;
  skos:notation "VT"@en;
  skosxl:prefLabel :xl_en_81fc9b34 .

:c_ed68836f a skos:Concept;
  dct:created "2018-04-21T14:22:52.627Z"^^xsd:dateTime;
  dct:modified "2018-07-22T07:46:49.735Z"^^xsd:dateTime;
  skos:broader :c_b8f9acb4;
  skos:inScheme :conceptScheme_751925ed;
  skos:notation "ECO"@en;
  skos:prefLabel "ecologist"@en;
  skosxl:prefLabel :xl_en_9f2328c7 .

:c_fb85aed5 a skos:Concept;
  dct:created "2018-04-21T14:23:03.635Z"^^xsd:dateTime;
  skos:broader :c_b8f9acb4;
  skos:inScheme :conceptScheme_751925ed;
  skos:prefLabel "environmental assessor"@en;
  skosxl:prefLabel :xl_en_b1cb3ed5 .

:xl_en_c531fffd a skosxl:Label;
  skosxl:literalForm "environmental and geological roles"@en .

:xl_en_f799f626 a skosxl:Label;
  skosxl:literalForm "agree design brief"@en .

:xl_en_bcefd2db a skosxl:Label;
  skosxl:literalForm "iso 55001:2014 asset management"@en .

:c_bcd787cb a skos:Concept;
  dct:created "2018-04-21T14:35:01.711Z"^^xsd:dateTime;
  skos:broader :c_ba4a8cbb;
  skos:inScheme :conceptScheme_751925ed;
  skos:prefLabel "access consultant"@en;
  skosxl:prefLabel :xl_en_e1857ce4 .

:c_fcba3610 a skos:Concept;
  dct:created "2018-04-21T14:35:11.664Z"^^xsd:dateTime;
  skos:broader :c_ba4a8cbb;
  skos:inScheme :conceptScheme_751925ed;
  skos:prefLabel "catering consultant"@en;
  skosxl:prefLabel :xl_en_24c31b75 .

:xl_en_7ac09f7e a skosxl:Label;
  skosxl:literalForm "specialist roles"@en .

:c_bba5abb9 a skos:Concept;
  dc:source "zero carbon hub appendices - closing the gap between design and as-built performance - appendix c";
  dct:created "2018-04-07T19:47:40.166Z"^^xsd:dateTime;
  dct:modified "2018-07-24T16:59:25.915Z"^^xsd:dateTime;
  skos:broader :c_281f6d96;
  skos:inScheme :conceptScheme_751925ed;
  skos:prefLabel "site plan"@en;
  skosxl:prefLabel :xl_en_02ad786d .

:xl_en_02ad786d a skosxl:Label;
  skosxl:literalForm "site plan"@en .

:xl_en_8640cb95 a skosxl:Label;
  skosxl:literalForm "water engineer"@en .

:xl_en_436338f3 a skosxl:Label;
  skosxl:literalForm "bs 11000-1:2010 collaborative business relationships"@en .

:xl_en_e1857ce4 a skosxl:Label;
  skosxl:literalForm "access consultant"@en .

:xl_en_68bbe786 a skosxl:Label;
  dct:modified "2018-07-20T21:53:00.835Z"^^xsd:dateTime;
  skosxl:literalForm "common data environment"@en .

:c_be027528 a skos:Concept;
  dct:created "2018-04-21T14:44:20.745Z"^^xsd:dateTime;
  dct:modified "2018-07-22T07:22:24.858Z"^^xsd:dateTime;
  skos:broader :c_d7f03766;
  skos:inScheme :conceptScheme_751925ed;
  skos:notation "T"@en;
  skos:prefLabel "town and country planner"@en;
  skosxl:prefLabel :xl_en_02bdb69d .

:xl_en_02bdb69d a skosxl:Label;
  dct:modified "2018-07-22T07:21:59.505Z"^^xsd:dateTime;
  skosxl:literalForm "town and country planner"@en .

:xl_en_ccbbc2c1 a skosxl:Label;
  skosxl:literalForm "handover and close out"@en .

:c_c03abf22 a skos:Concept;
  dct:created "2018-04-21T14:27:26.793Z"^^xsd:dateTime;
  skos:broader :c_fbcae061;
  skos:inScheme :conceptScheme_751925ed;
  skos:prefLabel "chief executive officer"@en;
  skosxl:prefLabel :xl_en_a74bd3c7 .

:xl_en_a74bd3c7 a skosxl:Label;
  skosxl:literalForm "chief executive officer"@en .

:xl_en_de124a5c a skosxl:Label;
  skosxl:literalForm "electrical engineer"@en .

:c_c26a3327 a skos:Concept;
  dct:created "2018-03-28T15:50:37.063Z"^^xsd:dateTime;
  dct:modified "2018-07-20T19:46:32.011Z"^^xsd:dateTime;
  skos:broader :c_a314e31f;
  skos:hiddenLabel """2.1.6
"""@en;
  skos:inScheme :conceptScheme_751925ed;
  skos:prefLabel "Develop and Implement Integrated Project Management Plan (PMP Baseline)"@en;
  skosxl:hiddenLabel :xl_en_453bc190;
  skosxl:prefLabel :xl_en_5177dd8e .

:xl_en_453bc190 a skosxl:Label;
  skosxl:literalForm """2.1.6
"""@en .

:xl_en_5177dd8e a skosxl:Label;
  dct:modified "2018-03-28T15:52:03.853Z"^^xsd:dateTime;
  skosxl:literalForm "Develop and Implement Integrated Project Management Plan (PMP Baseline)"@en .

:c_c315cc73 a skos:Concept;
  dct:created "2018-03-28T15:34:23.269Z"^^xsd:dateTime;
  dct:modified "2018-07-20T19:46:57.234Z"^^xsd:dateTime;
  skos:broader :c_a314e31f;
  skos:hiddenLabel """2.1.10
"""@en;
  skos:inScheme :conceptScheme_751925ed;
  skos:prefLabel "Evaluate Costs And Benefits"@en;
  skosxl:hiddenLabel :xl_en_80102184;
  skosxl:prefLabel :xl_en_9fabc4e2 .

:xl_en_80102184 a skosxl:Label;
  skosxl:literalForm """2.1.10
"""@en .

:xl_en_9fabc4e2 a skosxl:Label;
  dct:modified "2018-03-28T15:36:48.120Z"^^xsd:dateTime;
  skosxl:literalForm "Evaluate Costs And Benefits"@en .

:xl_en_865b7696 a skosxl:Label;
  skosxl:literalForm "acoustic engineers"@en .

:c_c6f08cf1 a skos:Concept;
  dct:created "2018-04-21T14:28:09.645Z"^^xsd:dateTime;
  skos:broader :c_fbcae061;
  skos:inScheme :conceptScheme_751925ed;
  skos:prefLabel "executive director"@en;
  skosxl:prefLabel :xl_en_2ecf19e8 .

:xl_en_2ecf19e8 a skosxl:Label;
  skosxl:literalForm "executive director"@en .

:c_da9ab00d a skos:Concept;
  dct:created "2018-04-07T19:48:04.181Z"^^xsd:dateTime;
  dct:modified "2018-04-21T15:34:36.439Z"^^xsd:dateTime;
  skos:broader :c_c76077ab;
  skos:inScheme :conceptScheme_751925ed;
  skos:prefLabel "concept layout"@en;
  skos:related :c_86013584;
  skosxl:prefLabel :xl_en_52df7f0e .

:xl_en_4a44a158 a skosxl:Label;
  dct:modified "2018-08-11T12:19:48.255Z"^^xsd:dateTime;
  skosxl:literalForm "drawing building"@en .

:xl_en_d0c4090d a skosxl:Label;
  skosxl:literalForm "bim level 1"@en .

:c_e2623996 a skos:Concept;
  dct:created "2018-04-21T15:11:03.821Z"^^xsd:dateTime;
  dct:modified "2018-10-13T05:16:24.050Z"^^xsd:dateTime;
  skos:broader :c_c7d2ad4d;
  skos:inScheme :conceptScheme_751925ed;
  skos:notation "10"@en;
  skos:prefLabel "brief"@en;
  skosxl:prefLabel :xl_en_e7f12805 .

:xl_en_e4618c12 a skosxl:Label;
  dct:modified "2018-05-12T21:37:32.538Z"^^xsd:dateTime;
  skosxl:literalForm "preparation and brief"@en .

:xl_en_f97f9a08 a skosxl:Label;
  dct:modified "2018-04-21T06:56:30.004Z"^^xsd:dateTime;
  skosxl:literalForm "occupational groups"@en .

:xl_en_0d4f3cf5 a skosxl:Label;
  skosxl:literalForm "cost consultant"@en .

:xl_en_859d9d06 a skosxl:Label;
  skosxl:literalForm "viability"@en .

:xl_en_8b493f51 a skosxl:Label;
  skosxl:literalForm "client"@en .

:xl_en_3f00a2dd a skosxl:Label;
  dct:modified "2018-07-20T22:05:33.941Z"^^xsd:dateTime;
  skosxl:literalForm "organization information requirements"@en .

:xl_en_d1442c80 a skosxl:Label;
  skosxl:literalForm "commissioning engineer"@en .

:c_e231ef90 a skos:Concept;
  dct:created "2018-04-21T07:06:22.985Z"^^xsd:dateTime;
  dct:modified "2018-07-22T07:39:45.702Z"^^xsd:dateTime;
  skos:broader :c_d63bf876;
  skos:inScheme :conceptScheme_751925ed;
  skos:notation "L"@en;
  skos:prefLabel "landscape architect"@en;
  skosxl:prefLabel :xl_en_be1fad1a .

:c_e8742734 a skos:Concept;
  dct:created "2018-04-21T07:06:47.231Z"^^xsd:dateTime;
  skos:broader :c_d63bf876;
  skos:inScheme :conceptScheme_751925ed;
  skos:prefLabel "lighting designer"@en;
  skosxl:prefLabel :xl_en_481dc285 .

:xl_en_aa53329a a skosxl:Label;
  skosxl:literalForm "architectural roles"@en .

:c_d63e56d7 a skos:Concept;
  dct:created "2018-04-21T14:52:21.081Z"^^xsd:dateTime;
  skos:broader :c_da75b83b;
  skos:inScheme :conceptScheme_751925ed;
  skos:prefLabel "road engineer"@en;
  skosxl:prefLabel :xl_en_46e9ee51 .

:xl_en_46e9ee51 a skosxl:Label;
  skosxl:literalForm "road engineer"@en .

:c_f74d9794 a skos:Concept;
  dct:created "2018-04-21T14:43:53.442Z"^^xsd:dateTime;
  skos:broader :c_d7f03766;
  skos:inScheme :conceptScheme_751925ed;
  skos:prefLabel "master-planning consultant"@en;
  skosxl:prefLabel :xl_en_e4f4a022 .

:xl_en_7d7cec2b a skosxl:Label;
  skosxl:literalForm "surveyor and planner roles"@en .

:xl_en_328696a6 a skosxl:Label;
  skosxl:literalForm "local authority policy"@en .

:xl_en_9f70c651 a skosxl:Label;
  skosxl:literalForm "environmental consultant"@en .

:c_dddfdc05 a skos:Concept;
  dct:created "2018-04-21T14:52:12.089Z"^^xsd:dateTime;
  skos:broader :c_da75b83b;
  skos:inScheme :conceptScheme_751925ed;
  skos:prefLabel "rail engineer"@en;
  skosxl:prefLabel :xl_en_8a7654a7 .

:c_ed7dd1f7 a skos:Concept;
  dct:created "2018-04-21T14:52:02.840Z"^^xsd:dateTime;
  dct:modified "2018-07-21T15:55:08.438Z"^^xsd:dateTime;
  skos:broader :c_da75b83b;
  skos:inScheme :conceptScheme_751925ed;
  skos:notation "highway"@en;
  skos:prefLabel "highways consultant"@en;
  skosxl:prefLabel :xl_en_253e3cb2 .

:c_fcea3a25 a skos:Concept;
  dct:created "2018-04-21T14:52:31.107Z"^^xsd:dateTime;
  skos:broader :c_da75b83b;
  skos:inScheme :conceptScheme_751925ed;
  skos:prefLabel "traffic appraisal, modelling and economics (TAME) consultant"@en;
  skosxl:prefLabel :xl_en_3d64890d .

:xl_en_f1e3fb75 a skosxl:Label;
  skosxl:literalForm "transport roles"@en .

:xl_en_52df7f0e a skosxl:Label;
  skosxl:literalForm "concept layout"@en .

:c_dc99fe05 dct:created "2018-04-07T19:42:55.911Z"^^xsd:dateTime .

:xl_en_81fc9b34 a skosxl:Label;
  dct:modified "2018-07-22T07:10:18.149Z"^^xsd:dateTime;
  skosxl:literalForm "geographical and land surveyor"@en .

:xl_en_f6592c32 a skosxl:Label;
  skosxl:literalForm "health and safety consultant"@en .

:xl_en_8a7654a7 a skosxl:Label;
  skosxl:literalForm "rail engineer"@en .

:xl_en_a3c9f952 a skosxl:Label;
  dct:modified "2018-05-12T22:11:11.471Z"^^xsd:dateTime;
  skosxl:literalForm "bs 1192-1 2007 + a2:2016 collaborative production"@en .

:c_e0edea38 a skos:Concept;
  dct:created "2018-03-28T15:46:56.619Z"^^xsd:dateTime;
  dct:modified "2018-07-20T19:47:21.389Z"^^xsd:dateTime;
  skos:broader :c_a314e31f;
  skos:hiddenLabel """2.1.3
"""@en;
  skos:inScheme :conceptScheme_751925ed;
  skos:prefLabel "Select Plan"@en;
  skosxl:hiddenLabel :xl_en_6cb57c20;
  skosxl:prefLabel :xl_en_af2c11a0 .

:xl_en_6cb57c20 a skosxl:Label;
  skosxl:literalForm """2.1.3
"""@en .

:xl_en_af2c11a0 a skosxl:Label;
  skosxl:literalForm "Select Plan"@en .

:c_e162c613 dct:created "2018-05-26T11:01:47.267Z"^^xsd:dateTime .

:xl_en_be1fad1a a skosxl:Label;
  skosxl:literalForm "landscape architect"@en .

:xl_en_e7f12805 a skosxl:Label;
  skosxl:literalForm "brief"@en .

:xl_en_ac6bbf19 a skosxl:Label;
  dct:modified "2018-07-22T07:17:22.900Z"^^xsd:dateTime;
  skosxl:literalForm "mechanical engineer"@en .

:xl_en_111e4da6 a skosxl:Label;
  dct:modified "2018-05-12T21:37:08.540Z"^^xsd:dateTime;
  skosxl:literalForm "developed design"@en .

:xl_en_481dc285 a skosxl:Label;
  skosxl:literalForm "lighting designer"@en .

:c_e8b12fa7 a skos:Concept;
  dct:created "2018-04-21T14:27:38.374Z"^^xsd:dateTime;
  skos:broader :c_fbcae061;
  skos:inScheme :conceptScheme_751925ed;
  skos:prefLabel "chief financial officer"@en;
  skosxl:prefLabel :xl_en_abdc466a .

:xl_en_abdc466a a skosxl:Label;
  skosxl:literalForm "chief financial officer"@en .

:c_e9100418 a skos:Concept;
  dct:created "2018-04-21T14:28:19.986Z"^^xsd:dateTime;
  skos:broader :c_fbcae061;
  skos:inScheme :conceptScheme_751925ed;
  skos:prefLabel "manager"@en;
  skosxl:prefLabel :xl_en_8a9538bc .

:xl_en_8a9538bc a skosxl:Label;
  skosxl:literalForm "manager"@en .

:xl_en_6a8a0f84 a skosxl:Label;
  skosxl:literalForm "employer"@en .

:xl_en_c5d7135d a skosxl:Label;
  skosxl:literalForm "construction operative"@en .

:c_e9b3a976 a skos:Concept;
  dct:created "2018-04-21T14:29:23.490Z"^^xsd:dateTime;
  skos:broader :c_fbcae061;
  skos:inScheme :conceptScheme_751925ed;
  skos:prefLabel "vice president"@en;
  skosxl:prefLabel :xl_en_677f42fb .

:xl_en_677f42fb a skosxl:Label;
  skosxl:literalForm "vice president"@en .

:xl_en_9f2328c7 a skosxl:Label;
  skosxl:literalForm "ecologist"@en .

:xl_en_253e3cb2 a skosxl:Label;
  skosxl:literalForm "highways consultant"@en .

:xl_en_638d7b83 a skosxl:Label;
  dct:modified "2018-07-22T07:06:52.770Z"^^xsd:dateTime;
  skosxl:literalForm "facilities engineer"@en .

:xl_en_5728ead4 a skosxl:Label;
  dct:modified "2018-06-02T00:23:04.344Z"^^xsd:dateTime;
  skosxl:literalForm "knowledge, information and data"@en .

:xl_en_e4f4a022 a skosxl:Label;
  skosxl:literalForm "master-planning consultant"@en .

:c_fa6f2225 a skos:Concept;
  dct:created "2018-04-21T14:27:16.893Z"^^xsd:dateTime;
  skos:broader :c_fbcae061;
  skos:inScheme :conceptScheme_751925ed;
  skos:prefLabel "chairman"@en;
  skosxl:prefLabel :xl_en_b07bb222 .

:xl_en_b07bb222 a skosxl:Label;
  skosxl:literalForm "chairman"@en .

:xl_en_eb6c78c3 a skosxl:Label;
  skosxl:literalForm "building information modeling"@en .

:xl_en_b1cb3ed5 a skosxl:Label;
  skosxl:literalForm "environmental assessor"@en .

:c_fc8d6da5 a skos:Concept;
  dct:created "2018-04-21T14:27:47.797Z"^^xsd:dateTime;
  skos:broader :c_fbcae061;
  skos:inScheme :conceptScheme_751925ed;
  skos:prefLabel "chief operating officer"@en;
  skosxl:prefLabel :xl_en_4a6a0b46 .

:xl_en_610d53f7 a skosxl:Label;
  skosxl:literalForm "organization roles"@en .

:xl_en_4a6a0b46 a skosxl:Label;
  skosxl:literalForm "chief operating officer"@en .

:xl_en_24c31b75 a skosxl:Label;
  skosxl:literalForm "catering consultant"@en .

:xl_en_3d64890d a skosxl:Label;
  skosxl:literalForm "traffic appraisal, modelling and economics (TAME) consultant"@en .

:xl_en_8f54ec97 a skosxl:Label;
  dct:modified "2018-07-20T22:06:41.669Z"^^xsd:dateTime;
  skosxl:literalForm "project implementation plan"@en .


:skosCollection_4ff8449c dct:created "2018-04-07T20:06:25.388Z"^^xsd:dateTime .

:skosCollection_c85ed09f dct:created "2018-03-28T14:43:50.385Z"^^xsd:dateTime .


:xl_en_d34f5762 dct:modified "2018-06-01T23:31:11.865Z"^^xsd:dateTime;
  skosxl:literalForm "P"@en .

:c_52608161 a skos:Concept;
  dc:source "zero carbon hub appendices - closing the gap between design and as-built performance - evidence review report appendices";
  dct:created "2018-07-10T20:25:25.047Z"^^xsd:dateTime;
  dct:modified "2020-10-31T05:34:30.592Z"^^xsd:dateTime;
  olo:index "5.1"^^xsd:positiveInteger;
  skos:broader :c_91ece774;
  skos:inScheme :conceptScheme_751925ed;
  skos:notation "51";
  skosxl:prefLabel :xl_en_83260c5d .

:xl_en_83260c5d a skosxl:Label;
  skosxl:literalForm "oversite"@en .

:c_b470c6f5 a skos:Concept;
  dct:created "2018-07-10T20:39:21.525Z"^^xsd:dateTime;
  skos:broader :c_c76077ab;
  skos:inScheme :conceptScheme_751925ed;
  skos:notation "FND"@en;
  skos:prefLabel "foundation"@en;
  skosxl:prefLabel :xl_en_b07b3938 .

:xl_en_b07b3938 a skosxl:Label;
  skosxl:literalForm "foundation"@en .

:skosCollection_059e795f a skos:Collection;
  dc:source "Managing health and safety in construction Construction (Design and Management) Regulations 2015";
  dct:created "2018-07-10T20:30:48.194Z"^^xsd:dateTime;
  dct:modified "2019-11-30T10:52:21.514Z"^^xsd:dateTime;
  skos:definition "The health and safety file is defined as a file appropriate to the characteristics of the project, containing relevant health and safety information to be taken into account during any subsequent project. The file is only required for projects involving more than one contractor.";
  skos:member :skosCollection_1f48022e, :skosCollection_4d3f42cb, :skosCollection_77325868,
    :skosCollection_b565257c, :skosCollection_dca655b9;
  skosxl:prefLabel :xl_en_9e4d8faa .

:xl_en_9e4d8faa a skosxl:Label;
  skosxl:literalForm "contents of health and safety file (housing)"@en .

:skosCollection_f8d24590 a skos:Collection;
  dct:created "2018-07-20T18:20:26.828Z"^^xsd:dateTime;
  rdfs:label "fire safety"@en;
  skosxl:prefLabel :xl_en_0b1ccf6d .

:xl_en_0b1ccf6d a skosxl:Label;
  skosxl:literalForm "fire safety"@en .

:c_01bda236 a skos:Concept;
  dct:created "2018-07-21T13:21:56.402Z"^^xsd:dateTime;
  dct:modified "2020-10-31T05:00:41.149Z"^^xsd:dateTime;
  skos:broader :c_2664d806;
  skos:inScheme :conceptScheme_751925ed;
  skos:notation "LA"@en;
  skosxl:prefLabel :xl_en_f2787772 .

:xl_en_f2787772 a skosxl:Label;
  skosxl:literalForm "local authority"@en .

:c_02f182a2 a skos:Concept;
  dc:source "Interim Advice Note 184/16 Highways England CAD and Data Standard"@en;
  dct:created "2018-08-11T13:06:19.239Z"^^xsd:dateTime;
  dct:modified "2020-10-31T05:14:52.204Z"^^xsd:dateTime;
  skos:broader :c_46f0d5a6;
  skos:inScheme :conceptScheme_751925ed;
  skos:notation "SGT"@en;
  skosxl:prefLabel :xl_en_89c67217 .

:c_46f0d5a6 a skos:Concept;
  dc:source "Interim Advice Note 184/16 Highways England CAD and Data Standard"@en;
  dct:created "2018-08-11T12:53:36.125Z"^^xsd:dateTime;
  dct:modified "2020-10-31T05:02:48.913Z"^^xsd:dateTime;
  skos:broader :c_3f7d46c0;
  skos:inScheme :conceptScheme_751925ed;
  skos:narrower :c_02f182a2, :c_0b45b235, :c_1b065c63, :c_412f9c62, :c_6c31e8f5, :c_6ceaacc1,
    :c_9ef52cee, :c_a02e9571, :c_b932ae7e;
  skosxl:prefLabel :xl_en_394d95a5 .

:xl_en_89c67217 a skosxl:Label;
  skosxl:literalForm "geotechnical (structures)"@en .

:c_03f66e64 a skos:Concept;
  dc:source "Interim Advice Note 184/16 Highways England CAD and Data Standard"@en;
  dct:created "2018-08-11T08:45:43.398Z"^^xsd:dateTime;
  dct:modified "2020-10-31T05:41:19.528Z"^^xsd:dateTime;
  skos:broader :c_3f7d46c0;
  skos:inScheme :conceptScheme_751925ed;
  skos:narrower :c_692f83c4, :c_7e8703b2, :c_bce20c84;
  skosxl:prefLabel :xl_en_0a2325af .

:c_3f7d46c0 a skos:Concept;
  dc:source "BS ENISO 19650-1 Organization of information about construction works — Information management using building information modelling Part 1: Concepts and principles"@en;
  dct:created "2018-08-11T08:27:21.017Z"^^xsd:dateTime;
  skos:broader :c_19203ba1;
  skos:definition "spatial, functional or system-based subdivision of an information model"@en;
  skos:inScheme :conceptScheme_751925ed;
  skos:narrower :c_03f66e64, :c_2bf70455, :c_46f0d5a6, :c_6bc1fab9, :c_9739e9be, :c_9af04a0c,
    :c_e54483d8;
  skos:prefLabel "volume"@en;
  skosxl:prefLabel :xl_en_55d842e3 .

:c_692f83c4 a skos:Concept;
  dc:source "Interim Advice Note 184/16 Highways England CAD and Data Standard"@en;
  dct:created "2018-08-11T12:38:14.873Z"^^xsd:dateTime;
  dct:modified "2020-10-31T05:11:09.353Z"^^xsd:dateTime;
  skos:broader :c_03f66e64;
  skos:inScheme :conceptScheme_751925ed;
  skos:notation "HGN"@en;
  skosxl:prefLabel :xl_en_777f97b2 .

:c_7e8703b2 a skos:Concept;
  dc:source "Interim Advice Note 184/16 Highways England CAD and Data Standard"@en;
  dct:created "2018-08-11T09:12:49.966Z"^^xsd:dateTime;
  dct:modified "2020-10-31T05:38:45.233Z"^^xsd:dateTime;
  skos:broader :c_03f66e64;
  skos:inScheme :conceptScheme_751925ed;
  skos:notation "GHS"@en;
  skosxl:prefLabel :xl_en_b077dd14 .

:c_bce20c84 a skos:Concept;
  dc:source "Interim Advice Note 184/16 Highways England CAD and Data Standard"@en;
  dct:created "2018-08-11T08:47:03.861Z"^^xsd:dateTime;
  dct:modified "2020-10-31T05:28:02.327Z"^^xsd:dateTime;
  skos:broader :c_03f66e64;
  skos:inScheme :conceptScheme_751925ed;
  skos:notation "GEN"@en;
  skosxl:prefLabel :xl_en_f7217563 .

:xl_en_0a2325af a skosxl:Label;
  dct:modified "2018-08-11T12:59:35.527Z"^^xsd:dateTime;
  skosxl:literalForm "general"@en .

:c_04a3b08d a skos:Concept;
  dc:source "Interim Advice Note 184/16 Highways England CAD and Data Standard"@en;
  dct:created "2018-08-11T12:46:49.816Z"^^xsd:dateTime;
  dct:modified "2020-10-31T05:18:51.227Z"^^xsd:dateTime;
  skos:broader :c_2bf70455;
  skos:inScheme :conceptScheme_751925ed;
  skos:notation "HRR"@en;
  skosxl:prefLabel :xl_en_25ebd53f .

:c_2bf70455 a skos:Concept;
  dc:source "Interim Advice Note 184/16 Highways England CAD and Data Standard"@en;
  dct:created "2018-08-11T09:15:56.999Z"^^xsd:dateTime;
  dct:modified "2020-10-30T20:24:39.483Z"^^xsd:dateTime;
  skos:broader :c_3f7d46c0;
  skos:inScheme :conceptScheme_751925ed;
  skos:narrower :c_04a3b08d, :c_14426eb2, :c_250f029d, :c_2ce0c940, :c_34b987d4, :c_3fd4eac3,
    :c_59dcd59c, :c_5e5901cb, :c_6cd2fa76, :c_71eda773, :c_76b17e4d, :c_7f9323cb, :c_80aeab06,
    :c_9e61f9a1, :c_a1cd3dcb, :c_ade56523;
  skosxl:prefLabel :xl_en_0c8b3250 .

:xl_en_25ebd53f a skosxl:Label;
  skosxl:literalForm "road restraint system (vehicle and pedestrian)"@en .

:c_086e071c a skos:Concept;
  dc:source "Interim Advice Note 184/16 Highways England CAD and Data Standard"@en;
  dct:created "2018-08-11T14:27:32.696Z"^^xsd:dateTime;
  dct:modified "2020-10-31T05:07:19.240Z"^^xsd:dateTime;
  skos:broader :c_6bc1fab9;
  skos:inScheme :conceptScheme_751925ed;
  skos:notation "VAB"@en;
  skosxl:prefLabel :xl_en_819a5c2a .

:c_6bc1fab9 a skos:Concept;
  dc:source "Interim Advice Note 184/16 Highways England CAD and Data Standard"@en;
  dct:created "2018-08-11T14:26:40.474Z"^^xsd:dateTime;
  dct:modified "2020-10-31T04:44:55.140Z"^^xsd:dateTime;
  skos:broader :c_3f7d46c0;
  skos:inScheme :conceptScheme_751925ed;
  skos:narrower :c_086e071c, :c_13d79d5e, :c_1e1d6eeb, :c_36ce18a2, :c_4a7bbbda, :c_5d8254a8,
    :c_adba6615, :c_b227f284, :c_b65fa6fd, :c_d8e2bacb, :c_d9ed5f11, :c_ed146474, :c_f443f164;
  skosxl:prefLabel :xl_en_a3532349 .

:xl_en_819a5c2a a skosxl:Label;
  skosxl:literalForm "asbestos survey"@en .

:c_08fa2f6e a skos:Concept;
  dc:source """production information a code of procedure for the construction industry
Organization of information about construction works — Information management using building information modelling - Part 2:Delivery phase of assets"""@en;
  dct:created "2018-07-22T14:37:46.078Z"^^xsd:dateTime;
  dct:modified "2020-10-31T04:45:12.563Z"^^xsd:dateTime;
  skos:broader :c_e5b1b611;
  skos:inScheme :conceptScheme_751925ed;
  skos:notation "M1"@en;
  skosxl:prefLabel :xl_en_8a9dc80b .

:c_e5b1b611 a skos:Concept;
  dct:created "2018-07-22T14:24:54.897Z"^^xsd:dateTime;
  dct:modified "2020-10-31T05:21:25.403Z"^^xsd:dateTime;
  skos:broader :c_19203ba1;
  skos:inScheme :conceptScheme_751925ed;
  skos:narrower :c_08fa2f6e, :c_2b89905f, :c_2d69d738, :c_443bf05e, :c_55b465e8, :c_5cd4aa00,
    :c_5f10d43b, :c_607b5b8a, :c_79de880f, :c_87804062, :c_87bf8d98, :c_930416d1, :c_b019c6a7,
    :c_c0f70902, :c_cf6c5d63, :c_da247d5e, :c_e4e408ec, :c_ede99420, :c_fa052d43, :c_fb2c64cc;
  skosxl:prefLabel :xl_en_763d939a .

:xl_en_8a9dc80b a skosxl:Label;
  skosxl:literalForm "mezzanine above level 01"@en .

:c_0a40b44e a skos:Concept;
  dc:source """production information a code of procedure for the construction industry
Organization of information about construction works — Information management using building information modelling - Part 2:Delivery phase of assets"""@en;
  dct:created "2018-07-22T13:34:12.629Z"^^xsd:dateTime;
  dct:modified "2020-10-31T05:18:16.501Z"^^xsd:dateTime;
  skos:broader :c_618864b7;
  skos:editorialNote "Used by Commercial only"@en;
  skos:inScheme :conceptScheme_751925ed;
  skos:notation "BQ"@en;
  skosxl:prefLabel :xl_en_6e1e73f0 .

:c_618864b7 a skos:Concept;
  dct:created "2018-07-22T11:14:59.756Z"^^xsd:dateTime;
  dct:modified "2020-10-31T05:36:48.995Z"^^xsd:dateTime;
  skos:broader :c_19203ba1;
  skos:inScheme :conceptScheme_751925ed;
  skos:narrower :c_05a3b5d1, :c_0a40b44e, :c_0d978f6c, :c_1081a7c2, :c_1e5f46db, :c_1f84f905,
    :c_2238ee39, :c_240f4112, :c_2592b8ec, :c_2a6e874e, :c_2cb0f320, :c_35bd7cc0, :c_3c21373f,
    :c_41bc9708, :c_4fb142b4, :c_536a60e1, :c_5ac38c99, :c_5d17180d, :c_68039062, :c_701139f9,
    :c_8046ed58, :c_8d5846c3, :c_9328238a, :c_9832f0b7, :c_98522fb2, :c_98ba4c18, :c_9b0e72da,
    :c_9e9aa534, :c_9ebfa246, :c_a47e6a9b, :c_a7289a25, :c_abd6f00f, :c_b3508a0f, :c_b707f1ea,
    :c_c989802e, :c_d0784080, :c_d37e6d79, :c_d6230a5f, :c_d71b62e2, :c_db373352, :c_e2fbc29a,
    :c_e8a3f333, :c_e8d35302, :c_ecc8ec55, :c_ef4fcc0c, :c_ef814787, :c_fcfbbcd0;
  skosxl:prefLabel :xl_en_3aeb39fa .

:xl_en_6e1e73f0 a skosxl:Label;
  skosxl:literalForm "bill of quantities"@en .

:c_0b45b235 a skos:Concept;
  dc:source "Interim Advice Note 184/16 Highways England CAD and Data Standard"@en;
  dct:created "2018-08-11T13:12:58.470Z"^^xsd:dateTime;
  dct:modified "2020-10-31T05:20:36.984Z"^^xsd:dateTime;
  skos:broader :c_46f0d5a6;
  skos:inScheme :conceptScheme_751925ed;
  skos:notation "SRW"@en;
  skosxl:prefLabel :xl_en_19b880d8 .

:xl_en_19b880d8 a skosxl:Label;
  skosxl:literalForm "retaining walls"@en .

:c_0d978f6c a skos:Concept;
  dc:source """production information a code of procedure for the construction industry
Organization of information about construction works — Information management using building information modelling - Part 2:Delivery phase of assets"""@en;
  dct:created "2018-07-22T13:59:01.668Z"^^xsd:dateTime;
  dct:modified "2020-10-30T20:45:29.044Z"^^xsd:dateTime;
  skos:broader :c_618864b7;
  skos:inScheme :conceptScheme_751925ed;
  skos:notation "RI"@en;
  skosxl:prefLabel :xl_en_14367ebb .

:xl_en_14367ebb a skosxl:Label;
  skosxl:literalForm "request for information"@en .

:c_0fc93a91 a skos:Concept;
  dc:source "Interim Advice Note 184/16 Highways England CAD and Data Standard"@en;
  dct:created "2018-08-11T14:55:57.866Z"^^xsd:dateTime;
  dct:modified "2020-10-31T05:12:12.878Z"^^xsd:dateTime;
  skos:broader :c_9739e9be;
  skos:inScheme :conceptScheme_751925ed;
  skos:notation "LLO"@en;
  skosxl:prefLabel :xl_en_2c9dd2e8 .

:c_9739e9be a skos:Concept;
  dc:source "Interim Advice Note 184/16 Highways England CAD and Data Standard"@en;
  dct:created "2018-08-11T14:52:20.961Z"^^xsd:dateTime;
  skos:broader :c_3f7d46c0;
  skos:inScheme :conceptScheme_751925ed;
  skos:narrower :c_0fc93a91, :c_3c5e3daa;
  skos:prefLabel "legal"@en;
  skosxl:prefLabel :xl_en_9381849e .

:xl_en_2c9dd2e8 a skosxl:Label;
  skosxl:literalForm "land ownership boundaries"@en .

:c_10975b72 a skos:Concept;
  dc:source "Building a Safer Future – Independent Review of Building Regulations and Fire Safety: Final Report"@en;
  dct:created "2018-07-28T16:39:24.186Z"^^xsd:dateTime;
  dct:modified "2020-10-30T20:23:17.307Z"^^xsd:dateTime;
  skos:broader :c_43a1e1f6;
  skos:definition "This is the key stages in the building life-cycle of which the dutyholder has to satisfy the Joint Competent Authority (JCA) that their plans are robust; that their understanding and management of risk is appropriately detailed; and that they can properly account for the safety of the as-built building"@en;
  skos:inScheme :conceptScheme_751925ed;
  skosxl:prefLabel :xl_en_755e2568 .

:xl_en_755e2568 a skosxl:Label;
  skosxl:literalForm "gateway points"@en .

:c_11f27c78 a skos:Concept;
  dct:created "2018-07-21T13:19:33.611Z"^^xsd:dateTime;
  dct:modified "2020-10-31T04:56:06.240Z"^^xsd:dateTime;
  skos:broader :c_2664d806;
  skos:inScheme :conceptScheme_751925ed;
  skos:notation "MA"@en;
  skosxl:prefLabel :xl_en_c2bb1ae6 .

:xl_en_c2bb1ae6 a skosxl:Label;
  dct:modified "2018-07-22T07:42:30.249Z"^^xsd:dateTime;
  skosxl:literalForm "managing agent"@en .

:c_129a5ec6 a skos:Concept;
  dc:source "zero carbon hub appendices - closing the gap between design and as-built performance - evidence review report appendices";
  dct:created "2018-07-20T20:57:46.487Z"^^xsd:dateTime;
  dct:modified "2020-10-31T05:17:10.795Z"^^xsd:dateTime;
  olo:index "5.6"^^xsd:positiveInteger;
  skos:broader :c_91ece774;
  skos:inScheme :conceptScheme_751925ed;
  skos:notation "56";
  skosxl:prefLabel :xl_en_d31d2539 .

:xl_en_d31d2539 a skosxl:Label;
  skosxl:literalForm "second fix"@en .

:c_13d79d5e a skos:Concept;
  dc:source "Interim Advice Note 184/16 Highways England CAD and Data Standard"@en;
  dct:created "2018-08-11T14:50:31.782Z"^^xsd:dateTime;
  dct:modified "2020-10-31T05:20:02.321Z"^^xsd:dateTime;
  skos:broader :c_6bc1fab9;
  skos:inScheme :conceptScheme_751925ed;
  skos:notation "VUT"@en;
  skosxl:prefLabel :xl_en_ecd8dae6 .

:xl_en_ecd8dae6 a skosxl:Label;
  skosxl:literalForm "utilities"@en .

:c_14426eb2 a skos:Concept;
  dc:source "Interim Advice Note 184/16 Highways England CAD and Data Standard"@en;
  dct:created "2018-08-11T11:19:37.416Z"^^xsd:dateTime;
  dct:modified "2020-10-30T20:39:15.521Z"^^xsd:dateTime;
  skos:broader :c_2bf70455;
  skos:inScheme :conceptScheme_751925ed;
  skos:notation "HMC"@en;
  skosxl:prefLabel :xl_en_af9cd54a .

:xl_en_af9cd54a a skosxl:Label;
  skosxl:literalForm "motorway communications"@en .

:c_161ac3be a skos:Concept;
  dc:source "Interim Advice Note 184/16 Highways England CAD and Data Standard"@en;
  dct:created "2018-08-11T13:50:07.309Z"^^xsd:dateTime;
  dct:modified "2020-10-30T20:35:55.509Z"^^xsd:dateTime;
  skos:broader :c_e54483d8;
  skos:inScheme :conceptScheme_751925ed;
  skos:notation "EAQ"@en;
  skosxl:prefLabel :xl_en_71337efd .

:c_e54483d8 a skos:Concept;
  dc:source "Interim Advice Note 184/16 Highways England CAD and Data Standard"@en;
  dct:created "2018-08-11T13:46:50.721Z"^^xsd:dateTime;
  dct:modified "2020-10-30T20:38:19.586Z"^^xsd:dateTime;
  skos:broader :c_3f7d46c0;
  skos:inScheme :conceptScheme_751925ed;
  skos:narrower :c_161ac3be, :c_3e2995a1, :c_49cc400a, :c_73726e27, :c_75f1aa77, :c_8b778c41,
    :c_8cad0fd2, :c_90ff7ddf, :c_a9c2e902, :c_b2e826d0, :c_edf75137;
  skosxl:prefLabel :xl_en_54371a61 .

:xl_en_71337efd a skosxl:Label;
  skosxl:literalForm "air quality"@en .

:c_281f6d96 a skos:Concept;
  dct:created "2018-07-24T16:58:22.993Z"^^xsd:dateTime;
  dct:modified "2020-10-30T20:25:12.864Z"^^xsd:dateTime;
  skos:broader :c_19203ba1;
  skos:inScheme :conceptScheme_751925ed;
  skos:narrower :c_3c4ef6f5, :c_6c460406, :c_bba5abb9, :c_c4204198;
  skosxl:prefLabel :xl_en_4f2f2bdc .

:c_73619d2a a skos:Concept;
  dct:created "2018-07-24T17:33:38.007Z"^^xsd:dateTime;
  dct:modified "2020-10-30T20:25:34.965Z"^^xsd:dateTime;
  skos:broader :c_19203ba1;
  skos:inScheme :conceptScheme_751925ed;
  skos:narrower :c_fbbe4f85;
  skosxl:prefLabel :xl_en_a579548c .

:c_b7ef2137 a skos:Concept;
  dct:created "2018-07-22T11:08:11.305Z"^^xsd:dateTime;
  dct:modified "2020-10-31T05:30:23.813Z"^^xsd:dateTime;
  skos:broader :c_19203ba1;
  skos:inScheme :conceptScheme_751925ed;
  skos:narrower :c_26348e8a, :c_4dc03e66, :c_55457a29, :c_624f6410, :c_8741d02b, :c_a34bfc84,
    :c_ac25e497, :c_bfc844fa, :c_c4c44bc2, :c_e9882180, :c_f84ebdc2, :c_f897a1c6;
  skosxl:prefLabel :xl_en_43d42d70 .

:c_f29587ff a skos:Concept;
  dct:created "2018-08-11T12:03:31.265Z"^^xsd:dateTime;
  dct:modified "2020-10-31T05:07:36.862Z"^^xsd:dateTime;
  skos:broader :c_19203ba1;
  skos:inScheme :conceptScheme_751925ed;
  skos:narrower :c_32bf6806, :c_46da6c1c, :c_49888cc9, :c_6859ada6, :c_ac615319, :c_b2459321,
    :c_f23ce991, :c_f8a6d299;
  skosxl:prefLabel :xl_en_bfd696fb .

:xl_en_96c8608e a skosxl:Label;
  skosxl:literalForm "loi"@en .

:c_1b065c63 a skos:Concept;
  dc:source "Interim Advice Note 184/16 Highways England CAD and Data Standard"@en;
  dct:created "2018-08-11T13:14:30.002Z"^^xsd:dateTime;
  dct:modified "2020-10-30T20:46:42.797Z"^^xsd:dateTime;
  skos:broader :c_46f0d5a6;
  skos:inScheme :conceptScheme_751925ed;
  skos:notation "SSP"@en;
  skosxl:prefLabel :xl_en_28ec3ce6 .

:xl_en_28ec3ce6 a skosxl:Label;
  skosxl:literalForm "special structures"@en .

:c_1e1d6eeb a skos:Concept;
  dc:source "Interim Advice Note 184/16 Highways England CAD and Data Standard"@en;
  dct:created "2018-08-11T14:43:32.870Z"^^xsd:dateTime;
  skos:broader :c_6bc1fab9;
  skos:inScheme :conceptScheme_751925ed;
  skos:notation "VSM"@en;
  skos:prefLabel "structures management"@en;
  skosxl:prefLabel :xl_en_23d15909 .

:xl_en_23d15909 a skosxl:Label;
  skosxl:literalForm "structures management"@en .

:c_1e5f46db a skos:Concept;
  dc:source """production information a code of procedure for the construction industry
Organization of information about construction works — Information management using building information modelling - Part 2:Delivery phase of assets"""@en;
  dct:created "2018-07-22T14:00:29.605Z"^^xsd:dateTime;
  dct:modified "2020-10-31T05:39:05.055Z"^^xsd:dateTime;
  skos:broader :c_618864b7;
  skos:inScheme :conceptScheme_751925ed;
  skos:narrower :c_8ec4ead3;
  skos:notation "RP"@en;
  skosxl:prefLabel :xl_en_c49e318a .

:c_8ec4ead3 a skos:Concept;
  dc:source "BS ISO 6707-2-2017-Buildings and civil engineering works. Vocabulary. Contract and communication terms"@en;
  dct:created "2018-07-24T17:12:36.624Z"^^xsd:dateTime;
  dct:modified "2020-10-31T05:21:01.590Z"^^xsd:dateTime;
  skos:broader :c_1e5f46db;
  skos:inScheme :conceptScheme_751925ed;
  skosxl:prefLabel :xl_en_9e9f2102 .

:xl_en_c49e318a a skosxl:Label;
  skosxl:literalForm "report"@en .

:xl_en_2de5ebbe a skosxl:Label;
  skosxl:literalForm "sb-imp"@en .

:c_1f84f905 a skos:Concept;
  dc:source """production information a code of procedure for the construction industry
Organization of information about construction works — Information management using building information modelling - Part 2:Delivery phase of assets"""@en;
  dct:created "2018-07-22T13:41:36.384Z"^^xsd:dateTime;
  dct:modified "2020-10-31T05:27:12.559Z"^^xsd:dateTime;
  skos:broader :c_618864b7;
  skos:inScheme :conceptScheme_751925ed;
  skos:notation "FN"@en;
  skosxl:prefLabel :xl_en_b5343ca3 .

:xl_en_b5343ca3 a skosxl:Label;
  skosxl:literalForm "file note"@en .

:c_240f4112 a skos:Concept;
  dc:source """production information a code of procedure for the construction industry
Organization of information about construction works — Information management using building information modelling - Part 2:Delivery phase of assets"""@en;
  dct:created "2018-07-22T13:39:53.219Z"^^xsd:dateTime;
  dct:modified "2020-10-31T04:45:28.479Z"^^xsd:dateTime;
  skos:broader :c_618864b7;
  skos:inScheme :conceptScheme_751925ed;
  skos:notation "DB"@en;
  skosxl:prefLabel :xl_en_e9d48530 .

:xl_en_e9d48530 a skosxl:Label;
  skosxl:literalForm "database"@en .

:c_49e95986 a skos:Concept;
  dct:created "2018-07-22T07:13:30.076Z"^^xsd:dateTime;
  dct:modified "2020-10-30T20:31:43.711Z"^^xsd:dateTime;
  skos:broader :c_2425ea08;
  skos:inScheme :conceptScheme_751925ed;
  skos:notation "H"@en;
  skosxl:prefLabel :xl_en_4ae15d25 .

:c_5060b718 a skos:Concept;
  dct:created "2018-07-21T12:59:43.767Z"^^xsd:dateTime;
  dct:modified "2020-10-30T20:49:55.031Z"^^xsd:dateTime;
  skos:broader :c_2425ea08;
  skos:inScheme :conceptScheme_751925ed;
  skosxl:prefLabel :xl_en_8d330048 .

:c_24506d00 a skos:Concept;
  dc:source "production information a code of procedure for the construction industry"@en;
  dct:created "2018-07-22T15:34:57.481Z"^^xsd:dateTime;
  dct:modified "2020-10-31T05:19:30.439Z"^^xsd:dateTime;
  skos:broader :c_c76077ab;
  skos:inScheme :conceptScheme_751925ed;
  skosxl:prefLabel :xl_en_c6289ef2 .

:xl_en_c6289ef2 a skosxl:Label;
  skosxl:literalForm "services electrical"@en .

:c_250f029d a skos:Concept;
  dc:source "Interim Advice Note 184/16 Highways England CAD and Data Standard"@en;
  dct:created "2018-08-11T09:35:23.053Z"^^xsd:dateTime;
  dct:modified "2020-10-31T05:05:25.149Z"^^xsd:dateTime;
  skos:broader :c_2bf70455;
  skos:inScheme :conceptScheme_751925ed;
  skos:notation "HDG"@en;
  skosxl:prefLabel :xl_en_9725b761 .

:xl_en_9725b761 a skosxl:Label;
  skosxl:literalForm "drainage"@en .

:c_26348e8a a skos:Concept;
  dc:source "organization of information about construction works — information management using building information modelling - part 2: delivery phase of assets"@en;
  dct:created "2018-07-22T11:21:27.626Z"^^xsd:dateTime;
  dct:modified "2020-10-31T04:48:52.378Z"^^xsd:dateTime;
  rdfs:isDefinedBy :c_263f8b4d;
  skos:broader :c_b7ef2137;
  skos:inScheme :conceptScheme_751925ed;
  skos:notation "VS"@en;
  skosxl:prefLabel :xl_en_e6349ebd .

:c_263f8b4d a skos:Concept;
  dct:created "2018-07-22T11:34:27.411Z"^^xsd:dateTime;
  skos:broader :c_aca16e26;
  skos:inScheme :conceptScheme_751925ed;
  skosxl:prefLabel :xl_en_57dad9d7 .

:xl_en_e6349ebd a skosxl:Label;
  skosxl:literalForm "visualization"@en .

:xl_en_57dad9d7 a skosxl:Label;
  dct:modified "2018-07-22T11:35:22.260Z"^^xsd:dateTime;
  skosxl:literalForm "ISO-DIS 19650-2 organization of information about construction works — information management using building information modelling - part 2: delivery phase of assets"@en .

:c_46f20ab0 a skos:Concept;
  dct:created "2018-07-22T07:28:51.447Z"^^xsd:dateTime;
  dct:modified "2020-10-31T05:13:34.767Z"^^xsd:dateTime;
  skos:broader :c_2664d806;
  skos:inScheme :conceptScheme_751925ed;
  skos:notation "Z"@en;
  skosxl:prefLabel :xl_en_596e8563 .

:c_9509873f a skos:Concept;
  dc:source "Building a Safer Future – Independent Review of Building Regulations and Fire Safety: Final Report"@en;
  dct:created "2018-07-28T16:23:29.008Z"^^xsd:dateTime;
  dct:modified "2020-10-31T05:39:19.526Z"^^xsd:dateTime;
  skos:broader :c_2664d806;
  skos:definition """Local Authority Building Control In this report local authority building control services are referred to as Local Authority Building Control – each local authority remains individually responsible for the delivery of building control services in its area"""@en;
  skos:inScheme :conceptScheme_751925ed;
  skos:notation "LABC"@en;
  skosxl:prefLabel :xl_en_38527472 .

:c_277602e6 dct:created "2018-08-11T09:08:09.653Z"^^xsd:dateTime .

:c_3c4ef6f5 a skos:Concept;
  dc:source "production information a code of procedure for the construction industry"@en;
  dct:created "2018-07-22T15:30:59.791Z"^^xsd:dateTime;
  dct:modified "2020-10-31T05:34:49.214Z"^^xsd:dateTime;
  skos:broader :c_281f6d96;
  skos:inScheme :conceptScheme_751925ed;
  skosxl:prefLabel :xl_en_23933c65 .

:c_6c460406 a skos:Concept;
  dc:source "production information a code of procedure for the construction industry"@en;
  dct:created "2018-07-22T15:32:46.072Z"^^xsd:dateTime;
  skos:broader :c_281f6d96;
  skos:inScheme :conceptScheme_751925ed;
  skos:prefLabel "services piped and ducted"@en;
  skosxl:prefLabel :xl_en_3380ad87 .

:c_c4204198 a skos:Concept;
  dc:source "production information a code of procedure for the construction industry"@en;
  dct:created "2018-07-22T15:40:17.272Z"^^xsd:dateTime;
  dct:modified "2020-10-30T20:57:37.673Z"^^xsd:dateTime;
  skos:broader :c_281f6d96;
  skos:inScheme :conceptScheme_751925ed;
  skosxl:prefLabel :xl_en_813a8fc3 .

:xl_en_4f2f2bdc a skosxl:Label;
  dct:modified "2018-08-11T12:20:36.234Z"^^xsd:dateTime;
  skosxl:literalForm "drawings civil (housing)"@en .

:xl_en_0049082b a skosxl:Label;
  skosxl:literalForm "bass"@en .

:c_d5bcf8c5 a skos:Concept;
  dc:source "BS ISO 6707-2-2017-Buildings and civil engineering works. Vocabulary. Contract and communication terms"@en;
  dct:created "2018-07-24T16:55:47.612Z"^^xsd:dateTime;
  dct:modified "2020-10-31T08:44:54.231Z"^^xsd:dateTime;
  skos:broader :c_261a288e;
  skos:definition "collection of information models that express knowledge about kinds of things (concepts) and that are stored and retrieved as electronic information"@en;
  skos:inScheme :conceptScheme_751925ed;
  skosxl:prefLabel :xl_en_043a03d3 .

:xl_en_3c41ea90 a skosxl:Label;
  skosxl:literalForm "lod"@en .

:c_2a6e874e a skos:Concept;
  dc:source """production information a code of procedure for the construction industry
Organization of information about construction works — Information management using building information modelling - Part 2:Delivery phase of assets"""@en;
  dct:created "2018-07-22T13:52:43.779Z"^^xsd:dateTime;
  dct:modified "2020-10-31T05:41:34.674Z"^^xsd:dateTime;
  skos:broader :c_618864b7;
  skos:inScheme :conceptScheme_751925ed;
  skos:notation "MS"@en;
  skosxl:prefLabel :xl_en_5b26d4a3 .

:xl_en_5b26d4a3 a skosxl:Label;
  skosxl:literalForm "method statement"@en .

:xl_en_42f4c7a1 a skosxl:Label;
  skosxl:literalForm "air"@en .

:c_2ce0c940 a skos:Concept;
  dc:source "Interim Advice Note 184/16 Highways England CAD and Data Standard"@en;
  dct:created "2018-08-11T11:16:40.686Z"^^xsd:dateTime;
  skos:broader :c_2bf70455;
  skos:inScheme :conceptScheme_751925ed;
  skos:notation "HKF"@en;
  skos:prefLabel "kerbs, footways and paved areas"@en;
  skosxl:prefLabel :xl_en_abe554b5 .

:c_34b987d4 a skos:Concept;
  dc:source "Interim Advice Note 184/16 Highways England CAD and Data Standard"@en;
  dct:created "2018-08-11T11:28:23.797Z"^^xsd:dateTime;
  dct:modified "2020-10-31T05:15:10.939Z"^^xsd:dateTime;
  skos:broader :c_2bf70455;
  skos:inScheme :conceptScheme_751925ed;
  skos:notation "HPV"@en;
  skosxl:prefLabel :xl_en_4b48058c .

:c_3fd4eac3 a skos:Concept;
  dc:source "Interim Advice Note 184/16 Highways England CAD and Data Standard"@en;
  dct:created "2018-08-11T11:18:11.372Z"^^xsd:dateTime;
  dct:modified "2020-10-31T05:00:18.839Z"^^xsd:dateTime;
  skos:broader :c_2bf70455;
  skos:inScheme :conceptScheme_751925ed;
  skos:notation "HLG"@en;
  skosxl:prefLabel :xl_en_850232a1 .

:c_59dcd59c a skos:Concept;
  dc:source "Interim Advice Note 184/16 Highways England CAD and Data Standard"@en;
  dct:created "2018-08-11T09:29:41.478Z"^^xsd:dateTime;
  dct:modified "2020-10-31T05:16:16.784Z"^^xsd:dateTime;
  skos:broader :c_2bf70455;
  skos:inScheme :conceptScheme_751925ed;
  skos:notation "HAC"@en;
  skosxl:prefLabel :xl_en_3c0a3e73 .

:c_5e5901cb a skos:Concept;
  dc:source "Interim Advice Note 184/16 Highways England CAD and Data Standard"@en;
  dct:created "2018-08-11T12:50:15.363Z"^^xsd:dateTime;
  skos:broader :c_2bf70455;
  skos:inScheme :conceptScheme_751925ed;
  skos:notation "HSN"@en;
  skos:prefLabel "traffic signs"@en;
  skosxl:prefLabel :xl_en_98e4302d .

:c_6cd2fa76 a skos:Concept;
  dc:source "Interim Advice Note 184/16 Highways England CAD and Data Standard"@en;
  dct:created "2018-08-11T10:01:07.959Z"^^xsd:dateTime;
  dct:modified "2020-10-30T20:36:12.680Z"^^xsd:dateTime;
  skos:broader :c_2bf70455;
  skos:inScheme :conceptScheme_751925ed;
  skos:notation "HEL"@en;
  skosxl:prefLabel :xl_en_a74e7a5b .

:c_71eda773 a skos:Concept;
  dc:source "Interim Advice Note 184/16 Highways England CAD and Data Standard"@en;
  dct:created "2018-08-11T10:03:17.064Z"^^xsd:dateTime;
  dct:modified "2020-10-31T05:11:40.060Z"^^xsd:dateTime;
  skos:broader :c_2bf70455;
  skos:inScheme :conceptScheme_751925ed;
  skos:notation "HFE"@en;
  skosxl:prefLabel :xl_en_4e277135 .

:c_76b17e4d a skos:Concept;
  dc:source "Interim Advice Note 184/16 Highways England CAD and Data Standard"@en;
  dct:created "2018-08-11T12:48:41.516Z"^^xsd:dateTime;
  dct:modified "2020-10-30T20:58:34.349Z"^^xsd:dateTime;
  skos:broader :c_2bf70455;
  skos:inScheme :conceptScheme_751925ed;
  skos:notation "HSC"@en;
  skosxl:prefLabel :xl_en_fd157b83 .

:c_7f9323cb a skos:Concept;
  dc:source "Interim Advice Note 184/16 Highways England CAD and Data Standard"@en;
  dct:created "2018-08-11T11:26:40.993Z"^^xsd:dateTime;
  dct:modified "2020-10-31T05:23:04.860Z"^^xsd:dateTime;
  skos:broader :c_2bf70455;
  skos:inScheme :conceptScheme_751925ed;
  skos:notation "HML"@en;
  skosxl:prefLabel :xl_en_ad12bf3f .

:c_80aeab06 a skos:Concept;
  dc:source "Interim Advice Note 184/16 Highways England CAD and Data Standard"@en;
  dct:created "2018-08-11T12:51:50.473Z"^^xsd:dateTime;
  dct:modified "2020-10-31T04:45:44.286Z"^^xsd:dateTime;
  skos:broader :c_2bf70455;
  skos:inScheme :conceptScheme_751925ed;
  skos:notation "HSR"@en;
  skosxl:prefLabel :xl_en_f642504c .

:c_9e61f9a1 a skos:Concept;
  dc:source "Interim Advice Note 184/16 Highways England CAD and Data Standard"@en;
  dct:created "2018-08-11T11:20:58.489Z"^^xsd:dateTime;
  dct:modified "2020-10-30T20:35:38.643Z"^^xsd:dateTime;
  skos:broader :c_2bf70455;
  skos:inScheme :conceptScheme_751925ed;
  skos:notation "HMK"@en;
  skosxl:prefLabel :xl_en_1b010294 .

:c_a1cd3dcb a skos:Concept;
  dc:source "Interim Advice Note 184/16 Highways England CAD and Data Standard"@en;
  dct:created "2018-08-11T11:12:57.728Z"^^xsd:dateTime;
  dct:modified "2020-10-31T05:06:57.932Z"^^xsd:dateTime;
  skos:broader :c_2bf70455;
  skos:inScheme :conceptScheme_751925ed;
  skos:notation "HGT"@en;
  skosxl:prefLabel :xl_en_bce41bc8 .

:c_ade56523 a skos:Concept;
  dc:source "Interim Advice Note 184/16 Highways England CAD and Data Standard"@en;
  dct:created "2018-08-11T09:33:13.625Z"^^xsd:dateTime;
  dct:modified "2020-10-31T05:11:23.433Z"^^xsd:dateTime;
  skos:broader :c_2bf70455;
  skos:inScheme :conceptScheme_751925ed;
  skos:notation "HAW"@en;
  skosxl:prefLabel :xl_en_b537b614 .

:xl_en_0c8b3250 a skosxl:Label;
  skosxl:literalForm "highways"@en .

:c_2cb0f320 a skos:Concept;
  dc:source """production information a code of procedure for the construction industry
Organization of information about construction works — Information management using building information modelling - Part 2:Delivery phase of assets"""@en;
  dct:created "2018-07-22T14:06:52.508Z"^^xsd:dateTime;
  dct:modified "2020-10-30T20:37:25.208Z"^^xsd:dateTime;
  skos:broader :c_618864b7;
  skos:inScheme :conceptScheme_751925ed;
  skos:notation "SN"@en;
  skosxl:prefLabel :xl_en_108b8fec .

:xl_en_108b8fec a skosxl:Label;
  skosxl:literalForm "snagging list"@en .

:xl_en_abe554b5 a skosxl:Label;
  skosxl:literalForm "kerbs, footways and paved areas"@en .

:c_2d69d738 a skos:Concept;
  dc:source """production information a code of procedure for the construction industry
Organization of information about construction works — Information management using building information modelling - Part 2:Delivery phase of assets"""@en;
  dct:created "2018-07-22T14:26:20.798Z"^^xsd:dateTime;
  dct:modified "2020-10-31T04:46:21.534Z"^^xsd:dateTime;
  skos:broader :c_e5b1b611;
  skos:inScheme :conceptScheme_751925ed;
  skos:notation "ZZ"@en;
  skosxl:prefLabel :xl_en_5a85847f .

:xl_en_5a85847f a skosxl:Label;
  skosxl:literalForm "multiple levels"@en .

:xl_en_f987d3fd a skosxl:Label;
  skosxl:literalForm "smp"@en .

:xl_en_511d9a71 a skosxl:Label;
  skosxl:literalForm "basmp"@en .

:c_32bf6806 a skos:Concept;
  dc:source "zero carbon hub appendices - closing the gap between design and as-built performance - appendix c";
  dct:created "2018-07-20T20:19:32.289Z"^^xsd:dateTime;
  skos:broader :c_f29587ff;
  skos:inScheme :conceptScheme_751925ed;
  skos:notation "SAP"@en;
  skos:prefLabel "standard assessment procedure worksheet: as built"@en;
  skosxl:altLabel :xl_en_310fdd79;
  skosxl:prefLabel :xl_en_ec0ff6cd .

:xl_en_310fdd79 a skosxl:Label;
  skosxl:literalForm "sap"@en .

:xl_en_ec0ff6cd a skosxl:Label;
  dct:modified "2020-10-31T05:49:47.848Z"^^xsd:dateTime .

:c_32da9577 a skos:Concept;
  dc:source "production information a code of procedure for the construction industry"@en;
  dct:created "2018-07-22T15:27:38.904Z"^^xsd:dateTime;
  skos:broader :c_c76077ab;
  skos:inScheme :conceptScheme_751925ed;
  skos:notation "RP"@en;
  skos:prefLabel "roof structure"@en;
  skosxl:prefLabel :xl_en_500aaf3e .

:xl_en_500aaf3e a skosxl:Label;
  skosxl:literalForm "roof structure"@en .

:xl_en_4b48058c a skosxl:Label;
  skosxl:literalForm "road pavements"@en .

:c_35bd7cc0 a skos:Concept;
  dc:source """production information a code of procedure for the construction industry
Organization of information about construction works — Information management using building information modelling - Part 2:Delivery phase of assets"""@en;
  dct:created "2018-07-22T13:48:03.427Z"^^xsd:dateTime;
  dct:modified "2020-10-31T05:40:26.072Z"^^xsd:dateTime;
  skos:broader :c_618864b7;
  skos:inScheme :conceptScheme_751925ed;
  skos:notation "IE"@en;
  skosxl:prefLabel :xl_en_a1e88f38 .

:xl_en_a1e88f38 a skosxl:Label;
  skosxl:literalForm "information exchange file"@en .

:c_36ce18a2 a skos:Concept;
  dc:source "Interim Advice Note 184/16 Highways England CAD and Data Standard"@en;
  dct:created "2018-08-11T14:48:44.284Z"^^xsd:dateTime;
  dct:modified "2020-10-31T05:10:52.980Z"^^xsd:dateTime;
  skos:broader :c_6bc1fab9;
  skos:inScheme :conceptScheme_751925ed;
  skos:notation "VTR"@en;
  skosxl:prefLabel :xl_en_d5ae8031 .

:xl_en_d5ae8031 a skosxl:Label;
  skosxl:literalForm "traffic survey"@en .

:c_3c21373f a skos:Concept;
  dc:source """production information a code of procedure for the construction industry
Organization of information about construction works — Information management using building information modelling - Part 2:Delivery phase of assets"""@en;
  dct:created "2018-07-22T14:01:59.303Z"^^xsd:dateTime;
  skos:broader :c_618864b7;
  skos:inScheme :conceptScheme_751925ed;
  skos:notation "SA"@en;
  skos:prefLabel "schedule of accommodation"@en;
  skosxl:prefLabel :xl_en_206a9ea8 .

:xl_en_206a9ea8 a skosxl:Label;
  skosxl:literalForm "schedule of accommodation"@en .

:xl_en_23933c65 a skosxl:Label;
  skosxl:literalForm "setting out plan"@en .

:c_3c5e3daa a skos:Concept;
  dc:source "Interim Advice Note 184/16 Highways England CAD and Data Standard"@en;
  dct:created "2018-08-11T14:53:17.584Z"^^xsd:dateTime;
  skos:broader :c_9739e9be;
  skos:inScheme :conceptScheme_751925ed;
  skos:notation "LSI"@en;
  skos:prefLabel "statutory instruments"@en;
  skosxl:prefLabel :xl_en_c7d8a973 .

:xl_en_c7d8a973 a skosxl:Label;
  skosxl:literalForm "statutory instruments"@en .

:c_3e2995a1 a skos:Concept;
  dc:source "Interim Advice Note 184/16 Highways England CAD and Data Standard"@en;
  dct:created "2018-08-11T13:56:38.825Z"^^xsd:dateTime;
  skos:broader :c_e54483d8;
  skos:inScheme :conceptScheme_751925ed;
  skos:notation "EGT"@en;
  skos:prefLabel "geology and soils"@en;
  skosxl:prefLabel :xl_en_54e1fbf9 .

:xl_en_54e1fbf9 a skosxl:Label;
  skosxl:literalForm "geology and soils"@en .

:xl_en_32357ece a skosxl:Label;
  skosxl:literalForm "eir"@en .

:xl_en_98ded33c a skosxl:Label;
  skosxl:literalForm """
employers information requirements"""@en .

:c_9af04a0c a skos:Concept;
  dc:source "Interim Advice Note 184/16 Highways England CAD and Data Standard"@en;
  dct:created "2018-08-11T14:57:47.855Z"^^xsd:dateTime;
  dct:modified "2020-10-30T20:36:31.726Z"^^xsd:dateTime;
  skos:broader :c_3f7d46c0;
  skos:inScheme :conceptScheme_751925ed;
  skos:narrower :c_ace7ce12, :c_eb6b96ad;
  skosxl:prefLabel :xl_en_06a2f565 .

:xl_en_55d842e3 a skosxl:Label;
  skosxl:literalForm "volume"@en .

:xl_en_850232a1 a skosxl:Label;
  skosxl:literalForm "road lighting"@en .

:xl_en_0a7cb84d a skosxl:Label;
  skosxl:literalForm "midp"@en .

:c_412f9c62 a skos:Concept;
  dc:source "Interim Advice Note 184/16 Highways England CAD and Data Standard"@en;
  dct:created "2018-08-11T13:09:52.000Z"^^xsd:dateTime;
  dct:modified "2020-10-31T04:47:00.018Z"^^xsd:dateTime;
  skos:broader :c_46f0d5a6;
  skos:inScheme :conceptScheme_751925ed;
  skos:notation "SMA"@en;
  skosxl:prefLabel :xl_en_58af5e0a .

:xl_en_58af5e0a a skosxl:Label;
  skosxl:literalForm "masts"@en .

:c_443bf05e a skos:Concept;
  dct:created "2018-07-22T14:46:12.820Z"^^xsd:dateTime;
  dct:modified "2020-10-30T20:38:58.269Z"^^xsd:dateTime;
  skos:broader :c_e5b1b611;
  skos:inScheme :conceptScheme_751925ed;
  skos:notation "PLT"@en;
  skosxl:prefLabel :xl_en_c4de547f .

:xl_en_c4de547f a skosxl:Label;
  skosxl:literalForm "plot"@en .

:c_447a9eee a skos:Concept;
  dc:source "zero carbon hub appendices - closing the gap between design and as-built performance - evidence review report appendices";
  dct:created "2018-07-20T20:54:28.033Z"^^xsd:dateTime;
  dct:modified "2020-10-30T20:46:08.112Z"^^xsd:dateTime;
  olo:index "5.4"^^xsd:positiveInteger;
  skos:broader :c_91ece774;
  skos:inScheme :conceptScheme_751925ed;
  skos:notation "54";
  skosxl:prefLabel :xl_en_e81acf13 .

:xl_en_e81acf13 a skosxl:Label;
  skosxl:literalForm "first fix"@en .

:c_4553c077 dct:created "2018-07-22T14:24:33.455Z"^^xsd:dateTime .

:c_46da6c1c a skos:Concept;
  dc:source "zero carbon hub appendices - closing the gap between design and as-built performance - appendix c";
  dct:created "2018-07-20T20:16:52.243Z"^^xsd:dateTime;
  dct:modified "2020-10-31T05:15:58.312Z"^^xsd:dateTime;
  skos:broader :c_f29587ff;
  skos:inScheme :conceptScheme_751925ed;
  skosxl:prefLabel :xl_en_7aade648 .

:xl_en_7aade648 a skosxl:Label;
  skosxl:literalForm "product specific plain language compliance report: as built"@en .

:c_6c31e8f5 a skos:Concept;
  dc:source "Interim Advice Note 184/16 Highways England CAD and Data Standard"@en;
  dct:created "2018-08-11T13:00:02.862Z"^^xsd:dateTime;
  dct:modified "2020-10-31T05:20:20.152Z"^^xsd:dateTime;
  skos:broader :c_46f0d5a6;
  skos:inScheme :conceptScheme_751925ed;
  skos:notation "SGN"@en;
  skosxl:prefLabel :xl_en_120eef77 .

:c_6ceaacc1 a skos:Concept;
  dc:source "Interim Advice Note 184/16 Highways England CAD and Data Standard"@en;
  dct:created "2018-08-11T13:16:18.703Z"^^xsd:dateTime;
  dct:modified "2020-10-30T20:39:46.908Z"^^xsd:dateTime;
  skos:broader :c_46f0d5a6;
  skos:inScheme :conceptScheme_751925ed;
  skos:notation "STU"@en;
  skosxl:prefLabel :xl_en_a423da25 .

:c_9ef52cee a skos:Concept;
  dc:source "Interim Advice Note 184/16 Highways England CAD and Data Standard"@en;
  dct:created "2018-08-11T12:55:44.938Z"^^xsd:dateTime;
  dct:modified "2020-10-30T20:49:38.224Z"^^xsd:dateTime;
  skos:broader :c_46f0d5a6;
  skos:inScheme :conceptScheme_751925ed;
  skos:notation "SBR"@en;
  skosxl:prefLabel :xl_en_09b0def2 .

:c_a02e9571 a skos:Concept;
  dc:source "Interim Advice Note 184/16 Highways England CAD and Data Standard"@en;
  dct:created "2018-08-11T13:11:32.620Z"^^xsd:dateTime;
  dct:modified "2020-10-31T05:30:45.951Z"^^xsd:dateTime;
  skos:broader :c_46f0d5a6;
  skos:inScheme :conceptScheme_751925ed;
  skos:notation "SMN"@en;
  skosxl:prefLabel :xl_en_2f190d8d .

:c_b932ae7e a skos:Concept;
  dc:source "Interim Advice Note 184/16 Highways England CAD and Data Standard"@en;
  dct:created "2018-08-11T13:08:07.606Z"^^xsd:dateTime;
  dct:modified "2020-10-31T05:33:51.473Z"^^xsd:dateTime;
  skos:broader :c_46f0d5a6;
  skos:inScheme :conceptScheme_751925ed;
  skos:notation "SGY"@en;
  skosxl:prefLabel :xl_en_ea6f60b0 .

:xl_en_394d95a5 a skosxl:Label;
  dct:modified "2018-08-11T12:54:14.355Z"^^xsd:dateTime;
  skosxl:literalForm "structures"@en .

:xl_en_596e8563 a skosxl:Label;
  dct:modified "2018-07-22T07:31:17.376Z"^^xsd:dateTime;
  skosxl:literalForm "general no-disciplinary"@en .

:c_49888cc9 a skos:Concept;
  dc:source "zero carbon hub appendices - closing the gap between design and as-built performance - appendix c";
  dct:created "2018-07-20T20:30:34.362Z"^^xsd:dateTime;
  dct:modified "2020-10-30T20:27:46.965Z"^^xsd:dateTime;
  skos:broader :c_f29587ff;
  skos:inScheme :conceptScheme_751925ed;
  skos:notation "CML"@en;
  skosxl:altLabel :xl_en_d1eea4cb;
  skosxl:prefLabel :xl_en_8a04c8ea .

:xl_en_d1eea4cb a skosxl:Label;
  skosxl:literalForm "cml"@en .

:xl_en_8a04c8ea a skosxl:Label;
  skosxl:literalForm "council of mortgage lenders certificate"@en .

:c_49cc400a a skos:Concept;
  dc:source "Interim Advice Note 184/16 Highways England CAD and Data Standard"@en;
  dct:created "2018-08-11T14:07:25.496Z"^^xsd:dateTime;
  skos:broader :c_e54483d8;
  skos:inScheme :conceptScheme_751925ed;
  skos:notation "EWE"@en;
  skos:prefLabel "water environment"@en;
  skosxl:prefLabel :xl_en_7316b527 .

:xl_en_7316b527 a skosxl:Label;
  skosxl:literalForm "water environment"@en .

:xl_en_4ae15d25 a skosxl:Label;
  skosxl:literalForm "heating and ventilation designer"@en .

:c_4a7bbbda a skos:Concept;
  dc:source "Interim Advice Note 184/16 Highways England CAD and Data Standard"@en;
  dct:created "2018-08-11T14:36:00.547Z"^^xsd:dateTime;
  dct:modified "2020-10-31T04:58:47.661Z"^^xsd:dateTime;
  skos:broader :c_6bc1fab9;
  skos:inScheme :conceptScheme_751925ed;
  skos:notation "VGN"@en;
  skosxl:prefLabel :xl_en_4a0407d3 .

:xl_en_4a0407d3 a skosxl:Label;
  skosxl:literalForm "survey general"@en .

:c_4d73ba7d a skos:Concept;
  dc:source "zero carbon hub appendices - closing the gap between design and as-built performance - evidence review report appendices";
  dct:created "2018-07-20T20:52:57.642Z"^^xsd:dateTime;
  dct:modified "2020-10-31T05:22:33.369Z"^^xsd:dateTime;
  olo:index "5.3"^^xsd:positiveInteger;
  skos:broader :c_91ece774;
  skos:inScheme :conceptScheme_751925ed;
  skos:notation "53";
  skosxl:prefLabel :xl_en_38ac8537 .

:xl_en_38ac8537 a skosxl:Label;
  skosxl:literalForm "roof to weathertight"@en .

:c_4dc03e66 a skos:Concept;
  dc:source "organization of information about construction works — information management using building information modelling - part 2: delivery phase of assets"@en;
  dct:created "2018-07-22T11:15:47.063Z"^^xsd:dateTime;
  dct:modified "2020-10-31T04:51:37.852Z"^^xsd:dateTime;
  rdfs:isDefinedBy :c_263f8b4d;
  skos:broader :c_b7ef2137;
  skos:inScheme :conceptScheme_751925ed;
  skos:notation "CR"@en;
  skosxl:prefLabel :xl_en_b6c7816a .

:xl_en_b6c7816a a skosxl:Label;
  skosxl:literalForm "clash rendition"@en .

:xl_en_44ca1675 a skosxl:Label;
  skosxl:literalForm "aim"@en .

:c_4fb142b4 a skos:Concept;
  dc:source """production information a code of procedure for the construction industry
Organization of information about construction works — Information management using building information modelling - Part 2:Delivery phase of assets"""@en;
  dct:created "2018-07-22T13:44:52.215Z"^^xsd:dateTime;
  dct:modified "2020-10-30T20:35:20.469Z"^^xsd:dateTime;
  skos:broader :c_618864b7;
  skos:inScheme :conceptScheme_751925ed;
  skos:notation "HS"@en;
  skosxl:prefLabel :xl_en_c744d996 .

:xl_en_c744d996 a skosxl:Label;
  dct:modified "2018-07-22T13:46:30.894Z"^^xsd:dateTime;
  skosxl:literalForm "health and safety (document type)"@en .

:xl_en_8d330048 a skosxl:Label;
  skosxl:literalForm "infrastructure engineer"@en .

:c_52aaa84e dct:created "2018-07-24T17:09:26.522Z"^^xsd:dateTime .

:c_533afc9b dct:created "2018-07-20T21:00:25.877Z"^^xsd:dateTime .

:c_f569343b a skos:Concept;
  dc:source "Building a Safer Future – Independent Review of Building Regulations and Fire Safety: Final Report"@en;
  dct:created "2018-07-28T16:32:21.066Z"^^xsd:dateTime;
  dct:modified "2020-10-31T05:42:22.193Z"^^xsd:dateTime;
  skos:broader :c_54bbebe2;
  skos:definition """building safety manager  Named individual (natural person) with the relevant skills, knowledge and expertise to be responsible for the day to day management of the building and act as a point of contact for residents on building safety"""@en;
  skos:inScheme :conceptScheme_751925ed;
  skos:notation "BSM"@en;
  skosxl:prefLabel :xl_en_b3950513 .

:c_55457a29 a skos:Concept;
  dc:source "organization of information about construction works — information management using building information modelling - part 2: delivery phase of assets"@en;
  dct:created "2018-07-22T11:08:52.319Z"^^xsd:dateTime;
  dct:modified "2020-10-30T20:45:07.982Z"^^xsd:dateTime;
  rdfs:isDefinedBy :c_263f8b4d;
  skos:broader :c_b7ef2137;
  skos:inScheme :conceptScheme_751925ed;
  skos:notation "AF"@en;
  skosxl:prefLabel :xl_en_45228085 .

:xl_en_45228085 a skosxl:Label;
  dct:modified "2018-07-22T11:11:43.239Z"^^xsd:dateTime;
  skosxl:literalForm "animation file of a model"@en .

:xl_en_3c0a3e73 a skosxl:Label;
  dct:modified "2018-08-11T09:31:59.483Z"^^xsd:dateTime;
  skosxl:literalForm "highway approvals and consents"@en .

:xl_en_cff63d0f a skosxl:Label;
  skosxl:literalForm "tidp"@en .

:c_5cd4aa00 a skos:Concept;
  dc:source """production information a code of procedure for the construction industry
Organization of information about construction works — Information management using building information modelling - Part 2:Delivery phase of assets"""@en;
  dct:created "2018-07-22T14:28:02.999Z"^^xsd:dateTime;
  dct:modified "2020-10-30T20:46:24.677Z"^^xsd:dateTime;
  skos:broader :c_e5b1b611;
  skos:inScheme :conceptScheme_751925ed;
  skos:notation "XX"@en;
  skosxl:prefLabel :xl_en_b63c3d8e .

:xl_en_b63c3d8e a skosxl:Label;
  skosxl:literalForm "no level applicable"@en .

:c_5d6a79d1 a skos:Concept;
  dct:created "2018-07-24T16:53:47.755Z"^^xsd:dateTime;
  skos:broader :c_a314e31f;
  skos:inScheme :conceptScheme_751925ed;
  skosxl:prefLabel :xl_en_6334086e .

:xl_en_6334086e a skosxl:Label;
  skosxl:literalForm "operational manual"@en .

:c_5d8254a8 a skos:Concept;
  dc:source "Interim Advice Note 184/16 Highways England CAD and Data Standard"@en;
  dct:created "2018-08-11T14:31:25.548Z"^^xsd:dateTime;
  skos:broader :c_6bc1fab9;
  skos:inScheme :conceptScheme_751925ed;
  skos:notation "VDS"@en;
  skos:prefLabel "drainage survey"@en;
  skosxl:prefLabel :xl_en_fbe57598 .

:xl_en_fbe57598 a skosxl:Label;
  skosxl:literalForm "drainage survey"@en .

:xl_en_98e4302d a skosxl:Label;
  skosxl:literalForm "traffic signs"@en .

:c_607b5b8a a skos:Concept;
  dc:source """production information a code of procedure for the construction industry
Organization of information about construction works — Information management using building information modelling - Part 2:Delivery phase of assets"""@en;
  dct:created "2018-07-22T14:31:37.578Z"^^xsd:dateTime;
  dct:modified "2020-10-31T05:22:50.883Z"^^xsd:dateTime;
  skos:broader :c_e5b1b611;
  skos:inScheme :conceptScheme_751925ed;
  skos:notation "00"@en;
  skosxl:prefLabel :xl_en_6e0de239 .

:xl_en_6e0de239 a skosxl:Label;
  skosxl:literalForm "base level of building where ground floor is not appropriate"@en .

:c_701139f9 a skos:Concept;
  dc:source """production information a code of procedure for the construction industry
Organization of information about construction works — Information management using building information modelling - Part 2:Delivery phase of assets"""@en;
  dct:created "2018-07-22T14:10:19.124Z"^^xsd:dateTime;
  dct:modified "2020-10-31T04:47:36.946Z"^^xsd:dateTime;
  skos:broader :c_618864b7;
  skos:editorialNote """Topographical, structural inspection,
Environmental, socio-economic,
Geotechnical
investigation, coring investigations,
materials investigation, condition"""@en;
  skos:inScheme :conceptScheme_751925ed;
  skos:narrower :c_bf7feeca, :c_eed60aa2;
  skos:notation "SU"@en;
  skosxl:prefLabel :xl_en_69eafeaa .

:c_9328238a a skos:Concept;
  dc:source """production information a code of procedure for the construction industry
Organization of information about construction works — Information management using building information modelling - Part 2:Delivery phase of assets"""@en;
  dct:created "2018-07-22T14:03:49.760Z"^^xsd:dateTime;
  dct:modified "2020-10-31T05:23:20.184Z"^^xsd:dateTime;
  skos:broader :c_618864b7;
  skos:editorialNote """Structural calcs, pavement calcs,
hydraulic calcs"""@en;
  skos:inScheme :conceptScheme_751925ed;
  skos:notation "CA"@en;
  skosxl:prefLabel :xl_en_4a589b21 .

:c_9b0e72da a skos:Concept;
  dc:source """production information a code of procedure for the construction industry
Organization of information about construction works — Information management using building information modelling - Part 2:Delivery phase of assets"""@en;
  dct:created "2018-07-22T13:50:57.697Z"^^xsd:dateTime;
  skos:broader :c_618864b7;
  skos:inScheme :conceptScheme_751925ed;
  skos:notation "MI"@en;
  skos:prefLabel "minutes action notes"@en;
  skosxl:prefLabel :xl_en_98adba90 .

:c_abd6f00f a skos:Concept;
  dct:created "2018-07-22T13:36:34.312Z"^^xsd:dateTime;
  skos:broader :c_618864b7;
  skos:inScheme :conceptScheme_751925ed;
  skosxl:prefLabel :xl_en_70a2d128 .

:c_b707f1ea a skos:Concept;
  dc:source """production information a code of procedure for the construction industry
Organization of information about construction works — Information management using building information modelling - Part 2:Delivery phase of assets"""@en;
  dct:created "2018-07-22T13:38:28.600Z"^^xsd:dateTime;
  dct:modified "2020-10-31T05:23:37.768Z"^^xsd:dateTime;
  skos:broader :c_618864b7;
  skos:inScheme :conceptScheme_751925ed;
  skos:notation "CP"@en;
  skosxl:prefLabel :xl_en_6ac4d708 .

:c_d0784080 a skos:Concept;
  dc:source """production information a code of procedure for the construction industry
Organization of information about construction works — Information management using building information modelling - Part 2:Delivery phase of assets"""@en;
  dct:created "2018-07-22T14:08:24.447Z"^^xsd:dateTime;
  dct:modified "2020-10-31T05:25:51.221Z"^^xsd:dateTime;
  skos:broader :c_618864b7;
  skos:inScheme :conceptScheme_751925ed;
  skos:notation "SP"@en;
  skosxl:prefLabel :xl_en_5882c3fa .

:c_d6230a5f a skos:Concept;
  dc:source """production information a code of procedure for the construction industry
Organization of information about construction works — Information management using building information modelling - Part 2:Delivery phase of assets"""@en;
  dct:created "2018-07-22T13:57:37.815Z"^^xsd:dateTime;
  dct:modified "2020-10-31T05:25:30.812Z"^^xsd:dateTime;
  skos:broader :c_618864b7;
  skos:inScheme :conceptScheme_751925ed;
  skos:notation "RD"@en;
  skosxl:prefLabel :xl_en_e48cb670 .

:c_ecc8ec55 a skos:Concept;
  dc:source """production information a code of procedure for the construction industry
Organization of information about construction works — Information management using building information modelling - Part 2:Delivery phase of assets"""@en;
  dct:created "2018-07-22T14:05:27.156Z"^^xsd:dateTime;
  skos:broader :c_618864b7;
  skos:inScheme :conceptScheme_751925ed;
  skos:notation "SH"@en;
  skos:prefLabel "schedule"@en;
  skosxl:prefLabel :xl_en_4e0710f8 .

:c_ef814787 a skos:Concept;
  dc:source """production information a code of procedure for the construction industry
Organization of information about construction works — Information management using building information modelling - Part 2:Delivery phase of assets"""@en;
  dct:created "2018-07-22T13:54:27.003Z"^^xsd:dateTime;
  dct:modified "2020-10-30T20:47:17.389Z"^^xsd:dateTime;
  skos:broader :c_618864b7;
  skos:inScheme :conceptScheme_751925ed;
  skos:notation "PP"@en;
  skosxl:prefLabel :xl_en_8d7d10e7 .

:c_fcfbbcd0 a skos:Concept;
  dc:source """production information a code of procedure for the construction industry
Organization of information about construction works — Information management using building information modelling - Part 2:Delivery phase of assets"""@en;
  dct:created "2018-07-22T13:56:05.268Z"^^xsd:dateTime;
  dct:modified "2020-10-31T05:17:57.485Z"^^xsd:dateTime;
  skos:broader :c_618864b7;
  skos:inScheme :conceptScheme_751925ed;
  skos:notation "PR"@en;
  skosxl:prefLabel :xl_en_66d2d261 .

:xl_en_3aeb39fa a skosxl:Label;
  skosxl:literalForm "document type"@en .

:c_6859ada6 a skos:Concept;
  dc:source "zero carbon hub appendices - closing the gap between design and as-built performance - appendix c";
  dct:created "2018-07-20T20:09:04.533Z"^^xsd:dateTime;
  dct:modified "2020-10-31T05:13:49.234Z"^^xsd:dateTime;
  skos:broader :c_f29587ff;
  skos:inScheme :conceptScheme_751925ed;
  skos:notation "ME SPEC"@en;
  skosxl:prefLabel :xl_en_dde3e6ee .

:xl_en_dde3e6ee a skosxl:Label;
  skosxl:literalForm "mechanical and electrical specification"@en .

:xl_en_777f97b2 a skosxl:Label;
  dct:modified "2018-08-11T12:59:12.410Z"^^xsd:dateTime;
  skosxl:literalForm "general (highways)"@en .

:c_adba6615 a skos:Concept;
  dc:source "Interim Advice Note 184/16 Highways England CAD and Data Standard"@en;
  dct:created "2018-08-11T14:47:01.050Z"^^xsd:dateTime;
  dct:modified "2020-10-31T05:08:31.235Z"^^xsd:dateTime;
  skos:broader :c_6bc1fab9;
  skos:inScheme :conceptScheme_751925ed;
  skos:notation "VTO"@en;
  skosxl:prefLabel :xl_en_90a100d1 .

:c_b227f284 a skos:Concept;
  dc:source "Interim Advice Note 184/16 Highways England CAD and Data Standard"@en;
  dct:created "2018-08-11T14:39:54.185Z"^^xsd:dateTime;
  dct:modified "2020-10-31T04:41:33.184Z"^^xsd:dateTime;
  skos:broader :c_6bc1fab9;
  skos:inScheme :conceptScheme_751925ed;
  skos:notation "VNR"@en;
  skosxl:prefLabel :xl_en_c6d8c858 .

:c_b65fa6fd a skos:Concept;
  dc:source "Interim Advice Note 184/16 Highways England CAD and Data Standard"@en;
  dct:created "2018-08-11T14:34:02.076Z"^^xsd:dateTime;
  dct:modified "2020-10-31T04:47:53.661Z"^^xsd:dateTime;
  skos:broader :c_6bc1fab9;
  skos:inScheme :conceptScheme_751925ed;
  skos:notation "VES"@en;
  skosxl:prefLabel :xl_en_93c72188 .

:c_d8e2bacb a skos:Concept;
  dc:source "Interim Advice Note 184/16 Highways England CAD and Data Standard"@en;
  dct:created "2018-08-11T14:37:43.628Z"^^xsd:dateTime;
  dct:modified "2020-10-31T05:38:31.059Z"^^xsd:dateTime;
  skos:broader :c_6bc1fab9;
  skos:inScheme :conceptScheme_751925ed;
  skos:notation "VGT"@en;
  skosxl:prefLabel :xl_en_3ede09f4 .

:c_d9ed5f11 a skos:Concept;
  dc:source "Interim Advice Note 184/16 Highways England CAD and Data Standard"@en;
  dct:created "2018-08-11T14:41:50.194Z"^^xsd:dateTime;
  dct:modified "2020-10-31T05:11:57.243Z"^^xsd:dateTime;
  skos:broader :c_6bc1fab9;
  skos:inScheme :conceptScheme_751925ed;
  skos:notation "VPS"@en;
  skosxl:prefLabel :xl_en_f2311450 .

:c_ed146474 a skos:Concept;
  dc:source "Interim Advice Note 184/16 Highways England CAD and Data Standard"@en;
  dct:created "2018-08-11T14:45:15.681Z"^^xsd:dateTime;
  skos:broader :c_6bc1fab9;
  skos:inScheme :conceptScheme_751925ed;
  skos:notation "VSS"@en;
  skos:prefLabel "stakeholder surveys"@en;
  skosxl:prefLabel :xl_en_414b9605 .

:c_f443f164 a skos:Concept;
  dc:source "Interim Advice Note 184/16 Highways England CAD and Data Standard"@en;
  dct:created "2018-08-11T14:29:38.977Z"^^xsd:dateTime;
  dct:modified "2020-10-30T21:01:08.559Z"^^xsd:dateTime;
  skos:broader :c_6bc1fab9;
  skos:inScheme :conceptScheme_751925ed;
  skos:notation "VAS"@en;
  skosxl:prefLabel :xl_en_98f021db .

:xl_en_a3532349 a skosxl:Label;
  skosxl:literalForm "survey (volume)"@en .

:xl_en_120eef77 a skosxl:Label;
  skosxl:literalForm "general (structures)"@en .

:xl_en_3380ad87 a skosxl:Label;
  skosxl:literalForm "services piped and ducted"@en .

:xl_en_a74e7a5b a skosxl:Label;
  skosxl:literalForm "power / electrical"@en .

:xl_en_a423da25 a skosxl:Label;
  skosxl:literalForm "tunnels"@en .

:c_bf7feeca a skos:Concept;
  dct:created "2018-07-24T17:11:09.735Z"^^xsd:dateTime;
  skos:broader :c_701139f9;
  skos:inScheme :conceptScheme_751925ed;
  skosxl:prefLabel :xl_en_395273d6 .

:c_eed60aa2 a skos:Concept;
  dc:source "BS ISO 6707-2-2017-Buildings and civil engineering works. Vocabulary. Contract and communication terms"@en;
  dct:created "2018-07-24T17:10:02.154Z"^^xsd:dateTime;
  dct:modified "2020-10-30T20:36:50.069Z"^^xsd:dateTime;
  skos:broader :c_701139f9;
  skos:inScheme :conceptScheme_751925ed;
  skosxl:prefLabel :xl_en_1b49474f .

:xl_en_69eafeaa a skosxl:Label;
  skosxl:literalForm "survey"@en .

:xl_en_4e277135 a skosxl:Label;
  skosxl:literalForm "fencing"@en .

:c_fbbe4f85 a skos:Concept;
  dc:source "zero carbon hub appendices - closing the gap between design and as-built performance - appendix c";
  dct:created "2018-07-20T20:14:15.814Z"^^xsd:dateTime;
  skos:broader :c_73619d2a;
  skos:inScheme :conceptScheme_751925ed;
  skos:prefLabel "water heating"@en;
  skosxl:prefLabel :xl_en_e3200bfa .

:xl_en_a579548c a skosxl:Label;
  dct:modified "2018-07-28T16:46:18.870Z"^^xsd:dateTime;
  skosxl:literalForm "mechanical and electrical"@en .

:c_73726e27 a skos:Concept;
  dc:source "Interim Advice Note 184/16 Highways England CAD and Data Standard"@en;
  dct:created "2018-08-11T13:48:11.818Z"^^xsd:dateTime;
  dct:modified "2020-10-31T04:57:54.585Z"^^xsd:dateTime;
  skos:broader :c_e54483d8;
  skos:inScheme :conceptScheme_751925ed;
  skos:notation "EAC"@en;
  skosxl:prefLabel :xl_en_d2436a52 .

:xl_en_d2436a52 a skosxl:Label;
  skosxl:literalForm "environmental approvals and consents"@en .

:c_75f1aa77 a skos:Concept;
  dc:source "Interim Advice Note 184/16 Highways England CAD and Data Standard"@en;
  dct:created "2018-08-11T13:54:16.180Z"^^xsd:dateTime;
  dct:modified "2020-10-30T20:46:58.411Z"^^xsd:dateTime;
  skos:broader :c_e54483d8;
  skos:inScheme :conceptScheme_751925ed;
  skos:notation "EGN"@en;
  skosxl:prefLabel :xl_en_e99e658b .

:xl_en_e99e658b a skosxl:Label;
  dct:modified "2018-08-11T13:55:10.158Z"^^xsd:dateTime;
  skosxl:literalForm "general (environment)"@en .

:xl_en_fd157b83 a skosxl:Label;
  skosxl:literalForm "site clearance"@en .

:c_793b849c dct:created "2018-08-11T13:05:19.050Z"^^xsd:dateTime .

:xl_en_b077dd14 a skosxl:Label;
  skosxl:literalForm "health and safety (volume)"@en .

:xl_en_ad12bf3f a skosxl:Label;
  skosxl:literalForm "mainline geometric layout"@en .

:xl_en_7274bb0f a skosxl:Label;
  skosxl:literalForm "pim"@en .

:xl_en_f642504c a skosxl:Label;
  skosxl:literalForm "side roads geometric layout"@en .

:xl_en_8715993d a skosxl:Label;
  skosxl:literalForm "cobie"@en .

:c_83498fa1 a skos:Concept;
  dct:created "2018-07-24T16:52:31.684Z"^^xsd:dateTime;
  skos:broader :c_a314e31f;
  skos:inScheme :conceptScheme_751925ed;
  skosxl:prefLabel :xl_en_f8f9fd3f .

:xl_en_f8f9fd3f a skosxl:Label;
  skosxl:literalForm "as-built drawing"@en .

:c_86ec4f8f a skos:Concept;
  dc:source "zero carbon hub appendices - closing the gap between design and as-built performance - evidence review report appendices";
  dct:created "2018-07-20T21:03:28.939Z"^^xsd:dateTime;
  dct:modified "2020-10-30T20:23:44.911Z"^^xsd:dateTime;
  olo:index "6"^^xsd:positiveInteger;
  skos:broader :c_c02e3a4e;
  skos:inScheme :conceptScheme_751925ed;
  skos:notation "60";
  skosxl:prefLabel :xl_en_2cad77a8 .

:xl_en_2cad77a8 a skosxl:Label;
  skosxl:literalForm "testing and commissioning"@en .

:c_876afb3f a skos:Concept;
  dc:source "zero carbon hub appendices - closing the gap between design and as-built performance - evidence review report appendices";
  dct:created "2018-07-20T20:49:10.127Z"^^xsd:dateTime;
  olo:index "5.2"^^xsd:positiveInteger;
  skos:broader :c_91ece774;
  skos:inScheme :conceptScheme_751925ed;
  skos:notation "52";
  skos:note "including roof structure";
  skos:prefLabel "joist to roof"@en;
  skosxl:prefLabel :xl_en_670428ce .

:xl_en_670428ce a skosxl:Label;
  dct:modified "2020-10-31T05:54:37.374Z"^^xsd:dateTime .

:c_87804062 a skos:Concept;
  dc:source """production information a code of procedure for the construction industry
Organization of information about construction works — Information management using building information modelling - Part 2:Delivery phase of assets"""@en;
  dct:created "2018-07-22T14:34:02.722Z"^^xsd:dateTime;
  dct:modified "2020-10-31T05:16:32.575Z"^^xsd:dateTime;
  skos:broader :c_e5b1b611;
  skos:inScheme :conceptScheme_751925ed;
  skos:notation "01"@en;
  skosxl:prefLabel :xl_en_eb7d0a12 .

:xl_en_eb7d0a12 a skosxl:Label;
  dct:modified "2018-07-22T14:35:43.310Z"^^xsd:dateTime;
  skosxl:literalForm "floor 01"@en .

:c_87bf8d98 a skos:Concept;
  dc:source """production information a code of procedure for the construction industry
Organization of information about construction works — Information management using building information modelling - Part 2:Delivery phase of assets"""@en;
  dct:created "2018-07-22T14:36:02.373Z"^^xsd:dateTime;
  dct:modified "2020-10-31T05:10:19.276Z"^^xsd:dateTime;
  skos:broader :c_e5b1b611;
  skos:inScheme :conceptScheme_751925ed;
  skos:notation "02"@en;
  skosxl:prefLabel :xl_en_ad8735fa .

:xl_en_ad8735fa a skosxl:Label;
  skosxl:literalForm "floor 02"@en .

:c_8b778c41 a skos:Concept;
  dc:source "Interim Advice Note 184/16 Highways England CAD and Data Standard"@en;
  dct:created "2018-08-11T14:04:05.302Z"^^xsd:dateTime;
  dct:modified "2020-10-31T05:32:55.932Z"^^xsd:dateTime;
  skos:broader :c_e54483d8;
  skos:inScheme :conceptScheme_751925ed;
  skos:notation "ENV"@en;
  skosxl:prefLabel :xl_en_b2637b46 .

:xl_en_b2637b46 a skosxl:Label;
  skosxl:literalForm "noise and vibration"@en .

:c_8cad0fd2 a skos:Concept;
  dc:source "Interim Advice Note 184/16 Highways England CAD and Data Standard"@en;
  dct:created "2018-08-11T14:02:08.560Z"^^xsd:dateTime;
  skos:broader :c_e54483d8;
  skos:inScheme :conceptScheme_751925ed;
  skos:notation "ENM"@en;
  skos:prefLabel "non motorised users"@en;
  skosxl:prefLabel :xl_en_8405c522 .

:xl_en_8405c522 a skosxl:Label;
  dct:modified "2018-08-11T14:03:00.687Z"^^xsd:dateTime;
  skosxl:literalForm "non motorised users"@en .

:xl_en_9e9f2102 a skosxl:Label;
  skosxl:literalForm "feasibility study"@en .

:xl_en_913b3693 a skosxl:Label;
  skosxl:literalForm "plqs"@en .

:c_90ff7ddf a skos:Concept;
  dc:source "Interim Advice Note 184/16 Highways England CAD and Data Standard"@en;
  dct:created "2018-08-11T13:51:37.079Z"^^xsd:dateTime;
  dct:modified "2020-10-31T04:54:42.605Z"^^xsd:dateTime;
  skos:broader :c_e54483d8;
  skos:inScheme :conceptScheme_751925ed;
  skos:notation "EBD"@en;
  skosxl:prefLabel :xl_en_42b22dc8 .

:xl_en_42b22dc8 a skosxl:Label;
  skosxl:literalForm "biodiversity"@en .

:c_9d7853dc a skos:Concept;
  dc:source "zero carbon hub appendices - closing the gap between design and as-built performance - evidence review report appendices";
  dct:created "2018-07-20T20:56:41.258Z"^^xsd:dateTime;
  dct:modified "2020-10-31T05:19:07.132Z"^^xsd:dateTime;
  olo:index "5.5"^^xsd:positiveInteger;
  skos:broader :c_91ece774;
  skos:inScheme :conceptScheme_751925ed;
  skos:notation "55";
  skosxl:prefLabel :xl_en_621ee2b6 .

:c_b39bb643 a skos:Concept;
  dc:source "zero carbon hub appendices - closing the gap between design and as-built performance - evidence review report appendices";
  dct:created "2018-07-20T20:59:09.057Z"^^xsd:dateTime;
  dct:modified "2020-10-31T05:01:03.207Z"^^xsd:dateTime;
  olo:index "5.7"^^xsd:positiveInteger;
  skos:broader :c_91ece774;
  skos:inScheme :conceptScheme_751925ed;
  skos:notation "57";
  skosxl:prefLabel :xl_en_4b523657 .

:xl_en_4a589b21 a skosxl:Label;
  skosxl:literalForm "calculations"@en .

:xl_en_38527472 a skosxl:Label;
  dct:modified "2018-07-28T16:24:06.260Z"^^xsd:dateTime;
  skosxl:literalForm "local authority building control"@en .

:xl_en_9381849e a skosxl:Label;
  skosxl:literalForm "legal"@en .

:c_ace7ce12 a skos:Concept;
  dc:source "Interim Advice Note 184/16 Highways England CAD and Data Standard"@en;
  dct:created "2018-08-11T14:58:45.534Z"^^xsd:dateTime;
  dct:modified "2020-10-30T20:30:07.752Z"^^xsd:dateTime;
  skos:broader :c_9af04a0c;
  skos:inScheme :conceptScheme_751925ed;
  skos:notation "TTM"@en;
  skosxl:prefLabel :xl_en_327048fe .

:c_eb6b96ad a skos:Concept;
  dc:source "Interim Advice Note 184/16 Highways England CAD and Data Standard"@en;
  dct:created "2018-08-11T15:00:51.419Z"^^xsd:dateTime;
  dct:modified "2020-10-30T20:30:25.619Z"^^xsd:dateTime;
  skos:broader :c_9af04a0c;
  skos:inScheme :conceptScheme_751925ed;
  skos:notation "TTW"@en;
  skosxl:prefLabel :xl_en_c21780ac .

:xl_en_06a2f565 a skosxl:Label;
  skosxl:literalForm "temporary"@en .

:xl_en_98adba90 a skosxl:Label;
  skosxl:literalForm "minutes action notes"@en .

:xl_en_621ee2b6 a skosxl:Label;
  skosxl:literalForm "dry lining and plaster"@en .

:xl_en_1b010294 a skosxl:Label;
  skosxl:literalForm "road markings"@en .

:xl_en_09b0def2 a skosxl:Label;
  skosxl:literalForm "bridges and major culverts"@en .

:xl_en_2f190d8d a skosxl:Label;
  skosxl:literalForm "minor structures and culverts"@en .

:xl_en_bce41bc8 a skosxl:Label;
  dct:modified "2018-08-11T13:05:46.598Z"^^xsd:dateTime;
  skosxl:literalForm "geotechnical (highways)"@en .

:c_a34bfc84 a skos:Concept;
  dc:source "organization of information about construction works — information management using building information modelling - part 2: delivery phase of assets"@en;
  dct:created "2018-07-22T11:19:03.959Z"^^xsd:dateTime;
  dct:modified "2020-10-31T05:26:06.422Z"^^xsd:dateTime;
  rdfs:isDefinedBy :c_263f8b4d;
  skos:broader :c_b7ef2137;
  skos:inScheme :conceptScheme_751925ed;
  skos:notation "M3"@en;
  skosxl:prefLabel :xl_en_7a6f26b1 .

:xl_en_7a6f26b1 a skosxl:Label;
  dct:modified "2018-07-28T16:45:31.302Z"^^xsd:dateTime;
  skosxl:literalForm "model 3d"@en .

:c_a9c2e902 a skos:Concept;
  dc:source "Interim Advice Note 184/16 Highways England CAD and Data Standard"@en;
  dct:created "2018-08-11T14:00:10.107Z"^^xsd:dateTime;
  skos:broader :c_e54483d8;
  skos:inScheme :conceptScheme_751925ed;
  skos:notation "ELS"@en;
  skos:prefLabel "landscape"@en;
  skosxl:prefLabel :xl_en_568677e9 .

:xl_en_568677e9 a skosxl:Label;
  skosxl:literalForm "landscape"@en .

:xl_en_70a2d128 a skosxl:Label;
  skosxl:literalForm "correspondence"@en .

:c_ac615319 a skos:Concept;
  dc:source "zero carbon hub appendices - closing the gap between design and as-built performance - appendix c";
  dct:created "2018-07-20T20:22:54.254Z"^^xsd:dateTime;
  dct:modified "2020-10-31T05:09:13.293Z"^^xsd:dateTime;
  skos:broader :c_f29587ff;
  skos:inScheme :conceptScheme_751925ed;
  skos:notation "ATTMA"@en;
  skos:prefLabel "air tightness certificate"@en;
  skosxl:altLabel :xl_en_91bd8550;
  skosxl:prefLabel :xl_en_285f3771 .

:c_adba6615 skos:prefLabel "topographical"@en .

:c_55b465e8 skos:prefLabel "section 1"@en .

:xl_en_91bd8550 a skosxl:Label;
  skosxl:literalForm "attma"@en .

:xl_en_285f3771 a skosxl:Label;
  dct:modified "2018-07-24T17:18:06.611Z"^^xsd:dateTime;
  skosxl:literalForm "air tightness certificate"@en .

:xl_en_327048fe a skosxl:Label;
  skosxl:literalForm "traffic management"@en .

:xl_en_90a100d1 a skosxl:Label;
  skosxl:literalForm "topographical"@en .

:xl_en_b537b614 a skosxl:Label;
  skosxl:literalForm "accommodation works"@en .

:xl_en_9717bf9a a skosxl:Label;
  skosxl:literalForm "plans"@en .

:c_b019c6a7 a skos:Concept;
  dc:source """production information a code of procedure for the construction industry
Organization of information about construction works — Information management using building information modelling - Part 2:Delivery phase of assets"""@en;
  dct:created "2018-07-22T14:39:34.010Z"^^xsd:dateTime;
  dct:modified "2020-10-31T05:06:37.028Z"^^xsd:dateTime;
  skos:broader :c_e5b1b611;
  skos:inScheme :conceptScheme_751925ed;
  skos:notation "M2"@en;
  skosxl:prefLabel :xl_en_843ef43e .

:xl_en_843ef43e a skosxl:Label;
  skosxl:literalForm "mezzanine above level 02"@en .

:xl_en_ca2d0e57 a skosxl:Label;
  skosxl:literalForm "bep"@en .

:xl_en_c6d8c858 a skosxl:Label;
  skosxl:literalForm "national road telecommunications services (NRTS)"@en .

:c_b2459321 a skos:Concept;
  dc:source "zero carbon hub appendices - closing the gap between design and as-built performance - appendix c";
  dct:created "2018-07-20T20:03:06.287Z"^^xsd:dateTime;
  dct:modified "2020-10-31T05:38:02.113Z"^^xsd:dateTime;
  skos:broader :c_f29587ff;
  skos:inScheme :conceptScheme_751925ed;
  skos:notation "CONST SPEC"@en;
  skosxl:altLabel :xl_en_45e6bbda;
  skosxl:prefLabel :xl_en_eb7d5dd2 .

:xl_en_45e6bbda a skosxl:Label;
  skosxl:literalForm "construct spec"@en .

:xl_en_eb7d5dd2 a skosxl:Label;
  skosxl:literalForm "construction specification"@en .

:c_b2e826d0 a skos:Concept;
  dc:source "Interim Advice Note 184/16 Highways England CAD and Data Standard"@en;
  dct:created "2018-08-11T13:58:27.429Z"^^xsd:dateTime;
  dct:modified "2020-10-30T20:59:47.155Z"^^xsd:dateTime;
  skos:broader :c_e54483d8;
  skos:inScheme :conceptScheme_751925ed;
  skos:notation "EHR"@en;
  skosxl:prefLabel :xl_en_85806c81 .

:xl_en_85806c81 a skosxl:Label;
  skosxl:literalForm "heritage/historic resources"@en .

:xl_en_4b523657 a skosxl:Label;
  skosxl:literalForm "finals and build complete"@en .

:c_b4f95391 a skos:Concept;
  dc:source "production information a code of procedure for the construction industry"@en;
  dct:created "2018-07-22T08:34:53.685Z"^^xsd:dateTime;
  dct:modified "2020-10-30T20:32:27.124Z"^^xsd:dateTime;
  skos:broader :c_c76077ab;
  skos:inScheme :conceptScheme_751925ed;
  skos:notation "SUP"@en;
  skos:related :c_2eb971b3;
  skosxl:prefLabel :xl_en_2f18cca0 .

:xl_en_2f18cca0 a skosxl:Label;
  skosxl:literalForm "superstructure"@en .

:c_b65b6f3f dct:created "2018-07-22T13:43:09.626Z"^^xsd:dateTime .

:xl_en_93c72188 a skosxl:Label;
  skosxl:literalForm "environmental survey"@en .

:c_be22475b a skos:Concept;
  dct:created "2018-07-24T17:21:40.033Z"^^xsd:dateTime;
  skos:broader :c_b67efcfb;
  skos:inScheme :conceptScheme_751925ed;
  skosxl:prefLabel :xl_en_fa04c4ec .

:xl_en_6ac4d708 a skosxl:Label;
  skosxl:literalForm "cost plan"@en .

:c_bfc844fa a skos:Concept;
  dc:source "organization of information about construction works — information management using building information modelling - part 2: delivery phase of assets"@en;
  dct:created "2018-07-22T11:20:21.855Z"^^xsd:dateTime;
  dct:modified "2020-10-30T20:27:24.765Z"^^xsd:dateTime;
  rdfs:isDefinedBy :c_263f8b4d;
  skos:broader :c_b7ef2137;
  skos:inScheme :conceptScheme_751925ed;
  skos:notation "MR"@en;
  skosxl:prefLabel :xl_en_43be086e .

:c_c4c44bc2 a skos:Concept;
  dc:source "organization of information about construction works — information management using building information modelling - part 2: delivery phase of assets"@en;
  dct:created "2018-07-22T11:18:11.072Z"^^xsd:dateTime;
  dct:modified "2020-10-31T04:58:26.078Z"^^xsd:dateTime;
  rdfs:isDefinedBy :c_263f8b4d;
  skos:broader :c_b7ef2137;
  skos:inScheme :conceptScheme_751925ed;
  skos:notation "M2"@en;
  skosxl:prefLabel :xl_en_80861017 .

:c_e9882180 a skos:Concept;
  dc:source "organization of information about construction works — information management using building information modelling - part 2: delivery phase of assets"@en;
  dct:created "2018-07-22T11:13:14.842Z"^^xsd:dateTime;
  dct:modified "2020-10-31T05:34:09.852Z"^^xsd:dateTime;
  rdfs:isDefinedBy :c_263f8b4d;
  skos:broader :c_b7ef2137;
  skos:inScheme :conceptScheme_751925ed;
  skos:notation "CM"@en;
  skosxl:prefLabel :xl_en_dc6b68be .

:c_f84ebdc2 a skos:Concept;
  dc:source "organization of information about construction works — information management using building information modelling - part 2: delivery phase of assets"@en;
  dct:created "2018-07-22T11:17:13.973Z"^^xsd:dateTime;
  rdfs:isDefinedBy :c_263f8b4d;
  skos:broader :c_b7ef2137;
  skos:inScheme :conceptScheme_751925ed;
  skos:notation "DR"@en;
  skos:prefLabel "drawing 2d"@en;
  skosxl:prefLabel :xl_en_6932328a .

:xl_en_43d42d70 a skosxl:Label;
  skosxl:literalForm "drawing type"@en .

:xl_en_ea6f60b0 a skosxl:Label;
  skosxl:literalForm "gantries"@en .

:c_db8a3f56 a skos:Concept;
  dct:created "2018-07-22T07:25:54.049Z"^^xsd:dateTime;
  dct:modified "2020-10-30T20:37:43.396Z"^^xsd:dateTime;
  skos:broader :c_ba4a8cbb;
  skos:inScheme :conceptScheme_751925ed;
  skos:notation "Y"@en;
  skosxl:prefLabel :xl_en_b5295211 .

:xl_en_f7217563 a skosxl:Label;
  skosxl:literalForm "scheme wide generic information"@en .

:xl_en_f2eee9b5 a skosxl:Label;
  skosxl:literalForm "cde"@en .

:xl_en_fa04c4ec a skosxl:Label;
  skosxl:literalForm "site manager"@en .

:xl_en_395273d6 a skosxl:Label;
  skosxl:literalForm "building survey"@en .

:xl_en_43be086e a skosxl:Label;
  skosxl:literalForm "model rendition for other renditions, e.g. thermal analysis, etc"@en .

:c_c0f70902 a skos:Concept;
  dc:source """production information a code of procedure for the construction industry
Organization of information about construction works — Information management using building information modelling - Part 2:Delivery phase of assets"""@en;
  dct:created "2018-07-22T14:29:39.867Z"^^xsd:dateTime;
  skos:broader :c_e5b1b611;
  skos:inScheme :conceptScheme_751925ed;
  skos:notation "GF"@en;
  skos:prefLabel "ground floor"@en;
  skosxl:prefLabel :xl_en_1e89b441 .

:xl_en_1e89b441 a skosxl:Label;
  skosxl:literalForm "ground floor"@en .

:xl_en_813a8fc3 a skosxl:Label;
  skosxl:literalForm "building services drainage"@en .

:xl_en_80861017 a skosxl:Label;
  dct:modified "2018-07-28T16:45:09.969Z"^^xsd:dateTime;
  skosxl:literalForm "model 2d"@en .

:c_d837a7ac a skos:Concept;
  dc:source "production information a code of procedure for the construction industry"@en;
  dct:created "2018-07-22T15:38:30.194Z"^^xsd:dateTime;
  dct:modified "2020-10-31T04:56:28.329Z"^^xsd:dateTime;
  skos:broader :c_c76077ab;
  skos:inScheme :conceptScheme_751925ed;
  skosxl:prefLabel :xl_en_b06ae72b .

:xl_en_5882c3fa a skosxl:Label;
  skosxl:literalForm "specification"@en .

:xl_en_1ec12f25 a skosxl:Label;
  skosxl:literalForm "oir"@en .

:xl_en_a28bbbe3 a skosxl:Label;
  skosxl:literalForm "approved document b"@en .

:xl_en_043a03d3 a skosxl:Label;
  skosxl:literalForm "knowledge library"@en .

:xl_en_e48cb670 a skosxl:Label;
  skosxl:literalForm "room data sheet"@en .

:xl_en_b06ae72b a skosxl:Label;
  skosxl:literalForm "substructure plan"@en .

:xl_en_3ede09f4 a skosxl:Label;
  skosxl:literalForm "geotechnical investigation"@en .

:xl_en_f2311450 a skosxl:Label;
  skosxl:literalForm "pavement systems"@en .

:c_da247d5e a skos:Concept;
  dct:created "2018-07-22T14:44:38.361Z"^^xsd:dateTime;
  dct:modified "2020-10-30T20:32:06.394Z"^^xsd:dateTime;
  skos:broader :c_e5b1b611;
  skos:inScheme :conceptScheme_751925ed;
  skos:notation "BLK"@en;
  skosxl:prefLabel :xl_en_a0cda785 .

:xl_en_a0cda785 a skosxl:Label;
  skosxl:literalForm "block"@en .

:xl_en_b5295211 a skosxl:Label;
  skosxl:literalForm "specialist designer"@en .

:xl_en_ecb8813d a skosxl:Label;
  skosxl:literalForm "health"@en .

:c_e4e408ec a skos:Concept;
  dc:source """production information a code of procedure for the construction industry
Organization of information about construction works — Information management using building information modelling - Part 2:Delivery phase of assets"""@en;
  dct:created "2018-07-22T14:41:10.793Z"^^xsd:dateTime;
  dct:modified "2020-10-31T04:55:48.245Z"^^xsd:dateTime;
  skos:broader :c_e5b1b611;
  skos:inScheme :conceptScheme_751925ed;
  skos:notation "B1"@en;
  skosxl:prefLabel :xl_en_e3ab5149 .

:xl_en_e3ab5149 a skosxl:Label;
  skosxl:literalForm "basement level 01"@en .

:c_edf75137 a skos:Concept;
  dc:source "Interim Advice Note 184/16 Highways England CAD and Data Standard"@en;
  dct:created "2018-08-11T14:05:46.598Z"^^xsd:dateTime;
  dct:modified "2020-10-30T20:59:27.559Z"^^xsd:dateTime;
  skos:broader :c_e54483d8;
  skos:inScheme :conceptScheme_751925ed;
  skos:notation "ETS"@en;
  skosxl:prefLabel :xl_en_7f471531 .

:xl_en_54371a61 a skosxl:Label;
  skosxl:literalForm "environment"@en .

:c_fb2c64cc a skos:Concept;
  dc:source """production information a code of procedure for the construction industry
Organization of information about construction works — Information management using building information modelling - Part 2:Delivery phase of assets"""@en;
  dct:created "2018-07-22T14:43:00.462Z"^^xsd:dateTime;
  dct:modified "2020-10-31T05:32:00.564Z"^^xsd:dateTime;
  skos:broader :c_e5b1b611;
  skos:inScheme :conceptScheme_751925ed;
  skos:notation "B2"@en;
  skosxl:prefLabel :xl_en_9da77174 .

:xl_en_763d939a a skosxl:Label;
  skosxl:literalForm "level location"@en .

:xl_en_dc6b68be a skosxl:Label;
  skosxl:literalForm "combined model combined multidiscipline model"@en .

:xl_en_c21780ac a skosxl:Label;
  skosxl:literalForm "temporary works"@en .

:xl_en_4e0710f8 a skosxl:Label;
  skosxl:literalForm "schedule"@en .

:xl_en_414b9605 a skosxl:Label;
  skosxl:literalForm "stakeholder surveys"@en .

:xl_en_7f471531 a skosxl:Label;
  skosxl:literalForm "townscape"@en .

:xl_en_1b49474f a skosxl:Label;
  skosxl:literalForm "land survey"@en .

:xl_en_8d7d10e7 a skosxl:Label;
  skosxl:literalForm "presentation"@en .

:c_f23ce991 a skos:Concept;
  dc:source "zero carbon hub appendices - closing the gap between design and as-built performance - appendix c";
  dct:created "2018-07-20T20:26:54.985Z"^^xsd:dateTime;
  skos:broader :c_f29587ff;
  skos:inScheme :conceptScheme_751925ed;
  skos:notation "EPC"@en;
  skos:prefLabel "energy performance certificate"@en;
  skosxl:prefLabel :xl_en_db0d74d0 .

:xl_en_db0d74d0 a skosxl:Label;
  skosxl:literalForm "energy performance certificate"@en .

:c_f8a6d299 a skos:Concept;
  dc:source "zero carbon hub appendices - closing the gap between design and as-built performance - appendix c";
  dct:created "2018-07-20T20:25:28.784Z"^^xsd:dateTime;
  dct:modified "2020-10-31T05:14:34.730Z"^^xsd:dateTime;
  skos:broader :c_f29587ff;
  skos:inScheme :conceptScheme_751925ed;
  skos:notation "COMP CERT"@en;
  skosxl:prefLabel :xl_en_b98d6f54 .

:xl_en_bfd696fb a skosxl:Label;
  dct:modified "2018-08-11T12:11:13.729Z"^^xsd:dateTime;
  skosxl:literalForm "documents (housing)"@en .

:xl_en_98f021db a skosxl:Label;
  skosxl:literalForm "accident statistics"@en .

:c_f46087b4 a skos:Concept;
  dc:source "BS ISO 6707-2-2017-Buildings and civil engineering works. Vocabulary. Contract and communication terms"@en;
  dct:created "2018-07-24T16:54:21.325Z"^^xsd:dateTime;
  dct:modified "2019-11-30T10:57:47.911Z"^^xsd:dateTime;
  skos:broader :c_a314e31f;
  skos:inScheme :conceptScheme_751925ed;
  skosxl:prefLabel :xl_en_ee9363f1 .

:xl_en_ee9363f1 a skosxl:Label;
  skosxl:literalForm "maintenance manual"@en .

:c_f479d1cb dct:created "2018-08-11T14:26:15.280Z"^^xsd:dateTime .

:xl_en_b3950513 a skosxl:Label;
  skosxl:literalForm "building safety manager"@en .

:xl_en_6932328a a skosxl:Label;
  dct:modified "2018-07-28T16:44:52.366Z"^^xsd:dateTime;
  skosxl:literalForm "drawing 2d"@en .

:xl_en_b98d6f54 a skosxl:Label;
  skosxl:literalForm "completion certificate"@en .

:xl_en_d4ddf75e a skosxl:Label;
  skosxl:literalForm "bim"@en .

:xl_en_9da77174 a skosxl:Label;
  skosxl:literalForm "basement level 02"@en .

:xl_en_e3200bfa a skosxl:Label;
  skosxl:literalForm "water heating"@en .

:xl_en_66d2d261 a skosxl:Label;
  skosxl:literalForm "programme"@en .

:xl_en_74b321d9 a skosxl:Label;
  skosxl:literalForm "pip"@en .

:skosCollection_1f48022e a skos:Collection;
  dct:created "2018-07-20T22:28:49.785Z"^^xsd:dateTime;
  dct:modified "2019-11-30T10:53:26.550Z"^^xsd:dateTime;
  skos:member :c_05a3b5d1, :c_0a40b44e, :c_0d978f6c, :c_1081a7c2, :c_1e5f46db, :c_1f84f905,
    :c_2238ee39, :c_240f4112, :c_2592b8ec, :c_2a6e874e, :c_2cb0f320, :c_32bf6806, :c_35bd7cc0,
    :c_3c21373f, :c_41bc9708, :c_49888cc9, :c_4fb142b4, :c_536a60e1, :c_5ac38c99, :c_5d17180d,
    :c_68039062, :c_6859ada6, :c_701139f9, :c_8046ed58, :c_8d5846c3, :c_8ec4ead3, :c_9328238a,
    :c_9832f0b7, :c_98522fb2, :c_98ba4c18, :c_9b0e72da, :c_9e9aa534, :c_9ebfa246, :c_a47e6a9b,
    :c_a7289a25, :c_ac615319, :c_b2459321, :c_b3508a0f, :c_b707f1ea, :c_bf7feeca, :c_c989802e,
    :c_d0784080, :c_d37e6d79, :c_d6230a5f, :c_d71b62e2, :c_db373352, :c_e2fbc29a, :c_e8a3f333,
    :c_e8d35302, :c_ecc8ec55, :c_eed60aa2, :c_ef4fcc0c, :c_ef814787, :c_f23ce991, :c_f8a6d299,
    :c_fcfbbcd0;
  skosxl:prefLabel :xl_en_75c407e4 .

:skosCollection_4d3f42cb a skos:Collection;
  dct:created "2018-07-22T14:23:03.497Z"^^xsd:dateTime;
  dct:modified "2019-11-30T10:54:06.928Z"^^xsd:dateTime;
  skos:member :c_08fa2f6e, :c_2b89905f, :c_2d69d738, :c_443bf05e, :c_55b465e8, :c_5cd4aa00,
    :c_5f10d43b, :c_607b5b8a, :c_79de880f, :c_87804062, :c_87bf8d98, :c_930416d1, :c_b019c6a7,
    :c_c0f70902, :c_cf6c5d63, :c_da247d5e, :c_e4e408ec, :c_ede99420, :c_fa052d43, :c_fb2c64cc;
  skosxl:prefLabel :xl_en_fdd7e66a .

:skosCollection_77325868 a skos:Collection;
  dct:created "2018-07-20T22:28:41.750Z"^^xsd:dateTime;
  dct:modified "2019-11-30T10:55:28.192Z"^^xsd:dateTime;
  skos:member :c_01bda236, :c_0d539813, :c_105811e3, :c_11f27c78, :c_1258140e, :c_162b9e61,
    :c_1e86ab1c, :c_20cde89c, :c_2eb971b3, :c_324b2ef1, :c_369e4bb6, :c_36f0ebbb, :c_386bb74f,
    :c_3c62e145, :c_46f20ab0, :c_49e95986, :c_4a31c73a, :c_517519ce, :c_55d219f9, :c_69e09153,
    :c_717bb7fd, :c_782fa318, :c_7b22749d, :c_86ba3858, :c_87ff7e6c, :c_901951db, :c_9260f33c,
    :c_9509873f, :c_974b12d0, :c_97ba48a0, :c_9a568eaa, :c_9e715393, :c_b0503f89, :c_b781cfae,
    :c_b7c13cf0, :c_b86b8a23, :c_bd6073c7, :c_be027528, :c_c048d0a8, :c_c4f5d4fc, :c_d0f52b80,
    :c_d19fc7a3, :c_db8a3f56, :c_dca128d9, :c_de6816aa, :c_e231ef90, :c_ed68836f, :c_edaf8450,
    :c_f569343b;
  skosxl:prefLabel :xl_en_7196b0dc .

:skosCollection_b565257c a skos:Collection;
  dct:created "2018-07-22T15:11:25.899Z"^^xsd:dateTime;
  dct:modified "2019-11-30T10:55:03.114Z"^^xsd:dateTime;
  skos:member :c_24506d00, :c_26348e8a, :c_32da9577, :c_3c4ef6f5, :c_5ae807c5, :c_624f6410,
    :c_6c460406, :c_8741d02b, :c_9c1d7995, :c_9d3f953f, :c_ac25e497, :c_af7e5693, :c_b470c6f5,
    :c_b4f95391, :c_bba5abb9, :c_c4204198, :c_d837a7ac, :c_f897a1c6;
  skosxl:prefLabel :xl_en_34cc7b6c .

:skosCollection_dca655b9 a skos:Collection;
  dct:created "2018-08-11T08:38:02.655Z"^^xsd:dateTime;
  dct:modified "2019-11-30T10:54:36.633Z"^^xsd:dateTime;
  skos:member :c_02f182a2, :c_04a3b08d, :c_086e071c, :c_0b45b235, :c_0fc93a91, :c_13d79d5e,
    :c_14426eb2, :c_161ac3be, :c_1b065c63, :c_1e1d6eeb, :c_250f029d, :c_2ce0c940, :c_34b987d4,
    :c_36ce18a2, :c_3c5e3daa, :c_3e2995a1, :c_3fd4eac3, :c_412f9c62, :c_49cc400a, :c_4a7bbbda,
    :c_59dcd59c, :c_5d8254a8, :c_5e5901cb, :c_692f83c4, :c_6c31e8f5, :c_6cd2fa76, :c_6ceaacc1,
    :c_71eda773, :c_73726e27, :c_75f1aa77, :c_76b17e4d, :c_7e8703b2, :c_7f9323cb, :c_80aeab06,
    :c_8b778c41, :c_8cad0fd2, :c_90ff7ddf, :c_9e61f9a1, :c_9ef52cee, :c_a1cd3dcb, :c_a9c2e902,
    :c_ace7ce12, :c_adba6615, :c_ade56523, :c_b227f284, :c_b2e826d0, :c_b65fa6fd, :c_b932ae7e,
    :c_bce20c84, :c_d8e2bacb, :c_d9ed5f11, :c_eb6b96ad, :c_ed146474, :c_edf75137, :c_f443f164;
  skosxl:prefLabel :xl_en_70364cc4 .

:xl_en_75c407e4 a skosxl:Label;
  dct:modified "2018-07-22T15:10:35.034Z"^^xsd:dateTime;
  skosxl:literalForm "type documents"@en .

:skosCollection_301a56ed a skos:Collection;
  dct:created "2018-07-20T20:32:00.722Z"^^xsd:dateTime;
  dct:modified "2019-11-30T10:52:46.682Z"^^xsd:dateTime;
  skos:member :c_32bf6806, :c_46da6c1c, :c_49888cc9, :c_6859ada6, :c_9c1d7995, :c_9d3f953f,
    :c_ac615319, :c_af7e5693, :c_b2459321, :c_f23ce991, :c_f8a6d299, :c_fbbe4f85;
  skos:prefLabel "handover pack (housing)"@en .

:skosCollection_3063372a skos:prefLabel "development stages (housing)"@en .

:skosCollection_059e795f skos:prefLabel "contents of health and safety file (housing)"@en .

:skosCollection_42952ecf dct:created "2018-08-11T08:35:23.556Z"^^xsd:dateTime .

:xl_en_fdd7e66a a skosxl:Label;
  skosxl:literalForm "location"@en .

:xl_en_7196b0dc a skosxl:Label;
  skosxl:literalForm "role"@en .

:xl_en_34cc7b6c a skosxl:Label;
  skosxl:literalForm "type drawings"@en .

:xl_en_70364cc4 a skosxl:Label;
  skosxl:literalForm "volumes"@en .

:c_05a3b5d1 a skos:Concept;
  dc:source "Interim Advice Note 184/16 Highways England CAD and Data Standard"@en;
  dct:created "2018-08-19T12:11:03.729Z"^^xsd:dateTime;
  dct:modified "2020-10-31T05:19:45.216Z"^^xsd:dateTime;
  skos:broader :c_618864b7;
  skos:editorialNote """Functional specification
(PLQ, Non-technical requirements)"""@en;
  skos:inScheme :conceptScheme_751925ed;
  skos:notation "FS"@en;
  skosxl:prefLabel :xl_en_73c840ba .

:xl_en_73c840ba a skosxl:Label;
  skosxl:literalForm "functional specification"@en .

:c_0d539813 a skos:Concept;
  dc:source "Interim Advice Note 184/16 Highways England CAD and Data Standard"@en;
  dct:created "2018-08-22T15:39:20.195Z"^^xsd:dateTime;
  dct:modified "2020-10-31T04:49:11.825Z"^^xsd:dateTime;
  skos:broader :c_2425ea08;
  skos:inScheme :conceptScheme_751925ed;
  skos:notation "EO"@en;
  skosxl:prefLabel :xl_en_0de5013f .

:xl_en_0de5013f a skosxl:Label;
  skosxl:literalForm "lighting engineer"@en .

:c_1081a7c2 a skos:Concept;
  dc:source "Interim Advice Note 184/16 Highways England CAD and Data Standard"@en;
  dct:created "2018-08-20T10:02:52.653Z"^^xsd:dateTime;
  dct:modified "2020-10-31T04:52:50.311Z"^^xsd:dateTime;
  skos:broader :c_618864b7;
  skos:editorialNote "Design change requests etc"@en;
  skos:inScheme :conceptScheme_751925ed;
  skos:notation "RS"@en;
  skosxl:prefLabel :xl_en_b79235bf .

:xl_en_b79235bf a skosxl:Label;
  dct:modified "2018-08-20T10:03:17.659Z"^^xsd:dateTime;
  skosxl:literalForm "site change request"@en .

:c_1258140e a skos:Concept;
  dc:source "Interim Advice Note 184/16 Highways England CAD and Data Standard"@en;
  dct:created "2018-08-20T15:43:09.733Z"^^xsd:dateTime;
  dct:modified "2020-10-31T05:25:14.851Z"^^xsd:dateTime;
  skos:broader :c_2425ea08;
  skos:inScheme :conceptScheme_751925ed;
  skos:notation "CH"@en;
  skosxl:prefLabel :xl_en_50bf8f3c .

:xl_en_50bf8f3c a skosxl:Label;
  skosxl:literalForm "civil-highways"@en .

:c_1e86ab1c a skos:Concept;
  dc:source "Interim Advice Note 184/16 Highways England CAD and Data Standard"@en;
  dct:created "2018-08-22T15:41:48.732Z"^^xsd:dateTime;
  dct:modified "2020-10-31T05:18:33.150Z"^^xsd:dateTime;
  skos:broader :c_b8f9acb4;
  skos:inScheme :conceptScheme_751925ed;
  skos:notation "GI"@en;
  skosxl:prefLabel :xl_en_1ce2b898 .

:xl_en_1ce2b898 a skosxl:Label;
  dct:modified "2018-08-22T15:44:13.156Z"^^xsd:dateTime;
  skosxl:literalForm "geospatial (role)"@en .

:c_2238ee39 a skos:Concept;
  dc:source "Interim Advice Note 184/16 Highways England CAD and Data Standard"@en;
  dct:created "2018-08-19T09:02:57.891Z"^^xsd:dateTime;
  dct:modified "2020-10-31T05:08:13.518Z"^^xsd:dateTime;
  skos:broader :c_618864b7;
  skos:editorialNote "Used by Commercial only"@en;
  skos:inScheme :conceptScheme_751925ed;
  skos:notation "CD"@en;
  skosxl:prefLabel :xl_en_c0714244 .

:xl_en_c0714244 a skosxl:Label;
  skosxl:literalForm "contract documents"@en .

:c_36f0ebbb a skos:Concept;
  dc:source "Interim Advice Note 184/16 Highways England CAD and Data Standard"@en;
  dct:created "2018-08-20T10:23:00.210Z"^^xsd:dateTime;
  dct:modified "2020-10-31T05:40:41.833Z"^^xsd:dateTime;
  skos:broader :c_2425ea08;
  skos:inScheme :conceptScheme_751925ed;
  skos:notation "CB"@en;
  skosxl:prefLabel :xl_en_347754f2 .

:c_386bb74f a skos:Concept;
  dc:source "Interim Advice Note 184/16 Highways England CAD and Data Standard"@en;
  dct:created "2018-08-22T15:37:05.718Z"^^xsd:dateTime;
  dct:modified "2020-10-30T20:34:22.447Z"^^xsd:dateTime;
  skos:broader :c_2425ea08;
  skos:inScheme :conceptScheme_751925ed;
  skos:notation "EC"@en;
  skosxl:prefLabel :xl_en_045311bc .

:c_782fa318 a skos:Concept;
  dc:source "Interim Advice Note 184/16 Highways England CAD and Data Standard"@en;
  dct:created "2018-08-20T15:40:56.475Z"^^xsd:dateTime;
  dct:modified "2020-10-31T05:12:46.816Z"^^xsd:dateTime;
  skos:broader :c_2425ea08;
  skos:inScheme :conceptScheme_751925ed;
  skos:notation "CE"@en;
  skosxl:prefLabel :xl_en_d5ef7cd5 .

:c_9260f33c a skos:Concept;
  dc:source "Interim Advice Note 184/16 Highways England CAD and Data Standard"@en;
  dct:created "2018-08-22T15:55:17.630Z"^^xsd:dateTime;
  skos:broader :c_2425ea08;
  skos:inScheme :conceptScheme_751925ed;
  skos:notation "TR"@en;
  skos:prefLabel "civil-traffic modelling"@en;
  skosxl:prefLabel :xl_en_2c20be11 .

:c_bd6073c7 a skos:Concept;
  dc:source "Interim Advice Note 184/16 Highways England CAD and Data Standard"@en;
  dct:created "2018-08-22T15:34:28.350Z"^^xsd:dateTime;
  dct:modified "2020-10-31T05:37:28.859Z"^^xsd:dateTime;
  skos:broader :c_2425ea08;
  skos:inScheme :conceptScheme_751925ed;
  skos:notation "CW"@en;
  skosxl:prefLabel :xl_en_ec48942c .

:c_c4f5d4fc a skos:Concept;
  dc:source "Interim Advice Note 184/16 Highways England CAD and Data Standard"@en;
  dct:created "2018-08-20T10:25:07.495Z"^^xsd:dateTime;
  dct:modified "2020-10-31T05:24:20.935Z"^^xsd:dateTime;
  skos:broader :c_2425ea08;
  skos:inScheme :conceptScheme_751925ed;
  skos:notation "CD"@en;
  skosxl:prefLabel :xl_en_ac6f7f83 .

:c_edaf8450 a skos:Concept;
  dc:source "Interim Advice Note 184/16 Highways England CAD and Data Standard"@en;
  dct:created "2018-08-22T15:31:52.072Z"^^xsd:dateTime;
  dct:modified "2020-10-31T05:07:52.170Z"^^xsd:dateTime;
  skos:broader :c_2425ea08;
  skos:inScheme :conceptScheme_751925ed;
  skos:notation "CU"@en;
  skosxl:prefLabel :xl_en_95dff570 .

:c_2592b8ec a skos:Concept;
  dc:source "Interim Advice Note 184/16 Highways England CAD and Data Standard"@en;
  dct:created "2018-08-19T11:59:20.190Z"^^xsd:dateTime;
  skos:broader :c_618864b7;
  skos:inScheme :conceptScheme_751925ed;
  skos:notation "DT"@en;
  skos:prefLabel "document transmittal note"@en;
  skosxl:prefLabel :xl_en_7f20258e .

:xl_en_7f20258e a skosxl:Label;
  skosxl:literalForm "document transmittal note"@en .

:c_b781cfae a skos:Concept;
  dc:source "Interim Advice Note 184/16 Highways England CAD and Data Standard"@en;
  dct:created "2018-08-22T16:08:27.500Z"^^xsd:dateTime;
  skos:broader :c_2664d806;
  skos:inScheme :conceptScheme_751925ed;
  skos:notation "ZQ"@en;
  skos:prefLabel "quality assurance (role)"@en;
  skosxl:prefLabel :xl_en_099ffa2a .

:c_2b89905f a skos:Concept;
  dct:created "2018-08-19T08:12:22.315Z"^^xsd:dateTime;
  dct:modified "2020-10-30T20:45:49.143Z"^^xsd:dateTime;
  skos:broader :c_e5b1b611;
  skos:inScheme :conceptScheme_751925ed;
  skos:notation "L1"@en;
  skosxl:prefLabel :xl_en_09354c3d .

:xl_en_09354c3d a skosxl:Label;
  dc:source """production information a code of procedure for the construction industry
Organization of information about construction works — Information management using building information modelling - Part 2:Delivery phase of assets"""@en;
  skos:notation "L1"@en;
  skosxl:literalForm "link 1"@en .

:c_369e4bb6 a skos:Concept;
  dc:source "Interim Advice Note 184/16 Highways England CAD and Data Standard"@en;
  dct:created "2018-08-22T15:52:04.737Z"^^xsd:dateTime;
  dct:modified "2020-10-31T05:13:04.860Z"^^xsd:dateTime;
  skos:broader :c_b8f9acb4;
  skos:inScheme :conceptScheme_751925ed;
  skos:notation "LH"@en;
  skosxl:prefLabel :xl_en_7c5bf386 .

:xl_en_7c5bf386 a skosxl:Label;
  skosxl:literalForm "landscape and environment-heritage"@en .

:xl_en_347754f2 a skosxl:Label;
  dct:modified "2018-08-20T15:40:03.130Z"^^xsd:dateTime;
  skosxl:literalForm "civil-bridges and structures"@en .

:xl_en_045311bc a skosxl:Label;
  skosxl:literalForm "electrical-control systems and technology"@en .

:c_38840388 a skos:Concept;
  dct:created "2018-08-20T15:44:47.263Z"^^xsd:dateTime;
  skos:broader :c_2425ea08;
  skos:inScheme :conceptScheme_751925ed;
  skosxl:prefLabel :xl_en_dc1fb585 .

:xl_en_dc1fb585 a skosxl:Label;
  skosxl:literalForm "civil-tunnels"@en .

:c_41bc9708 a skos:Concept;
  dc:source "Interim Advice Note 184/16 Highways England CAD and Data Standard"@en;
  dct:created "2018-08-20T10:05:08.552Z"^^xsd:dateTime;
  dct:modified "2020-10-31T05:39:52.057Z"^^xsd:dateTime;
  skos:broader :c_618864b7;
  skos:editorialNote """To cover Human Resources and
contractual discussions"""@en;
  skos:inScheme :conceptScheme_751925ed;
  skos:notation "RT"@en;
  skosxl:prefLabel :xl_en_cdf4625c .

:xl_en_cdf4625c a skosxl:Label;
  skosxl:literalForm "reconciliation"@en .

:c_517519ce a skos:Concept;
  dc:source "Interim Advice Note 184/16 Highways England CAD and Data Standard"@en;
  dct:created "2018-08-22T16:01:10.127Z"^^xsd:dateTime;
  dct:modified "2020-10-31T05:26:38.415Z"^^xsd:dateTime;
  skos:broader :c_d7f03766;
  skos:inScheme :conceptScheme_751925ed;
  skos:notation "ZC"@en;
  skosxl:prefLabel :xl_en_5bc2e3f7 .

:xl_en_5bc2e3f7 a skosxl:Label;
  dct:modified "2018-08-22T16:01:41.152Z"^^xsd:dateTime;
  skosxl:literalForm "commercial and cost management (role)"@en .

:c_536a60e1 a skos:Concept;
  dc:source "Interim Advice Note 184/16 Highways England CAD and Data Standard"@en;
  dct:created "2018-08-19T08:52:30.983Z"^^xsd:dateTime;
  dct:modified "2020-10-30T21:00:45.473Z"^^xsd:dateTime;
  skos:broader :c_618864b7;
  skos:editorialNote "Used by Commercial only"@en;
  skos:inScheme :conceptScheme_751925ed;
  skos:notation "CC"@en;
  skosxl:prefLabel :xl_en_0fcad60f .

:xl_en_0fcad60f a skosxl:Label;
  skosxl:literalForm "contract certificates"@en .

:c_86ba3858 a skos:Concept;
  dc:source "Interim Advice Note 184/16 Highways England CAD and Data Standard"@en;
  dct:created "2018-08-22T16:03:39.272Z"^^xsd:dateTime;
  dct:modified "2020-10-31T05:39:35.918Z"^^xsd:dateTime;
  skos:broader :c_54bbebe2;
  skos:inScheme :conceptScheme_751925ed;
  skos:notation "ZH"@en;
  skosxl:prefLabel :xl_en_93f0315c .

:c_55b465e8 a skos:Concept;
  dc:source "Interim Advice Note 184/16 Highways England CAD and Data Standard"@en;
  dct:created "2018-08-19T08:09:28.867Z"^^xsd:dateTime;
  dct:modified "2020-10-31T05:08:48.443Z"^^xsd:dateTime;
  skos:broader :c_e5b1b611;
  skos:inScheme :conceptScheme_751925ed;
  skos:notation "S1"@en;
  skosxl:prefLabel :xl_en_988b5593 .

:xl_en_988b5593 a skosxl:Label;
  dc:source """production information a code of procedure for the construction industry
Organization of information about construction works — Information management using building information modelling - Part 2:Delivery phase of assets"""@en;
  skos:notation "S1"@en;
  skosxl:literalForm "section 1"@en .

:c_5ac38c99 a skos:Concept;
  dc:source "Interim Advice Note 184/16 Highways England CAD and Data Standard"@en;
  dct:created "2018-08-20T09:43:12.513Z"^^xsd:dateTime;
  dct:modified "2020-10-31T04:57:19.871Z"^^xsd:dateTime;
  skos:broader :c_618864b7;
  skos:inScheme :conceptScheme_751925ed;
  skos:notation "LI"@en;
  skosxl:prefLabel :xl_en_3ab074bd .

:xl_en_3ab074bd a skosxl:Label;
  skosxl:literalForm "licence"@en .

:c_5d17180d a skos:Concept;
  dc:source "Interim Advice Note 184/16 Highways England CAD and Data Standard"@en;
  dct:created "2018-08-20T09:46:55.962Z"^^xsd:dateTime;
  dct:modified "2020-10-31T05:42:05.755Z"^^xsd:dateTime;
  skos:broader :c_618864b7;
  skos:inScheme :conceptScheme_751925ed;
  skos:notation "NC"@en;
  skosxl:prefLabel :xl_en_068c4260 .

:xl_en_068c4260 a skosxl:Label;
  skosxl:literalForm "non conformance report"@en .

:c_5f10d43b a skos:Concept;
  dc:source "Interim Advice Note 184/16 Highways England CAD and Data Standard"@en;
  dct:created "2018-08-19T08:13:43.805Z"^^xsd:dateTime;
  dct:modified "2020-10-31T05:06:00.545Z"^^xsd:dateTime;
  skos:broader :c_e5b1b611;
  skos:inScheme :conceptScheme_751925ed;
  skos:notation "ML"@en;
  skosxl:prefLabel :xl_en_2c97f758 .

:xl_en_2c97f758 a skosxl:Label;
  dc:source """production information a code of procedure for the construction industry
Organization of information about construction works — Information management using building information modelling - Part 2:Delivery phase of assets"""@en;
  skos:notation "ML"@en;
  skosxl:literalForm "mainline"@en .

:c_68039062 a skos:Concept;
  dc:source "Interim Advice Note 184/16 Highways England CAD and Data Standard"@en;
  dct:created "2018-08-20T09:40:17.561Z"^^xsd:dateTime;
  dct:modified "2020-10-30T20:47:53.872Z"^^xsd:dateTime;
  skos:broader :c_618864b7;
  skos:inScheme :conceptScheme_751925ed;
  skos:notation "IS"@en;
  skosxl:prefLabel :xl_en_785815a0 .

:c_8046ed58 a skos:Concept;
  dc:source "Interim Advice Note 184/16 Highways England CAD and Data Standard"@en;
  dct:created "2018-08-19T10:09:06.382Z"^^xsd:dateTime;
  skos:broader :c_618864b7;
  skos:editorialNote "Email, Fax, Letter, File Note, Memo"@en;
  skos:inScheme :conceptScheme_751925ed;
  skos:notation "CI"@en;
  skos:prefLabel "correspondence incoming"@en;
  skosxl:prefLabel :xl_en_df3fb955 .

:c_8d5846c3 a skos:Concept;
  dc:source "Interim Advice Note 184/16 Highways England CAD and Data Standard"@en;
  dct:created "2018-08-19T11:52:27.519Z"^^xsd:dateTime;
  dct:modified "2020-10-31T04:41:51.322Z"^^xsd:dateTime;
  skos:broader :c_618864b7;
  skos:inScheme :conceptScheme_751925ed;
  skos:notation "DS"@en;
  skosxl:prefLabel :xl_en_945bcfee .

:c_9832f0b7 a skos:Concept;
  dc:source "Interim Advice Note 184/16 Highways England CAD and Data Standard"@en;
  dct:created "2018-08-20T09:48:22.338Z"^^xsd:dateTime;
  dct:modified "2020-10-30T20:49:21.036Z"^^xsd:dateTime;
  skos:broader :c_618864b7;
  skos:inScheme :conceptScheme_751925ed;
  skos:notation "PH"@en;
  skosxl:prefLabel :xl_en_9dc1bd11 .

:c_98522fb2 a skos:Concept;
  dc:source "Interim Advice Note 184/16 Highways England CAD and Data Standard"@en;
  dct:created "2018-08-20T10:01:20.191Z"^^xsd:dateTime;
  dct:modified "2020-10-31T04:51:53.329Z"^^xsd:dateTime;
  skos:broader :c_618864b7;
  skos:inScheme :conceptScheme_751925ed;
  skos:notation "RM"@en;
  skosxl:prefLabel :xl_en_f7f3d2f3 .

:c_98ba4c18 a skos:Concept;
  dc:source "Interim Advice Note 184/16 Highways England CAD and Data Standard"@en;
  dct:created "2018-08-19T10:15:20.874Z"^^xsd:dateTime;
  dct:modified "2020-10-31T05:35:07.835Z"^^xsd:dateTime;
  skos:broader :c_618864b7;
  skos:inScheme :conceptScheme_751925ed;
  skos:notation "DF"@en;
  skosxl:prefLabel :xl_en_4f3a5af6 .

:c_9e9aa534 a skos:Concept;
  dc:source "Interim Advice Note 184/16 Highways England CAD and Data Standard"@en;
  dct:created "2018-08-20T09:50:20.260Z"^^xsd:dateTime;
  dct:modified "2020-10-31T05:05:08.348Z"^^xsd:dateTime;
  skos:broader :c_618864b7;
  skos:inScheme :conceptScheme_751925ed;
  skos:notation "PT"@en;
  skosxl:prefLabel :xl_en_8fa8020d .

:c_9ebfa246 a skos:Concept;
  dc:source "Interim Advice Note 184/16 Highways England CAD and Data Standard"@en;
  dct:created "2018-08-20T09:44:59.494Z"^^xsd:dateTime;
  dct:modified "2020-10-31T05:04:15.266Z"^^xsd:dateTime;
  skos:broader :c_618864b7;
  skos:inScheme :conceptScheme_751925ed;
  skos:notation "LN"@en;
  skosxl:prefLabel :xl_en_aba56f1e .

:c_a47e6a9b a skos:Concept;
  dc:source "Interim Advice Note 184/16 Highways England CAD and Data Standard"@en;
  dct:created "2018-08-19T11:43:38.985Z"^^xsd:dateTime;
  skos:broader :c_618864b7;
  skos:inScheme :conceptScheme_751925ed;
  skos:notation "DI"@en;
  skos:prefLabel "design site instruction"@en;
  skosxl:prefLabel :xl_en_c0901abd .

:c_a7289a25 a skos:Concept;
  dc:source "Interim Advice Note 184/16 Highways England CAD and Data Standard"@en;
  dct:created "2018-08-20T10:12:53.036Z"^^xsd:dateTime;
  skos:broader :c_618864b7;
  skos:editorialNote "Deliverables Tracker, MIDP, TIDP"@en;
  skos:inScheme :conceptScheme_751925ed;
  skos:notation "TK"@en;
  skos:prefLabel "tracker"@en;
  skosxl:prefLabel :xl_en_d3eb53d0 .

:c_b3508a0f a skos:Concept;
  dc:source "Interim Advice Note 184/16 Highways England CAD and Data Standard"@en;
  dct:created "2018-08-19T09:21:51.018Z"^^xsd:dateTime;
  skos:broader :c_618864b7;
  skos:editorialNote "Register of changes etc"@en;
  skos:inScheme :conceptScheme_751925ed;
  skos:notation "CH"@en;
  skos:prefLabel "change control document"@en;
  skosxl:prefLabel :xl_en_93d48f5b .

:c_c989802e a skos:Concept;
  dc:source "Interim Advice Note 184/16 Highways England CAD and Data Standard"@en;
  dct:created "2018-08-20T09:38:49.049Z"^^xsd:dateTime;
  dct:modified "2020-10-31T05:26:22.133Z"^^xsd:dateTime;
  skos:broader :c_618864b7;
  skos:inScheme :conceptScheme_751925ed;
  skos:notation "IN"@en;
  skosxl:prefLabel :xl_en_7ebb38ae .

:c_d37e6d79 a skos:Concept;
  dc:source "Interim Advice Note 184/16 Highways England CAD and Data Standard"@en;
  dct:created "2018-08-19T12:06:31.520Z"^^xsd:dateTime;
  dct:modified "2020-10-31T05:10:02.417Z"^^xsd:dateTime;
  skos:broader :c_618864b7;
  skos:editorialNote "Internal process forms"@en;
  skos:inScheme :conceptScheme_751925ed;
  skos:notation "FM"@en;
  skosxl:prefLabel :xl_en_2e2f6167 .

:c_d71b62e2 a skos:Concept;
  dc:source "Interim Advice Note 184/16 Highways England CAD and Data Standard"@en;
  dct:created "2018-08-19T12:03:09.340Z"^^xsd:dateTime;
  dct:modified "2020-10-31T05:42:37.275Z"^^xsd:dateTime;
  skos:broader :c_618864b7;
  skos:inScheme :conceptScheme_751925ed;
  skos:notation "EW"@en;
  skosxl:prefLabel :xl_en_86ca8f53 .

:c_db373352 a skos:Concept;
  dc:source "Interim Advice Note 184/16 Highways England CAD and Data Standard"@en;
  dct:created "2018-08-19T11:47:40.357Z"^^xsd:dateTime;
  dct:modified "2020-10-31T05:09:42.549Z"^^xsd:dateTime;
  skos:broader :c_618864b7;
  skos:editorialNote """Contractual notifications of
Design Changes"""@en;
  skos:inScheme :conceptScheme_751925ed;
  skos:notation "DN"@en;
  skosxl:prefLabel :xl_en_36537239 .

:c_e2fbc29a a skos:Concept;
  dc:source "Interim Advice Note 184/16 Highways England CAD and Data Standard"@en;
  dct:created "2018-08-20T09:51:38.605Z"^^xsd:dateTime;
  dct:modified "2020-10-31T04:42:32.565Z"^^xsd:dateTime;
  skos:broader :c_618864b7;
  skos:inScheme :conceptScheme_751925ed;
  skos:notation "RA"@en;
  skosxl:prefLabel :xl_en_47c2d55f .

:c_e8a3f333 a skos:Concept;
  dc:source "Interim Advice Note 184/16 Highways England CAD and Data Standard"@en;
  dct:created "2018-08-19T09:16:57.487Z"^^xsd:dateTime;
  dct:modified "2020-10-31T05:31:09.088Z"^^xsd:dateTime;
  skos:broader :c_618864b7;
  skos:editorialNote "Used by Commercial only"@en;
  skos:inScheme :conceptScheme_751925ed;
  skos:notation "CE"@en;
  skosxl:prefLabel :xl_en_a39943b3 .

:c_e8d35302 a skos:Concept;
  dc:source "Interim Advice Note 184/16 Highways England CAD and Data Standard"@en;
  dct:created "2018-08-20T09:37:26.605Z"^^xsd:dateTime;
  dct:modified "2020-10-30T20:47:35.777Z"^^xsd:dateTime;
  skos:broader :c_618864b7;
  skos:inScheme :conceptScheme_751925ed;
  skos:notation "IC"@en;
  skosxl:prefLabel :xl_en_c897327d .

:c_ef4fcc0c a skos:Concept;
  dc:source "Interim Advice Note 184/16 Highways England CAD and Data Standard"@en;
  dct:created "2018-08-20T09:41:49.405Z"^^xsd:dateTime;
  dct:modified "2020-10-31T05:40:59.502Z"^^xsd:dateTime;
  skos:broader :c_618864b7;
  skos:inScheme :conceptScheme_751925ed;
  skos:notation "IT"@en;
  skosxl:prefLabel :xl_en_e1702714 .

:c_624f6410 a skos:Concept;
  dc:source "Interim Advice Note 184/16 Highways England CAD and Data Standard"@en;
  dct:created "2018-08-20T09:34:18.313Z"^^xsd:dateTime;
  dct:modified "2020-10-31T05:05:43.130Z"^^xsd:dateTime;
  skos:broader :c_b7ef2137;
  skos:inScheme :conceptScheme_751925ed;
  skos:notation "GS"@en;
  skosxl:prefLabel :xl_en_93cced32 .

:xl_en_93cced32 a skosxl:Label;
  skosxl:literalForm "gis dataset"@en .

:xl_en_785815a0 a skosxl:Label;
  skosxl:literalForm "instruction"@en .

:c_6cbca36f dct:created "2018-08-20T10:00:12.829Z"^^xsd:dateTime .

:xl_en_d5ef7cd5 a skosxl:Label;
  skosxl:literalForm "civil-earthworks and geotechnics"@en .

:c_79de880f a skos:Concept;
  dc:source "Interim Advice Note 184/16 Highways England CAD and Data Standard"@en;
  dct:created "2018-08-19T08:10:06.896Z"^^xsd:dateTime;
  dct:modified "2020-10-31T05:17:43.655Z"^^xsd:dateTime;
  skos:broader :c_e5b1b611;
  skos:inScheme :conceptScheme_751925ed;
  skos:notation "S2"@en;
  skosxl:prefLabel :xl_en_d450f943 .

:xl_en_d450f943 a skosxl:Label;
  dc:source """production information a code of procedure for the construction industry
Organization of information about construction works — Information management using building information modelling - Part 2:Delivery phase of assets"""@en;
  skos:notation "S2"@en;
  skosxl:literalForm "section 2"@en .

:xl_en_df3fb955 a skosxl:Label;
  skosxl:literalForm "correspondence incoming"@en .

:xl_en_93f0315c a skosxl:Label;
  skosxl:literalForm "stakeholder liaison"@en .

:c_8741d02b a skos:Concept;
  dc:source "Interim Advice Note 184/16 Highways England CAD and Data Standard"@en;
  dct:created "2018-08-19T10:12:37.864Z"^^xsd:dateTime;
  dct:modified "2020-10-31T05:24:37.519Z"^^xsd:dateTime;
  skos:broader :c_b7ef2137;
  skos:editorialNote """Standard detail drawings and
content not included in the model"""@en;
  skos:inScheme :conceptScheme_751925ed;
  skos:notation "DE"@en;
  skosxl:prefLabel :xl_en_8e62ea51 .

:xl_en_8e62ea51 a skosxl:Label;
  skosxl:literalForm "detail drawing"@en .

:xl_en_945bcfee a skosxl:Label;
  skosxl:literalForm "diary-activity sheet"@en .

:xl_en_2c20be11 a skosxl:Label;
  skosxl:literalForm "civil-traffic modelling"@en .

:c_930416d1 a skos:Concept;
  dc:source "Interim Advice Note 184/16 Highways England CAD and Data Standard"@en;
  dct:created "2018-08-19T08:48:15.314Z"^^xsd:dateTime;
  dct:modified "2020-10-31T04:57:37.111Z"^^xsd:dateTime;
  skos:broader :c_e5b1b611;
  skos:inScheme :conceptScheme_751925ed;
  skos:notation "CR"@en;
  skosxl:prefLabel :xl_en_9c41fe5d .

:xl_en_9c41fe5d a skosxl:Label;
  skosxl:literalForm "central reservation"@en .

:xl_en_9dc1bd11 a skosxl:Label;
  skosxl:literalForm "photographs"@en .

:xl_en_f7f3d2f3 a skosxl:Label;
  skosxl:literalForm "rams-wasp"@en .

:xl_en_4f3a5af6 a skosxl:Label;
  skosxl:literalForm "departure submissions"@en .

:xl_en_1b847882 a skosxl:Label;
  skosxl:literalForm "legal"@en .

:xl_en_8fa8020d a skosxl:Label;
  skosxl:literalForm "permit"@en .

:xl_en_aba56f1e a skosxl:Label;
  skosxl:literalForm "legal notices-orders"@en .

:xl_en_c0901abd a skosxl:Label;
  skosxl:literalForm "design site instruction"@en .

:xl_en_d3eb53d0 a skosxl:Label;
  skosxl:literalForm "tracker"@en .

:c_ac25e497 a skos:Concept;
  dc:source "Interim Advice Note 184/16 Highways England CAD and Data Standard"@en;
  dct:created "2018-08-20T10:09:13.261Z"^^xsd:dateTime;
  dct:modified "2020-10-30T20:29:48.259Z"^^xsd:dateTime;
  skos:broader :c_b7ef2137;
  skos:editorialNote "Typically singular plan-section,not for HA approval"@en;
  skos:inScheme :conceptScheme_751925ed;
  skos:notation "SK"@en;
  skosxl:prefLabel :xl_en_f0feb4f0 .

:xl_en_f0feb4f0 a skosxl:Label;
  skosxl:literalForm "sketch"@en .

:xl_en_93d48f5b a skosxl:Label;
  skosxl:literalForm "change control document"@en .

:xl_en_099ffa2a a skosxl:Label;
  dct:modified "2018-08-22T16:09:54.495Z"^^xsd:dateTime;
  skosxl:literalForm "quality assurance (role)"@en .

:c_f897a1c6 a skos:Concept;
  dc:source "Interim Advice Note 184/16 Highways England CAD and Data Standard"@en;
  dct:created "2018-08-20T10:07:14.533Z"^^xsd:dateTime;
  skos:broader :c_b7ef2137;
  skos:editorialNote """Model based on chainage, eg for
communications drawings"""@en;
  skos:inScheme :conceptScheme_751925ed;
  skos:notation "SC"@en;
  skos:prefLabel "schematic"@en;
  skosxl:prefLabel :xl_en_f3446da3 .

:c_b86b8a23 a skos:Concept;
  dc:source "Interim Advice Note 184/16 Highways England CAD and Data Standard"@en;
  dct:created "2018-08-22T15:49:35.010Z"^^xsd:dateTime;
  dct:modified "2020-10-30T21:00:08.461Z"^^xsd:dateTime;
  skos:broader :c_b8f9acb4;
  skos:inScheme :conceptScheme_751925ed;
  skos:notation "LE"@en;
  skosxl:prefLabel :xl_en_8fb7d7ca .

:xl_en_8fb7d7ca a skosxl:Label;
  skosxl:literalForm "landscape and environment-environmentalist"@en .

:c_de6816aa a skos:Concept;
  dc:source "Interim Advice Note 184/16 Highways England CAD and Data Standard"@en;
  dct:created "2018-08-22T15:47:23.652Z"^^xsd:dateTime;
  dct:modified "2020-10-31T05:06:22.016Z"^^xsd:dateTime;
  skos:broader :c_b8f9acb4;
  skos:inScheme :conceptScheme_751925ed;
  skos:notation "LA"@en;
  skosxl:prefLabel :xl_en_b34686a9 .

:xl_en_ec48942c a skosxl:Label;
  skosxl:literalForm "civil-temporary works"@en .

:xl_en_ac6f7f83 a skosxl:Label;
  dct:modified "2018-08-20T15:40:18.175Z"^^xsd:dateTime;
  skosxl:literalForm "civil-drainage"@en .

:xl_en_7ebb38ae a skosxl:Label;
  skosxl:literalForm "invoice"@en .

:c_cf6c5d63 a skos:Concept;
  dc:source "Interim Advice Note 184/16 Highways England CAD and Data Standard"@en;
  dct:created "2018-08-19T08:13:17.254Z"^^xsd:dateTime;
  dct:modified "2020-10-31T05:10:37.034Z"^^xsd:dateTime;
  skos:broader :c_e5b1b611;
  skos:inScheme :conceptScheme_751925ed;
  skos:notation "JN"@en;
  skosxl:prefLabel :xl_en_9dc9ba74 .

:xl_en_9dc9ba74 a skosxl:Label;
  dct:modified "2018-08-19T08:38:20.850Z"^^xsd:dateTime;
  skosxl:literalForm "junction"@en .

:c_d19fc7a3 a skos:Concept;
  dc:source "Interim Advice Note 184/16 Highways England CAD and Data Standard"@en;
  dct:created "2018-08-20T10:20:47.431Z"^^xsd:dateTime;
  dct:modified "2019-11-30T10:59:43.483Z"^^xsd:dateTime;
  skos:broader :c_d63bf876;
  skos:inScheme :conceptScheme_751925ed;
  skos:notation "AX"@en;
  skos:prefLabel "architectural - general"@en;
  skosxl:prefLabel :xl_en_965bae0f .

:xl_en_965bae0f a skosxl:Label;
  skosxl:literalForm "architectural - general"@en .

:xl_en_2e2f6167 a skosxl:Label;
  skosxl:literalForm "forms"@en .

:xl_en_86ca8f53 a skosxl:Label;
  skosxl:literalForm "early warning"@en .

:xl_en_36537239 a skosxl:Label;
  skosxl:literalForm "design change notice"@en .

:xl_en_b34686a9 a skosxl:Label;
  skosxl:literalForm "landscape and environment-air and noise"@en .

:xl_en_47c2d55f a skosxl:Label;
  skosxl:literalForm "risk assessment"@en .

:c_ede99420 a skos:Concept;
  dc:source "Interim Advice Note 184/16 Highways England CAD and Data Standard"@en;
  dct:created "2018-08-19T08:15:48.037Z"^^xsd:dateTime;
  dct:modified "2020-10-31T05:31:27.167Z"^^xsd:dateTime;
  skos:broader :c_e5b1b611;
  skos:inScheme :conceptScheme_751925ed;
  skos:notation "SR"@en;
  skosxl:prefLabel :xl_en_29757dce .

:c_fa052d43 a skos:Concept;
  dc:source "Interim Advice Note 184/16 Highways England CAD and Data Standard"@en;
  dct:created "2018-08-19T08:43:25.336Z"^^xsd:dateTime;
  dct:modified "2020-10-31T05:31:40.994Z"^^xsd:dateTime;
  skos:broader :c_e5b1b611;
  skos:example """For individual assets like gantry, retaining walls these will be numbered GY or RT then the
asset number e.g."""@en;
  skos:inScheme :conceptScheme_751925ed;
  skos:notation "ID"@en;
  skosxl:prefLabel :xl_en_072055b5 .

:xl_en_a39943b3 a skosxl:Label;
  skosxl:literalForm "compensation events"@en .

:xl_en_c897327d a skosxl:Label;
  skosxl:literalForm "confirmation of verbal instruction"@en .

:xl_en_95dff570 a skosxl:Label;
  skosxl:literalForm "civil-utilities"@en .

:xl_en_29757dce a skosxl:Label;
  dc:source """production information a code of procedure for the construction industry
Organization of information about construction works — Information management using building information modelling - Part 2:Delivery phase of assets"""@en;
  skos:notation "SR"@en;
  skosxl:literalForm "slip road"@en .

:xl_en_e1702714 a skosxl:Label;
  skosxl:literalForm "inspection and test plan"@en .

:xl_en_f3446da3 a skosxl:Label;
  skosxl:literalForm "schematic"@en .

:xl_en_072055b5 a skosxl:Label;
  skosxl:literalForm "individual asset"@en .

:c_2df70b84 a skos:Concept;
  dc:source "zero carbon hub appendices - closing the gap between design and as-built performance - evidence review report appendices"@en;
  dct:created "2018-10-13T05:27:18.574Z"^^xsd:dateTime;
  dct:modified "2020-10-31T05:33:10.388Z"^^xsd:dateTime;
  olo:index "5"^^xsd:positiveInteger;
  skos:broader :c_91ece774;
  skos:inScheme :conceptScheme_751925ed;
  skos:notation "50"@en;
  skosxl:prefLabel :xl_en_a620c80c .

:xl_en_a620c80c a skosxl:Label;
  skosxl:literalForm "substructure"@en .

:skosCollection_3063372a a skos:Collection;
  dct:created "2018-10-25T12:33:12.091Z"^^xsd:dateTime;
  dct:modified "2019-11-30T10:51:39.869Z"^^xsd:dateTime;
  skos:member :c_1fbd8b11, :c_72030014, :c_8d825e3a, :c_91ece774, :c_c7d2ad4d, :c_e85c9613;
  skosxl:prefLabel :xl_en_979d65f7 .

:xl_en_979d65f7 a skosxl:Label;
  skosxl:literalForm "development stages (housing)"@en .

:conceptScheme_751925ed dc:contributor """HM Government
"""@en;
  dc:description "Scope of controlled vocabulary to follow"@en .

:skosCollection_f8d24590 skos:prefLabel "fire safety"@en .

:skosCollection_1f48022e skos:prefLabel "type documents"@en .

:skosCollection_4d3f42cb skos:prefLabel "location"@en .

:skosCollection_dca655b9 skos:prefLabel "volumes"@en .

:skosCollection_b565257c skos:prefLabel "type drawings"@en .

:skosCollection_77325868 skos:prefLabel "role"@en .

:c_5d6a79d1 dct:modified "2019-11-30T10:56:42.344Z"^^xsd:dateTime;
  skos:prefLabel "operational manual"@en .

:c_83498fa1 dct:modified "2019-11-30T10:57:14.060Z"^^xsd:dateTime;
  skos:prefLabel "as-built drawing"@en .

:c_f46087b4 skos:prefLabel "maintenance manual"@en .

:c_263f8b4d dct:modified "2019-11-30T10:58:42.421Z"^^xsd:dateTime;
  skos:prefLabel "ISO-DIS 19650-2 organization of information about construction works — information management using building information modelling - part 2: delivery phase of assets"@en .

<http://buildvoc.co.uk/resource/> owl:imports <http://purl.org/dc/elements/1.1/>,
    <http://purl.org/dc/terms/>, <http://www.w3.org/ns/dcat> .

:c_10975b72 skos:prefLabel "gateway points"@en .

:c_86ec4f8f skos:prefLabel "testing and commissioning"@en .

:c_3f7d46c0 dct:modified "2020-10-31T05:02:22.548Z"^^xsd:dateTime .

:c_2bf70455 skos:prefLabel "highways"@en .

:c_281f6d96 skos:prefLabel "drawings civil (housing)"@en .

:c_73619d2a skos:prefLabel "mechanical and electrical"@en .

:c_fbbe4f85 dct:modified "2020-10-31T05:57:11.926Z"^^xsd:dateTime .

:c_bfc844fa skos:prefLabel "model rendition for other renditions, e.g. thermal analysis, etc"@en .

:c_49888cc9 skos:prefLabel "council of mortgage lenders certificate"@en .

:c_f23ce991 dct:modified "2020-10-31T05:55:13.373Z"^^xsd:dateTime .

:c_2a55a494 skos:prefLabel "level of detail"@en .

:c_c7b03ed3 dct:modified "2020-10-31T05:56:39.845Z"^^xsd:dateTime .

:c_32da9577 dct:modified "2020-10-31T05:56:56.654Z"^^xsd:dateTime .

:c_b470c6f5 dct:modified "2020-10-31T05:44:39.641Z"^^xsd:dateTime .

:c_ac25e497 skos:prefLabel "sketch"@en .

:c_ace7ce12 skos:prefLabel "traffic management"@en .

:c_eb6b96ad skos:prefLabel "temporary works"@en .

:c_0d6f0660 dct:modified "2020-10-31T05:48:52.625Z"^^xsd:dateTime .

:c_8f194b82 skos:prefLabel "plain language questions"@en .

:c_7d508f5e skos:prefLabel "bim level 2"@en .

:c_49e95986 skos:prefLabel "heating and ventilation designer"@en .

:c_da247d5e skos:prefLabel "block"@en .

:c_b4f95391 skos:prefLabel "superstructure"@en .

:c_386bb74f skos:prefLabel "electrical-control systems and technology"@en .

:c_3c21373f dct:modified "2020-10-31T05:46:15.146Z"^^xsd:dateTime .

:c_bf7feeca dct:modified "2020-10-31T05:57:58.032Z"^^xsd:dateTime;
  skos:prefLabel "building survey"@en .

:c_4fb142b4 skos:prefLabel "health and safety (document type)"@en .

:c_9e61f9a1 skos:prefLabel "road markings"@en .

:c_161ac3be skos:prefLabel "air quality"@en .

:c_6cd2fa76 skos:prefLabel "power / electrical"@en .

:c_9af04a0c skos:prefLabel "temporary"@en .

:c_eed60aa2 skos:prefLabel "land survey"@en .

:c_6c460406 dct:modified "2020-10-31T05:54:04.931Z"^^xsd:dateTime .

:c_2cb0f320 skos:prefLabel "snagging list"@en .

:c_db8a3f56 skos:prefLabel "specialist designer"@en .

:c_7b22749d skos:prefLabel "contractor"@en .

:c_e54483d8 skos:prefLabel "environment"@en .

:c_49cc400a dct:modified "2020-10-31T05:48:35.386Z"^^xsd:dateTime .

:c_443bf05e skos:prefLabel "plot"@en .

:c_14426eb2 skos:prefLabel "motorway communications"@en .

:c_3e2995a1 dct:modified "2020-10-31T05:53:10.482Z"^^xsd:dateTime .

:c_6ceaacc1 skos:prefLabel "tunnels"@en .

:c_8cad0fd2 dct:modified "2020-10-31T05:56:02.367Z"^^xsd:dateTime .

:c_55457a29 skos:prefLabel "animation file of a model"@en .

:c_0d978f6c skos:prefLabel "request for information"@en .

:c_2b89905f skos:prefLabel "link 1"@en .

:c_447a9eee skos:prefLabel "first fix"@en .

:c_5cd4aa00 skos:prefLabel "no level applicable"@en .

:c_1b065c63 skos:prefLabel "special structures"@en .

:c_75f1aa77 skos:prefLabel "general (environment)"@en .

:c_ef814787 skos:prefLabel "presentation"@en .

:c_e8d35302 skos:prefLabel "confirmation of verbal instruction"@en .

:c_68039062 skos:prefLabel "instruction"@en .

:c_9f1a47e2 dct:modified "2020-10-31T05:50:19.883Z"^^xsd:dateTime .

:c_5d8254a8 dct:modified "2020-10-31T05:46:33.554Z"^^xsd:dateTime .

:c_9832f0b7 skos:prefLabel "photographs"@en .

:c_9ef52cee skos:prefLabel "bridges and major culverts"@en .

:c_5060b718 skos:prefLabel "infrastructure engineer"@en .

:c_b046bfd7 dct:modified "2020-10-31T05:53:28.382Z"^^xsd:dateTime .

:c_c4204198 skos:prefLabel "building services drainage"@en .

:c_d0fec206 dct:modified "2020-10-31T05:47:08.049Z"^^xsd:dateTime .

:c_76b17e4d skos:prefLabel "site clearance"@en .

:c_b3508a0f dct:modified "2020-10-31T05:53:48.020Z"^^xsd:dateTime .

:c_edf75137 skos:prefLabel "townscape"@en .

:c_b2e826d0 skos:prefLabel "heritage/historic resources"@en .

:c_b86b8a23 skos:prefLabel "landscape and environment-environmentalist"@en .

:c_800d8fbb skos:prefLabel "project information model"@en .

:c_536a60e1 skos:prefLabel "contract certificates"@en .

:c_f443f164 skos:prefLabel "accident statistics"@en .

:c_b227f284 skos:prefLabel "national road telecommunications services (NRTS)"@en .

:c_8d5846c3 skos:prefLabel "diary-activity sheet"@en .

:c_3c5e3daa dct:modified "2020-10-31T05:44:55.674Z"^^xsd:dateTime .

:c_e2fbc29a skos:prefLabel "risk assessment"@en .

:c_5e5901cb dct:modified "2020-10-31T05:52:02.163Z"^^xsd:dateTime .

:c_6bc1fab9 skos:prefLabel "survey (volume)"@en .

:c_08fa2f6e skos:prefLabel "mezzanine above level 01"@en .

:c_240f4112 skos:prefLabel "database"@en .

:c_80aeab06 skos:prefLabel "side roads geometric layout"@en .

:c_2592b8ec dct:modified "2020-10-31T05:54:52.784Z"^^xsd:dateTime .

:c_2d69d738 skos:prefLabel "multiple levels"@en .

:c_8046ed58 dct:modified "2020-10-31T05:50:36.893Z"^^xsd:dateTime .

:c_412f9c62 skos:prefLabel "masts"@en .

:c_ecc8ec55 dct:modified "2020-10-31T05:57:43.371Z"^^xsd:dateTime .

:c_701139f9 skos:prefLabel "survey"@en .

:c_b65fa6fd skos:prefLabel "environmental survey"@en .

:c_9260f33c dct:modified "2020-10-31T05:48:19.442Z"^^xsd:dateTime .

:c_c0f70902 dct:modified "2020-10-31T05:57:26.589Z"^^xsd:dateTime .

:c_26348e8a skos:prefLabel "visualization"@en .

:c_0d539813 skos:prefLabel "lighting engineer"@en .

:c_818585d8 dct:modified "2020-10-31T04:51:19.484Z"^^xsd:dateTime .

:c_4dc03e66 skos:prefLabel "clash rendition"@en .

:c_98522fb2 skos:prefLabel "rams-wasp"@en .

:c_3f128faf dct:modified "2020-10-31T04:52:26.638Z"^^xsd:dateTime .

:c_1081a7c2 skos:prefLabel "site change request"@en .

:c_b781cfae dct:modified "2020-10-31T05:50:53.718Z"^^xsd:dateTime .

:c_9739e9be dct:modified "2020-10-31T04:53:54.920Z"^^xsd:dateTime .

:c_90ff7ddf skos:prefLabel "biodiversity"@en .

:c_e4e408ec skos:prefLabel "basement level 01"@en .

:c_11f27c78 skos:prefLabel "managing agent"@en .

:c_d837a7ac skos:prefLabel "substructure plan"@en .

:c_9b0e72da dct:modified "2020-10-31T05:47:52.635Z"^^xsd:dateTime .

:c_1e1d6eeb dct:modified "2020-10-31T05:44:21.986Z"^^xsd:dateTime .

:c_5ac38c99 skos:prefLabel "licence"@en .

:c_930416d1 skos:prefLabel "central reservation"@en .

:c_73726e27 skos:prefLabel "environmental approvals and consents"@en .

:c_f84ebdc2 dct:modified "2020-10-31T05:50:05.114Z"^^xsd:dateTime .

:c_c4c44bc2 skos:prefLabel "model 2d"@en .

:c_4a7bbbda skos:prefLabel "survey general"@en .

:c_ed146474 dct:modified "2020-10-31T05:46:50.008Z"^^xsd:dateTime .

:c_3fd4eac3 skos:prefLabel "road lighting"@en .

:c_01bda236 skos:prefLabel "local authority"@en .

:c_b39bb643 skos:prefLabel "finals and build complete"@en .

:c_46f0d5a6 skos:prefLabel "structures"@en .

:c_38840388 dct:modified "2020-10-31T05:03:24.202Z"^^xsd:dateTime;
  skos:prefLabel "civil-tunnels"@en .

:c_a9c2e902 dct:modified "2020-10-31T05:04:00.373Z"^^xsd:dateTime .

:c_9ebfa246 skos:prefLabel "legal notices-orders"@en .

:c_f897a1c6 dct:modified "2020-10-31T05:04:46.624Z"^^xsd:dateTime .

:c_9e9aa534 skos:prefLabel "permit"@en .

:c_250f029d skos:prefLabel "drainage"@en .

:c_624f6410 skos:prefLabel "gis dataset"@en .

:c_5f10d43b skos:prefLabel "mainline"@en .

:c_de6816aa skos:prefLabel "landscape and environment-air and noise"@en .

:c_b019c6a7 skos:prefLabel "mezzanine above level 02"@en .

:c_a1cd3dcb skos:prefLabel "geotechnical (highways)"@en .

:c_086e071c skos:prefLabel "asbestos survey"@en .

:c_f29587ff skos:prefLabel "documents (housing)"@en .

:c_edaf8450 skos:prefLabel "civil-utilities"@en .

:c_2238ee39 skos:prefLabel "contract documents"@en .

:c_db373352 skos:prefLabel "design change notice"@en .

:c_d37e6d79 skos:prefLabel "forms"@en .

:c_87bf8d98 skos:prefLabel "floor 02"@en .

:c_cf6c5d63 skos:prefLabel "junction"@en .

:c_36ce18a2 skos:prefLabel "traffic survey"@en .

:c_692f83c4 skos:prefLabel "general (highways)"@en .

:c_ade56523 skos:prefLabel "accommodation works"@en .

:c_71eda773 skos:prefLabel "fencing"@en .

:c_d9ed5f11 skos:prefLabel "pavement systems"@en .

:c_0fc93a91 skos:prefLabel "land ownership boundaries"@en .

:c_abd6f00f dct:modified "2020-10-31T05:12:31.807Z"^^xsd:dateTime;
  skos:prefLabel "correspondence"@en .

:c_782fa318 skos:prefLabel "civil-earthworks and geotechnics"@en .

:c_369e4bb6 skos:prefLabel "landscape and environment-heritage"@en .

:c_2a84910f skos:prefLabel "asset information requirements"@en .

:c_46f20ab0 skos:prefLabel "general no-disciplinary"@en .

:c_6859ada6 skos:prefLabel "mechanical and electrical specification"@en .

:c_2ce0c940 dct:modified "2020-10-31T05:14:16.717Z"^^xsd:dateTime .

:c_f8a6d299 skos:prefLabel "completion certificate"@en .

:c_02f182a2 skos:prefLabel "geotechnical (structures)"@en .

:c_34b987d4 skos:prefLabel "road pavements"@en .

:c_19a61f73 skos:prefLabel "level of information"@en .

:c_46da6c1c skos:prefLabel "product specific plain language compliance report: as built"@en .

:c_59dcd59c skos:prefLabel "highway approvals and consents"@en .

:c_87804062 skos:prefLabel "floor 01"@en .

:c_08498a44 skos:prefLabel "bim level 0"@en .

:c_129a5ec6 skos:prefLabel "second fix"@en .

:c_32bf6806 dct:modified "2020-10-31T05:49:37.020Z"^^xsd:dateTime .

:c_79de880f skos:prefLabel "section 2"@en .

:c_fcfbbcd0 skos:prefLabel "programme"@en .

:c_0a40b44e skos:prefLabel "bill of quantities"@en .

:c_1e86ab1c skos:prefLabel "geospatial (role)"@en .

:c_04a3b08d skos:prefLabel "road restraint system (vehicle and pedestrian)"@en .

:c_9d7853dc skos:prefLabel "dry lining and plaster"@en .

:c_24506d00 skos:prefLabel "services electrical"@en .

:c_05a3b5d1 skos:prefLabel "functional specification"@en .

:c_13d79d5e skos:prefLabel "utilities"@en .

:c_6c31e8f5 skos:prefLabel "general (structures)"@en .

:c_0b45b235 skos:prefLabel "retaining walls"@en .

:c_8ec4ead3 skos:prefLabel "feasibility study"@en .

:c_e5b1b611 skos:prefLabel "level location"@en .

:c_4d73ba7d skos:prefLabel "roof to weathertight"@en .

:c_607b5b8a skos:prefLabel "base level of building where ground floor is not appropriate"@en .

:c_7f9323cb skos:prefLabel "mainline geometric layout"@en .

:c_9328238a skos:prefLabel "calculations"@en .

:c_b707f1ea skos:prefLabel "cost plan"@en .

:c_a47e6a9b dct:modified "2020-10-31T05:56:18.268Z"^^xsd:dateTime .

:c_c4f5d4fc skos:prefLabel "civil-drainage"@en .

:c_8741d02b skos:prefLabel "detail drawing"@en .

:c_1258140e skos:prefLabel "civil-highways"@en .

:c_d6230a5f skos:prefLabel "room data sheet"@en .

:c_d0784080 skos:prefLabel "specification"@en .

:c_a34bfc84 skos:prefLabel "model 3d"@en .

:c_c989802e skos:prefLabel "invoice"@en .

:c_517519ce skos:prefLabel "commercial and cost management (role)"@en .

:c_ff860f3e skos:prefLabel "project implementation plan"@en .

:c_1f84f905 skos:prefLabel "file note"@en .

:c_be22475b dct:modified "2020-10-31T05:27:30.728Z"^^xsd:dateTime;
  skos:prefLabel "site manager"@en .

:c_3fdd4da0 skos:prefLabel "master information delivery plan"@en .

:c_bce20c84 skos:prefLabel "scheme wide generic information"@en .

:c_a7289a25 dct:modified "2020-10-31T05:28:32.967Z"^^xsd:dateTime .

:c_b0503f89 skos:prefLabel "sub-contractor"@en .

:c_b7ef2137 skos:prefLabel "drawing type"@en .

:c_a02e9571 skos:prefLabel "minor structures and culverts"@en .

:c_e8a3f333 skos:prefLabel "compensation events"@en .

:c_ede99420 skos:prefLabel "slip road"@en .

:c_fa052d43 skos:prefLabel "individual asset"@en .

:c_fb2c64cc skos:prefLabel "basement level 02"@en .

:c_717bb7fd skos:prefLabel "health and safety adviser"@en .

:c_d5bcf8c5 skos:prefLabel "knowledge library"@en .

:c_8b778c41 skos:prefLabel "noise and vibration"@en .

:c_2df70b84 skos:prefLabel "substructure"@en .

:c_28df75da skos:prefLabel "built asset security strategy"@en .

:c_b932ae7e skos:prefLabel "gantries"@en .

:c_e9882180 skos:prefLabel "combined model combined multidiscipline model"@en .

:c_52608161 skos:prefLabel "oversite"@en .

:c_3c4ef6f5 skos:prefLabel "setting out plan"@en .

:c_98ba4c18 skos:prefLabel "departure submissions"@en .

:c_876afb3f dct:modified "2020-10-31T05:54:28.696Z"^^xsd:dateTime .

:c_618864b7 skos:prefLabel "document type"@en .

:c_5bc1704c skos:prefLabel "task information delivery plan"@en .

:c_bd6073c7 skos:prefLabel "civil-temporary works"@en .

:c_31175b54 skos:prefLabel "built asset security management plan"@en .

:c_b2459321 skos:prefLabel "construction specification"@en .

:c_2e6cd3a6 skos:prefLabel "standard methods and procedures"@en .

:c_d8e2bacb skos:prefLabel "geotechnical investigation"@en .

:c_7e8703b2 skos:prefLabel "health and safety (volume)"@en .

:c_1e5f46db skos:prefLabel "report"@en .

:c_9509873f skos:prefLabel "local authority building control"@en .

:c_86ba3858 skos:prefLabel "stakeholder liaison"@en .

:c_41bc9708 skos:prefLabel "reconciliation"@en .

:c_dca128d9 skos:prefLabel "geographical and land surveyor"@en .

:c_35bd7cc0 skos:prefLabel "information exchange file"@en .

:c_36f0ebbb skos:prefLabel "civil-bridges and structures"@en .

:c_ef4fcc0c skos:prefLabel "inspection and test plan"@en .

:c_03f66e64 skos:prefLabel "general"@en .

:c_2a6e874e skos:prefLabel "method statement"@en .

:c_1efc9178 skos:prefLabel "security breach / incident management plan"@en .

:c_5d17180d skos:prefLabel "non conformance report"@en .

:c_f569343b skos:prefLabel "building safety manager"@en .

:c_d71b62e2 skos:prefLabel "early warning"@en .

:xl_en_5e0bcc99 skosxl:literalForm "guide to bs1192"@en .

:c_026699d9 skos:prefLabel "inconsistency"@en .

:xl_en_ec0ff6cd skosxl:literalForm "standard assessment procedure worksheet: as built"@en .

:xl_en_7589e5ba skosxl:literalForm "initiate feasibility study"@en .

:xl_en_670428ce skosxl:literalForm "joist to roof"@en .

:c_261a288e a skos:Concept;
  dct:created "2020-10-31T08:16:44.529Z"^^xsd:dateTime;
  dct:modified "2020-10-31T08:43:42.402Z"^^xsd:dateTime;
  skos:broader :c_084a4f3a;
  skos:definition "part of management that is responsible for the management of records and the guidance and supervision of knowledge work that is related to any records"@en;
  skos:exactMatch <http://urn.fi/URN:NBN:fi:au:tt:t129>;
  skos:inScheme :conceptScheme_751925ed;
  skos:narrower :c_0987399d, :c_57245cc9, :c_6dd048e6, :c_93444f60;
  skos:prefLabel "records management"@en .

:c_295c3f50 dct:modified "2020-10-31T08:54:10.480Z"^^xsd:dateTime;
  owl:deprecated true .

:c_0987399d a skos:Concept;
  dct:created "2020-10-31T08:19:42.521Z"^^xsd:dateTime;
  dct:modified "2020-10-31T08:23:33.826Z"^^xsd:dateTime;
  skos:broader :c_261a288e;
  skos:definition "document that has been made or received in connection with the activities of an organisation or private individual and which is then stored as evidence and information property"@en;
  skos:exactMatch <http://urn.fi/URN:NBN:fi:au:tt:t77>;
  skos:inScheme :conceptScheme_751925ed;
  skos:prefLabel "record"@en .

:c_93444f60 a skos:Concept;
  dct:created "2020-10-31T08:24:25.743Z"^^xsd:dateTime;
  dct:modified "2020-10-31T08:26:20.680Z"^^xsd:dateTime;
  skos:broader :c_261a288e;
  skos:definition """
process of adding records to an archive (records)"""@en;
  skos:exactMatch <http://urn.fi/URN:NBN:fi:au:tt:t49>;
  skos:inScheme :conceptScheme_751925ed;
  skos:note "Archiving plays a central role in ensuring the usability of an archive, and it enables the record-specific management of materials, especially the screening of materials as well as their provision according to the Finnish Personal Data Act and the Act on the Openness of Government Activities."@en;
  skos:prefLabel "archiving"@en .

:c_6dd048e6 a skos:Concept;
  dct:created "2020-10-31T08:27:05.856Z"^^xsd:dateTime;
  dct:modified "2020-10-31T08:27:40.222Z"^^xsd:dateTime;
  skos:broader :c_261a288e;
  skos:definition """
information that is part of the information content or metadata of a record"""@en;
  skos:inScheme :conceptScheme_751925ed;
  skos:prefLabel "records data"@en .

:c_084a4f3a a skos:Concept;
  dct:modified "2020-10-31T09:30:47.509Z"^^xsd:dateTime;
  skos:broader :c_f6f95a83;
  skos:narrower :c_261a288e, :c_4dd7fd6a, :c_bd21cb81, :c_cbb9bfe9, :c_fb07c266 .

:c_7710af58 a skos:Concept;
  dct:created "2020-10-31T08:54:25.843Z"^^xsd:dateTime;
  dct:modified "2020-10-31T08:58:14.515Z"^^xsd:dateTime;
  skos:broader :c_084a4f3a;
  skos:definition "part of the data acquisition process where the desired information is searched from data sources"@en;
  skos:exactMatch <http://urn.fi/URN:NBN:fi:au:tt:t99>;
  skos:inScheme :conceptScheme_751925ed;
  skos:prefLabel "information retrieval"@en .

:c_cbb9bfe9 a skos:Concept;
  dct:created "2020-10-31T09:03:11.749Z"^^xsd:dateTime;
  dct:modified "2020-10-31T09:05:17.241Z"^^xsd:dateTime;
  skos:broader :c_084a4f3a;
  skos:definition """activity that aims to satisfy one's need for information
"""@en;
  skos:exactMatch <http://urn.fi/URN:NBN:fi:au:tt:t1>;
  skos:inScheme :conceptScheme_751925ed;
  skos:note "To ensure a successful data acquisition process, the relevant channels and information sources must be identified and utilised – for example, an expert in the field can act as an information source by participating in an interview or survey."@en;
  skos:prefLabel "data acquisition"@en .

:c_733ad8a3 a skos:Concept;
  dct:created "2020-11-01T09:34:30.175Z"^^xsd:dateTime;
  skos:broader :c_a314e31f;
  skos:inScheme :conceptScheme_751925ed;
  skos:prefLabel "duties"@en .

:c_09f6c52a skos:definition "The Project BIM Protocol sets out the obligations of the principal members of the Project Team in respect of the use of BIM on the Project."@en .

:c_57245cc9 a skos:Concept;
  skos:broader :c_261a288e;
  skos:inScheme :conceptScheme_751925ed;
  skos:prefLabel "audit documentation"@en .

